@prefix : <http://data.europa.eu/949/> .
@prefix cc: <http://creativecommons.org/ns#> .
@prefix vs: <http://www.w3.org/2003/06/sw-vocab-status/ns#> .
@prefix dct: <http://purl.org/dc/terms/> .
@prefix era: <http://data.europa.eu/949/> .
@prefix gsp: <http://www.opengis.net/ont/geosparql#> .
@prefix org: <http://www.w3.org/ns/org#> .
@prefix owl: <http://www.w3.org/2002/07/owl#> .
@prefix rdf: <http://www.w3.org/1999/02/22-rdf-syntax-ns#> .
@prefix wgs: <http://www.w3.org/2003/01/geo/wgs84_pos#> .
@prefix xml: <http://www.w3.org/XML/1998/namespace> .
@prefix xsd: <http://www.w3.org/2001/XMLSchema#> .
@prefix rdfs: <http://www.w3.org/2000/01/rdf-schema#> .
@prefix skos: <http://www.w3.org/2004/02/skos/core#> .
@prefix schema: <https://schema.org/> .
@prefix scheme: <http://data.europa.eu/949/schemes/> .
@prefix opTypes: <http://data.europa.eu/949/concepts/op-types/> .
@prefix osmClass: <http://data.europa.eu/949/concepts/osmClass/> .
@base <http://data.europa.eu/949/> .

<http://data.europa.eu/949/> rdf:type owl:Ontology ;
                              owl:imports gsp: ;
                              cc:license <https://creativecommons.org/licenses/by/4.0/> ;
                              dct:author "Edna Ruckhaus" ,
                                         "Oscar Corcho" ;
                              dct:contributor <https://dylanvanassche.be/#me> ,
                                              <https://julianrojas.org/#me> ,
                                              <https://pietercolpaert.be/#me> ,
                                              "Ivo Velitchkov" ,
                                              "Marina Aguado" ,
                                              "Polymnia Vasilopoulou" ,
                                              "Wouter Beek" ;
                              dct:issued "2020-07-29"^^xsd:date ;
                              dct:modified "2023-04-05"^^xsd:date ;
                              dct:publisher "European Union Agency for Railways" ;
                              dct:title "ERA vocabulary"@en ;
                              rdfs:comment """This is the human and machine readable Vocabulary/Ontology governed by the European Union Agency for Railways. It represents the concepts and relationships linked to the sectorial legal framework and the use cases under the AgencyÂ´s remit. Currently, this vocabulary covers the European railway infrastructure and the vehicles authorized to operate over it. It is a semantic/browsable representation of the [RINF](https://www.era.europa.eu/sites/default/files/registers/docs/rinf_application_guide_for_register_en.pdf) and [ERATV](https://www.era.europa.eu/sites/default/files/registers/docs/iu-eratv_application_guide_for_register_2016-797_en.pdf) application guides that were built by domain experts in the RINF and ERATV working parties.
Since version 2.6.0, the ontology includes the routebook concepts described in appendix D2 \"Elements the infrastructure manager has to provide to the railway undertaking for the Route Book\" (https://eur-lex.europa.eu/eli/reg_impl/2019/773/oj) and the appendix D3 \"ERTMS trackside engineering information relevant to operation that the infrastructure manager shall provide to the railway undertaking\"."""@en ;
                              rdfs:label "ERA vocabulary"@en ;
                              owl:priorVersion "https://git.fpfis.eu/datateam/ERA/era-vocabulary/-/releases/v3.0.0"^^xsd:anyURI ;
                              owl:versionInfo "v3.0.1"^^xsd:string ;
                              owl:versionURI "https://git.fpfis.eu/datateam/ERA/era-vocabulary/-/releases/v3.0.1"^^xsd:anyURI .

#################################################################
#    Annotation properties
#################################################################

###  http://creativecommons.org/ns#license
cc:license rdf:type owl:AnnotationProperty .


###  http://data.europa.eu/949/appendixD2Index
era:appendixD2Index rdf:type owl:AnnotationProperty ;
                    rdfs:comment "The index of a vocabulary term in Appendix D2 Elements the infrastructure manager has to provide to the railway undertaking for the Route Book from the document Commission Implementing Regulation (EU) 2019/773 of 16 May 2019 on the technical specification for interoperability relating to the operation and traffic management subsystem of the rail system within the European Union and repealing Decision 2012/757/EU."@en ;
                    rdfs:isDefinedBy <http://data.europa.eu/949/> ;
                    rdfs:label "Appendix D2 index"@en ;
                    skos:definition "The index of a vocabulary term in Appendix D2 Elements the infrastructure manager has to provide to the railway undertaking for the Route Book from the document Commission Implementing Regulation (EU) 2019/773 of 16 May 2019 on the technical specification for interoperability relating to the operation and traffic management subsystem of the rail system within the European Union and repealing Decision 2012/757/EU."@en .


###  http://data.europa.eu/949/appendixD3Index
era:appendixD3Index rdf:type owl:AnnotationProperty ;
                    dct:created "2022-11-04"^^xsd:date ;
                    rdfs:comment "The index of a vocabulary term in Appendix D3 ERTMS trackside engineering information relevant to operation that the infrastructure manager shall provide to the railway undertaking."@en ;
                    rdfs:isDefinedBy <http://data.europa.eu/949/> ;
                    rdfs:label "Appendix D3 index"@en ;
                    vs:term_status "stable" .


###  http://data.europa.eu/949/canonicalURI
era:canonicalURI rdf:type owl:AnnotationProperty ;
                 dct:created "2022-12-13"^^xsd:date ;
                 rdfs:comment "The canonical URI is defined for each instance of a Feature, e.g. section of line, operational point. URIs generated through RML mappings include a part with the validity start and end dates. The canonical URI is the URI stripped of its validity start and end dates during the post-processing of the RDF file."@en ;
                 rdfs:isDefinedBy <http://data.europa.eu/949/> ;
                 rdfs:label "Canonical URI"@en ;
                 rdfs:range xsd:anyURI ;
                 rdfs:domain era:Feature .


###  http://data.europa.eu/949/eratvIndex
era:eratvIndex rdf:type owl:AnnotationProperty ;
               dct:created "2020-11-03"^^xsd:date ;
               dct:modified "2020-11-03"^^xsd:date ;
               rdfs:comment "Index code used in the original definition of a parameter in ERATV."@en ;
               rdfs:isDefinedBy <http://data.europa.eu/949/> ;
               rdfs:label "ERATV index"@en ;
               vs:term_status "stable" .


###  http://data.europa.eu/949/inSkosConceptScheme
era:inSkosConceptScheme rdf:type owl:AnnotationProperty ;
                        dct:created "2022-11-17"^^xsd:date ;
                        rdfs:comment "Property that links an object SKOS property to a the URI of the corresponding SKOS Concept Scheme."@en ;
                        rdfs:isDefinedBy <http://data.europa.eu/949/> ;
                        rdfs:label "in SKOS Concept Scheme"@en ;
                        vs:term_status "stable" ;
                        rdfs:range xsd:anyURI .


###  http://data.europa.eu/949/rinfIndex
era:rinfIndex rdf:type owl:AnnotationProperty ;
              dct:created "2020-11-03"^^xsd:date ;
              dct:modified "2020-11-03"^^xsd:date ;
              rdfs:comment "Index code used in the original definition of a parameter in RINF."@en ;
              rdfs:isDefinedBy <http://data.europa.eu/949/> ;
              rdfs:label "RINF index"@en ;
              vs:term_status "stable" .


###  http://data.europa.eu/949/usedInRCCCalculations
era:usedInRCCCalculations rdf:type owl:AnnotationProperty ;
                          dct:created "2023-04-12"^^xsd:date ;
                          rdfs:comment """Indicates whether a RINF parameter is used in Route Compatibility Check calculations according to Commission Implementing Regulation (EU) 2019/773 of 16 May 2019 on the technical specification for interoperability relating to the operation and traffic management subsystem of the rail system within the European Union and repealing Decision.
https://eur-lex.europa.eu/eli/reg_impl/2019/773/oj#:~:text=Commission%20Implementing%20Regulation."""@en ;
                          rdfs:isDefinedBy <http://data.europa.eu/949/> ;
                          rdfs:label "Parameter is used in Route Compatibility Check (RCC) calculations"@en ;
                          rdfs:range xsd:boolean .


###  http://purl.org/dc/elements/1.1/date
<http://purl.org/dc/elements/1.1/date> rdf:type owl:AnnotationProperty .


###  http://purl.org/dc/elements/1.1/description
<http://purl.org/dc/elements/1.1/description> rdf:type owl:AnnotationProperty .


###  http://purl.org/dc/elements/1.1/source
<http://purl.org/dc/elements/1.1/source> rdf:type owl:AnnotationProperty .


###  http://purl.org/dc/elements/1.1/title
<http://purl.org/dc/elements/1.1/title> rdf:type owl:AnnotationProperty .


###  http://purl.org/dc/terms/author
dct:author rdf:type owl:AnnotationProperty .


###  http://purl.org/dc/terms/contributor
dct:contributor rdf:type owl:AnnotationProperty .


###  http://purl.org/dc/terms/created
dct:created rdf:type owl:AnnotationProperty .


###  http://purl.org/dc/terms/description
dct:description rdf:type owl:AnnotationProperty .


###  http://purl.org/dc/terms/isReplacedBy
dct:isReplacedBy rdf:type owl:AnnotationProperty .


###  http://purl.org/dc/terms/issued
dct:issued rdf:type owl:AnnotationProperty .


###  http://purl.org/dc/terms/modified
dct:modified rdf:type owl:AnnotationProperty .


###  http://purl.org/dc/terms/publisher
dct:publisher rdf:type owl:AnnotationProperty .


###  http://purl.org/dc/terms/source
dct:source rdf:type owl:AnnotationProperty .


###  http://purl.org/dc/terms/title
dct:title rdf:type owl:AnnotationProperty .


###  http://www.w3.org/2002/07/owl#versionURI
owl:versionURI rdf:type owl:AnnotationProperty .


###  http://www.w3.org/2003/01/geo/wgs84_pos#alt
wgs:alt rdf:type owl:AnnotationProperty ;
        rdfs:comment """The WGS84 altitude of a SpatialThing (decimal meters 
above the local reference ellipsoid).""" ;
        rdfs:label "altitude" ;
        rdfs:domain wgs:SpatialThing .


###  http://www.w3.org/2003/01/geo/wgs84_pos#lat
wgs:lat rdf:type owl:AnnotationProperty ;
        rdfs:comment "The WGS84 latitude of a SpatialThing (decimal degrees)." ;
        rdfs:label "latitude" ;
        rdfs:domain wgs:SpatialThing .


###  http://www.w3.org/2003/01/geo/wgs84_pos#location
wgs:location rdf:type owl:AnnotationProperty ;
             rdfs:subPropertyOf <http://xmlns.com/foaf/0.1/based_near> ;
             rdfs:range wgs:SpatialThing .


###  http://www.w3.org/2003/01/geo/wgs84_pos#long
wgs:long rdf:type owl:AnnotationProperty ;
         rdfs:comment "The WGS84 longitude of a SpatialThing (decimal degrees)." ;
         rdfs:label "longitude" ;
         rdfs:domain wgs:SpatialThing .


###  http://www.w3.org/2003/06/sw-vocab-status/ns#term_status
vs:term_status rdf:type owl:AnnotationProperty .


###  http://www.w3.org/2004/02/skos/core#definition
skos:definition rdf:type owl:AnnotationProperty .


###  http://www.w3.org/2004/02/skos/core#scopeNote
skos:scopeNote rdf:type owl:AnnotationProperty .


###  http://xmlns.com/foaf/0.1/based_near
<http://xmlns.com/foaf/0.1/based_near> rdf:type owl:AnnotationProperty .


#################################################################
#    Datatypes
#################################################################

###  http://www.opengis.net/ont/geosparql#wktLiteral
gsp:wktLiteral rdf:type rdfs:Datatype .


###  http://www.w3.org/2001/XMLSchema#date
xsd:date rdf:type rdfs:Datatype .


#################################################################
#    Object Properties
#################################################################

###  http://data.europa.eu/949/TSIMagneticFields
era:TSIMagneticFields rdf:type owl:ObjectProperty ,
                               owl:FunctionalProperty ;
                      rdfs:domain [ rdf:type owl:Class ;
                                    owl:unionOf ( era:SubsetWithCommonCharacteristics
                                                  era:Track
                                                )
                                  ] ;
                      rdfs:range skos:Concept ;
                      era:inSkosConceptScheme <http://data.europa.eu/949/concepts/tsi-compliances/TSICompliances> ;
                      era:rinfIndex "1.1.1.3.9.1" ,
                                    "1.2.1.1.8.1" ;
                      dct:created "2021-08-09"^^xsd:date ;
                      dct:modified "2021-09-12"^^xsd:date ;
                      rdfs:comment "Indication whether rules exist and are compliant with the TSI. The allowed values for this property belong to the SKOS Concept Scheme http://data.europa.eu/949/concepts/tsi-compliances/TSICompliances."@en ;
                      rdfs:isDefinedBy <http://data.europa.eu/949/> ;
                      rdfs:label "Existence and TSI compliance of rules for magnetic fields emitted by a vehicle"@en ;
                      vs:term_status "stable" .


###  http://data.europa.eu/949/TSITractionHarmonics
era:TSITractionHarmonics rdf:type owl:ObjectProperty ,
                                  owl:FunctionalProperty ;
                         rdfs:domain [ rdf:type owl:Class ;
                                       owl:unionOf ( era:SubsetWithCommonCharacteristics
                                                     era:Track
                                                   )
                                     ] ;
                         rdfs:range skos:Concept ;
                         era:inSkosConceptScheme <http://data.europa.eu/949/concepts/tsi-compliances/TSICompliances> ;
                         era:rinfIndex "1.1.1.3.9.2" ,
                                       "1.2.1.1.8.2" ;
                         dct:created "2021-08-09"^^xsd:date ;
                         dct:modified "2021-09-12"^^xsd:date ;
                         rdfs:comment "Indication whether rules exist and are compliant with the TSI. The allowed values for this property belong to the SKOS Concept Scheme http://data.europa.eu/949/concepts/tsi-compliances/TSICompliances."@en ;
                         rdfs:isDefinedBy <http://data.europa.eu/949/> ;
                         rdfs:label "Existence and TSI compliance of limits in harmonics in the traction current of vehicles"@en ;
                         vs:term_status "stable" .


###  http://data.europa.eu/949/atoCommunicationSystem
era:atoCommunicationSystem rdf:type owl:ObjectProperty ;
                           rdfs:domain [ rdf:type owl:Class ;
                                         owl:unionOf ( era:SubsetWithCommonCharacteristics
                                                       era:Track
                                                     )
                                       ] ;
                           rdfs:range skos:Concept ;
                           era:rinfIndex "1.1.1.3.13.3" ,
                                         "1.2.1.1.10.3" ;
                           dct:created "2023-03-14"^^xsd:date ;
                           rdfs:comment """Supported ATO communication systems from trackside.
The allowed values for this property belong to a SKOS Concept Scheme."""@en ;
                           rdfs:isDefinedBy <http://data.europa.eu/949/> ;
                           rdfs:label "ATO communication system"@en ;
                           vs:term_status "unstable" .


###  http://data.europa.eu/949/atoGradeAutomation
era:atoGradeAutomation rdf:type owl:ObjectProperty ;
                       rdfs:domain [ rdf:type owl:Class ;
                                     owl:unionOf ( era:SubsetWithCommonCharacteristics
                                                   era:Track
                                                 )
                                   ] ;
                       rdfs:range skos:Concept ;
                       era:rinfIndex "1.1.1.3.13.1" ,
                                     "1.2.1.1.10.1" ;
                       dct:created "2023-03-14"^^xsd:date ;
                       rdfs:comment """ATO grade of automation installed lineside.
The allowed values for this property belong to a SKOS Concept Scheme."""@en ;
                       rdfs:isDefinedBy <http://data.europa.eu/949/> ;
                       rdfs:label "ATO Grade of Automation"@en ;
                       vs:term_status "unstable" .


###  http://data.europa.eu/949/atoSystemVersion
era:atoSystemVersion rdf:type owl:ObjectProperty ;
                     rdfs:domain [ rdf:type owl:Class ;
                                   owl:unionOf ( era:SubsetWithCommonCharacteristics
                                                 era:Track
                                               )
                                 ] ;
                     rdfs:range skos:Concept ;
                     era:rinfIndex "1.1.1.3.13.2" ,
                                   "1.2.1.1.10.2" ;
                     dct:created "2023-03-14"^^xsd:date ;
                     rdfs:comment """ATO system version according to the specification referenced in Appendix A-1, index [C].
The allowed values for this property belong to a SKOS Concept Scheme."""@en ;
                     rdfs:isDefinedBy <http://data.europa.eu/949/> ;
                     rdfs:label "ATO System version"@en ;
                     vs:term_status "unstable" .


###  http://data.europa.eu/949/authorizedCountry
era:authorizedCountry rdf:type owl:ObjectProperty ;
                      rdfs:domain era:VehicleType ;
                      rdfs:range skos:Concept ;
                      era:inSkosConceptScheme <http://publications.europa.eu/resource/authority/country> ;
                      dct:created "2020-09-30"^^xsd:date ;
                      dct:modified "2020-09-30"^^xsd:date ;
                      rdfs:comment "Indicates the country(ies) in where a vehicle type has been authorized to operate. The allowed values for this property belong to the SKOS Concept Scheme http://publications.europa.eu/resource/authority/country"@en ;
                      rdfs:isDefinedBy <http://data.europa.eu/949/> ;
                      rdfs:label "Authorized country"@en ;
                      vs:term_status "stable" .


###  http://data.europa.eu/949/axleBearingConditionMonitoring
era:axleBearingConditionMonitoring rdf:type owl:ObjectProperty ;
                                   rdfs:domain era:VehicleType ;
                                   rdfs:range skos:Concept ;
                                   era:eratvIndex "4.9.2" ;
                                   era:inSkosConceptScheme <http://data.europa.eu/949/concepts/axle-monitoring/AxleBearingMonitoring> ;
                                   dct:created "2020-08-24"^^xsd:date ;
                                   dct:modified "2021-08-02"^^xsd:date ;
                                   rdfs:comment "Axle bearing condition monitoring. The allowed values for this property belong to the SKOS Concept Scheme http://data.europa.eu/949/concepts/axle-monitoring/AxleBearingMonitoring"@en ;
                                   rdfs:isDefinedBy <http://data.europa.eu/949/> ;
                                   rdfs:label "Axle bearing condition monitoring"@en ;
                                   vs:term_status "stable" .


###  http://data.europa.eu/949/borderPointOf
era:borderPointOf rdf:type owl:ObjectProperty ;
                  owl:inverseOf era:opInfoPerCountry ;
                  rdfs:domain era:OperationalPoint ;
                  rdfs:range era:OperationalPoint ;
                  dct:created "2023-01-20"^^xsd:date ;
                  rdfs:comment "Relates the information that each country maintains on a border point, to the operational point that represents the general information on the border point."@en ;
                  rdfs:isDefinedBy <http://data.europa.eu/949/> ;
                  rdfs:label "Border point of"@en ;
                  vs:term_status "stable" .


###  http://data.europa.eu/949/cantDeficiencyBasicSSP
era:cantDeficiencyBasicSSP rdf:type owl:ObjectProperty ;
                           rdfs:domain [ rdf:type owl:Class ;
                                         owl:unionOf ( era:SubsetWithCommonCharacteristics
                                                       era:Track
                                                     )
                                       ] ;
                           rdfs:range skos:Concept ;
                           era:rinfIndex "1.1.1.3.2.14" ,
                                         "1.2.1.1.1.14" ;
                           dct:created "2023-03-14"^^xsd:date ;
                           rdfs:comment """Essential information for drivers of trains with a worse (lower) tolerated cant deficiency than those for which the ETCS trackside provides SSP (Static Speed Profiles) in conjunction with 1.1.1.3.2.14.1 
According to the specification referenced in Appendix A-1, index [C]."""@en ;
                           rdfs:isDefinedBy <http://data.europa.eu/949/> ;
                           rdfs:label "Cant Deficiency used for the basic SSP"@en ;
                           vs:term_status "stable" .


###  http://data.europa.eu/949/category
era:category rdf:type owl:ObjectProperty ,
                      owl:FunctionalProperty ;
             rdfs:domain era:VehicleType ;
             rdfs:range skos:Concept ;
             era:eratvIndex 1.4 ;
             era:inSkosConceptScheme <http://data.europa.eu/949/concepts/vehicle-types/Categories> ;
             dct:created "2020-07-29"^^xsd:date ;
             dct:modified "2021-08-03"^^xsd:date ;
             rdfs:comment "Vehicle category. The allowed values for this property belong to the SKOS Concept Scheme http://data.europa.eu/949/concepts/vehicle-types/Categories."@en ;
             rdfs:isDefinedBy <http://data.europa.eu/949/> ;
             rdfs:label "Vehicle category"@en ;
             vs:term_status "stable" .


###  http://data.europa.eu/949/certificate
era:certificate rdf:type owl:ObjectProperty ;
                rdfs:domain era:VehicleType ;
                rdfs:range era:Certificate ;
                dct:created "2022-06-15"^^xsd:date ;
                dct:modified "2022-11-15"^^xsd:date ;
                rdfs:comment "Denotes a certificate for this particular vehicleType."@en ;
                rdfs:isDefinedBy <http://data.europa.eu/949/> ;
                rdfs:label "Certificate"@en ;
                vs:term_status "stable" .


###  http://data.europa.eu/949/companyCodeCategory
era:companyCodeCategory rdf:type owl:ObjectProperty ;
                        rdfs:range skos:Concept ;
                        era:inSkosConceptScheme <http://data.europa.eu/949/concepts/company-code-categories/CompanyCodeCategories> ;
                        dct:created "2023-04-04"^^xsd:date ;
                        rdfs:comment """Category of a Railway company. Can be Infrastructure, Freight or Passenger.
The allowed values for this property belong to the SKOS concept scheme http://data.europa.eu/949/concepts/company-code-categories/CompanyCodeCategories"""@en ;
                        rdfs:isDefinedBy <http://data.europa.eu/949/> ;
                        rdfs:label "Company code category"@en ;
                        vs:term_status "stable" .


###  http://data.europa.eu/949/conditionsUseReflectivePlates
era:conditionsUseReflectivePlates rdf:type owl:ObjectProperty ;
                                  rdfs:domain [ rdf:type owl:Class ;
                                                owl:unionOf ( era:SubsetWithCommonCharacteristics
                                                              era:Track
                                                            )
                                              ] ;
                                  rdfs:range skos:Concept ;
                                  era:rinfIndex "1.1.1.1.7.12.1" ;
                                  dct:created "2023-03-14"^^xsd:date ;
                                  rdfs:comment """Details of any conditions for using the reflective plates on freight corridors. Specific case for Portugal and Spain until 1.1.2025 and Belgium and France until 1.1.2026.
The allowed values for this property belong to a SKOS Concept Scheme."""@en ;
                                  rdfs:isDefinedBy <http://data.europa.eu/949/> ;
                                  rdfs:label "Conditions for use of reflective plates"@en ;
                                  vs:term_status "unstable" .


###  http://data.europa.eu/949/contactLineSystem
era:contactLineSystem rdf:type owl:ObjectProperty ;
                      rdfs:domain [ rdf:type owl:Class ;
                                    owl:unionOf ( era:SubsetWithCommonCharacteristics
                                                  era:Track
                                                )
                                  ] ;
                      rdfs:range era:ContactLineSystem ;
                      dct:created "2020-08-24"^^xsd:date ;
                      dct:modified "2021-09-11"^^xsd:date ;
                      rdfs:comment "Contact line system present in the section of line."@en ;
                      rdfs:isDefinedBy <http://data.europa.eu/949/> ;
                      rdfs:label "Contact line system"@en ;
                      vs:term_status "stable" .


###  http://data.europa.eu/949/contactLineSystemType
era:contactLineSystemType rdf:type owl:ObjectProperty ;
                          rdfs:domain era:ContactLineSystem ;
                          rdfs:range skos:Concept ;
                          era:inSkosConceptScheme <http://data.europa.eu/949/concepts/contact-line-systems/ContactLineSystems> ;
                          era:rinfIndex "1.1.1.2.2.1.1" ;
                          era:usedInRCCCalculations "true"^^xsd:boolean ;
                          dct:created "2021-08-06"^^xsd:date ;
                          dct:modified "2021-08-06"^^xsd:date ;
                          rdfs:comment "Indication of the type of the contact line system. The allowed values for this property belong to the SKOS Concept Scheme http://data.europa.eu/949/concepts/contact-line-systems/ContactLineSystems"@en ;
                          rdfs:isDefinedBy <http://data.europa.eu/949/> ;
                          rdfs:label "Type of contact line system"@en ;
                          vs:term_status "stable" .


###  http://data.europa.eu/949/contactStripMaterial
era:contactStripMaterial rdf:type owl:ObjectProperty ;
                         rdfs:domain [ rdf:type owl:Class ;
                                       owl:unionOf ( era:SubsetWithCommonCharacteristics
                                                     era:Track
                                                     era:VehicleType
                                                   )
                                     ] ;
                         rdfs:range skos:Concept ;
                         era:eratvIndex "4.10.10" ;
                         era:inSkosConceptScheme <http://data.europa.eu/949/concepts/contact-strip-materials/ContactStripMaterials> ;
                         era:rinfIndex "1.1.1.2.3.4" ;
                         era:usedInRCCCalculations "true"^^xsd:boolean ;
                         dct:created "2020-08-25"^^xsd:date ;
                         dct:modified "2021-09-12"^^xsd:date ;
                         rdfs:comment "Indication of which contact strip materials are permitted to be used. The allowed values for this property belong to the SKOS Concept Scheme http://data.europa.eu/949/concepts/contact-strip-materials/ContactStripMaterials"@en ;
                         rdfs:isDefinedBy <http://data.europa.eu/949/> ;
                         rdfs:label "Permitted contact strip material"@en ;
                         vs:term_status "stable" .


###  http://data.europa.eu/949/dataGSMRNetwork
era:dataGSMRNetwork rdf:type owl:ObjectProperty ,
                             owl:FunctionalProperty ;
                    rdfs:domain era:VehicleType ;
                    rdfs:range skos:Concept ;
                    era:eratvIndex "4.13.2.11" ;
                    era:inSkosConceptScheme <http://data.europa.eu/949/concepts/gsmr-networks/GSMRNetworks> ;
                    dct:created "2020-08-31"^^xsd:date ;
                    dct:modified "2021-08-02"^^xsd:date ;
                    rdfs:comment "Data SIM Card GSM-R Home Network. The allowed values for this property belong to the SKOS Concept Scheme http://data.europa.eu/949/concepts/gsmr-networks/GSMRNetworks"@en ;
                    rdfs:isDefinedBy <http://data.europa.eu/949/> ;
                    rdfs:label "Data GSM-R network"@en ;
                    vs:term_status "stable" .


###  http://data.europa.eu/949/dataRadioCompatible
era:dataRadioCompatible rdf:type owl:ObjectProperty ;
                        rdfs:domain [ rdf:type owl:Class ;
                                      owl:unionOf ( era:SubsetWithCommonCharacteristics
                                                    era:Track
                                                    era:VehicleType
                                                  )
                                    ] ;
                        rdfs:range skos:Concept ;
                        era:eratvIndex "4.13.2.8" ;
                        era:inSkosConceptScheme <http://data.europa.eu/949/concepts/radio-system-compatibilities-data/RadioSystemCompatibilitiesData> ;
                        era:rinfIndex "1.1.1.3.3.10" ,
                                      "1.2.1.1.2.10" ;
                        dct:created "2020-08-31"^^xsd:date ;
                        dct:modified "2021-09-12"^^xsd:date ;
                        rdfs:comment """Radio requirements used for demonstrating technical compatibility data.
 The allowed values for this property belong to the SKOS Concept Scheme http://data.europa.eu/949/concepts/radio-system-compatibilities-data/RadioSystemCompatibilitiesData."""@en ;
                        rdfs:isDefinedBy <http://data.europa.eu/949/> ;
                        rdfs:label "Radio system compatibility data"@en ;
                        vs:term_status "stable" .


###  http://data.europa.eu/949/definesSubset
era:definesSubset rdf:type owl:ObjectProperty ;
                  rdfs:domain era:InfrastructureManager ;
                  rdfs:range era:SubsetWithCommonCharacteristics ;
                  dct:created "2022-11-04"^^xsd:date ;
                  dct:modified "2023-03-14"^^xsd:date ;
                  rdfs:comment "For the purposes of the register of infrastructure, each infrastructure manager may describe its railway network optionally via common characteristic subsets."@en ;
                  rdfs:isDefinedBy <http://data.europa.eu/949/> ;
                  rdfs:label "Defines subset"@en ;
                  vs:term_status "stable" .


###  http://data.europa.eu/949/eddyCurrentBraking
era:eddyCurrentBraking rdf:type owl:ObjectProperty ,
                                owl:FunctionalProperty ;
                       rdfs:domain [ rdf:type owl:Class ;
                                     owl:unionOf ( era:SubsetWithCommonCharacteristics
                                                   era:Track
                                                 )
                                   ] ;
                       rdfs:range skos:Concept ;
                       era:appendixD2Index "3.4.5" ;
                       era:inSkosConceptScheme <http://data.europa.eu/949/concepts/eddy-current-braking/EddyCurrentBraking> ;
                       era:rinfIndex "1.1.1.1.6.2" ,
                                     "1.2.1.0.4.2" ;
                       era:usedInRCCCalculations "true"^^xsd:boolean ;
                       dct:created "2020-08-24"^^xsd:date ;
                       dct:modified "2022-09-06"^^xsd:date ;
                       dct:source <https://eur-lex.europa.eu/eli/reg_impl/2019/773/oj> ;
                       rdfs:comment """Indication of limitations on the use of eddy current brakes. The allowed values for this property belong to the SKOS Concept Scheme http://data.europa.eu/949/concepts/eddy-current-braking/EddyCurrentBraking
This property has been modified to be a RINF parameter (its eratvIndex is deleted). It is treated as a SKOS by RINF and as a boolean by ERATV. A new ERATV datatype property has been defined, eddyCurrentBrakingFitted with boolean values.
In https://eur-lex.europa.eu/eli/reg_impl/2019/773/oj 3.4.5 Permissibility to use Eddy-current brake."""@en ;
                       rdfs:isDefinedBy <http://data.europa.eu/949/> ;
                       rdfs:label "Use of eddy current brakes"@en ;
                       vs:term_status "stable" .


###  http://data.europa.eu/949/elementA
era:elementA rdf:type owl:ObjectProperty ;
             rdfs:domain era:NetRelation ;
             rdfs:range era:NetElement ;
             era:rinfIndex "1.1.1.0.1.2" ,
                           "1.2.4.1" ;
             dct:created "2021-04-01"^^xsd:date ;
             dct:modified "2023-03-14"^^xsd:date ;
             rdfs:comment """References the first topological object in an oriented relation.
Indicates the object that corresponds to a section of line, an operational point or a track inside an operational point connected at start."""@en ;
             rdfs:isDefinedBy <http://data.europa.eu/949/> ;
             rdfs:label "Element A"@en ;
             rdfs:seeAlso <https://rsm-evolution.org/220927_RSM/EARoot/EA2/EA2/EA290.html> ;
             vs:term_status "stable" ;
             skos:altLabel "Internal connection"@en .


###  http://data.europa.eu/949/elementB
era:elementB rdf:type owl:ObjectProperty ;
             rdfs:domain era:NetRelation ;
             rdfs:range era:NetElement ;
             era:rinfIndex "1.1.1.0.1.2" ,
                           "1.2.4.1" ;
             dct:created "2021-04-01"^^xsd:date ;
             dct:modified "2023-03-14"^^xsd:date ;
             rdfs:comment """References the second topological object in an oriented relation.
Indicates the object that corresponds to a section of line, an operational point or a track inside an operational point connected at end."""@en ;
             rdfs:isDefinedBy <http://data.europa.eu/949/> ;
             rdfs:label "Element B"@en ;
             rdfs:seeAlso <https://rsm-evolution.org/220927_RSM/EARoot/EA2/EA2/EA290.html> ;
             vs:term_status "stable" ;
             skos:altLabel "Internal connection"@en .


###  http://data.europa.eu/949/elementPart
era:elementPart rdf:type owl:ObjectProperty ;
                rdfs:domain era:NetElement ;
                rdfs:range era:NetElement ;
                dct:created "2021-04-01"^^xsd:date ;
                dct:modified "2021-04-01"^^xsd:date ;
                rdfs:comment "References the topology object of a higher-granularity level which contains a lower-granularity topology object."@en ;
                rdfs:isDefinedBy <http://data.europa.eu/949/> ;
                rdfs:label "Element part"@en ;
                rdfs:seeAlso <https://rsm-evolution.org/220927_RSM/EARoot/EA2/EA2/EA284.html> ;
                vs:term_status "stable" .


###  http://data.europa.eu/949/endCouplingType
era:endCouplingType rdf:type owl:ObjectProperty ;
                    rdfs:domain era:VehicleType ;
                    rdfs:range skos:Concept ;
                    era:eratvIndex "4.9.1" ;
                    era:inSkosConceptScheme <http://data.europa.eu/949/concepts/end-coupling-type/EndCouplingType> ;
                    dct:created "2021-08-31"^^xsd:date ;
                    dct:modified "2021-08-31"^^xsd:date ;
                    rdfs:comment "Type of end coupling (indicating tensile and compressive forces). The allowed values for this property belong to the SKOS Concept Scheme http://data.europa.eu/949/concepts/end-coupling-type/EndCouplingType."@en ;
                    rdfs:isDefinedBy <http://data.europa.eu/949/> ;
                    rdfs:label "End coupling type"@en ;
                    vs:term_status "stable" .


###  http://data.europa.eu/949/endLocation
era:endLocation rdf:type owl:ObjectProperty ;
                rdfs:subPropertyOf gsp:hasGeometry ,
                                   wgs:location ;
                rdfs:domain era:Tunnel ;
                rdfs:range [ rdf:type owl:Class ;
                             owl:unionOf ( gsp:Geometry
                                           wgs:Point
                                         )
                           ] ;
                era:rinfIndex "1.1.1.1.8.4" ;
                dct:created "2020-07-29"^^xsd:date ;
                dct:modified "2021-08-11"^^xsd:date ;
                rdfs:comment "Geographical coordinates in decimal degrees and km of the line at the end of a tunnel."@en ;
                rdfs:isDefinedBy <http://data.europa.eu/949/> ;
                rdfs:label "End of tunnel"@en ;
                vs:term_status "stable" .


###  http://data.europa.eu/949/energySupplySystem
era:energySupplySystem rdf:type owl:ObjectProperty ;
                       rdfs:domain [ rdf:type owl:Class ;
                                     owl:unionOf ( era:ContactLineSystem
                                                   era:VehicleType
                                                 )
                                   ] ;
                       rdfs:range skos:Concept ;
                       era:appendixD2Index "3.3.1" ;
                       era:eratvIndex "4.10.1" ;
                       era:inSkosConceptScheme <http://data.europa.eu/949/concepts/energy-supply-systems/EnergySupplySystems> ;
                       era:rinfIndex "1.1.1.2.2.1.2" ;
                       era:usedInRCCCalculations "true"^^xsd:boolean ;
                       dct:created "2020-08-24"^^xsd:date ;
                       dct:modified "2021-08-06"^^xsd:date ;
                       dct:source <https://eur-lex.europa.eu/eli/reg_impl/2019/773/oj> ;
                       rdfs:comment """Indication of the traction supply system (nominal voltage and frequency). The allowed values for this property belong to the SKOS Concept Scheme http://data.europa.eu/949/concepts/energy-supply-systems/EnergySupplySystems
In https://eur-lex.europa.eu/eli/reg_impl/2019/773/oj 3.3.1 Energy supply system (voltage and frequency)."""@en ;
                       rdfs:isDefinedBy <http://data.europa.eu/949/> ;
                       rdfs:label "Energy supply system"@en ;
                       vs:term_status "stable" .


###  http://data.europa.eu/949/etcsBaseline
era:etcsBaseline rdf:type owl:ObjectProperty ;
                 rdfs:domain [ rdf:type owl:Class ;
                               owl:unionOf ( era:ETCSLevel
                                             era:VehicleType
                                           )
                             ] ;
                 rdfs:range skos:Concept ;
                 era:eratvIndex "4.13.1.2" ;
                 era:inSkosConceptScheme <http://data.europa.eu/949/concepts/etcs-baselines/ETCSBaselines> ;
                 era:rinfIndex "1.1.1.3.2.2" ,
                               "1.2.1.1.1.2" ;
                 dct:created "2021-08-07"^^xsd:date ;
                 dct:modified "2021-08-31"^^xsd:date ;
                 rdfs:comment "ETCS baseline installed lineside. The allowed values for this property belong to the SKOS Concept Scheme http://data.europa.eu/949/concepts/etcs-baselines/ETCSBaselines"@en ;
                 rdfs:isDefinedBy <http://data.europa.eu/949/> ;
                 rdfs:label "ETCS baseline"@en ;
                 vs:term_status "stable" .


###  http://data.europa.eu/949/etcsDegradedSituation
era:etcsDegradedSituation rdf:type owl:ObjectProperty ;
                          rdfs:domain [ rdf:type owl:Class ;
                                        owl:unionOf ( era:SubsetWithCommonCharacteristics
                                                      era:Track
                                                    )
                                      ] ;
                          rdfs:range skos:Concept ;
                          era:appendixD2Index "3.1.7" ;
                          era:inSkosConceptScheme <http://data.europa.eu/949/concepts/etcs-situation/ETCSSituations> ;
                          era:rinfIndex "1.1.1.3.10.1" ,
                                        "1.2.1.1.9.1" ;
                          dct:created "2021-08-09"^^xsd:date ;
                          dct:modified "2021-09-12"^^xsd:date ;
                          dct:source <https://eur-lex.europa.eu/eli/reg_impl/2019/773/oj> ;
                          rdfs:comment """ERTMS / ETCS application level for degraded situation related to the track side equipment. The allowed values for this property belong to the SKOS Concept Scheme http://data.europa.eu/949/concepts/etcs-situation/ETCSSituations
In https://eur-lex.europa.eu/eli/reg_impl/2019/773/oj 3.1.7 Means of Communication with the traffic management/control centre in normal, degraded and emergency situation."""@en ;
                          rdfs:isDefinedBy <http://data.europa.eu/949/> ;
                          rdfs:label "ETCS level for degraded situation"@en ;
                          vs:term_status "stable" .


###  http://data.europa.eu/949/etcsEquipmentOnBoardLevel
era:etcsEquipmentOnBoardLevel rdf:type owl:ObjectProperty ,
                                       owl:FunctionalProperty ;
                              rdfs:domain era:VehicleType ;
                              rdfs:range skos:Concept ;
                              era:eratvIndex "4.13.1.1" ;
                              era:inSkosConceptScheme <http://data.europa.eu/949/concepts/etcs-equipment-on-board-level/ETCSEquipmentLevels> ;
                              dct:created "2021-08-31"^^xsd:date ;
                              dct:modified "2021-08-31"^^xsd:date ;
                              rdfs:comment "ETCS equipment on-board and its level. The allowed values for this property belong to the SKOS Concept Scheme http://data.europa.eu/949/concepts/etcs-equipment-on-board-level/ETCSEquipmentLevels."@en ;
                              rdfs:isDefinedBy <http://data.europa.eu/949/> ;
                              rdfs:label "ETCS equipment level"@en ;
                              vs:term_status "stable" .


###  http://data.europa.eu/949/etcsInfill
era:etcsInfill rdf:type owl:ObjectProperty ,
                        owl:FunctionalProperty ;
               rdfs:domain [ rdf:type owl:Class ;
                             owl:unionOf ( era:SubsetWithCommonCharacteristics
                                           era:Track
                                           era:VehicleType
                                         )
                           ] ;
               rdfs:range skos:Concept ;
               era:eratvIndex "4.13.1.3" ;
               era:inSkosConceptScheme <http://data.europa.eu/949/concepts/etcs-infills/ETCSInfills> ;
               era:rinfIndex "1.1.1.3.2.4" ,
                             "1.2.1.1.1.4" ;
               dct:created "2021-08-08"^^xsd:date ;
               dct:modified "2021-09-12"^^xsd:date ;
               rdfs:comment "Information about installed trackside equipment capable to transmit infill information by loop or Global System for Mobile communications for Railways (GSM-R) for level 1 installations."@en ;
               rdfs:isDefinedBy <http://data.europa.eu/949/> ;
               rdfs:label "ETCS infill installed lineside"@en ;
               vs:term_status "stable" .


###  http://data.europa.eu/949/etcsLevel
era:etcsLevel rdf:type owl:ObjectProperty ;
              rdfs:domain [ rdf:type owl:Class ;
                            owl:unionOf ( era:SubsetWithCommonCharacteristics
                                          era:Track
                                        )
                          ] ;
              rdfs:range era:ETCSLevel ;
              era:rinfIndex "1.2.1.1.1.1" ;
              dct:created "2021-08-07"^^xsd:date ;
              dct:modified "2021-09-12"^^xsd:date ;
              rdfs:comment "ETCS application level related to the track side equipment. The allowed values for this property belong to the SKOS Concept Scheme http://data.europa.eu/949/concepts/etcs-levels/ETCSLevels"@en ;
              rdfs:isDefinedBy <http://data.europa.eu/949/> ;
              rdfs:label "Etcs level"@en ;
              vs:term_status "stable" .


###  http://data.europa.eu/949/etcsLevelType
era:etcsLevelType rdf:type owl:ObjectProperty ;
                  rdfs:domain era:ETCSLevel ;
                  rdfs:range skos:Concept ;
                  era:inSkosConceptScheme <http://data.europa.eu/949/concepts/etcs-levels/ETCSLevels> ;
                  era:rinfIndex "1.1.1.3.2.1" ,
                                "1.2.1.1.1.1" ;
                  dct:created "2021-08-07"^^xsd:date ;
                  dct:modified "2021-08-07"^^xsd:date ;
                  rdfs:comment "ETCS application level related to the track side equipment. The allowed values for this property belong to the SKOS Concept Scheme http://data.europa.eu/949/concepts/etcs-levels/ETCSLevels"@en ;
                  rdfs:isDefinedBy <http://data.europa.eu/949/> ;
                  rdfs:label "ETCS level type"@en ;
                  vs:term_status "stable" .


###  http://data.europa.eu/949/etcsMVersion
era:etcsMVersion rdf:type owl:ObjectProperty ,
                          owl:FunctionalProperty ;
                 rdfs:domain [ rdf:type owl:Class ;
                               owl:unionOf ( era:SubsetWithCommonCharacteristics
                                             era:Track
                                           )
                             ] ;
                 rdfs:range skos:Concept ;
                 era:inSkosConceptScheme <http://data.europa.eu/949/concepts/etcs-m-versions/ETCSMVersions> ;
                 era:rinfIndex "1.1.1.3.2.10" ,
                               "1.2.1.1.1.10" ;
                 era:usedInRCCCalculations "true"^^xsd:boolean ;
                 dct:created "2021-08-08"^^xsd:date ;
                 dct:modified "2021-09-12"^^xsd:date ;
                 rdfs:comment "ETCS M_version according to the specification referenced in Appendix A-1, index [C]. The allowed values for this property belong to the SKOS Concept Scheme http://data.europa.eu/949/concepts/etcs-m-versions/ETCSMVersions"@en ;
                 rdfs:isDefinedBy <http://data.europa.eu/949/> ;
                 rdfs:label "ETCS M_version"@en ;
                 vs:term_status "stable" .


###  http://data.europa.eu/949/etcsSystemCompatibility
era:etcsSystemCompatibility rdf:type owl:ObjectProperty ;
                            rdfs:domain [ rdf:type owl:Class ;
                                          owl:unionOf ( era:Track
                                                        era:VehicleType
                                                      )
                                        ] ;
                            rdfs:range skos:Concept ;
                            era:eratvIndex "4.13.1.8" ;
                            era:inSkosConceptScheme <http://data.europa.eu/949/concepts/etcs-system-compatibilities/ETCSSystemCompatibilities> ;
                            era:rinfIndex "1.1.1.3.2.9" ,
                                          "1.2.1.1.1.9" ;
                            era:usedInRCCCalculations "true"^^xsd:boolean ;
                            dct:created "2020-08-31"^^xsd:date ;
                            dct:modified "2021-09-12"^^xsd:date ;
                            rdfs:comment "ETCS requirements used for demonstrating technical compatibility. The allowed values for this property belong to the SKOS Concept Scheme http://data.europa.eu/949/concepts/etcs-system-compatibilities/ETCSSystemCompatibilities"@en ;
                            rdfs:isDefinedBy <http://data.europa.eu/949/> ;
                            rdfs:label "ETCS system compatibility"@en ;
                            vs:term_status "stable" .


###  http://data.europa.eu/949/etcsTransmittedTrackConditions
era:etcsTransmittedTrackConditions rdf:type owl:ObjectProperty ;
                                   rdfs:domain [ rdf:type owl:Class ;
                                                 owl:unionOf ( era:SubsetWithCommonCharacteristics
                                                               era:Track
                                                             )
                                               ] ;
                                   rdfs:range skos:Concept ;
                                   era:appendixD3Index "1.1" ;
                                   era:rinfIndex "1.1.1.3.2.12.1" ,
                                                 "1.2.1.1.1.12.1" ;
                                   dct:created "2022-11-16"^^xsd:date ;
                                   dct:modified "2023-03-14"^^xsd:date ;
                                   rdfs:comment """According to the specification referenced in Appendix A-1, index [C]. 
In https://www.era.europa.eu/sites/default/files/filesystem/ertms/ccs_tsi_annex_a_-_mandatory_specifications/set_of_specifications_3_etcs_b3_r2_gsm-r_b1/index004_-_subset-026_v360.zip
Chapter 5, section 5.18.1.1.
The allowed values for this property belong to a SKOS Concept Scheme."""@en ;
                                   rdfs:isDefinedBy <http://data.europa.eu/949/> ;
                                   rdfs:label "Track conditions which can be transmitted"@en ;
                                   vs:term_status "unstable" .


###  http://data.europa.eu/949/fireSafetyCategory
era:fireSafetyCategory rdf:type owl:ObjectProperty ,
                                owl:FunctionalProperty ;
                       rdfs:domain era:VehicleType ;
                       rdfs:range skos:Concept ;
                       era:eratvIndex "4.4.1" ;
                       era:inSkosConceptScheme <http://data.europa.eu/949/concepts/rolling-stock-fire/Categories> ;
                       dct:created "2020-08-29"^^xsd:date ;
                       dct:modified "2021-08-03"^^xsd:date ;
                       rdfs:comment "Fire safety category for tunnels. The allowed values for this property belong to the SKOS Concept Scheme http://data.europa.eu/949/concepts/rolling-stock-fire/Categories."@en ;
                       rdfs:isDefinedBy <http://data.europa.eu/949/> ;
                       rdfs:label "Fire safety category"@en ;
                       vs:term_status "stable" .


###  http://data.europa.eu/949/freightCorridor
era:freightCorridor rdf:type owl:ObjectProperty ;
                    rdfs:domain [ rdf:type owl:Class ;
                                  owl:unionOf ( era:SubsetWithCommonCharacteristics
                                                era:Track
                                              )
                                ] ;
                    rdfs:range skos:Concept ;
                    era:inSkosConceptScheme <http://data.europa.eu/949/concepts/freight-corridor/FreightCorridors> ;
                    era:rinfIndex "1.1.1.1.2.3" ,
                                  "1.2.1.0.2.3" ;
                    dct:created "2021-08-03"^^xsd:date ;
                    dct:modified "2023-03-14"^^xsd:date ;
                    rdfs:comment """Indication whether the line is designated to a Railway Freight Corridor. 
The allowed values for this property belong to the SKOS Concept Scheme http://data.europa.eu/949/concepts/freight-corridor/FreightCorridors"""@en ;
                    rdfs:isDefinedBy <http://data.europa.eu/949/> ;
                    rdfs:label "Part of a Railway freight corridor"@en ;
                    vs:term_status "stable" .


###  http://data.europa.eu/949/frenchTrainDetectionSystemLimitation
era:frenchTrainDetectionSystemLimitation rdf:type owl:ObjectProperty ;
                                         rdfs:domain era:TrainDetectionSystem ;
                                         rdfs:range skos:Concept ;
                                         era:inSkosConceptScheme <http://data.europa.eu/949/concepts/train-detection/FrenchTrainDetectionSystemLimitations> ;
                                         era:rinfIndex "1.1.1.3.7.1.4" ,
                                                       "1.2.1.1.6.3" ;
                                         dct:created "2020-08-24"^^xsd:date ;
                                         dct:isReplacedBy era:frenchTrainDetectionSystemLimitationApplicable ,
                                                          era:frenchTrainDetectionSystemLimitationNumber ,
                                                          era:tdsFrenchTrainDetectionSystemLimitation ;
                                         dct:modified "2022-04-05"^^xsd:date ;
                                         rdfs:comment """Specific for route compatibility check on French network. The allowed values for this property belong to the SKOS Concept Scheme http://data.europa.eu/949/concepts/train-detection/FrenchTrainDetectionSystemLimitations.
Deprecated because of replacement by a class, an object property and two datatype properties. The reason is that the property is composed of two values: A boolean [Y/N] and  a number N is between 1 and 8."""@en ;
                                         rdfs:isDefinedBy <http://data.europa.eu/949/> ;
                                         rdfs:label "Section with train detection limitation, only for the French network"@en ;
                                         owl:deprecated "true"^^xsd:boolean ;
                                         vs:term_status "stable" .


###  http://data.europa.eu/949/frenchTrainDetectionSystemLimitationNumber
era:frenchTrainDetectionSystemLimitationNumber rdf:type owl:ObjectProperty ;
                                               rdfs:domain era:FrenchTrainDetectionSystemLimitation ;
                                               rdfs:range skos:Concept ;
                                               era:inSkosConceptScheme <http://data.europa.eu/949/concepts/train-detection-numbers/FrenchTrainDetectionSystemLimitationNumbers> ;
                                               era:rinfIndex "1.1.1.3.7.1.4" ;
                                               era:usedInRCCCalculations "true"^^xsd:boolean ;
                                               dct:created "2023-04-05"^^xsd:date ;
                                               rdfs:comment """Part of the section with train detection limitation that indicates the type of train detection limitation.
The allowed values for this property belong to the SKOS Concept Scheme http://data.europa.eu/949/concepts/train-detection-numbers/FrenchTrainDetectionSystemLimitationNumbers."""@en ;
                                               rdfs:isDefinedBy <http://data.europa.eu/949/> ;
                                               rdfs:label "Section with train detection limitation number, only for French  network"@en ;
                                               vs:term_status "stable" .


###  http://data.europa.eu/949/frequencyBandsForDetection
era:frequencyBandsForDetection rdf:type owl:ObjectProperty ;
                               rdfs:domain era:TrainDetectionSystem ;
                               rdfs:range skos:Concept ;
                               era:rinfIndex "1.1.1.3.4.2" ,
                                             "1.2.1.1.3.2" ;
                               dct:created "2023-03-14"^^xsd:date ;
                               rdfs:comment """Bands of the frequency management of the train detection systems as defined in the specification referenced in Appendix A-1, index [D], and in the specific cases or technical documents referred to in Article 13 of TSI CCS when they are available.
The allowed values for this property belong to a SKOS Concept Scheme."""@en ;
                               rdfs:isDefinedBy <http://data.europa.eu/949/> ;
                               rdfs:label "Frequency bands for detection"@en ;
                               vs:term_status "unstable" .


###  http://data.europa.eu/949/gaugingProfile
era:gaugingProfile rdf:type owl:ObjectProperty ;
                   rdfs:domain [ rdf:type owl:Class ;
                                 owl:unionOf ( era:SubsetWithCommonCharacteristics
                                               era:Track
                                               era:VehicleType
                                             )
                               ] ;
                   rdfs:range skos:Concept ;
                   era:eratvIndex "4.2.1" ;
                   era:inSkosConceptScheme <http://data.europa.eu/949/concepts/gaugings/GaugingProfiles> ;
                   era:rinfIndex "1.1.1.1.3.1.1" ,
                                 "1.2.1.0.3.4" ;
                   era:usedInRCCCalculations "true"^^xsd:boolean ;
                   dct:created "2020-07-29"^^xsd:date ;
                   dct:modified "2023-03-14"^^xsd:date ;
                   rdfs:comment """Gauges as defined in European standard or other local gauges, including lower or upper part.
In accordance with point 7.3.2.2 of LOC&PAS TSI, sections of lines of the United Kingdom of Great Britain network may not have gauge reference profile.
The allowed values for this property belong to the SKOS Concept Scheme http://data.europa.eu/949/concepts/gaugings/GaugingProfiles"""@en ;
                   rdfs:isDefinedBy <http://data.europa.eu/949/> ;
                   rdfs:label "Gauging"@en ;
                   vs:term_status "stable" .


###  http://data.europa.eu/949/gsmRActiveMobiles
era:gsmRActiveMobiles rdf:type owl:ObjectProperty ,
                               owl:FunctionalProperty ;
                      rdfs:domain [ rdf:type owl:Class ;
                                    owl:unionOf ( era:SubsetWithCommonCharacteristics
                                                  era:Track
                                                )
                                  ] ;
                      rdfs:range skos:Concept ;
                      era:inSkosConceptScheme <http://data.europa.eu/949/concepts/gsmr-number-active-mobiles/NumberActiveMobiles> ;
                      era:rinfIndex "1.1.1.3.3.2" ,
                                    "1.2.1.1.2.2" ;
                      dct:created "2021-08-08"^^xsd:date ;
                      dct:modified "2021-09-12"^^xsd:date ;
                      rdfs:comment """Number of simultaneous communication session on board for ETCS level R required for a smooth running of the train. This relates to the radio block centre (RBC) handling of communication sessions. Not safety critical and no matter of interoperability.
The allowed values for this property belong to the SKOS Concept Scheme http://data.europa.eu/949/concepts/gsmr-number-active-mobiles/NumberActiveMobiles"""@en ;
                      rdfs:isDefinedBy <http://data.europa.eu/949/> ;
                      rdfs:label "Number of active GSM-R mobiles (EDOR) or simultaneous communication session on-board for ETCS Level 2 (or level 3) needed to perform radio block centre handovers without having an operational disruption"@en ;
                      vs:term_status "stable" .


###  http://data.europa.eu/949/gsmROptionalFunctions
era:gsmROptionalFunctions rdf:type owl:ObjectProperty ;
                          rdfs:domain [ rdf:type owl:Class ;
                                        owl:unionOf ( era:SubsetWithCommonCharacteristics
                                                      era:Track
                                                    )
                                      ] ;
                          rdfs:range skos:Concept ;
                          era:inSkosConceptScheme <http://data.europa.eu/949/concepts/gsmr-optional-functions/OptionalFunctions> ;
                          era:rinfIndex "1.1.1.3.3.3" ,
                                        "1.2.1.1.2.3" ;
                          dct:created "2021-08-08"^^xsd:date ;
                          dct:modified "2021-09-12"^^xsd:date ;
                          rdfs:comment "Use of optional GSM-R functions which might improve operation on the line. They are for information only and not for network access criteria. The allowed values for this property belong to the SKOS Concept Scheme http://data.europa.eu/949/concepts/gsmr-optional-functions/OptionalFunctions"@en ;
                          rdfs:isDefinedBy <http://data.europa.eu/949/> ;
                          rdfs:label "Optional GSM-R functions"@en ;
                          vs:term_status "stable" .


###  http://data.europa.eu/949/gsmRRadioDataCommunication
era:gsmRRadioDataCommunication rdf:type owl:ObjectProperty ,
                                        owl:FunctionalProperty ;
                               rdfs:domain era:VehicleType ;
                               rdfs:range skos:Concept ;
                               era:eratvIndex "4.13.2.7" ;
                               era:inSkosConceptScheme <http://data.europa.eu/949/concepts/gsm-r-radio-data-communication/GSMRRadioDataCommunications> ;
                               dct:created "2021-08-31"^^xsd:date ;
                               dct:modified "2021-08-31"^^xsd:date ;
                               rdfs:comment "GSM-R Radio Data communication on board and its Baseline. The allowed values for this property belong to the SKOS Concept Scheme http://data.europa.eu/949/concepts/gsm-r-radio-data-communication/GSMRRadioDataCommunications."@en ;
                               rdfs:isDefinedBy <http://data.europa.eu/949/> ;
                               rdfs:label "GSM-R radio data communication"@en ;
                               vs:term_status "stable" .


###  http://data.europa.eu/949/gsmRVersion
era:gsmRVersion rdf:type owl:ObjectProperty ,
                         owl:FunctionalProperty ;
                rdfs:domain [ rdf:type owl:Class ;
                              owl:unionOf ( era:SubsetWithCommonCharacteristics
                                            era:Track
                                            era:VehicleType
                                          )
                            ] ;
                rdfs:range skos:Concept ;
                era:eratvIndex "4.13.2.1" ;
                era:inSkosConceptScheme <http://data.europa.eu/949/concepts/gsmr-versions/GSMRVersions> ;
                era:rinfIndex "1.1.1.3.3.1" ,
                              "1.2.1.1.2.1" ;
                dct:created "2021-08-08"^^xsd:date ;
                dct:modified "2021-09-12"^^xsd:date ;
                rdfs:comment "GSM-R functional requirements specification and system requirements specification in accordance with the specification respectively referenced in Appendix A-1, index [E] and index [F], version number installed lineside. The allowed values for this property belong to the SKOS Concept Scheme http://data.europa.eu/949/concepts/gsmr-versions/GSMRVersions"@en ;
                rdfs:isDefinedBy <http://data.europa.eu/949/> ;
                rdfs:label "GSM-R version"@en ;
                vs:term_status "stable" .


###  http://data.europa.eu/949/gsmrConstraintsOperateOnlyInCircuitSwitch
era:gsmrConstraintsOperateOnlyInCircuitSwitch rdf:type owl:ObjectProperty ;
                                              rdfs:domain [ rdf:type owl:Class ;
                                                            owl:unionOf ( era:SubsetWithCommonCharacteristics
                                                                          era:Track
                                                                        )
                                                          ] ;
                                              rdfs:range skos:Concept ;
                                              era:appendixD3Index "2.2" ;
                                              era:rinfIndex "1.2.1.1.2.12" ;
                                              dct:created "2023-03-14"^^xsd:date ;
                                              rdfs:comment """These constraints, where applicable, are meant to manage the limited number of circuit-switched radio connections that can be handled simultaneously by a Radio Block Center.
The allowed values for this property are taken from a SKOS concept scheme."""@en ;
                                              rdfs:isDefinedBy <http://data.europa.eu/949/> ;
                                              rdfs:label "Specific constraints imposed by the GSM-R network operator on ETCS on-board units only able to operate in circuit-switch"@en ;
                                              vs:term_status "stable" .


###  http://data.europa.eu/949/gsmrNetworkCoverage
era:gsmrNetworkCoverage rdf:type owl:ObjectProperty ;
                        rdfs:domain [ rdf:type owl:Class ;
                                      owl:unionOf ( era:SubsetWithCommonCharacteristics
                                                    era:Track
                                                  )
                                    ] ;
                        rdfs:range skos:Concept ;
                        era:inSkosConceptScheme <http://data.europa.eu/949/concepts/gsmr-networks/GSMRNetworks> ;
                        era:rinfIndex "1.1.1.3.3.5" ,
                                      "1.2.1.1.2.5" ;
                        era:usedInRCCCalculations "true"^^xsd:boolean ;
                        dct:created "2020-08-31"^^xsd:date ;
                        dct:modified "2021-09-12"^^xsd:date ;
                        rdfs:comment "List of GSM-R networks which are covered by a roaming agreement. The allowed values for this property belong to the SKOS Concept Scheme http://data.europa.eu/949/concepts/gsmr-networks/GSMRNetworks"@en ;
                        rdfs:isDefinedBy <http://data.europa.eu/949/> ;
                        rdfs:label "GSM-R networks covered by a roaming agreement"@en ;
                        vs:term_status "stable" .


###  http://data.europa.eu/949/hasAbstraction
era:hasAbstraction rdf:type owl:ObjectProperty ;
                   owl:inverseOf era:hasImplementation ;
                   rdfs:domain era:InfrastructureObject ;
                   rdfs:range era:NetElement ;
                   dct:created "2020-07-29"^^xsd:date ;
                   dct:modified "2022-10-27"^^xsd:date ;
                   rdfs:comment "Property that links a physical entity with its topological abstraction representation."@en ;
                   rdfs:isDefinedBy <http://data.europa.eu/949/> ;
                   rdfs:label "Has abstraction"@en ;
                   vs:term_status "stable" .


###  http://data.europa.eu/949/hasImplementation
era:hasImplementation rdf:type owl:ObjectProperty ;
                      rdfs:domain era:NetElement ;
                      rdfs:range era:InfrastructureObject ;
                      dct:created "2020-07-29"^^xsd:date ;
                      dct:modified "2022-10-27"^^xsd:date ;
                      rdfs:comment "Property that links a topological abstraction entity with its physical representation."@en ;
                      rdfs:isDefinedBy <http://data.europa.eu/949/> ;
                      rdfs:label "Has implementation"@en ;
                      vs:term_status "stable" .


###  http://data.europa.eu/949/hasSignal
era:hasSignal rdf:type owl:ObjectProperty ;
              rdfs:domain era:NetElement ;
              rdfs:range era:Signal ;
              dct:created "2021-04-01"^^xsd:date ;
              dct:modified "2022-11-15"^^xsd:date ;
              rdfs:comment "References a signal associated with a topology object."@en ,
                           "The reason for deprecation is that it is a property of era:netElement and signals are not part of the topological layer but of the physical layer."@en ;
              rdfs:isDefinedBy <http://data.europa.eu/949/> ;
              rdfs:label "Has signal"@en ;
              owl:deprecated "true"^^xsd:boolean ;
              vs:term_status "stable" .


###  http://data.europa.eu/949/hotAxleBoxDetectorDirection
era:hotAxleBoxDetectorDirection rdf:type owl:ObjectProperty ;
                                rdfs:subPropertyOf owl:topObjectProperty ;
                                rdfs:domain [ rdf:type owl:Class ;
                                              owl:unionOf ( era:SubsetWithCommonCharacteristics
                                                            era:Track
                                                          )
                                            ] ;
                                rdfs:range skos:Concept ;
                                era:inSkosConceptScheme <http://data.europa.eu/949/concepts/hot-axle/HotAxleBoxDetectorDirections> ;
                                era:rinfIndex "1.1.1.1.7.9" ;
                                era:usedInRCCCalculations "true"^^xsd:boolean ;
                                dct:created "2022-07-08"^^xsd:date ;
                                rdfs:comment """Specific for the French Italian and Swedish networks.
Applicable if trackside HABD is not TSI compliant, direction of measurement of trackside Hot Axle Box Detector.
If the direction of measurement is:
â	the same as the direction defined by the start and end of the SoL: (N)
â	the opposite to the direction defined by the start and end of the SoL: (O)
â	both directions: (B).
This property was previously a datatype property with domain Track and range string. As its values are a list of three predefined values, it is now a SKOS. The allowed values for this property belong to the SKOS Concept Scheme http://data.europa.eu/949/concepts/hot-axle/HotAxleBoxDetectorDirections"""@en ;
                                rdfs:isDefinedBy <http://data.europa.eu/949/> ;
                                rdfs:label "Hot axle box detector direction"@en ;
                                vs:term_status "stable" .


###  http://data.europa.eu/949/inCountry
era:inCountry rdf:type owl:ObjectProperty ;
              rdfs:domain era:InfrastructureObject ;
              rdfs:range skos:Concept ;
              era:inSkosConceptScheme <http://publications.europa.eu/resource/authority/country> ;
              dct:created "2020-09-01"^^xsd:date ;
              dct:modified "2020-11-20"^^xsd:date ;
              rdfs:comment "Indicates the country in which an entity resides. The allowed values for this property belong to the SKOS Concept Scheme http://publications.europa.eu/resource/authority/country"@en ;
              rdfs:isDefinedBy <http://data.europa.eu/949/> ;
              rdfs:label "In country"@en ;
              vs:term_status "stable" .


###  http://data.europa.eu/949/infrastructureMgr
era:infrastructureMgr rdf:type owl:ObjectProperty ;
                      rdfs:domain era:InfrastructureObject ;
                      rdfs:range era:InfrastructureManager ;
                      dct:created "2022-07-07"^^xsd:date ;
                      rdfs:comment "Relates any feature implemented in the European railway infrastructure with its infrastructure manager."@en ;
                      rdfs:isDefinedBy <http://data.europa.eu/949/> ;
                      rdfs:label "Infrastructure manager"@en ;
                      vs:term_status "stable" .


###  http://data.europa.eu/949/legacyRadioSystem
era:legacyRadioSystem rdf:type owl:ObjectProperty ;
                      rdfs:domain [ rdf:type owl:Class ;
                                    owl:unionOf ( era:SubsetWithCommonCharacteristics
                                                  era:Track
                                                  era:VehicleType
                                                )
                                  ] ;
                      rdfs:range skos:Concept ;
                      era:appendixD2Index "3.2.8" ;
                      era:eratvIndex "4.13.2.3" ;
                      era:inSkosConceptScheme <http://data.europa.eu/949/concepts/legacy-radio-systems/LegacyRadioSystems> ;
                      era:rinfIndex "1.1.1.3.6.1" ,
                                    "1.2.1.1.5.1" ;
                      era:usedInRCCCalculations "true"^^xsd:boolean ;
                      dct:created "2020-08-31"^^xsd:date ;
                      dct:modified "2021-09-12"^^xsd:date ;
                      dct:source <https://eur-lex.europa.eu/eli/reg_impl/2019/773/oj> ;
                      rdfs:comment """Indication of radio legacy systems installed. The allowed values for this property belong to the SKOS Concept Scheme http://data.europa.eu/949/concepts/legacy-radio-systems/LegacyRadioSystems
In https://eur-lex.europa.eu/eli/reg_impl/2019/773/oj 3.2.8 Type of track to train radio equipment."""@en ;
                      rdfs:isDefinedBy <http://data.europa.eu/949/> ;
                      rdfs:label "Other radio systems installed (Radio Legacy Systems)"@en ;
                      vs:term_status "stable" .


###  http://data.europa.eu/949/lineCategory
era:lineCategory rdf:type owl:ObjectProperty ;
                 rdfs:domain [ rdf:type owl:Class ;
                               owl:unionOf ( era:SubsetWithCommonCharacteristics
                                             era:Track
                                           )
                             ] ;
                 rdfs:range skos:Concept ;
                 era:inSkosConceptScheme <http://data.europa.eu/949/concepts/line-category/LineCategories> ;
                 era:rinfIndex "1.1.1.1.2.2" ,
                               "1.2.1.0.2.2" ;
                 dct:created "2021-08-02"^^xsd:date ;
                 dct:modified "2023-03-14"^^xsd:date ;
                 rdfs:comment """Classification of a line according to the INF TSI. â Commission Regulation (EU) No 1299/2014. 
In https://eur-lex.europa.eu/legal-content/EN/TXT/HTML/?uri=CELEX:32019R0777&from=EN#ntr3-LI2019139EN.01031601-E0003
The allowed values for this property belong to the SKOS Concept Scheme http://data.europa.eu/949/concepts/line-category/LineCategories"""@en ;
                 rdfs:isDefinedBy <http://data.europa.eu/949/> ;
                 rdfs:label "Category of line"@en ;
                 vs:term_status "stable" .


###  http://data.europa.eu/949/lineNationalId
era:lineNationalId rdf:type owl:ObjectProperty ,
                            owl:FunctionalProperty ;
                   rdfs:domain [ rdf:type owl:Class ;
                                 owl:unionOf ( era:LineReference
                                               era:SectionOfLine
                                             )
                               ] ;
                   rdfs:range era:NationalRailwayLine ;
                   era:appendixD2Index "2.2.1.1" ;
                   era:rinfIndex "1.1.0.0.0.2" ;
                   dct:created "2020-09-30"^^xsd:date ;
                   dct:modified "2023-03-14"^^xsd:date ;
                   rdfs:comment "Unique line identification or unique line number within Member State."@en ;
                   rdfs:isDefinedBy <http://data.europa.eu/949/> ;
                   rdfs:label "National line identification"@en ;
                   vs:term_status "stable" .


###  http://data.europa.eu/949/lineReference
era:lineReference rdf:type owl:ObjectProperty ;
                  rdfs:domain era:InfrastructureObject ;
                  rdfs:range era:LineReference ;
                  dct:created "2021-01-29"^^xsd:date ;
                  dct:modified "2023-03-14"^^xsd:date ;
                  rdfs:comment "Indicates a relationship with a national railway line at a specific kilometer point."@en ;
                  rdfs:isDefinedBy <http://data.europa.eu/949/> ;
                  rdfs:label "Railway location of Operational point"@en ;
                  vs:term_status "stable" .


###  http://data.europa.eu/949/linesideDistanceIndicationAppearance
era:linesideDistanceIndicationAppearance rdf:type owl:ObjectProperty ;
                                         rdfs:domain [ rdf:type owl:Class ;
                                                       owl:unionOf ( era:SubsetWithCommonCharacteristics
                                                                     era:Track
                                                                   )
                                                     ] ;
                                         rdfs:range skos:Concept ;
                                         era:appendixD2Index "3.1.3" ;
                                         era:rinfIndex "1.1.1.0.0.3" ;
                                         dct:created "2022-10-27"^^xsd:date ;
                                         dct:modified "2023-03-14"^^xsd:date ;
                                         dct:source <https://eur-lex.europa.eu/eli/reg_impl/2019/773/oj> ;
                                         rdfs:comment """Indication of types of appearance of track lineside distance indications. 
The allowed values for this property are taken from a SKOS concept scheme.
In https://eur-lex.europa.eu/eli/reg_impl/2019/773/oj 3.1.3 Lineside indications of distance (frequency, appearance and positioning)."""@en ;
                                         rdfs:isDefinedBy <http://data.europa.eu/949/> ;
                                         rdfs:label "Lineside distance indication appearance"@en ;
                                         vs:term_status "unstable" .


###  http://data.europa.eu/949/linesideDistanceIndicationPositioning
era:linesideDistanceIndicationPositioning rdf:type owl:ObjectProperty ;
                                          rdfs:subPropertyOf owl:topObjectProperty ;
                                          rdfs:domain [ rdf:type owl:Class ;
                                                        owl:unionOf ( era:SubsetWithCommonCharacteristics
                                                                      era:Track
                                                                    )
                                                      ] ;
                                          rdfs:range skos:Concept ;
                                          era:appendixD2Index "3.1.3" ;
                                          era:rinfIndex "1.1.1.0.0.3" ;
                                          dct:created "2023-03-14"^^xsd:date ;
                                          dct:source <https://eur-lex.europa.eu/eli/reg_impl/2019/773/oj> ;
                                          rdfs:comment """Indication of the side along the track where the lineside indication is positioned (left or right).
The allowed values for this property are taken from a SKOS concept scheme.
In https://eur-lex.europa.eu/eli/reg_impl/2019/773/oj 3.1.3 Lineside indications of distance (frequency, appearance and positioning)."""@en ;
                                          rdfs:isDefinedBy <http://data.europa.eu/949/> ;
                                          rdfs:label "Lineside distance indication positioning"@en ;
                                          vs:term_status "unstable" .


###  http://data.europa.eu/949/loadCapability
era:loadCapability rdf:type owl:ObjectProperty ;
                   rdfs:domain [ rdf:type owl:Class ;
                                 owl:unionOf ( era:SubsetWithCommonCharacteristics
                                               era:Track
                                             )
                               ] ;
                   rdfs:range skos:Concept ;
                   era:inSkosConceptScheme <http://data.europa.eu/949/concepts/load-capabilities/LoadCapabilities> ;
                   era:rinfIndex "1.1.1.1.2.4" ;
                   dct:created "2020-08-24"^^xsd:date ;
                   dct:isReplacedBy era:LoadCapability ,
                                    era:loadCapabilityLineCategory ,
                                    era:loadCapabilitySpeed ,
                                    era:trackLoadCapability ;
                   dct:modified "2023-01-20"^^xsd:date ;
                   rdfs:comment "A combination of the line category and speed at the weakest point of the track. The allowed values for this property belong to the SKOS Concept Scheme http://data.europa.eu/949/concepts/load-capabilities/LoadCapabilities. The reason for deprecation is that the load capability property 1.1.1.1.2.4 was defined incorrectly as a SKOS property. It is composed of two values: (1)  line category, and (2) speed. Only line category is a list of predefined values (SKOS), whereas speed is an integer (according to the RINF application guide)."@en ;
                   rdfs:isDefinedBy <http://data.europa.eu/949/> ;
                   rdfs:label "Load Capability"@en ;
                   owl:deprecated "true"^^xsd:boolean ;
                   vs:term_status "stable" .


###  http://data.europa.eu/949/loadCapabilityLineCategory
era:loadCapabilityLineCategory rdf:type owl:ObjectProperty ;
                               rdfs:domain era:LoadCapability ;
                               rdfs:range skos:Concept ;
                               era:inSkosConceptScheme <http://data.europa.eu/949/concepts/load-capability-line-categories/LoadCapabilityLineCategories> ;
                               era:rinfIndex "1.1.1.1.2.4" ;
                               era:usedInRCCCalculations "true"^^xsd:boolean ;
                               dct:created "2023-01-20"^^xsd:date ;
                               rdfs:comment """Part of the load capability of a track that corresponds to the line category of the load model. 
The load capability is a value selected from the list of load models representing: line category which is amended by value of speed [km/h] permitted for a specific load model. The list of values may also be Route Availability which is amended by value of speed [miles/h] permitted for a specific load model.
The allowed values for this property belong to the SKOS Concept Scheme http://data.europa.eu/949/concepts/load-capability-line-categories/LoadCapabilityLineCategories"""@en ;
                               rdfs:isDefinedBy <http://data.europa.eu/949/> ;
                               rdfs:label "Load capability line category"@en ;
                               vs:term_status "stable" .


###  http://data.europa.eu/949/mNvcontact
era:mNvcontact rdf:type owl:ObjectProperty ;
               rdfs:domain [ rdf:type owl:Class ;
                             owl:unionOf ( era:SubsetWithCommonCharacteristics
                                           era:Track
                                         )
                           ] ;
               rdfs:range skos:Concept ;
               era:appendixD3Index "1.5.9" ;
               era:rinfIndex "1.1.1.3.2.16.9" ,
                             "1.2.1.1.1.16.9Â " ;
               dct:created "2022-11-07"^^xsd:date ;
               dct:modified "2023-03-14"^^xsd:date ;
               rdfs:comment """On-Board system reaction when T_NVCONTACT expires.  
According to the specification referenced in Appendix A-1, index [C]. 
In https://www.era.europa.eu/sites/default/files/filesystem/ertms/ccs_tsi_annex_a_-_mandatory_specifications/set_of_specifications_3_etcs_b3_r2_gsm-r_b1/index004_-_subset-026_v360.zip
 Subset 26, chapter 7. 7.5.1.74 M_NVCONTACT.
The allowed values for this concept belong to a SKOS concept scheme."""@en ;
               rdfs:isDefinedBy <http://data.europa.eu/949/> ;
               rdfs:label "M_NVCONTACT"@en ;
               vs:term_status "unstable" .


###  http://data.europa.eu/949/magneticBraking
era:magneticBraking rdf:type owl:ObjectProperty ,
                             owl:FunctionalProperty ;
                    rdfs:domain [ rdf:type owl:Class ;
                                  owl:unionOf ( era:SubsetWithCommonCharacteristics
                                                era:Track
                                              )
                                ] ;
                    rdfs:range skos:Concept ;
                    era:appendixD2Index "3.4.6" ;
                    era:inSkosConceptScheme <http://data.europa.eu/949/concepts/magnetic-braking/MagneticBraking> ;
                    era:rinfIndex "1.1.1.1.6.3" ,
                                  "1.2.1.0.4.3" ;
                    era:usedInRCCCalculations "true"^^xsd:boolean ;
                    dct:created "2020-08-24"^^xsd:date ;
                    dct:modified "2022-09-12"^^xsd:date ;
                    dct:source <https://eur-lex.europa.eu/eli/reg_impl/2019/773/oj> ;
                    rdfs:comment """Indication of limitations on the use of magnetic brakes. The allowed values for this property belong to the SKOS Concept Scheme http://data.europa.eu/949/concepts/magnetic-braking/MagneticBraking.
This property has been modified to be a RINF parameter (its eratvIndex is deleted). It is treated as a SKOS by RINF and as a boolean by ERATV. A new ERATV datatype property has been defined, magneticBrakingFitted with boolean values.
In 3.4.6 https://eur-lex.europa.eu/eli/reg_impl/2019/773/oj Permissibility to use magnetic brake."""@en ;
                    rdfs:isDefinedBy <http://data.europa.eu/949/> ;
                    rdfs:label "Use of magnetic brakes"@en ;
                    vs:term_status "stable" .


###  http://data.europa.eu/949/manufacturer
era:manufacturer rdf:type owl:ObjectProperty ;
                 rdfs:domain era:VehicleType ;
                 rdfs:range era:Manufacturer ;
                 dct:created "2020-07-29"^^xsd:date ;
                 dct:modified "2020-11-19"^^xsd:date ;
                 rdfs:comment "Vehicle manufacturer company."@en ;
                 rdfs:isDefinedBy <http://data.europa.eu/949/> ;
                 rdfs:label "Manufacturer"@en ;
                 vs:term_status "stable" .


###  http://data.europa.eu/949/manufacturingCountry
era:manufacturingCountry rdf:type owl:ObjectProperty ;
                         rdfs:domain [ rdf:type owl:Class ;
                                       owl:unionOf ( era:Vehicle
                                                     era:VehicleType
                                                   )
                                     ] ;
                         rdfs:range skos:Concept ;
                         era:inSkosConceptScheme <http://publications.europa.eu/resource/authority/country> ;
                         dct:created "2020-09-30"^^xsd:date ;
                         dct:modified "2020-11-22"^^xsd:date ;
                         rdfs:comment "Indicates the country in which a vehicle or vehicle type is manufactured. The allowed values for this property belong to the SKOS Concept Scheme http://publications.europa.eu/resource/authority/country"@en ;
                         rdfs:isDefinedBy <http://data.europa.eu/949/> ;
                         rdfs:label "Manufacturing country"@en ;
                         vs:term_status "stable" .


###  http://data.europa.eu/949/maxSandingOutput
era:maxSandingOutput rdf:type owl:ObjectProperty ;
                     rdfs:domain era:TrainDetectionSystem ;
                     rdfs:range skos:Concept ;
                     era:inSkosConceptScheme <http://data.europa.eu/949/concepts/max-amount-sandings/MaxAmountSandings> ;
                     era:rinfIndex "1.1.1.3.7.17" ;
                     dct:created "2021-08-08"^^xsd:date ;
                     dct:modified "2023-03-14"^^xsd:date ;
                     rdfs:comment "Deprecated according to the ammendment to the Regulation (EU) 2019/777. Maximum amount of sand accepted on the track within value of sanding output for 30s, given in grams. The allowed values for this property belong to the SKOS Concept Scheme http://data.europa.eu/949/concepts/max-amount-sandings/MaxAmountSandings"@en ;
                     rdfs:isDefinedBy <http://data.europa.eu/949/> ;
                     rdfs:label "Maximum amount of sand"@en ;
                     owl:deprecated "true"^^xsd:boolean ;
                     vs:term_status "stable" .


###  http://data.europa.eu/949/minAxleLoadVehicleCategory
era:minAxleLoadVehicleCategory rdf:type owl:ObjectProperty ;
                               rdfs:domain era:MinAxleLoadVehicleCategory ;
                               rdfs:range skos:Concept ;
                               era:inSkosConceptScheme <http://data.europa.eu/949/concepts/min-axle-load-vehicle-categories/MinAxleLoadVehicleCategories> ;
                               era:rinfIndex "1.1.1.3.7.11.1" ;
                               dct:created "2021-08-08"^^xsd:date ;
                               dct:modified "2023-03-14"^^xsd:date ;
                               rdfs:comment "Deprecated according to the ammendment to the Regulation (EU) 2019/777. Represents the category of vehicle which is amended by value of minimum permitted axle load [tons] (property minAxleLoad). The allowed values for this property belong to the SKOS Concept Scheme http://data.europa.eu/949/concepts/min-axle-load-vehicle-categories/MinAxleLoadVehicleCategories."@en ;
                               rdfs:isDefinedBy <http://data.europa.eu/949/> ;
                               rdfs:label "Minimum axle load vehicle category"@en ;
                               owl:deprecated "true"^^xsd:boolean ;
                               vs:term_status "stable" .


###  http://data.europa.eu/949/navigability
era:navigability rdf:type owl:ObjectProperty ;
                 rdfs:domain era:NetRelation ;
                 rdfs:range skos:Concept ;
                 era:inSkosConceptScheme <http://data.europa.eu/949/concepts/navigabilities/Navigabilities> ;
                 era:rinfIndex "1.1.1.0.1.2" ,
                               "1.2.4.1" ;
                 dct:created "2021-04-01"^^xsd:date ;
                 dct:modified "2021-08-03"^^xsd:date ;
                 dct:source <https://rsm-evolution.org/220927_RSM/EARoot/EA2/EA2/EA286.html> ;
                 rdfs:comment "Indicates the navigation possibilities between two related topological objects. The allowed values for this property belong to the SKOS Concept Scheme http://data.europa.eu/949/concepts/navigabilities/Navigabilities."@en ;
                 rdfs:isDefinedBy <http://data.europa.eu/949/> ;
                 rdfs:label "Navigability"@en ;
                 vs:term_status "stable" ;
                 skos:altLabel "Internal connection"@en .


###  http://data.europa.eu/949/netElement
era:netElement rdf:type owl:ObjectProperty ;
               rdfs:range era:NetElement ;
               dct:created "2021-04-01"^^xsd:date ;
               dct:modified "2022-09-06"^^xsd:date ;
               rdfs:comment """References an associated topological object.
The reason for deprecating this property is that it is defined as \"References an associated topological object.\" and the vocabulary has already a property \"hasAbstraction\" which relates the implementation layer with the topological layer, https://citnet.tech.ec.europa.eu/CITnet/confluence/pages/viewpage.action?pageId=1122974879."""@en ;
               rdfs:isDefinedBy <http://data.europa.eu/949/> ;
               rdfs:label "Net element"@en ;
               owl:deprecated "true"^^xsd:boolean ;
               vs:term_status "stable" .


###  http://data.europa.eu/949/notApplicable
era:notApplicable rdf:type owl:ObjectProperty ;
                  dct:created "2021-09-13"^^xsd:date ;
                  dct:modified "2021-09-13"^^xsd:date ;
                  rdfs:comment "Reference to a property that is not applicable."@en ;
                  rdfs:isDefinedBy <http://data.europa.eu/949/> ;
                  rdfs:label "Not applicable"@en ;
                  vs:term_status "unstable" .


###  http://data.europa.eu/949/notYetAvailable
era:notYetAvailable rdf:type owl:ObjectProperty ;
                    dct:created "2021-09-13"^^xsd:date ;
                    dct:modified "2021-09-13"^^xsd:date ;
                    rdfs:comment "Reference to a property that is not yet available."@en ;
                    rdfs:isDefinedBy <http://data.europa.eu/949/> ;
                    rdfs:label "Not yet available"@en ;
                    vs:term_status "unstable" .


###  http://data.europa.eu/949/opEnd
era:opEnd rdf:type owl:ObjectProperty ;
          rdfs:domain era:SectionOfLine ;
          rdfs:range era:OperationalPoint ;
          era:appendixD2Index "3.1.2" ;
          era:rinfIndex "1.1.0.0.0.4" ;
          dct:created "2021-09-09"^^xsd:date ;
          dct:modified "2023-03-14"^^xsd:date ;
          dct:source <https://eur-lex.europa.eu/eli/reg_impl/2019/773/oj> ;
          rdfs:comment """Unique OP ID at end of section of line (kilometres increasing from start OP to the end OP).
In https://eur-lex.europa.eu/eli/reg_impl/2019/773/oj 3.1.2 Line segment extremity 2."""@en ;
          rdfs:isDefinedBy <http://data.europa.eu/949/> ;
          rdfs:label "Operational Point at end of Section of Line"@en ;
          vs:term_status "stable" .


###  http://data.europa.eu/949/opInfoPerCountry
era:opInfoPerCountry rdf:type owl:ObjectProperty ;
                     rdfs:domain era:OperationalPoint ;
                     rdfs:range era:OperationalPoint ;
                     dct:created "2023-01-20"^^xsd:date ;
                     rdfs:comment "Relates an operational point that represents the general information of a  border point to the information that each country maintains for the border point."@en ;
                     rdfs:isDefinedBy <http://data.europa.eu/949/> ;
                     rdfs:label "Border point information per country"@en ;
                     vs:term_status "stable" .


###  http://data.europa.eu/949/opStart
era:opStart rdf:type owl:ObjectProperty ;
            rdfs:domain era:SectionOfLine ;
            rdfs:range era:OperationalPoint ;
            era:appendixD2Index "3.1.1" ;
            era:rinfIndex "1.1.0.0.0.3" ;
            dct:created "2021-09-09"^^xsd:date ;
            dct:modified "2023-03-14"^^xsd:date ;
            dct:source <https://eur-lex.europa.eu/eli/reg_impl/2019/773/oj> ;
            rdfs:comment """Unique OP ID at start of section of line (kilometres increasing from start OP to the end OP).
In https://eur-lex.europa.eu/eli/reg_impl/2019/773/oj 3.1.1 Line segment extremity 1."""@en ;
            rdfs:isDefinedBy <http://data.europa.eu/949/> ;
            rdfs:label "Operational Point at start of Section of Line"@en ;
            vs:term_status "stable" .


###  http://data.europa.eu/949/opType
era:opType rdf:type owl:ObjectProperty ,
                    owl:FunctionalProperty ;
           rdfs:domain era:OperationalPoint ;
           rdfs:range skos:Concept ;
           era:appendixD2Index "2.2.2" ,
                               "2.3.2" ;
           era:inSkosConceptScheme opTypes:OperationalPointTypes ;
           era:rinfIndex "1.2.0.0.0.4" ;
           dct:created "2020-07-29"^^xsd:date ;
           dct:modified "2021-08-03"^^xsd:date ;
           dct:source <https://eur-lex.europa.eu/eli/reg_impl/2019/773/oj> ;
           rdfs:comment """Type of facility in relation to the dominating operational functions. The allowed values for this property belong to the SKOS Concept Scheme http://data.europa.eu/949/concepts/op-types/OperationalPointTypes.
In https://eur-lex.europa.eu/eli/reg_impl/2019/773/oj 2.3.2 Type of location passenger terminal, freight terminal, yard, depot."""@en ;
           rdfs:isDefinedBy <http://data.europa.eu/949/> ;
           rdfs:label "Type of operational point"@en ;
           vs:term_status "stable" .


###  http://data.europa.eu/949/operatingLanguage
era:operatingLanguage rdf:type owl:ObjectProperty ;
                      rdfs:range skos:Concept ;
                      era:appendixD2Index "3.5.1" ;
                      era:rinfIndex "1.1.0.0.1.2" ,
                                    "1.2.0.0.0.8" ;
                      dct:created "2022-10-28"^^xsd:date ;
                      dct:modified "2023-03-14"^^xsd:date ;
                      dct:source <https://eur-lex.europa.eu/eli/reg_impl/2019/773/oj> ;
                      rdfs:comment """The language or languages used in daily operation by infrastructure manager and published in its Network Statement, for the communication of operational or safety related messages between the staff of the infrastructure manager and the railway undertaking.
The allowed values for this property belong to a SKOS Concept Scheme.
In 3.5.1 https://eur-lex.europa.eu/eli/reg_impl/2019/773/oj  Operating language."""@en ;
                      rdfs:isDefinedBy <http://data.europa.eu/949/> ;
                      rdfs:label "Operating language"@en ;
                      vs:term_status "unstable" .


###  http://data.europa.eu/949/operationalRegimeType
era:operationalRegimeType rdf:type owl:ObjectProperty ,
                                   owl:FunctionalProperty ;
                          rdfs:range skos:Concept ;
                          era:appendixD2Index "3.2.7" ;
                          era:rinfIndex "1.1.0.0.1.3" ;
                          dct:created "2022-10-27"^^xsd:date ;
                          dct:modified "2023-03-14"^^xsd:date ;
                          dct:source <https://eur-lex.europa.eu/eli/reg_impl/2019/773/oj> ;
                          rdfs:comment """Double track type. The allowed values for this property belong to a SKOS Concept Scheme.
In https://eur-lex.europa.eu/eli/reg_impl/2019/773/oj 3.2.7 Type of signalling system and corresponding operational regime (double track, reversible working, left or right hand running, etc.)."""@en ;
                          rdfs:isDefinedBy <http://data.europa.eu/949/> ;
                          rdfs:label "Operational regime type"@en ;
                          vs:term_status "unstable" .


###  http://data.europa.eu/949/operationalRestriction
era:operationalRestriction rdf:type owl:ObjectProperty ;
                           rdfs:domain era:Vehicle ;
                           rdfs:range skos:Concept ;
                           era:inSkosConceptScheme <http://data.europa.eu/949/concepts/restrictions/Restrictions> ;
                           dct:created "2020-11-23"^^xsd:date ;
                           dct:modified "2021-08-03"^^xsd:date ;
                           rdfs:comment "Indicates an operational restriction of vehicle or wagon. Parking brake type (if the vehicle is fitted with it). The allowed values for this property belong to the SKOS Concept Scheme http://data.europa.eu/949/concepts/restrictions/Restrictions."@en ;
                           rdfs:isDefinedBy <http://data.europa.eu/949/> ;
                           rdfs:label "Operational restriction"@en ;
                           vs:term_status "stable" .


###  http://data.europa.eu/949/osmClass
era:osmClass rdf:type owl:ObjectProperty ;
             rdfs:domain [ rdf:type owl:Class ;
                           owl:unionOf ( era:SubsetWithCommonCharacteristics
                                         era:Track
                                       )
                         ] ;
             rdfs:range skos:Concept ;
             era:inSkosConceptScheme <http://data.europa.eu/949/concepts/osmclass/OSMClasses> ;
             rdfs:isDefinedBy <http://data.europa.eu/949/> ;
             rdfs:label "Open street map class"@en ;
             vs:term_status "stable" ;
             skos:definition "Additional concept class according to OpenStreetMap. The allowed values for this property belong to the SKOS Concept Scheme http://data.europa.eu/949/concepts/osmclass/OSMClasses."@en .


###  http://data.europa.eu/949/otherCantDeficiencyBasicSSP
era:otherCantDeficiencyBasicSSP rdf:type owl:ObjectProperty ;
                                rdfs:domain [ rdf:type owl:Class ;
                                              owl:unionOf ( era:SubsetWithCommonCharacteristics
                                                            era:Track
                                                          )
                                            ] ;
                                rdfs:range skos:Concept ;
                                era:rinfIndex "1.1.1.3.2.14.1" ,
                                              "1.2.1.1.1.14.1" ;
                                dct:created "2023-03-14"^^xsd:date ;
                                rdfs:comment """Essential information for drivers of trains with a worse (lower) tolerated cant deficiency than those for which the ETCS trackside provides SSP (Static Speed Profiles) in conjunction with 1.1.1.3.2.14. 
According to the specification referenced in Appendix A-1, index [C]."""@en ;
                                rdfs:isDefinedBy <http://data.europa.eu/949/> ;
                                rdfs:label "Other Cant Deficiency train categories for which the ETCS trackside is configured to provide SSP"@en ;
                                vs:term_status "unstable" .


###  http://data.europa.eu/949/otherPantographHead
era:otherPantographHead rdf:type owl:ObjectProperty ;
                        rdfs:domain [ rdf:type owl:Class ;
                                      owl:unionOf ( era:SubsetWithCommonCharacteristics
                                                    era:Track
                                                  )
                                    ] ;
                        rdfs:range skos:Concept ;
                        era:inSkosConceptScheme <http://data.europa.eu/949/concepts/other-pantograph-heads/OtherPantographHeads> ;
                        era:rinfIndex "1.1.1.2.3.2" ;
                        era:usedInRCCCalculations "true"^^xsd:boolean ;
                        dct:created "2022-06-03"^^xsd:date ;
                        dct:modified "2022-06-03"^^xsd:date ;
                        rdfs:comment """Indication of pantograph heads which are allowed to be used.
The allowed values for this property belong to the SKOS Concept Scheme http://data.europa.eu/949/concepts/other-pantograph-heads/OtherPantographHeads."""@en ;
                        rdfs:isDefinedBy <http://data.europa.eu/949/> ;
                        rdfs:label "Accepted other pantograph heads"@en ;
                        vs:term_status "stable" .


###  http://data.europa.eu/949/otherTrainProtection
era:otherTrainProtection rdf:type owl:ObjectProperty ,
                                  owl:FunctionalProperty ;
                         rdfs:domain [ rdf:type owl:Class ;
                                       owl:unionOf ( era:SubsetWithCommonCharacteristics
                                                     era:Track
                                                   )
                                     ] ;
                         rdfs:range skos:Concept ;
                         era:inSkosConceptScheme <http://data.europa.eu/949/concepts/other-protection-control-warning/OtherProtectionControlWarnings> ;
                         era:rinfIndex "1.1.1.3.10.2" ,
                                       "1.2.1.1.9.2" ;
                         dct:created "2021-08-09"^^xsd:date ;
                         dct:modified "2021-09-12"^^xsd:date ;
                         rdfs:comment "Indication of existence of other system than ETCS for degraded situation. The allowed values for this property belong to the SKOS Concept Scheme http://data.europa.eu/949/concepts/other-protection-control-warning/OtherProtectionControlWarnings"@en ;
                         rdfs:isDefinedBy <http://data.europa.eu/949/> ;
                         rdfs:label "Other train protection, control and warning systems for degraded situation"@en ;
                         vs:term_status "stable" .


###  http://data.europa.eu/949/parkingBrakeType
era:parkingBrakeType rdf:type owl:ObjectProperty ;
                     rdfs:domain era:VehicleType ;
                     rdfs:range skos:Concept ;
                     era:eratvIndex "4.7.3.2" ;
                     era:inSkosConceptScheme <http://data.europa.eu/949/concepts/brake-parking-type/BrakeParkingType> ;
                     dct:created "2021-08-26"^^xsd:date ;
                     dct:modified "2021-08-26"^^xsd:date ;
                     rdfs:comment "Parking brake type (if the vehicle is fitted with it). The allowed values for this property belong to the SKOS Concept Scheme http://data.europa.eu/949/concepts/brake-parking-type/BrakeParkingType."@en ;
                     rdfs:isDefinedBy <http://data.europa.eu/949/> ;
                     rdfs:label "Parking brake type"@en ;
                     vs:term_status "stable" .


###  http://data.europa.eu/949/passesThroughTunnel
era:passesThroughTunnel rdf:type owl:ObjectProperty ;
                        rdfs:domain [ rdf:type owl:Class ;
                                      owl:unionOf ( era:SubsetWithCommonCharacteristics
                                                    era:Track
                                                  )
                                    ] ;
                        rdfs:range era:Tunnel ;
                        dct:created "2020-07-29"^^xsd:date ;
                        dct:modified "2022-10-27"^^xsd:date ;
                        rdfs:comment "References a tunnel that a track goes through."@en ;
                        rdfs:isDefinedBy <http://data.europa.eu/949/> ;
                        rdfs:label "Passes through tunnel"@en ;
                        vs:term_status "stable" .


###  http://data.europa.eu/949/platform
era:platform rdf:type owl:ObjectProperty ;
             rdfs:domain [ rdf:type owl:Class ;
                           owl:unionOf ( era:SubsetWithCommonCharacteristics
                                         era:Track
                                       )
                         ] ;
             rdfs:range era:Platform ;
             dct:created "2021-08-09"^^xsd:date ;
             dct:modified "2021-08-09"^^xsd:date ;
             rdfs:comment "Reference to a related platform."@en ;
             rdfs:isDefinedBy <http://data.europa.eu/949/> ;
             rdfs:label "Platform"@en ;
             vs:term_status "stable" .


###  http://data.europa.eu/949/platformHeight
era:platformHeight rdf:type owl:ObjectProperty ,
                            owl:FunctionalProperty ;
                   rdfs:domain era:Platform ;
                   rdfs:range skos:Concept ;
                   era:appendixD2Index "2.3.7" ;
                   era:inSkosConceptScheme <http://data.europa.eu/949/concepts/platform-heights/PlatformHeights> ;
                   era:rinfIndex "1.2.1.0.6.5" ;
                   era:usedInRCCCalculations "true"^^xsd:boolean ;
                   dct:created "2021-08-02"^^xsd:date ;
                   dct:modified "2021-08-02"^^xsd:date ;
                   dct:source <https://eur-lex.europa.eu/eli/reg_impl/2019/773/oj> ;
                   rdfs:comment """Distance between the upper surface of platform and running surface of the neighbouring track. It is the nominal value expressed in millimetres. The allowed values for this property belong to the SKOS Concept Scheme http://data.europa.eu/949/concepts/platform-heights/PlatformHeights
In https://eur-lex.europa.eu/eli/reg_impl/2019/773/oj 2.3.7 Height of platforms."""@en ;
                   rdfs:isDefinedBy <http://data.europa.eu/949/> ;
                   rdfs:label "Height of platform"@en ;
                   vs:term_status "stable" .


###  http://data.europa.eu/949/positionOnA
era:positionOnA rdf:type owl:ObjectProperty ;
                rdfs:domain era:NetRelation ;
                rdfs:range skos:Concept ;
                era:inSkosConceptScheme <http://data.europa.eu/949/concepts/relation-positions/RelationPositions> ;
                era:rinfIndex "1.1.1.0.1.2" ,
                              "1.2.4.1" ;
                dct:created "2021-04-03"^^xsd:date ;
                dct:modified "2021-08-03"^^xsd:date ;
                rdfs:comment "Determines the position of the topological object A in a relation. The allowed values for this property belong to the SKOS Concept Scheme http://data.europa.eu/949/concepts/relation-positions/RelationPositions."@en ;
                rdfs:isDefinedBy <http://data.europa.eu/949/> ;
                rdfs:label "Position on A"@en ;
                rdfs:seeAlso <https://rsm-evolution.org/220927_RSM/EARoot/EA2/EA2/EA291.html> ;
                vs:term_status "stable" ;
                skos:altLabel "Internal connection"@en .


###  http://data.europa.eu/949/positionOnB
era:positionOnB rdf:type owl:ObjectProperty ;
                rdfs:domain era:NetRelation ;
                rdfs:range skos:Concept ;
                era:inSkosConceptScheme <http://data.europa.eu/949/concepts/relation-positions/RelationPositions> ;
                era:rinfIndex "1.1.1.0.1.2" ,
                              "1.2.4.1" ;
                dct:created "2021-04-03"^^xsd:date ;
                dct:modified "2021-08-03"^^xsd:date ;
                rdfs:comment "Determines the position of the topological object B in a relation. The allowed values for this property belong to the SKOS Concept Scheme http://data.europa.eu/949/concepts/relation-positions/RelationPositions."@en ;
                rdfs:isDefinedBy <http://data.europa.eu/949/> ;
                rdfs:label "Position on B"@en ;
                rdfs:seeAlso <https://rsm-evolution.org/220927_RSM/EARoot/EA2/EA2/EA291.html> ;
                vs:term_status "stable" ;
                skos:altLabel "Internal connection"@en .


###  http://data.europa.eu/949/previousVehicleType
era:previousVehicleType rdf:type owl:ObjectProperty ,
                                 owl:FunctionalProperty ;
                        rdfs:domain era:VehicleType ;
                        rdfs:range era:VehicleType ;
                        dct:created "2022-06-15"^^xsd:date ;
                        dct:modified "2022-06-15"^^xsd:date ;
                        rdfs:comment "Denotes a the previous VehicleType."@en ;
                        rdfs:isDefinedBy <http://data.europa.eu/949/> ;
                        rdfs:label "Previous vehicle type"@en ;
                        vs:term_status "stable" .


###  http://data.europa.eu/949/profileNumberSemiTrailers
era:profileNumberSemiTrailers rdf:type owl:ObjectProperty ;
                              rdfs:domain [ rdf:type owl:Class ;
                                            owl:unionOf ( era:SubsetWithCommonCharacteristics
                                                          era:Track
                                                        )
                                          ] ;
                              rdfs:range skos:Concept ;
                              era:inSkosConceptScheme <http://data.europa.eu/949/concepts/profile-num-semi-trailers/ProfileNumbersSemiTrailers> ;
                              era:rinfIndex "1.1.1.1.3.5" ;
                              dct:created "2021-08-03"^^xsd:date ;
                              dct:modified "2023-03-14"^^xsd:date ;
                              rdfs:comment """Coding for combined transport for semi-trailers (for all freight and mixed-traffic lines) in accordance with the specification referenced in Appendix A-1, index [B].
The allowed values for this property belong to the SKOS Concept Scheme http://data.europa.eu/949/concepts/profile-num-semi-trailers/ProfileNumbersSemiTrailers"""@en ;
                              rdfs:isDefinedBy <http://data.europa.eu/949/> ;
                              rdfs:label "Standard combined transport profile number for semi-trailers"@en ;
                              vs:term_status "stable" .


###  http://data.europa.eu/949/profileNumberSwapBodies
era:profileNumberSwapBodies rdf:type owl:ObjectProperty ;
                            rdfs:domain [ rdf:type owl:Class ;
                                          owl:unionOf ( era:SubsetWithCommonCharacteristics
                                                        era:Track
                                                      )
                                        ] ;
                            rdfs:range skos:Concept ;
                            era:inSkosConceptScheme <http://data.europa.eu/949/concepts/profile-num-swap-bodies/ProfileNumbersSwapBodies> ;
                            era:rinfIndex "1.1.1.1.3.4" ;
                            dct:created "2021-08-03"^^xsd:date ;
                            dct:modified "2023-03-14"^^xsd:date ;
                            rdfs:comment "Coding for combined transport with swap bodies (for all freight and mixed-traffic lines) in accordance with the specification referenced in Appendix A-1, index [B]"@en ;
                            rdfs:isDefinedBy <http://data.europa.eu/949/> ;
                            rdfs:label "Standard combined transport profile number for swap bodies"@en ;
                            vs:term_status "stable" .


###  http://data.europa.eu/949/protectionLegacySystem
era:protectionLegacySystem rdf:type owl:ObjectProperty ;
                           rdfs:domain [ rdf:type owl:Class ;
                                         owl:unionOf ( era:SubsetWithCommonCharacteristics
                                                       era:Track
                                                       era:VehicleType
                                                     )
                                       ] ;
                           rdfs:range skos:Concept ;
                           era:eratvIndex "4.13.1.5" ;
                           era:inSkosConceptScheme <http://data.europa.eu/949/concepts/train-protection-legacy-systems/TrainProtectionLegacySystems> ;
                           era:rinfIndex "1.1.1.3.5.3" ,
                                         "1.2.1.1.4.1" ;
                           era:usedInRCCCalculations "true"^^xsd:boolean ;
                           dct:created "2020-08-31"^^xsd:date ;
                           dct:modified "2021-09-12"^^xsd:date ;
                           rdfs:comment "Indication of which class B system is installed. The allowed values for this property belong to the SKOS Concept Scheme http://data.europa.eu/949/concepts/train-protection-legacy-systems/TrainProtectionLegacySystems"@en ;
                           rdfs:isDefinedBy <http://data.europa.eu/949/> ;
                           rdfs:label "Train protection legacy system"@en ;
                           vs:term_status "stable" .


###  http://data.europa.eu/949/qNvdriverAdhes
era:qNvdriverAdhes rdf:type owl:ObjectProperty ;
                   rdfs:domain [ rdf:type owl:Class ;
                                 owl:unionOf ( era:SubsetWithCommonCharacteristics
                                               era:Track
                                             )
                               ] ;
                   rdfs:range skos:Concept ;
                   era:appendixD3Index "1.5.11" ;
                   era:rinfIndex "1.1.1.3.2.16.11" ,
                                 "1.2.1.1.1.16.11Â " ;
                   dct:created "2023-03-14"^^xsd:date ;
                   rdfs:comment """Qualifier determining whether the driver is allowed to modify the adhesion factor used by the ETCS on-board to calculate the braking curves. 
According to the specification referenced in Appendix A-1, index [C]. 
In https://www.era.europa.eu/sites/default/files/filesystem/ertms/ccs_tsi_annex_a_-_mandatory_specifications/set_of_specifications_3_etcs_b3_r2_gsm-r_b1/index004_-_subset-026_v360.zip
 Subset 26, chapter 7. 7.5.1.122 Q_NVDRIVER_ADHES.
The allowed values for this property belong to a SKOS Concept Scheme."""@en ;
                   rdfs:isDefinedBy <http://data.europa.eu/949/> ;
                   rdfs:label "Q_NVDRIVER_ADHES"@en ;
                   vs:term_status "stable" .


###  http://data.europa.eu/949/qNvemrrls
era:qNvemrrls rdf:type owl:ObjectProperty ;
              rdfs:domain [ rdf:type owl:Class ;
                            owl:unionOf ( era:SubsetWithCommonCharacteristics
                                          era:Track
                                        )
                          ] ;
              rdfs:range skos:Concept ;
              era:appendixD3Index "1.5.2" ;
              era:rinfIndex "1.1.1.3.2.16.2" ,
                            "1.2.1.1.1.16.2Â " ;
              dct:created "2023-03-14"^^xsd:date ;
              rdfs:comment """Qualifier defining whether the application of the emergency brake for reasons other than a trip can be revoked as soon as the conditions for it have disappeared or after the train has come to a complete standstill.
According to the specification referenced in Appendix A-1, index [C]. 
In https://www.era.europa.eu/sites/default/files/filesystem/ertms/ccs_tsi_annex_a_-_mandatory_specifications/set_of_specifications_3_etcs_b3_r2_gsm-r_b1/index004_-_subset-026_v360.zip
Subset 26, chapter 7. 7.5.1.123 Q_NVEMRRLS.
The allowed values for this property belong to a SKOS Concept Scheme."""@en ;
              rdfs:isDefinedBy <http://data.europa.eu/949/> ;
              rdfs:label "Q_NVEMRRLS"@en ;
              vs:term_status "unstable" .


###  http://data.europa.eu/949/quieterRoutesExemptedCountry
era:quieterRoutesExemptedCountry rdf:type owl:ObjectProperty ;
                                 rdfs:domain era:Vehicle ;
                                 rdfs:range skos:Concept ;
                                 era:inSkosConceptScheme <http://publications.europa.eu/resource/authority/country> ;
                                 dct:created "2020-11-23"^^xsd:date ;
                                 dct:modified "2020-11-23"^^xsd:date ;
                                 rdfs:comment "Country where a vehicle may operate without noise restrictions. The allowed values for this property belong to the SKOS Concept Scheme http://publications.europa.eu/resource/authority/country"@en ;
                                 rdfs:isDefinedBy <http://data.europa.eu/949/> ;
                                 rdfs:label "Quieter route exempted country"@en ;
                                 vs:term_status "stable" .


###  http://data.europa.eu/949/railInclination
era:railInclination rdf:type owl:ObjectProperty ,
                             owl:FunctionalProperty ;
                    rdfs:domain [ rdf:type owl:Class ;
                                  owl:unionOf ( era:SubsetWithCommonCharacteristics
                                                era:Track
                                                era:VehicleType
                                              )
                                ] ;
                    rdfs:range skos:Concept ;
                    era:eratvIndex "4.6.5" ;
                    era:inSkosConceptScheme <http://data.europa.eu/949/concepts/rail-inclinations/RailInclinations> ;
                    era:rinfIndex "1.1.1.1.4.3" ;
                    era:usedInRCCCalculations "true"^^xsd:boolean ;
                    dct:created "2020-08-24"^^xsd:date ;
                    dct:modified "2022-10-20"^^xsd:date ;
                    rdfs:comment """An angle defining the inclination of the head of a rail relative to the running surface. The allowed values for this property belong to the SKOS Concept Scheme http://data.europa.eu/949/concepts/rail-inclinations/RailInclinations
This property has been changed, its rinfIndex has been deleted. RINF treats this parameter as an integer. A new datatype property for RINF has been defined called railInclinationMeasurement.
This change was rolled back, RINF index was again added."""@en ;
                    rdfs:isDefinedBy <http://data.europa.eu/949/> ;
                    rdfs:label "Rail inclination"@en ;
                    vs:term_status "stable" .


###  http://data.europa.eu/949/reasonsEtcsRadioBlockCenterReject
era:reasonsEtcsRadioBlockCenterReject rdf:type owl:ObjectProperty ;
                                      rdfs:domain [ rdf:type owl:Class ;
                                                    owl:unionOf ( era:SubsetWithCommonCharacteristics
                                                                  era:Track
                                                                )
                                                  ] ;
                                      rdfs:range skos:Concept ;
                                      era:appendixD3Index "1.4" ;
                                      era:rinfIndex "1.1.1.3.2.15" ,
                                                    "1.2.1.1.1.15" ;
                                      dct:created "2022-11-07"^^xsd:date ;
                                      dct:modified "2023-03-14"^^xsd:date ;
                                      rdfs:comment """List of cases subject to system design choices made by the infrastructure manager according to the specification referenced in Appendix A-1, index [C]. 
In https://www.era.europa.eu/sites/default/files/filesystem/ertms/ccs_tsi_annex_a_-_mandatory_specifications/set_of_specifications_3_etcs_b3_r2_gsm-r_b1/index004_-_subset-026_v360.zip
Subset 26, Chapter 5 5.4 Procedure start of mission.
The allowed values for this property belong to a SKOS Concept Scheme."""@en ;
                                      rdfs:isDefinedBy <http://data.europa.eu/949/> ;
                                      rdfs:label "Reasons for which an ETCS Radio Block Center can reject a train"@en ;
                                      vs:term_status "unstable" .


###  http://data.europa.eu/949/rollingStockFireCategory
era:rollingStockFireCategory rdf:type owl:ObjectProperty ,
                                      owl:FunctionalProperty ;
                             rdfs:domain era:Tunnel ;
                             rdfs:range skos:Concept ;
                             era:appendixD2Index "3.2.3" ;
                             era:inSkosConceptScheme <http://data.europa.eu/949/concepts/rolling-stock-fire/Categories> ;
                             era:rinfIndex "1.1.1.1.8.10" ,
                                           "1.2.1.0.5.7" ,
                                           "1.2.2.0.5.7" ;
                             era:usedInRCCCalculations "true"^^xsd:boolean ;
                             dct:created "2020-07-29"^^xsd:date ;
                             dct:modified "2021-08-10"^^xsd:date ;
                             dct:source <https://eur-lex.europa.eu/eli/reg_impl/2019/773/oj> ;
                             rdfs:comment """Categorisation how a passenger train with a fire on board will continue to operate for a defined time period. The allowed values for this property belong to the SKOS Concept Scheme http://data.europa.eu/949/concepts/rolling-stock-fire/Categories.
In https://eur-lex.europa.eu/eli/reg_impl/2019/773/oj 3.2.3 Tunnels: location, name, length, specific information such as the existence of walkways and points of safe egress as well as the location of safe areas where evacuation of passengers may take place; fire safety categorisation."""@en ;
                             rdfs:isDefinedBy <http://data.europa.eu/949/> ;
                             rdfs:label "Fire category of rolling stock required"@en ;
                             vs:term_status "stable" .


###  http://data.europa.eu/949/safeConsistLengthInformationNecessary
era:safeConsistLengthInformationNecessary rdf:type owl:ObjectProperty ;
                                          rdfs:domain [ rdf:type owl:Class ;
                                                        owl:unionOf ( era:SubsetWithCommonCharacteristics
                                                                      era:Track
                                                                    )
                                                      ] ;
                                          rdfs:range skos:Concept ;
                                          era:rinfIndex "1.1.1.3.2.11" ,
                                                        "1.2.1.1.1.11" ;
                                          dct:created "2023-03-14"^^xsd:date ;
                                          rdfs:comment """Indication whether safe consist train length information from on-board is required to access the line for safety reasons and the required safety integrity level.
The allowed values for this property belong to a SKOS Concept Scheme."""@en ;
                                          rdfs:isDefinedBy <http://data.europa.eu/949/> ;
                                          rdfs:label "Safe consist length information from on-board necessary for access the line and SIL"@en ;
                                          vs:term_status "stable" .


###  http://data.europa.eu/949/siding
era:siding rdf:type owl:ObjectProperty ;
           rdfs:domain era:OperationalPoint ;
           rdfs:range era:Siding ;
           dct:created "2021-08-10"^^xsd:date ;
           dct:modified "2021-08-10"^^xsd:date ;
           rdfs:comment "Reference to a related siding."@en ;
           rdfs:isDefinedBy <http://data.europa.eu/949/> ;
           rdfs:label "Siding"@en ;
           vs:term_status "stable" .


###  http://data.europa.eu/949/signalOrientation
era:signalOrientation rdf:type owl:ObjectProperty ;
                      rdfs:domain era:Signal ;
                      rdfs:range skos:Concept ;
                      era:rinfIndex "1.1.1.3.14.3" ,
                                    "1.2.1.0.8.3" ;
                      dct:created "2023-03-14"^^xsd:date ;
                      rdfs:isDefinedBy <http://data.europa.eu/949/> ;
                      rdfs:label "Signal orientation"@en ;
                      owl:versionURI """indication if the signal refers to normal or opposite track direction.
The allowed values for this property belong to a SKOS Concept Scheme."""@en ;
                      vs:term_status "unstable" .


###  http://data.europa.eu/949/signalType
era:signalType rdf:type owl:ObjectProperty ;
               rdfs:domain era:Signal ;
               rdfs:range skos:Concept ;
               era:appendixD2Index "2.2.3" ;
               era:rinfIndex "1.1.1.3.14.2" ,
                             "1.2.1.0.8.2" ;
               dct:created "2022-10-27"^^xsd:date ;
               dct:modified "2023-03-14"^^xsd:date ;
               dct:source <https://eur-lex.europa.eu/eli/reg_impl/2019/773/oj> ;
               rdfs:comment """Location, type and name of all fixed signals relevant for trains.
The allowed values for this property belong to a SKOS Concept Scheme.
In https://eur-lex.europa.eu/eli/reg_impl/2019/773/oj 2.2.3 Location, type and name of all fixed signals relevant for trains."""@en ;
               rdfs:isDefinedBy <http://data.europa.eu/949/> ;
               rdfs:label "Type of signal"@en ;
               vs:term_status "unstable" .


###  http://data.europa.eu/949/signallingSystemType
era:signallingSystemType rdf:type owl:ObjectProperty ;
                         rdfs:range skos:Concept ;
                         era:appendixD2Index "3.2.7" ;
                         era:rinfIndex "1.1.0.0.1.3" ;
                         dct:created "2023-03-14"^^xsd:date ;
                         dct:source <https://eur-lex.europa.eu/eli/reg_impl/2019/773/oj> ;
                         rdfs:comment """Indication of the signalling system type of the signalling system. The allowed values for this property belong to a SKOS Concept Scheme.
In https://eur-lex.europa.eu/eli/reg_impl/2019/773/oj 3.2.7 Type of signalling system and corresponding operational regime (double track, reversible working, left or right hand running, etc.).
The allowed values for this property belong to a SKOS Concept Scheme."""@en ;
                         rdfs:isDefinedBy <http://data.europa.eu/949/> ;
                         rdfs:label "Signalling system type"@en ;
                         vs:term_status "unstable" .


###  http://data.europa.eu/949/snowIceHailConditions
era:snowIceHailConditions rdf:type owl:ObjectProperty ,
                                   owl:FunctionalProperty ;
                          rdfs:domain era:VehicleType ;
                          rdfs:range skos:Concept ;
                          era:eratvIndex "4.3.3" ;
                          era:inSkosConceptScheme <http://data.europa.eu/949/concepts/ice-conditions/IceConditions> ;
                          dct:created "2020-08-24"^^xsd:date ;
                          dct:modified "2021-08-02"^^xsd:date ;
                          rdfs:comment "Snow, ice and hail conditions. The allowed values for this property belong to the SKOS Concept Scheme http://data.europa.eu/949/concepts/ice-conditions/IceConditions"@en ;
                          rdfs:isDefinedBy <http://data.europa.eu/949/> ;
                          rdfs:label "Snow ice hail conditions"@en ;
                          vs:term_status "stable" .


###  http://data.europa.eu/949/solNature
era:solNature rdf:type owl:ObjectProperty ,
                       owl:FunctionalProperty ;
              rdfs:domain era:SectionOfLine ;
              rdfs:range skos:Concept ;
              era:inSkosConceptScheme <http://data.europa.eu/949/concepts/sol-natures/SoLNatures> ;
              era:rinfIndex "1.1.0.0.0.6" ;
              dct:created "2021-08-08"^^xsd:date ;
              dct:modified "2023-03-14"^^xsd:date ;
              rdfs:comment """Kind of section of line expressing size of presented data which depends on fact whether it connects OPs generated by division of a big node into several OPs or not.
The allowed values for this property belong to the SKOS Concept Scheme http://data.europa.eu/949/concepts/sol-natures/SoLNatures"""@en ;
              rdfs:isDefinedBy <http://data.europa.eu/949/> ;
              rdfs:label "Nature of Section of Line"@en ;
              vs:term_status "stable" .


###  http://data.europa.eu/949/specialAreaType
era:specialAreaType rdf:type owl:ObjectProperty ;
                    rdfs:domain era:SpecialArea ;
                    rdfs:range skos:Concept ;
                    era:appendixD2Index "3.2.3" ,
                                        "3.2.4" ,
                                        "3.2.5" ,
                                        "3.2.6" ,
                                        "3.3.5" ,
                                        "3.3.6" ;
                    era:rinfIndex "1.1.0.0.1.1" ;
                    dct:created "2022-10-27"^^xsd:date ;
                    dct:modified "2023-03-14"^^xsd:date ;
                    rdfs:comment """Indicates the special area or location types such as safe areas and restricted area types.
The allowed values of this property belong to a SKOS concept scheme.
In https://eur-lex.europa.eu/eli/reg_impl/2019/773/oj 
3.2.3 Tunnels: location, name, length, specific information such as the existence of walkways and points of safe egress as well as the location of safe areas where evacuation of passengers may take place; fire safety categorisation.
3.2.4 Non-stopping areas: identification, location, type.
3.2.5 Industrial risks â locations where it is dangerous for the driver to step out.
3.2.6 Locations of areas designated for testing the sanding equipment (if existing).
3.3.5 Location of neutral sections.
3.3.6 Location of areas that shall be passed with lowered pantographs."""@en ;
                    rdfs:isDefinedBy <http://data.europa.eu/949/> ;
                    rdfs:label "Special area type"@en ;
                    vs:term_status "unstable" .


###  http://data.europa.eu/949/specialTunnelArea
era:specialTunnelArea rdf:type owl:ObjectProperty ;
                      rdfs:domain era:Tunnel ;
                      rdfs:range era:SpecialTunnelArea ;
                      era:appendixD2Index "3.2.3" ;
                      dct:created "2022-10-27"^^xsd:date ;
                      dct:source <https://eur-lex.europa.eu/eli/reg_impl/2019/773/oj> ;
                      rdfs:comment """Relates a tunnel with a special area or location.
In https://eur-lex.europa.eu/eli/reg_impl/2019/773/oj 3.2.3 Tunnels: location, name, length, specific information such as the existence of walkways and points of safe egress as well as the location of safe areas where evacuation of passengers may take place; fire safety categorisation."""@en ;
                      rdfs:isDefinedBy "http://data.europa.eu/949/" ;
                      rdfs:label "Special tunnel area"@en ;
                      vs:term_status "stable" .


###  http://data.europa.eu/949/standardCombinedTransporRollerUnits
era:standardCombinedTransporRollerUnits rdf:type owl:ObjectProperty ;
                                        rdfs:domain [ rdf:type owl:Class ;
                                                      owl:unionOf ( era:SubsetWithCommonCharacteristics
                                                                    era:Track
                                                                  )
                                                    ] ;
                                        rdfs:range skos:Concept ;
                                        era:rinfIndex "1.1.1.1.3.9" ;
                                        dct:created "2023-03-14"^^xsd:date ;
                                        rdfs:comment """Coding for combined transport for roller units (for all freight and mixed-traffic lines) in accordance with the specification referenced in Appendix A-1, index [B]. 
The allowed values for this property belong to a SKOS Concept Scheme."""@en ;
                                        rdfs:isDefinedBy <http://data.europa.eu/949/> ;
                                        rdfs:label "Standard combined transport profile number for roller units"@en ;
                                        vs:term_status "unstable" .


###  http://data.europa.eu/949/standardCombinedTransportContainers
era:standardCombinedTransportContainers rdf:type owl:ObjectProperty ;
                                        rdfs:domain [ rdf:type owl:Class ;
                                                      owl:unionOf ( era:SubsetWithCommonCharacteristics
                                                                    era:Track
                                                                  )
                                                    ] ;
                                        rdfs:range skos:Concept ;
                                        era:rinfIndex "1.1.1.1.3.8" ;
                                        dct:created "2023-03-14"^^xsd:date ;
                                        rdfs:comment """Coding for combined transport for containers (for all freight and mixed-traffic lines) in accordance with the specification referenced in Appendix A-1, index [B].
The allowed values for this property belong to a SKOS Concept Scheme."""@en ;
                                        rdfs:isDefinedBy <http://data.europa.eu/949/> ;
                                        rdfs:label "Standard combined transport profile number for containers"@en ;
                                        vs:term_status "unstable" .


###  http://data.europa.eu/949/startLocation
era:startLocation rdf:type owl:ObjectProperty ;
                  rdfs:subPropertyOf gsp:hasGeometry ,
                                     wgs:location ;
                  rdfs:domain era:Tunnel ;
                  rdfs:range [ rdf:type owl:Class ;
                               owl:unionOf ( gsp:Geometry
                                             wgs:Point
                                           )
                             ] ;
                  era:rinfIndex "1.1.1.1.8.3" ;
                  dct:created "2020-07-29"^^xsd:date ;
                  dct:modified "2021-08-11"^^xsd:date ;
                  rdfs:comment "References the geolocation of the start of a tunnel."@en ;
                  rdfs:isDefinedBy <http://data.europa.eu/949/> ;
                  rdfs:label "Start of tunnel"@en ;
                  vs:term_status "stable" .


###  http://data.europa.eu/949/state
era:state rdf:type owl:ObjectProperty ,
                   owl:FunctionalProperty ;
          rdfs:domain era:Certificate ;
          rdfs:range skos:Concept ;
          era:inSkosConceptScheme <http://data.europa.eu/949/concepts/states/States> ;
          dct:created "2022-06-15"^^xsd:date ;
          dct:modified "2022-06-15"^^xsd:date ;
          rdfs:comment "Denoting the state of the certificate and range the following instances. The allowed values for this property belong to the SKOS Concept Scheme http://data.europa.eu/949/concepts/states/States."@en ;
          rdfs:label "State"@en ;
          vs:term_status "stable" .


###  http://data.europa.eu/949/subCategory
era:subCategory rdf:type owl:ObjectProperty ,
                         owl:FunctionalProperty ;
                rdfs:domain era:VehicleType ;
                rdfs:range skos:Concept ;
                era:eratvIndex 1.5 ;
                era:inSkosConceptScheme <http://data.europa.eu/949/concepts/vehicle-types/Categories> ;
                dct:created "2020-07-29"^^xsd:date ;
                dct:modified "2021-08-03"^^xsd:date ;
                rdfs:comment "Vehicle subcategory. The allowed values for this property belong to the SKOS Concept Scheme http://data.europa.eu/949/concepts/vehicle-types/Categories."@en ;
                rdfs:isDefinedBy <http://data.europa.eu/949/> ;
                rdfs:label "Vehicle subcategory"@en ;
                vs:term_status "stable" .


###  http://data.europa.eu/949/supportedPlatformHeight
era:supportedPlatformHeight rdf:type owl:ObjectProperty ;
                            rdfs:domain era:VehicleType ;
                            rdfs:range skos:Concept ;
                            era:eratvIndex "4.12.3.1" ;
                            era:inSkosConceptScheme <http://data.europa.eu/949/concepts/platform-heights/PlatformHeights> ;
                            dct:created "2020-07-29"^^xsd:date ;
                            dct:modified "2021-08-02"^^xsd:date ;
                            rdfs:comment "Platform height for which the vehicle is deÂ­signed. The allowed values for this property belong to the SKOS Concept Scheme http://data.europa.eu/949/concepts/platform-heights/PlatformHeights"@en ;
                            rdfs:isDefinedBy <http://data.europa.eu/949/> ;
                            rdfs:label "Supported platform height"@en ;
                            vs:term_status "stable" .


###  http://data.europa.eu/949/tdsFrenchTrainDetectionSystemLimitation
era:tdsFrenchTrainDetectionSystemLimitation rdf:type owl:ObjectProperty ;
                                            rdfs:domain era:TrainDetectionSystem ;
                                            rdfs:range era:FrenchTrainDetectionSystemLimitation ;
                                            era:rinfIndex "1.1.1.3.7.1.4" ;
                                            era:usedInRCCCalculations "true"^^xsd:boolean ;
                                            dct:created "2023-04-05"^^xsd:date ;
                                            rdfs:comment """Relates the class train detection system with the class that represents the section with train detection limitation. 
Specific for route compatibility check on French network."""@en ;
                                            rdfs:isDefinedBy <http://data.europa.eu/949/> ;
                                            rdfs:label "Section with train detection limitation, only for the French network"@en ;
                                            vs:term_status "stable" .


###  http://data.europa.eu/949/tdsMaximumMagneticField
era:tdsMaximumMagneticField rdf:type owl:ObjectProperty ;
                            rdfs:domain era:TrainDetectionSystem ;
                            rdfs:range era:MaximumMagneticField ;
                            era:rinfIndex "1.1.1.3.4.2.3" ,
                                          "1.2.1.1.3.2.3" ;
                            dct:created "2023-03-14"^^xsd:date ;
                            rdfs:comment """Relates the TrainDetectionSystem with the MaximumMagneticField.
The maximum magnetic field limits allowed for axle counters (in dBÂµA/m) for a defined frequency band.
It should be provided in 3 directions."""@en ;
                            rdfs:isDefinedBy <http://data.europa.eu/949/> ;
                            rdfs:label "Train detection system maximum magnetic field"@en ;
                            vs:term_status "stable" .


###  http://data.europa.eu/949/tdsMinAxleLoadVehicleCategory
era:tdsMinAxleLoadVehicleCategory rdf:type owl:ObjectProperty ;
                                  rdfs:domain era:TrainDetectionSystem ;
                                  rdfs:range era:MinAxleLoadVehicleCategory ;
                                  era:rinfIndex "1.1.1.3.7.11.1" ;
                                  dct:created "2023-01-25"^^xsd:date ;
                                  dct:modified "2023-03-14"^^xsd:date ;
                                  rdfs:comment "Deprecated according to the ammendment to the Regulation (EU) 2019/777. Indication of load given in tons depending of the category of vehicle."@en ;
                                  rdfs:isDefinedBy <http://data.europa.eu/949/> ;
                                  rdfs:label "Train detection system min axle load vehicle category"@en ;
                                  owl:deprecated "true"^^xsd:boolean ;
                                  vs:term_status "stable" .


###  http://data.europa.eu/949/temperatureRange
era:temperatureRange rdf:type owl:ObjectProperty ;
                     rdfs:domain [ rdf:type owl:Class ;
                                   owl:unionOf ( era:SubsetWithCommonCharacteristics
                                                 era:Track
                                               )
                                 ] ;
                     rdfs:range skos:Concept ;
                     era:inSkosConceptScheme <http://data.europa.eu/949/concepts/temperature-ranges/TemperatureRanges> ;
                     era:rinfIndex "1.1.1.1.2.6" ;
                     era:usedInRCCCalculations "true"^^xsd:boolean ;
                     dct:created "2023-01-20"^^xsd:date ;
                     rdfs:comment "Temperature range for unrestricted access to the line according European standard. The allowed values for this property belong to the SKOS Concept Scheme http://data.europa.eu/949/concepts/temperature-ranges/TemperatureRanges"@en ;
                     rdfs:isDefinedBy <http://data.europa.eu/949/> ;
                     rdfs:label "Temperature range"@en ;
                     vs:term_status "stable" .


###  http://data.europa.eu/949/tenClassification
era:tenClassification rdf:type owl:ObjectProperty ;
                      rdfs:domain [ rdf:type owl:Class ;
                                    owl:unionOf ( era:Platform
                                                  era:Siding
                                                  era:Track
                                                )
                                  ] ;
                      rdfs:range skos:Concept ;
                      era:inSkosConceptScheme <http://data.europa.eu/949/concepts/ten-classifications/TENClassifications> ;
                      era:rinfIndex "1.1.1.1.2.1" ,
                                    "1.2.1.0.2.1" ,
                                    "1.2.1.0.6.3" ,
                                    "1.2.2.0.0.3" ;
                      dct:created "2021-08-02"^^xsd:date ;
                      dct:modified "2021-09-10"^^xsd:date ;
                      rdfs:comment "Indication of the part of the trans-European network the line belongs to. The allowed values for this property belong to the SKOS Concept Scheme http://data.europa.eu/949/concepts/ten-classifications/TENClassifications."@en ;
                      rdfs:isDefinedBy <http://data.europa.eu/949/> ;
                      rdfs:label "TEN classification (of track, of platform, of siding)"@en ;
                      vs:term_status "stable" .


###  http://data.europa.eu/949/thermalCapacityTSIReference
era:thermalCapacityTSIReference rdf:type owl:ObjectProperty ,
                                         owl:FunctionalProperty ;
                                rdfs:domain era:VehicleType ;
                                rdfs:range skos:Concept ;
                                era:eratvIndex "4.7.2.1.1" ;
                                era:inSkosConceptScheme <http://data.europa.eu/949/concepts/thermal-capacity/ThermalCapacityTSIReferences> ;
                                dct:created "2020-08-24"^^xsd:date ;
                                dct:modified "2021-08-02"^^xsd:date ;
                                rdfs:comment "Reference case of a TSI thermal capacity. The allowed values for this property belong to the SKOS Concept Scheme http://data.europa.eu/949/concepts/thermal-capacity/ThermalCapacityTSIReferences"@en ;
                                rdfs:isDefinedBy <http://data.europa.eu/949/> ;
                                rdfs:label "Thermal capacity TSI reference"@en ;
                                vs:term_status "stable" .


###  http://data.europa.eu/949/track
era:track rdf:type owl:ObjectProperty ;
          rdfs:domain [ rdf:type owl:Class ;
                        owl:unionOf ( era:OperationalPoint
                                      era:SectionOfLine
                                      era:Signal
                                    )
                      ] ;
          rdfs:range era:Track ;
          dct:created "2021-08-09"^^xsd:date ;
          dct:modified "2021-09-09"^^xsd:date ;
          rdfs:comment "Reference to a related railway track."@en ;
          rdfs:isDefinedBy <http://data.europa.eu/949/> ;
          rdfs:label "Track"@en ;
          vs:term_status "stable" .


###  http://data.europa.eu/949/trackDirection
era:trackDirection rdf:type owl:ObjectProperty ,
                            owl:FunctionalProperty ;
                   rdfs:domain era:Track ;
                   rdfs:range skos:Concept ;
                   era:appendixD2Index "2.2.1.1" ;
                   era:inSkosConceptScheme <http://data.europa.eu/949/concepts/track-running-directions/TrackRunningDirections> ;
                   era:rinfIndex "1.1.1.0.0.2" ;
                   dct:created "2021-09-09"^^xsd:date ;
                   dct:modified "2023-03-14"^^xsd:date ;
                   rdfs:comment """The normal running direction is:
- The same as the direction defined by the start and end of the SoL: (N)
- The opposite to the direction defined by the start and end of the SoL: (O)
- Both directions: (B)
The allowed values for this property belong to the SKOS Concept Scheme http://data.europa.eu/949/concepts/track-running-directions/TrackRunningDirections."""@en ;
                   rdfs:isDefinedBy <http://data.europa.eu/949/> ;
                   rdfs:label "Normal running direction"@en ;
                   vs:term_status "stable" .


###  http://data.europa.eu/949/trackLoadCapability
era:trackLoadCapability rdf:type owl:ObjectProperty ;
                        rdfs:subPropertyOf owl:topObjectProperty ;
                        rdfs:domain [ rdf:type owl:Class ;
                                      owl:unionOf ( era:SubsetWithCommonCharacteristics
                                                    era:Track
                                                  )
                                    ] ;
                        rdfs:range era:LoadCapability ;
                        era:rinfIndex "1.1.1.1.2.4" ;
                        era:usedInRCCCalculations "true"^^xsd:boolean ;
                        dct:created "2023-01-20"^^xsd:date ;
                        rdfs:comment "Relates the track with the class LoadCapability. A combination of the line category and speed at the weakest point of the track."@en ;
                        rdfs:isDefinedBy <http://data.europa.eu/949/> ;
                        rdfs:label "Track load capability"@en ;
                        vs:term_status "stable" .


###  http://data.europa.eu/949/trackPhaseInfo
era:trackPhaseInfo rdf:type owl:ObjectProperty ;
                   rdfs:domain [ rdf:type owl:Class ;
                                 owl:unionOf ( era:SubsetWithCommonCharacteristics
                                               era:Track
                                             )
                               ] ;
                   rdfs:range era:PhaseInfo ;
                   era:rinfIndex "1.1.1.2.4.1.2" ;
                   dct:created "2023-04-05"^^xsd:date ;
                   rdfs:comment "Relates the Track with PhaseInfo. Indication of required several information on phase separation."@en ;
                   rdfs:isDefinedBy <http://data.europa.eu/949/> ;
                   rdfs:label "Track phase info"@en ;
                   vs:term_status "stable" .


###  http://data.europa.eu/949/trackRaisedPantographsDistanceAndSpeed
era:trackRaisedPantographsDistanceAndSpeed rdf:type owl:ObjectProperty ;
                                           rdfs:domain [ rdf:type owl:Class ;
                                                         owl:unionOf ( era:SubsetWithCommonCharacteristics
                                                                       era:Track
                                                                     )
                                                       ] ;
                                           rdfs:range era:RaisedPantographsDistanceAndSpeed ;
                                           era:rinfIndex "1.1.1.2.3.3" ;
                                           era:usedInRCCCalculations "true"^^xsd:boolean ;
                                           dct:created "2023-04-05" ;
                                           rdfs:comment "Relates the track with the class RaisePantporaphsDistanceAndSpeed. Indication of maximum number of raised pantographs per train allowed and minimum spacing centre line to centre line of adjacent pantograph heads, expressed in metres, at the given speed."@en ;
                                           rdfs:isDefinedBy <http://data.europa.eu/949/> ;
                                           rdfs:label "Track raised pantograph distance and speed"@en ;
                                           vs:term_status "stable" .


###  http://data.europa.eu/949/trackSystemSeparationInfo
era:trackSystemSeparationInfo rdf:type owl:ObjectProperty ;
                              rdfs:domain [ rdf:type owl:Class ;
                                            owl:unionOf ( era:SubsetWithCommonCharacteristics
                                                          era:Track
                                                        )
                                          ] ;
                              rdfs:range era:SystemSeparationInfo ;
                              era:rinfIndex "1.1.1.2.4.2.2" ;
                              dct:created "2023-04-05"^^xsd:date ;
                              rdfs:comment "Relates the Track with the SystemSeparationInfo. Indication of required several information on system separation."@en ;
                              rdfs:isDefinedBy <http://data.europa.eu/949/> ;
                              rdfs:label "Track system separation info"@en ;
                              vs:term_status "stable" .


###  http://data.europa.eu/949/trainDetectionSystem
era:trainDetectionSystem rdf:type owl:ObjectProperty ;
                         rdfs:domain [ rdf:type owl:Class ;
                                       owl:unionOf ( era:SubsetWithCommonCharacteristics
                                                     era:Track
                                                   )
                                     ] ;
                         rdfs:range era:TrainDetectionSystem ;
                         dct:created "2020-07-29"^^xsd:date ;
                         dct:modified "2021-09-12"^^xsd:date ;
                         rdfs:comment "Train detection systems installed in the section of line."@en ;
                         rdfs:isDefinedBy <http://data.europa.eu/949/> ;
                         rdfs:label "Train detection system"@en ;
                         vs:term_status "stable" .


###  http://data.europa.eu/949/trainDetectionSystemSpecificCheck
era:trainDetectionSystemSpecificCheck rdf:type owl:ObjectProperty ;
                                      rdfs:domain era:TrainDetectionSystem ;
                                      rdfs:range skos:Concept ;
                                      era:inSkosConceptScheme <http://data.europa.eu/949/concepts/train-detection-specific-checks/TrainDetectionSystemsSpecificChecks> ;
                                      era:rinfIndex "1.1.1.3.7.1.2" ,
                                                    "1.2.1.1.6.1" ;
                                      era:usedInRCCCalculations "true"^^xsd:boolean ;
                                      dct:created "2020-08-24"^^xsd:date ;
                                      dct:modified "2021-08-08"^^xsd:date ;
                                      rdfs:comment "Reference to the technical specification of train detection system, in accordance with the specification referenced in Appendix A-1, index [D]. The allowed values for this property belong to the SKOS Concept Scheme http://data.europa.eu/949/concepts/train-detection-specific-checks/TrainDetectionSystemsSpecificChecks"@en ;
                                      rdfs:isDefinedBy <http://data.europa.eu/949/> ;
                                      rdfs:label "Type of track circuits to which specific checks are needed"@en ;
                                      vs:term_status "stable" .


###  http://data.europa.eu/949/trainDetectionSystemType
era:trainDetectionSystemType rdf:type owl:ObjectProperty ;
                             rdfs:domain [ rdf:type owl:Class ;
                                           owl:unionOf ( era:TrainDetectionSystem
                                                         era:VehicleType
                                                       )
                                         ] ;
                             rdfs:range skos:Concept ;
                             era:eratvIndex "4.14.1" ;
                             era:inSkosConceptScheme <http://data.europa.eu/949/concepts/train-detection/TrainDetectionSystems> ;
                             era:rinfIndex "1.1.1.3.7.1.1" ,
                                           "1.2.1.1.3.1.1" ;
                             era:usedInRCCCalculations "true"^^xsd:boolean ;
                             dct:created "2021-08-07"^^xsd:date ;
                             dct:modified "2021-08-07"^^xsd:date ;
                             rdfs:comment "Indication of types of train detection systems installed. The allowed values for this property belong to the SKOS Concept Scheme http://data.europa.eu/949/concepts/train-detection/TrainDetectionSystems"@en ;
                             rdfs:isDefinedBy <http://data.europa.eu/949/> ;
                             rdfs:label "Type of train detection system"@en ;
                             vs:term_status "stable" .


###  http://data.europa.eu/949/tsiCompliantCompositeBrakeBlocks
era:tsiCompliantCompositeBrakeBlocks rdf:type owl:ObjectProperty ;
                                     rdfs:domain era:TrainDetectionSystem ;
                                     rdfs:range skos:Concept ;
                                     era:inSkosConceptScheme <http://data.europa.eu/949/concepts/tsi-compliances/TSICompliances> ;
                                     era:rinfIndex "1.1.1.3.7.21" ;
                                     dct:created "2021-08-08"^^xsd:date ;
                                     dct:modified "2023-03-14"^^xsd:date ;
                                     rdfs:comment "Deprecated according to the ammendment to the Regulation (EU) 2019/777. TSI compliance of rules on the use of composite brake blocks. The allowed values for this property belong to the SKOS Concept Scheme http://data.europa.eu/949/concepts/tsi-compliances/TSICompliances."@en ;
                                     rdfs:isDefinedBy <http://data.europa.eu/949/> ;
                                     rdfs:label "TSI compliance of rules on the use of composite brake blocks"@en ;
                                     owl:deprecated "true"^^xsd:boolean ;
                                     vs:term_status "stable" .


###  http://data.europa.eu/949/tsiCompliantFerromagneticWheel
era:tsiCompliantFerromagneticWheel rdf:type owl:ObjectProperty ;
                                   rdfs:domain era:TrainDetectionSystem ;
                                   rdfs:range skos:Concept ;
                                   era:inSkosConceptScheme <http://data.europa.eu/949/concepts/tsi-compliances/TSICompliances> ;
                                   era:rinfIndex "1.1.1.3.7.14" ;
                                   dct:created "2021-08-08"^^xsd:date ;
                                   dct:modified "2023-03-14"^^xsd:date ;
                                   rdfs:comment """Deprecated according to the ammendment to the Regulation (EU) 2019/777.TSI compliance of Ferromagnetic characteristics of wheel material required. The allowed values for this property belong to the SKOS Concept Scheme http://data.europa.eu/949/concepts/tsi-compliances/TSICompliances.

The concept scheme is temporarily non-deferenceable."""@en ;
                                   rdfs:isDefinedBy <http://data.europa.eu/949/> ;
                                   rdfs:label "TSI compliance of Ferromagnetic characteristics of wheel material required"@en ;
                                   owl:deprecated "true"^^xsd:boolean ;
                                   vs:term_status "stable" .


###  http://data.europa.eu/949/tsiCompliantMaxDistConsecutiveAxles
era:tsiCompliantMaxDistConsecutiveAxles rdf:type owl:ObjectProperty ;
                                        rdfs:domain era:TrainDetectionSystem ;
                                        rdfs:range skos:Concept ;
                                        era:inSkosConceptScheme <http://data.europa.eu/949/concepts/tsi-compliances/TSICompliances> ;
                                        era:rinfIndex "1.1.1.3.7.2.1" ;
                                        dct:created "2021-08-07"^^xsd:date ;
                                        dct:modified "2023-03-14"^^xsd:date ;
                                        rdfs:comment "Deprecated according to the ammendment to the Regulation (EU) 2019/777. Indication whether required distance between two consecutive axles is compliant with the TSI. The allowed values for this property belong to the SKOS Concept Scheme http://data.europa.eu/949/concepts/tsi-compliances/TSICompliances."@en ;
                                        rdfs:isDefinedBy <http://data.europa.eu/949/> ;
                                        rdfs:label "TSI compliance of maximum permitted distance between two consecutive axles"@en ;
                                        owl:deprecated "true"^^xsd:boolean ;
                                        vs:term_status "stable" .


###  http://data.europa.eu/949/tsiCompliantMaxImpedanceWheelset
era:tsiCompliantMaxImpedanceWheelset rdf:type owl:ObjectProperty ;
                                     rdfs:domain era:TrainDetectionSystem ;
                                     rdfs:range skos:Concept ;
                                     era:inSkosConceptScheme <http://data.europa.eu/949/concepts/tsi-compliances/TSICompliances> ;
                                     era:rinfIndex "1.1.1.3.7.15.1" ;
                                     dct:created "2021-08-08"^^xsd:date ;
                                     dct:modified "2023-03-14"^^xsd:date ;
                                     rdfs:comment "Deprecated according to the ammendment to the Regulation (EU) 2019/777. TSI compliance of maximum permitted impedance between opposite wheels of a wheelset. The allowed values for this property belong to the SKOS Concept Scheme http://data.europa.eu/949/concepts/tsi-compliances/TSICompliances."@en ;
                                     rdfs:isDefinedBy <http://data.europa.eu/949/> ;
                                     rdfs:label "TSI compliance of maximum permitted impedance between opposite wheels of a wheelset"@en ;
                                     owl:deprecated "true"^^xsd:boolean ;
                                     vs:term_status "stable" .


###  http://data.europa.eu/949/tsiCompliantMetalConstruction
era:tsiCompliantMetalConstruction rdf:type owl:ObjectProperty ;
                                  rdfs:domain era:TrainDetectionSystem ;
                                  rdfs:range skos:Concept ;
                                  era:inSkosConceptScheme <http://data.europa.eu/949/concepts/tsi-compliances/TSICompliances> ;
                                  era:rinfIndex "1.1.1.3.7.13" ;
                                  dct:created "2021-08-08"^^xsd:date ;
                                  dct:modified "2023-03-14"^^xsd:date ;
                                  rdfs:comment "Deprecated according to the ammendment to the Regulation (EU) 2019/777. TSI compliance of rules for vehicle metal construction. The allowed values for this property belong to the SKOS Concept Scheme http://data.europa.eu/949/concepts/tsi-compliances/TSICompliances."@en ;
                                  rdfs:isDefinedBy <http://data.europa.eu/949/> ;
                                  rdfs:label "TSI compliance of rules for vehicle metal construction"@en ;
                                  owl:deprecated "true"^^xsd:boolean ;
                                  vs:term_status "stable" .


###  http://data.europa.eu/949/tsiCompliantMetalFreeSpace
era:tsiCompliantMetalFreeSpace rdf:type owl:ObjectProperty ;
                               rdfs:domain era:TrainDetectionSystem ;
                               rdfs:range skos:Concept ;
                               era:inSkosConceptScheme <http://data.europa.eu/949/concepts/tsi-compliances/TSICompliances> ;
                               era:rinfIndex "1.1.1.3.7.12" ;
                               dct:created "2021-08-08"^^xsd:date ;
                               dct:modified "2023-03-14"^^xsd:date ;
                               rdfs:comment "Deprecated according to the ammendment to the Regulation (EU) 2019/777. TSI compliance of rules for metal-free space around wheels. The allowed values for this property belong to the SKOS Concept Scheme http://data.europa.eu/949/concepts/tsi-compliances/TSICompliances."@en ;
                               rdfs:isDefinedBy <http://data.europa.eu/949/> ;
                               rdfs:label "TSI compliance of rules for metal-free space around wheels"@en ;
                               owl:deprecated "true"^^xsd:boolean ;
                               vs:term_status "stable" .


###  http://data.europa.eu/949/tsiCompliantRSTShuntImpedance
era:tsiCompliantRSTShuntImpedance rdf:type owl:ObjectProperty ;
                                  rdfs:domain era:TrainDetectionSystem ;
                                  rdfs:range skos:Concept ;
                                  era:inSkosConceptScheme <http://data.europa.eu/949/concepts/tsi-compliances/TSICompliances> ;
                                  era:rinfIndex "1.1.1.3.7.23" ;
                                  dct:created "2021-08-08"^^xsd:date ;
                                  dct:modified "2023-03-14"^^xsd:date ;
                                  rdfs:comment "Deprecated according to the ammendment to the Regulation (EU) 2019/777. TSI compliance of rules on combination of RST characteristics influencing shunting impedance. The allowed values for this property belong to the SKOS Concept Scheme http://data.europa.eu/949/concepts/tsi-compliances/TSICompliances."@en ;
                                  rdfs:isDefinedBy <http://data.europa.eu/949/> ;
                                  rdfs:label "TSI compliance of rules on combination of RST characteristics influencing shunting impedance"@en ;
                                  owl:deprecated "true"^^xsd:boolean ;
                                  vs:term_status "stable" .


###  http://data.europa.eu/949/tsiCompliantSandCharacteristics
era:tsiCompliantSandCharacteristics rdf:type owl:ObjectProperty ;
                                    rdfs:domain era:TrainDetectionSystem ;
                                    rdfs:range skos:Concept ;
                                    era:inSkosConceptScheme <http://data.europa.eu/949/concepts/tsi-compliances/TSICompliances> ;
                                    era:rinfIndex "1.1.1.3.7.19" ;
                                    dct:created "2021-08-08"^^xsd:date ;
                                    dct:modified "2023-03-14"^^xsd:date ;
                                    rdfs:comment "Deprecated according to the ammendment to the Regulation (EU) 2019/777. TSI Compliance of rules on sand characteristics. The allowed values for this property belong to the SKOS Concept Scheme http://data.europa.eu/949/concepts/tsi-compliances/TSICompliances."@en ;
                                    rdfs:isDefinedBy <http://data.europa.eu/949/> ;
                                    rdfs:label "TSI Compliance of rules on sand characteristics"@en ;
                                    owl:deprecated "true"^^xsd:boolean ;
                                    vs:term_status "stable" .


###  http://data.europa.eu/949/tsiCompliantSanding
era:tsiCompliantSanding rdf:type owl:ObjectProperty ;
                        rdfs:domain era:TrainDetectionSystem ;
                        rdfs:range skos:Concept ;
                        era:inSkosConceptScheme <http://data.europa.eu/949/concepts/tsi-compliances/TSICompliances> ;
                        era:rinfIndex "1.1.1.3.7.16" ;
                        dct:created "2021-08-08"^^xsd:date ;
                        dct:modified "2023-03-14"^^xsd:date ;
                        rdfs:comment "Deprecated according to the ammendment to the Regulation (EU) 2019/777. TSI compliance of sanding rules to allow compatibility with track circuits. Too much sand brings the risk of not detecting trains in tracks equipped with track circuits. The allowed values for this property belong to the SKOS Concept Scheme http://data.europa.eu/949/concepts/tsi-compliances/TSICompliances."@en ;
                        rdfs:isDefinedBy <http://data.europa.eu/949/> ;
                        rdfs:label "TSI compliance of sanding"@en ;
                        owl:deprecated "true"^^xsd:boolean ;
                        vs:term_status "unstable" .


###  http://data.europa.eu/949/tsiCompliantShuntDevices
era:tsiCompliantShuntDevices rdf:type owl:ObjectProperty ;
                             rdfs:domain era:TrainDetectionSystem ;
                             rdfs:range skos:Concept ;
                             era:inSkosConceptScheme <http://data.europa.eu/949/concepts/tsi-compliances/TSICompliances> ;
                             era:rinfIndex "1.1.1.3.7.22" ;
                             dct:created "2021-08-08"^^xsd:date ;
                             dct:modified "2023-03-14"^^xsd:date ;
                             rdfs:comment "Deprecated according to the ammendment to the Regulation (EU) 2019/777. TSI compliance of rules on shunt assisting devices. The allowed values for this property belong to the SKOS Concept Scheme http://data.europa.eu/949/concepts/tsi-compliances/TSICompliances."@en ;
                             rdfs:isDefinedBy <http://data.europa.eu/949/> ;
                             rdfs:label "TSI compliance of rules on shunt assisting devices"@en ;
                             owl:deprecated "true"^^xsd:boolean ;
                             vs:term_status "stable" .


###  http://data.europa.eu/949/tsiPantographHead
era:tsiPantographHead rdf:type owl:ObjectProperty ;
                      rdfs:domain [ rdf:type owl:Class ;
                                    owl:unionOf ( era:SubsetWithCommonCharacteristics
                                                  era:Track
                                                )
                                  ] ;
                      rdfs:range skos:Concept ;
                      era:inSkosConceptScheme <http://data.europa.eu/949/concepts/compliant-pantograph-heads/CompliantPantographHeads> ;
                      era:rinfIndex "1.1.1.2.3.1" ;
                      era:usedInRCCCalculations "true"^^xsd:boolean ;
                      dct:created "2020-08-25"^^xsd:date ;
                      dct:modified "2021-09-11"^^xsd:date ;
                      rdfs:comment "Indication of TSI compliant pantograph heads which are allowed to be used. The allowed values for this property belong to the SKOS Concept Scheme http://data.europa.eu/949/concepts/compliant-pantograph-heads/CompliantPantographHeads."@en ;
                      rdfs:isDefinedBy <http://data.europa.eu/949/> ;
                      rdfs:label "Accepted TSI compliant pantograph heads"@en ;
                      vs:term_status "stable" .


###  http://data.europa.eu/949/typeVersionId
era:typeVersionId rdf:type owl:ObjectProperty ;
                  rdfs:domain era:VehicleType ;
                  rdfs:range skos:Concept ;
                  era:inSkosConceptScheme <http://data.europa.eu/949/concepts/version-ids/VehicleTypeVersionIds> ;
                  dct:created "2022-11-03"^^xsd:date ;
                  rdfs:comment """Indicates the registrationVersion with Ids 10,20 and 30 indicating registration according to Directive 2008/57/EC and implementing Decision 2011/665/EU, and 40 and 50 indicating registration according to regime described in Directive 2008/57/EC.
The allowed values for this property belong to the SKOS Concept Scheme http://data.europa.eu/949/concepts/type-version-ids/TypeVersionIds."""@en ;
                  rdfs:isDefinedBy <http://data.europa.eu/949/> ;
                  rdfs:label "Type version id"@en ;
                  vs:term_status "stable" .


###  http://data.europa.eu/949/vehicleKeeper
era:vehicleKeeper rdf:type owl:ObjectProperty ;
                  rdfs:domain era:Vehicle ;
                  rdfs:range era:VehicleKeeper ;
                  dct:created "2020-11-23"^^xsd:date ;
                  dct:modified "2020-11-23"^^xsd:date ;
                  rdfs:comment "Indicates the organization that owns/operated a vehicle or wagon."@en ;
                  rdfs:isDefinedBy <http://data.europa.eu/949/> ;
                  rdfs:label "Vehicle keeper"@en ;
                  vs:term_status "stable" .


###  http://data.europa.eu/949/vehicleType
era:vehicleType rdf:type owl:ObjectProperty ;
                rdfs:domain era:Vehicle ;
                rdfs:range era:VehicleType ;
                dct:created "2020-11-22"^^xsd:date ;
                dct:modified "2020-11-22"^^xsd:date ;
                rdfs:comment "Indicates the vehicle type of a specific vehicle or wagon."@en ;
                rdfs:isDefinedBy <http://data.europa.eu/949/> ;
                rdfs:label "Vehicle type"@en ;
                vs:term_status "stable" .


###  http://data.europa.eu/949/vehicleTypeMaximumSpeedAndCantDeficiency
era:vehicleTypeMaximumSpeedAndCantDeficiency rdf:type owl:ObjectProperty ;
                                             rdfs:domain era:VehicleType ;
                                             rdfs:range era:MaximumSpeedAndCantDeficiency ;
                                             era:eratvIndex "4.6.4" ;
                                             dct:created "2023-04-05"^^xsd:date ;
                                             rdfs:comment "Relates the vehicle type with its values of maximum speed and cant deficiency."@en ;
                                             rdfs:isDefinedBy <http://data.europa.eu/949/> ;
                                             rdfs:label "Vehicle type maximum speed and cant deficiency"@en ;
                                             vs:term_status "stable" .


###  http://data.europa.eu/949/voiceGSMRNetwork
era:voiceGSMRNetwork rdf:type owl:ObjectProperty ,
                              owl:FunctionalProperty ;
                     rdfs:domain era:VehicleType ;
                     rdfs:range skos:Concept ;
                     era:eratvIndex "4.13.2.10" ;
                     era:inSkosConceptScheme <http://data.europa.eu/949/concepts/gsmr-networks/GSMRNetworks> ;
                     dct:created "2020-08-31"^^xsd:date ;
                     dct:modified "2021-08-02"^^xsd:date ;
                     rdfs:comment "Voice SIM Card GSM-R Home Network. The allowed values for this property belong to the SKOS Concept Scheme http://data.europa.eu/949/concepts/gsmr-networks/GSMRNetworks"@en ;
                     rdfs:isDefinedBy <http://data.europa.eu/949/> ;
                     rdfs:label "Voice GSM-R network"@en ;
                     vs:term_status "stable" .


###  http://data.europa.eu/949/voiceRadioCompatible
era:voiceRadioCompatible rdf:type owl:ObjectProperty ;
                         rdfs:domain [ rdf:type owl:Class ;
                                       owl:unionOf ( era:Track
                                                     era:VehicleType
                                                   )
                                     ] ;
                         rdfs:range skos:Concept ;
                         era:eratvIndex "4.13.2.5" ;
                         era:inSkosConceptScheme <http://data.europa.eu/949/concepts/voice-radio-system-compatibilities/VoiceRadioSystemCompatibilities> ;
                         era:rinfIndex "1.1.1.3.3.9" ,
                                       "1.2.1.1.2.9" ;
                         dct:created "2020-08-31"^^xsd:date ;
                         dct:modified "2021-09-12"^^xsd:date ;
                         rdfs:comment """Radio requirements used for demonstrating technical compatibility voice.
 The allowed values for this property belong to the SKOS Concept Scheme http://data.europa.eu/949/concepts/voice-radio-system-compatibilities/VoiceRadioSystemCompatibilities. This concept scheme is temporatily non-deferenceable."""@en ;
                         rdfs:isDefinedBy <http://data.europa.eu/949/> ;
                         rdfs:label "Radio system compatibility voice"@en ;
                         vs:term_status "stable" .


###  http://data.europa.eu/949/wheelSetGauge
era:wheelSetGauge rdf:type owl:ObjectProperty ,
                           owl:FunctionalProperty ;
                  rdfs:domain [ rdf:type owl:Class ;
                                owl:unionOf ( era:Track
                                              era:VehicleType
                                            )
                              ] ;
                  rdfs:range skos:Concept ;
                  era:eratvIndex "4.1.3" ;
                  era:inSkosConceptScheme <http://data.europa.eu/949/concepts/nominal-track-gauges/NominalTrackGauges> ;
                  era:rinfIndex "1.1.1.1.4.1" ,
                                "1.2.1.0.4.1" ;
                  era:usedInRCCCalculations "true"^^xsd:boolean ;
                  dct:created "2020-07-29"^^xsd:date ;
                  dct:modified "2021-09-10"^^xsd:date ;
                  rdfs:comment "A single value expressed in millimetres that identifies the track and vehicle wheel set gauge. The allowed values for this property belong to the SKOS Concept Scheme http://data.europa.eu/949/concepts/nominal-track-gauges/NominalTrackGauges"@en ;
                  rdfs:isDefinedBy <http://data.europa.eu/949/> ;
                  rdfs:label "Nominal track gauge"@en ;
                  vs:term_status "stable" .


###  http://data.europa.eu/949/wheelSetGaugeChangeoverFacility
era:wheelSetGaugeChangeoverFacility rdf:type owl:ObjectProperty ,
                                             owl:FunctionalProperty ;
                                    rdfs:domain era:VehicleType ;
                                    rdfs:range skos:Concept ;
                                    era:eratvIndex "4.1.11" ;
                                    era:inSkosConceptScheme <http://data.europa.eu/949/concepts/gauge-changeover-facilities/GaugeChangeoverFacilities> ;
                                    dct:created "2020-09-01"^^xsd:date ;
                                    dct:modified "2021-08-25"^^xsd:date ;
                                    rdfs:comment "Wheelset gauge changeover facility. The allowed values for this property belong to the SKOS Concept Scheme http://data.europa.eu/949/concepts/gauge-changeover-facilities/GaugeChangeoverFacilities"@en ;
                                    rdfs:isDefinedBy <http://data.europa.eu/949/> ;
                                    rdfs:label "Wheelset gauge changeover facility"@en ;
                                    vs:term_status "stable" .


###  http://www.opengis.net/ont/geosparql#hasGeometry
gsp:hasGeometry rdf:type owl:ObjectProperty ;
                era:rinfIndex "1.1.0.0.1.1" ,
                              "1.1.1.0.1.1" ,
                              "1.1.1.3.14.6" ,
                              "1.2.0.0.0.5" ,
                              "1.2.1.0.8.5" ;
                era:usedInRCCCalculations "true"^^xsd:boolean .


###  http://www.w3.org/2003/01/geo/wgs84_pos#location
wgs:location rdf:type owl:ObjectProperty .


#################################################################
#    Data properties
#################################################################

###  http://data.europa.eu/949/IdPhoneErtmsRadioBlockCenter
era:IdPhoneErtmsRadioBlockCenter rdf:type owl:DatatypeProperty ;
                                 rdfs:domain [ rdf:type owl:Class ;
                                               owl:unionOf ( era:SubsetWithCommonCharacteristics
                                                             era:Track
                                                           )
                                             ] ;
                                 rdfs:range xsd:string ;
                                 era:rinfIndex "1.1.1.3.2.17" ,
                                               "1.2.1.1.1.17" ;
                                 dct:created "2023-03-14"^^xsd:date ;
                                 rdfs:comment "Unique RBC identification (NID_C+NID_RBC) and calling number (NID_RADIO) as defined in the specification referenced in Appendix A-1, index [C]."@en ;
                                 rdfs:isDefinedBy <http://data.europa.eu/949/> ;
                                 rdfs:label "ID and phone number of ERTMS/ETCS Radio Block Center"@en ;
                                 vs:term_status "stable" .


###  http://data.europa.eu/949/accelerationLevelCrossing
era:accelerationLevelCrossing rdf:type owl:DatatypeProperty ,
                                       owl:FunctionalProperty ;
                              rdfs:domain [ rdf:type owl:Class ;
                                            owl:unionOf ( era:SubsetWithCommonCharacteristics
                                                          era:Track
                                                        )
                                          ] ;
                              rdfs:range xsd:string ;
                              era:rinfIndex "1.1.1.1.7.3" ;
                              dct:created "2021-08-03"^^xsd:date ;
                              dct:modified "2021-09-11"^^xsd:date ;
                              rdfs:comment "Existence of limit for acceleration of train if stopping or recovering speed close to a level crossing expressed in a specific reference acceleration curve."@en ;
                              rdfs:isDefinedBy <http://data.europa.eu/949/> ;
                              rdfs:label "Acceleration allowed at level crossing"@en ;
                              vs:term_status "stable" .


###  http://data.europa.eu/949/additionalBrakingInformationDocument
era:additionalBrakingInformationDocument rdf:type owl:DatatypeProperty ;
                                         rdfs:domain [ rdf:type owl:Class ;
                                                       owl:unionOf ( era:SubsetWithCommonCharacteristics
                                                                     era:Track
                                                                   )
                                                     ] ;
                                         rdfs:range xsd:anyURI ;
                                         era:rinfIndex "1.1.1.3.11.3" ;
                                         era:usedInRCCCalculations "true"^^xsd:boolean ;
                                         dct:created "2020-08-24"^^xsd:date ;
                                         dct:modified "2021-09-12"^^xsd:date ;
                                         rdfs:comment "Electronic document available in two EU languages from the IM stored by the Agency providing additional information as defined in point (2) of point 4.2.2.6.2 of OPE TSI."@en ;
                                         rdfs:isDefinedBy <http://data.europa.eu/949/> ;
                                         rdfs:label "Documents available by the IM relating to braking performance"@en ;
                                         vs:term_status "stable" .


###  http://data.europa.eu/949/alternativeName
era:alternativeName rdf:type owl:DatatypeProperty ,
                             owl:FunctionalProperty ;
                    rdfs:domain era:VehicleType ;
                    rdfs:range xsd:string ;
                    era:eratvIndex 1.2 ;
                    dct:created "2020-07-29"^^xsd:date ;
                    dct:modified "2020-07-29"^^xsd:date ;
                    rdfs:comment "Alternative name of a vehicle."@en ;
                    rdfs:isDefinedBy <http://data.europa.eu/949/> ;
                    rdfs:label "Alternative name"@en ;
                    vs:term_status "stable" .


###  http://data.europa.eu/949/altitudeRange
era:altitudeRange rdf:type owl:DatatypeProperty ;
                  rdfs:domain era:VehicleType ;
                  rdfs:range xsd:string ;
                  era:eratvIndex "4.3.2" ;
                  dct:created "2021-08-26"^^xsd:date ;
                  dct:modified "2021-08-26"^^xsd:date ;
                  rdfs:comment "Altitude range."@en ;
                  rdfs:isDefinedBy <http://data.europa.eu/949/> ;
                  rdfs:label "Altitude range"@en ;
                  vs:term_status "stable" .


###  http://data.europa.eu/949/altitudeRangeDetail
era:altitudeRangeDetail rdf:type owl:DatatypeProperty ;
                        rdfs:domain era:VehicleType ;
                        rdfs:range xsd:integer ;
                        era:eratvIndex "4.3.2.1" ;
                        dct:created "2021-08-26"^^xsd:date ;
                        dct:modified "2021-08-26"^^xsd:date ;
                        rdfs:comment "Altitude range value for 'X' if value 'AX' is selected in altitude range."@en ;
                        rdfs:isDefinedBy <http://data.europa.eu/949/> ;
                        rdfs:label "Altitude range detail"@en ;
                        vs:term_status "stable" .


###  http://data.europa.eu/949/areaBoardingAid
era:areaBoardingAid rdf:type owl:DatatypeProperty ,
                             owl:FunctionalProperty ;
                    rdfs:domain era:Platform ;
                    rdfs:range xsd:integer ;
                    era:rinfIndex "1.2.1.0.6.7" ;
                    dct:created "2021-08-02"^^xsd:date ;
                    dct:modified "2023-01-20"^^xsd:date ;
                    rdfs:comment "Information of the train access level for which the boarding aid can be used. Data is presented as the vertical difference that is overcome by the platform boarding aid in millimetres. The value â0â means that the platform is not equipped with a platform boarding aid."@en ;
                    rdfs:isDefinedBy <http://data.europa.eu/949/> ;
                    rdfs:label "Information of the train access level for which the boarding aid can be used."@en ;
                    vs:term_status "stable" .


###  http://data.europa.eu/949/assistanceStartingTrain
era:assistanceStartingTrain rdf:type owl:DatatypeProperty ,
                                     owl:FunctionalProperty ;
                            rdfs:domain era:Platform ;
                            rdfs:range xsd:boolean ;
                            era:rinfIndex "1.2.1.0.6.6" ;
                            dct:created "2021-08-02"^^xsd:date ;
                            dct:modified "2021-08-02"^^xsd:date ;
                            rdfs:comment "Indication of existence of equipment or staff supporting the train crew in starting the train."@en ;
                            rdfs:isDefinedBy <http://data.europa.eu/949/> ;
                            rdfs:label "Existence of platform assistance for starting train"@en ;
                            vs:term_status "stable" .


###  http://data.europa.eu/949/atoErrorCorrectionsOnboard
era:atoErrorCorrectionsOnboard rdf:type owl:DatatypeProperty ;
                               rdfs:domain [ rdf:type owl:Class ;
                                             owl:unionOf ( era:SubsetWithCommonCharacteristics
                                                           era:Track
                                                         )
                                           ] ;
                               rdfs:range xsd:anyURI ;
                               era:rinfIndex "1.1.1.3.13.4" ;
                               dct:created "2023-03-14"^^xsd:date ;
                               rdfs:comment "List of unacceptable errors impacting the IM network that are required to be solved in the on-board according to the CCS TSI point 7.2.10.3 specification maintenance point."@en ;
                               rdfs:isDefinedBy <http://data.europa.eu/949/> ;
                               rdfs:label "ATO error corrections required for the on-board"@en ;
                               vs:term_status "stable" .


###  http://data.europa.eu/949/automaticDroppingDeviceRequired
era:automaticDroppingDeviceRequired rdf:type owl:DatatypeProperty ,
                                             owl:FunctionalProperty ;
                                    rdfs:domain [ rdf:type owl:Class ;
                                                  owl:unionOf ( era:SubsetWithCommonCharacteristics
                                                                era:Track
                                                              )
                                                ] ;
                                    rdfs:range xsd:boolean ;
                                    era:rinfIndex "1.1.1.2.5.3" ;
                                    era:usedInRCCCalculations "true"^^xsd:boolean ;
                                    dct:created "2020-08-25"^^xsd:date ;
                                    dct:modified "2021-09-12"^^xsd:date ;
                                    rdfs:comment "Indication of whether an automatic dropping device (ADD) required on the vehicle."@en ;
                                    rdfs:isDefinedBy <http://data.europa.eu/949/> ;
                                    rdfs:label "Automatic dropping device required"@en ;
                                    vs:term_status "stable" .


###  http://data.europa.eu/949/axleSpacing
era:axleSpacing rdf:type owl:DatatypeProperty ,
                         owl:FunctionalProperty ;
                rdfs:domain era:VehicleType ;
                rdfs:range xsd:string ;
                era:eratvIndex "4.5.3.4" ;
                dct:created "2020-08-24"^^xsd:date ;
                dct:modified "2021-08-26"^^xsd:date ;
                rdfs:comment "Position of the axles along the unit. a: Distance between axles; b: Distance from end axle to the end of the nearest coupling plane; c: distance between two inside axles."@en ;
                rdfs:isDefinedBy <http://data.europa.eu/949/> ;
                rdfs:label "Axle spacing"@en ;
                vs:term_status "stable" .


###  http://data.europa.eu/949/bigMetalMass
era:bigMetalMass rdf:type owl:DatatypeProperty ;
                 rdfs:domain [ rdf:type owl:Class ;
                               owl:unionOf ( era:SubsetWithCommonCharacteristics
                                             era:Track
                                           )
                             ] ;
                 rdfs:range xsd:boolean ;
                 era:rinfIndex "1.1.1.3.2.18" ,
                               "1.2.1.1.1.18" ;
                 dct:created "2023-03-14"^^xsd:date ;
                 rdfs:comment "Indication of existence of metal mass in the vicinity of the location, susceptible of perturbating the reading of balises by the on-board system."@en ;
                 rdfs:isDefinedBy <http://data.europa.eu/949/> ;
                 rdfs:label "Big metal mass"@en ;
                 vs:term_status "stable" .


###  http://data.europa.eu/949/boardingAids
era:boardingAids rdf:type owl:DatatypeProperty ;
                 rdfs:domain era:VehicleType ;
                 rdfs:range xsd:string ;
                 era:eratvIndex "4.12.3.2" ;
                 dct:created "2021-08-31"^^xsd:date ;
                 dct:modified "2021-08-31"^^xsd:date ;
                 rdfs:comment "Description of any integrated boarding aids (if provided)."@en ;
                 rdfs:isDefinedBy <http://data.europa.eu/949/> ;
                 rdfs:label "Boarding aids"@en ;
                 vs:term_status "stable" .


###  http://data.europa.eu/949/brakeWeightPercentage
era:brakeWeightPercentage rdf:type owl:DatatypeProperty ,
                                   owl:FunctionalProperty ;
                          rdfs:domain era:VehicleType ;
                          rdfs:range xsd:string ;
                          era:eratvIndex "4.7.6" ;
                          dct:created "2020-08-24"^^xsd:date ;
                          dct:modified "2021-08-26"^^xsd:date ;
                          rdfs:comment "Brake weight percentage (lambda) or Braked mass."@en ;
                          rdfs:isDefinedBy <http://data.europa.eu/949/> ;
                          rdfs:label "Brake weight percentage"@en ;
                          vs:term_status "stable" .


###  http://data.europa.eu/949/bridge
era:bridge rdf:type owl:DatatypeProperty ;
           rdfs:domain era:Track ;
           rdfs:range xsd:boolean ;
           rdfs:isDefinedBy <http://data.europa.eu/949/> ;
           rdfs:label "Is bridge"@en ;
           vs:term_status "stable" ;
           skos:definition "Whether or not a track is associated with a bridge."@en .


###  http://data.europa.eu/949/cantDefficiency
era:cantDefficiency rdf:type owl:DatatypeProperty ;
                    rdfs:domain era:VehicleType ;
                    rdfs:range xsd:integer ;
                    era:eratvIndex "4.6.1" ;
                    dct:created "2021-08-26"^^xsd:date ;
                    dct:modified "2021-08-26"^^xsd:date ;
                    rdfs:comment "Cant deficiency (maximum uncompensated lateral acceleration) for which the vehicle has been assessed. For dual gauge vehicles values for each gauge have to be indicated."@en ;
                    rdfs:isDefinedBy <http://data.europa.eu/949/> ;
                    rdfs:label "Cant defficiency"@en ;
                    vs:term_status "stable" .


###  http://data.europa.eu/949/cantDeficiency
era:cantDeficiency rdf:type owl:DatatypeProperty ,
                            owl:FunctionalProperty ;
                   rdfs:domain [ rdf:type owl:Class ;
                                 owl:unionOf ( era:SubsetWithCommonCharacteristics
                                               era:Track
                                             )
                               ] ;
                   rdfs:range xsd:integer ;
                   era:rinfIndex "1.1.1.1.4.2" ;
                   era:usedInRCCCalculations "true"^^xsd:boolean ;
                   dct:created "2020-08-24"^^xsd:date ;
                   dct:modified "2021-09-10"^^xsd:date ;
                   rdfs:comment "Maximum cant deficiency expressed in millimetres defined as difference between the applied cant and a higher equilibrium cant the line has been designed for."@en ;
                   rdfs:isDefinedBy <http://data.europa.eu/949/> ;
                   rdfs:label "Cant deficiency"@en ;
                   vs:term_status "stable" .


###  http://data.europa.eu/949/catenaryMaxRatedCurrent
era:catenaryMaxRatedCurrent rdf:type owl:DatatypeProperty ;
                            rdfs:domain era:VehicleType ;
                            rdfs:range xsd:double ;
                            era:eratvIndex "4.10.3" ;
                            dct:created "2021-08-31"^^xsd:date ;
                            dct:modified "2021-08-31"^^xsd:date ;
                            rdfs:comment "Maximum rated current from the catenary (to be indicated for each electrical energy supply system the vehicle is equipped for), given in A."@en ;
                            rdfs:isDefinedBy <http://data.europa.eu/949/> ;
                            rdfs:label "Catenary max rated current"@en ;
                            vs:term_status "stable" .


###  http://data.europa.eu/949/compatibilityProcedureDocument
era:compatibilityProcedureDocument rdf:type owl:DatatypeProperty ;
                                   rdfs:domain [ rdf:type owl:Class ;
                                                 owl:unionOf ( era:SubsetWithCommonCharacteristics
                                                               era:Track
                                                             )
                                               ] ;
                                   rdfs:range xsd:anyURI ;
                                   era:rinfIndex "1.1.1.1.2.4.4" ;
                                   era:usedInRCCCalculations "true"^^xsd:boolean ;
                                   dct:created "2023-03-14"^^xsd:date ;
                                   dct:modified "2021-09-10"^^xsd:date ;
                                   rdfs:comment """Electronic document available in two EU languages from the IM stored by the Agency with:
- precise procedures for the static and dynamic route compatibility checks;
Or
- relevant information for carrying out the checks for specific structures."""@en ;
                                   rdfs:isDefinedBy <http://data.europa.eu/949/> ;
                                   rdfs:label "Document with the procedure(s) for static and dynamic route compatibility checks"@en ;
                                   vs:term_status "stable" .


###  http://data.europa.eu/949/complianceInfTsi
era:complianceInfTsi rdf:type owl:DatatypeProperty ,
                              owl:FunctionalProperty ;
                     rdfs:domain era:Tunnel ;
                     rdfs:range xsd:boolean ;
                     era:rinfIndex "1.1.1.1.8.8.1" ;
                     dct:created "2021-08-03"^^xsd:date ;
                     dct:modified "2021-08-03"^^xsd:date ;
                     rdfs:comment "Compliance of the tunnel with INF TSI at the maximum permitted speed."@en ;
                     rdfs:isDefinedBy <http://data.europa.eu/949/> ;
                     rdfs:label "Compliance of the tunnel with INF TSI"@en ;
                     vs:term_status "stable" .


###  http://data.europa.eu/949/compositeBrakeBlockRetrofitted
era:compositeBrakeBlockRetrofitted rdf:type owl:DatatypeProperty ;
                                   rdfs:domain era:Vehicle ;
                                   rdfs:range xsd:boolean ;
                                   dct:created "2020-11-23"^^xsd:date ;
                                   dct:modified "2020-11-23"^^xsd:date ;
                                   rdfs:comment "Indicates if a vehicle's composite brake block is retrofitted"@en ;
                                   rdfs:isDefinedBy <http://data.europa.eu/949/> ;
                                   rdfs:label "Composite brake block retrofitted"@en ;
                                   vs:term_status "stable" .


###  http://data.europa.eu/949/conditionalRegenerativeBrake
era:conditionalRegenerativeBrake rdf:type owl:DatatypeProperty ;
                                 rdfs:domain era:ContactLineSystem ;
                                 rdfs:range xsd:boolean ;
                                 era:rinfIndex "1.1.1.2.2.4" ;
                                 era:usedInRCCCalculations "true"^^xsd:boolean ;
                                 dct:created "2020-08-24"^^xsd:date ;
                                 dct:modified "2023-01-20"^^xsd:date ;
                                 rdfs:comment "Indication whether regenerative braking is permitted, not permitted, or permitted under specific conditions."@en ;
                                 rdfs:isDefinedBy <http://data.europa.eu/949/> ;
                                 rdfs:label "Permission for regenerative braking"@en ;
                                 vs:term_status "stable" .


###  http://data.europa.eu/949/conditionsAppliedRegenerativeBraking
era:conditionsAppliedRegenerativeBraking rdf:type owl:DatatypeProperty ;
                                         rdfs:domain era:ContactLineSystem ;
                                         rdfs:range xsd:anyURI ;
                                         era:appendixD2Index "3.3.7" ;
                                         era:rinfIndex "1.1.1.2.2.4.1" ;
                                         dct:created "2022-11-10"^^xsd:date ;
                                         dct:modified "2023-03-14"^^xsd:date ;
                                         dct:source <https://eur-lex.europa.eu/eli/reg_impl/2019/773/oj> ;
                                         rdfs:comment """Name and/or reference of the document specifying the conditions applying in regards to regenerative braking.
In https://eur-lex.europa.eu/eli/reg_impl/2019/773/oj 3.3.7 Conditions applying with regard to regenerative braking."""@en ;
                                         rdfs:isDefinedBy <http://data.europa.eu/949/> ;
                                         rdfs:label "Conditions applying in regards to regenerative braking"@en ;
                                         vs:term_status "stable" .


###  http://data.europa.eu/949/conditionsChargingElectricEnergyStorage
era:conditionsChargingElectricEnergyStorage rdf:type owl:DatatypeProperty ;
                                            rdfs:domain era:ContactLineSystem ;
                                            rdfs:range xsd:anyURI ;
                                            era:rinfIndex "1.2.1.0.7.2" ;
                                            dct:created "2023-03-14"^^xsd:date ;
                                            rdfs:comment "Conditions set by IMs according to a standardised document."@en ;
                                            rdfs:isDefinedBy <http://data.europa.eu/949/> ;
                                            rdfs:label "Permitted conditions for charging electric energy storage for traction purposes at standstill"@en ;
                                            vs:term_status "stable" .


###  http://data.europa.eu/949/conditionsSwitchClassBSystems
era:conditionsSwitchClassBSystems rdf:type owl:DatatypeProperty ;
                                  rdfs:domain [ rdf:type owl:Class ;
                                                owl:unionOf ( era:SubsetWithCommonCharacteristics
                                                              era:Track
                                                            )
                                              ] ;
                                  rdfs:range xsd:anyURI ;
                                  era:appendixD2Index "3.4.3" ;
                                  era:rinfIndex "1.1.1.3.8.3" ,
                                                "1.2.1.1.7.3" ;
                                  dct:created "2022-10-28"^^xsd:date ;
                                  dct:modified "2023-03-14"^^xsd:date ;
                                  dct:source <https://eur-lex.europa.eu/eli/reg_impl/2019/773/oj> ;
                                  rdfs:comment """Name and/or reference of the document specifying the Special technical conditions required to switch over between ERTMS/ETCS and Class B systems.
In https://eur-lex.europa.eu/eli/reg_impl/2019/773/oj 3.4.3 Special technical conditions required to switch over between ERTMS/ETCS and Class B systems."""@en ;
                                  rdfs:isDefinedBy <http://data.europa.eu/949/> ;
                                  rdfs:label "Special technical conditions required to switch over between ERTMS/ETCS and Class B systems"@en ;
                                  vs:term_status "stable" .


###  http://data.europa.eu/949/conditionsSwitchTrainProtectionSystems
era:conditionsSwitchTrainProtectionSystems rdf:type owl:DatatypeProperty ;
                                           rdfs:domain [ rdf:type owl:Class ;
                                                         owl:unionOf ( era:SubsetWithCommonCharacteristics
                                                                       era:Track
                                                                     )
                                                       ] ;
                                           rdfs:range xsd:anyURI ;
                                           era:appendixD2Index "3.4.2" ;
                                           era:rinfIndex "1.1.1.3.8.1.1" ,
                                                         "1.2.1.1.7.1.1" ;
                                           dct:created "2022-10-28"^^xsd:date ;
                                           dct:source <https://eur-lex.europa.eu/eli/reg_impl/2019/773/oj> ;
                                           rdfs:comment """Conditions to switch over between different class B train protection, control and warning systems.
In https://eur-lex.europa.eu/eli/reg_impl/2019/773/oj 3.4.2 Special conditions to switch over between different class B train protection, control and warning systems."""@en ;
                                           rdfs:isDefinedBy <http://data.europa.eu/949/> ;
                                           rdfs:label "Special conditions to switch over between different class B train protection, control and warning systems"@en ;
                                           vs:term_status "stable" .


###  http://data.europa.eu/949/conditionsTrainFormation
era:conditionsTrainFormation rdf:type owl:DatatypeProperty ;
                             rdfs:domain era:VehicleType ;
                             rdfs:range xsd:string ;
                             era:eratvIndex "4.1.4" ;
                             dct:created "2021-08-25"^^xsd:date ;
                             dct:modified "2021-08-25"^^xsd:date ;
                             rdfs:comment "Conditions of use regarding train formation."@en ;
                             rdfs:isDefinedBy <http://data.europa.eu/949/> ;
                             rdfs:label "Conditions train formation"@en ;
                             vs:term_status "stable" .


###  http://data.europa.eu/949/contactStripMaterialMetallicContent
era:contactStripMaterialMetallicContent rdf:type owl:DatatypeProperty ;
                                        rdfs:domain [ rdf:type owl:Class ;
                                                      owl:unionOf ( era:SubsetWithCommonCharacteristics
                                                                    era:Track
                                                                  )
                                                    ] ;
                                        rdfs:range xsd:integer ;
                                        era:rinfIndex "1.1.1.2.3.4" ;
                                        era:usedInRCCCalculations "true"^^xsd:boolean ;
                                        dct:created "2023-01-25"^^xsd:date ;
                                        rdfs:comment "In case that the value of the property era:contactStripMaterial is \"impregnated carbon\", it is the metallic content in % (this value must be added). This is the maximum percentage allowed."@en ;
                                        rdfs:isDefinedBy <http://data.europa.eu/949/> ;
                                        rdfs:label "Contact strip material metallic content"@en ;
                                        vs:term_status "stable" .


###  http://data.europa.eu/949/crossSectionArea
era:crossSectionArea rdf:type owl:DatatypeProperty ,
                              owl:FunctionalProperty ;
                     rdfs:domain era:Tunnel ;
                     rdfs:range xsd:integer ;
                     era:rinfIndex "1.1.1.1.8.8" ;
                     dct:created "2021-08-03"^^xsd:date ;
                     dct:modified "2021-08-03"^^xsd:date ;
                     rdfs:comment "Smallest cross section area in square metres of the tunnel."@en ;
                     rdfs:isDefinedBy <http://data.europa.eu/949/> ;
                     rdfs:label "Cross section area"@en ;
                     vs:term_status "stable" .


###  http://data.europa.eu/949/currentLimitationRequired
era:currentLimitationRequired rdf:type owl:DatatypeProperty ;
                              rdfs:domain era:ContactLineSystem ;
                              rdfs:range xsd:boolean ;
                              era:rinfIndex "1.1.1.2.5.1" ;
                              era:usedInRCCCalculations "true"^^xsd:boolean ;
                              dct:created "2020-08-25"^^xsd:date ;
                              dct:modified "2021-09-12"^^xsd:date ;
                              rdfs:comment "Indication of whether an on board current or power limitation function on vehicles is required."@en ;
                              rdfs:isDefinedBy <http://data.europa.eu/949/> ;
                              rdfs:label "Current or power limitation on board required"@en ;
                              vs:term_status "stable" .


###  http://data.europa.eu/949/currentlyValid
era:currentlyValid rdf:type owl:DatatypeProperty ;
                   rdfs:domain era:Feature ;
                   rdfs:range xsd:boolean ;
                   dct:created "2022-12-13"^^xsd:date ;
                   rdfs:comment "Indicates whether a feature, e.g. operational point, is currently valid according to its validity start and end dates."@en ;
                   rdfs:isDefinedBy <http://data.europa.eu/949/> ;
                   rdfs:label "Currently valid"@en ;
                   vs:term_status "stable" .


###  http://data.europa.eu/949/dNvovtrp
era:dNvovtrp rdf:type owl:DatatypeProperty ;
             rdfs:domain [ rdf:type owl:Class ;
                           owl:unionOf ( era:SubsetWithCommonCharacteristics
                                         era:Track
                                       )
                         ] ;
             rdfs:range xsd:integer ;
             era:appendixD3Index "1.5.5" ;
             era:rinfIndex "1.1.1.3.2.16.5" ;
             dct:created "2022-11-07"^^xsd:date ;
             dct:modified "2023-03-14"^^xsd:date ;
             rdfs:comment """Maximum distance for overriding the train trip in metres
According to the specification referenced in Appendix A-1, index [C]. 
In Subset 26, chapter 7. 7.5.1.15 D_NVOVTRP https://www.era.europa.eu/sites/default/files/filesystem/ertms/ccs_tsi_annex_a_-_mandatory_specifications/set_of_specifications_3_etcs_b3_r2_gsm-r_b1/index004_-_subset-026_v360.zip."""@en ;
             rdfs:isDefinedBy <http://data.europa.eu/949/> ;
             rdfs:label "D_NVOVTRP"@en ;
             vs:term_status "stable" .


###  http://data.europa.eu/949/dNvpotrp
era:dNvpotrp rdf:type owl:DatatypeProperty ;
             rdfs:domain [ rdf:type owl:Class ;
                           owl:unionOf ( era:SubsetWithCommonCharacteristics
                                         era:Track
                                       )
                         ] ;
             rdfs:range xsd:integer ;
             era:appendixD3Index "1.5.7" ;
             era:rinfIndex "1.1.1.3.2.16.7" ,
                           "1.2.1.1.1.16.7Â " ;
             dct:created "2022-11-07"^^xsd:date ;
             dct:modified "2023-03-14" ;
             rdfs:comment """Maximum distance for reversing in Post Trip mode  in metres. 
According to the specification referenced in Appendix A-1, index [C]. 
In https://www.era.europa.eu/sites/default/files/filesystem/ertms/ccs_tsi_annex_a_-_mandatory_specifications/set_of_specifications_3_etcs_b3_r2_gsm-r_b1/index004_-_subset-026_v360.zip
 Subset 26, chapter 7. 7.5.1.16 D_NVPOTRP."""@en ;
             rdfs:isDefinedBy <http://data.europa.eu/949/> ;
             rdfs:label "D_NVPOTRP"@en ;
             vs:term_status "stable" .


###  http://data.europa.eu/949/dNvroll
era:dNvroll rdf:type owl:DatatypeProperty ;
            rdfs:domain [ rdf:type owl:Class ;
                          owl:unionOf ( era:SubsetWithCommonCharacteristics
                                        era:Track
                                      )
                        ] ;
            rdfs:range xsd:integer ;
            era:appendixD3Index "1.5.1" ;
            era:rinfIndex "1.1.1.3.2.16.1" ,
                          "1.2.1.1.1.16.1Â " ;
            dct:created "2022-11-07"^^xsd:date ;
            dct:modified "2023-03-14"^^xsd:date ;
            rdfs:comment """Parameter used by the ETCS on-board to supervise the distance allowed to be travelled under the roll-away protection and the reverse movement protection, in metres
According to the specification referenced in Appendix A-1, index [C].
In https://www.era.europa.eu/sites/default/files/filesystem/ertms/ccs_tsi_annex_a_-_mandatory_specifications/set_of_specifications_3_etcs_b3_r2_gsm-r_b1/index004_-_subset-026_v360.zip
 Subset 26, chapter 7. 7.5.1.17 D_NVROLL."""@en ;
            rdfs:isDefinedBy <http://data.europa.eu/949/> ;
            rdfs:label "D_NVROLL"@en ;
            vs:term_status "stable" .


###  http://data.europa.eu/949/dangerousGoodsTankCode
era:dangerousGoodsTankCode rdf:type owl:DatatypeProperty ;
                           rdfs:domain era:VehicleType ;
                           rdfs:range xsd:string ;
                           era:eratvIndex "4.1.9" ;
                           dct:created "2021-08-25"^^xsd:date ;
                           dct:modified "2021-08-25"^^xsd:date ;
                           rdfs:comment "Dangerous goods for which the vehicle is suitable (tank code)."@en ;
                           rdfs:isDefinedBy <http://data.europa.eu/949/> ;
                           rdfs:label "Dangerous goods tank code"@en ;
                           vs:term_status "stable" .


###  http://data.europa.eu/949/demonstrationENE
era:demonstrationENE rdf:type owl:DatatypeProperty ;
                     rdfs:domain [ rdf:type owl:Class ;
                                   owl:unionOf ( era:SubsetWithCommonCharacteristics
                                                 era:Track
                                               )
                                 ] ;
                     rdfs:range xsd:string ;
                     era:rinfIndex "1.1.1.2.1.2" ;
                     dct:created "2021-08-08"^^xsd:date ;
                     dct:modified "2021-09-11"^^xsd:date ;
                     rdfs:comment "Unique number for EI declarations following the same format requirements as specified for EC declarations in Annex VII of Commission Implementing Regulation (EU) 2019/250." ;
                     rdfs:label "EI declaration of demonstration for track (ENE)"@en ;
                     vs:term_status "stable" .


###  http://data.europa.eu/949/demonstrationINF
era:demonstrationINF rdf:type owl:DatatypeProperty ;
                     rdfs:domain [ rdf:type owl:Class ;
                                   owl:unionOf ( era:Siding
                                                 era:Track
                                               )
                                 ] ;
                     rdfs:range xsd:string ;
                     era:rinfIndex "1.1.1.1.1.2" ,
                                   "1.2.1.0.1.2" ,
                                   "1.2.2.0.1.2" ;
                     dct:created "2021-08-03"^^xsd:date ;
                     dct:modified "2023-03-14"^^xsd:date ;
                     rdfs:comment """Unique number for EI declarations following the same format requirements as specified for EC declarations in Annex VII of Commission Implementing Regulation (EU) 2019/250.
In https://eur-lex.europa.eu/legal-content/EN/TXT/HTML/?uri=CELEX:32019R0777&from=EN"""@en ;
                     rdfs:isDefinedBy <http://data.europa.eu/949/> ;
                     rdfs:label "EI declaration of demonstration for track/siding [INF]"@en ;
                     vs:term_status "stable" .


###  http://data.europa.eu/949/demonstrationSRT
era:demonstrationSRT rdf:type owl:DatatypeProperty ;
                     rdfs:domain era:Tunnel ;
                     rdfs:range xsd:string ;
                     era:rinfIndex "1.1.1.1.8.6" ,
                                   "1.2.1.0.5.4" ,
                                   "1.2.2.0.5.4" ;
                     dct:created "2021-08-03"^^xsd:date ;
                     dct:modified "2021-08-11"^^xsd:date ;
                     rdfs:comment "Unique number for EI declarations following the same format requirements as specified for EC declarations in Annex VII of Commission Implementing Regulation (EU) 2019/250."@en ;
                     rdfs:isDefinedBy <http://data.europa.eu/949/> ;
                     rdfs:label "EI declaration of demonstration for tunnel (SRT)"@en ;
                     vs:term_status "stable" .


###  http://data.europa.eu/949/designMassExceptionalPayload
era:designMassExceptionalPayload rdf:type owl:DatatypeProperty ,
                                          owl:FunctionalProperty ;
                                 rdfs:domain era:VehicleType ;
                                 rdfs:range xsd:integer ;
                                 era:eratvIndex "4.5.2.3" ;
                                 dct:created "2020-08-24"^^xsd:date ;
                                 dct:modified "2020-11-03"^^xsd:date ;
                                 rdfs:comment "Design mass under exceptional payload."@en ;
                                 rdfs:isDefinedBy <http://data.europa.eu/949/> ;
                                 rdfs:label "Design mass under exceptional payload"@en ;
                                 vs:term_status "stable" .


###  http://data.europa.eu/949/designMassNormalPayload
era:designMassNormalPayload rdf:type owl:DatatypeProperty ,
                                     owl:FunctionalProperty ;
                            rdfs:domain era:VehicleType ;
                            rdfs:range xsd:integer ;
                            era:eratvIndex "4.5.2.2" ;
                            dct:created "2020-08-24"^^xsd:date ;
                            dct:modified "2020-11-03"^^xsd:date ;
                            rdfs:comment "Design mass under normal payload."@en ;
                            rdfs:isDefinedBy <http://data.europa.eu/949/> ;
                            rdfs:label "Design mass under normal payload"@en ;
                            vs:term_status "stable" .


###  http://data.europa.eu/949/designMassWorkingOrder
era:designMassWorkingOrder rdf:type owl:DatatypeProperty ,
                                    owl:FunctionalProperty ;
                           rdfs:domain era:VehicleType ;
                           rdfs:range xsd:integer ;
                           era:eratvIndex "4.5.2.1" ;
                           dct:created "2020-08-24"^^xsd:date ;
                           dct:modified "2020-11-03"^^xsd:date ;
                           rdfs:comment "Design mass in working order."@en ;
                           rdfs:isDefinedBy <http://data.europa.eu/949/> ;
                           rdfs:label "Design mass in working order"@en ;
                           vs:term_status "stable" .


###  http://data.europa.eu/949/dieselThermalAllowed
era:dieselThermalAllowed rdf:type owl:DatatypeProperty ,
                                  owl:FunctionalProperty ;
                         rdfs:domain era:Tunnel ;
                         rdfs:range xsd:boolean ;
                         era:rinfIndex "1.2.1.0.5.9" ;
                         dct:created "2021-08-09"^^xsd:date ;
                         dct:modified "2021-08-09"^^xsd:date ;
                         rdfs:comment "Indication whether it is allowed to use diesel or other thermal traction in the tunnel."@en ;
                         rdfs:isDefinedBy <http://data.europa.eu/949/> ;
                         rdfs:label "Diesel or other thermal traction allowed"@en ;
                         vs:term_status "stable" .


###  http://data.europa.eu/949/digitalSchematicOverview
era:digitalSchematicOverview rdf:type owl:DatatypeProperty ;
                             rdfs:domain era:OperationalPoint ;
                             rdfs:range gsp:wktLiteral ;
                             era:rinfIndex "1.2.0.0.0.7.2" ;
                             dct:created "2023-03-14"^^xsd:date ;
                             rdfs:comment "Diagrammatic representation of the operational point in Well Known Text polyline"@en ;
                             rdfs:isDefinedBy <http://data.europa.eu/949/> ;
                             rdfs:label "Digital schematic overview"@en ;
                             vs:term_status "stable" .


###  http://data.europa.eu/949/distSignToPhaseEnd
era:distSignToPhaseEnd rdf:type owl:DatatypeProperty ,
                                owl:FunctionalProperty ;
                       rdfs:domain [ rdf:type owl:Class ;
                                     owl:unionOf ( era:SubsetWithCommonCharacteristics
                                                   era:Track
                                                 )
                                   ] ;
                       rdfs:range xsd:integer ;
                       era:rinfIndex "1.1.1.2.4.3" ;
                       era:usedInRCCCalculations "true"^^xsd:boolean ;
                       dct:created "2021-08-08"^^xsd:date ;
                       dct:modified "2021-09-12"^^xsd:date ;
                       rdfs:comment """Specific for route compatibility check on French network.
Distance between the signboard authorizing the driver to âraise pantographâ or âclose the circuit breakerâ after passing the phase separation and the end of the phase separation section."""@en ;
                       rdfs:isDefinedBy <http://data.europa.eu/949/> ;
                       rdfs:label "Distance between signboard and phase separation ending"@en ;
                       vs:term_status "stable" .


###  http://data.europa.eu/949/documentRestrictionPositionContactLineSeparation
era:documentRestrictionPositionContactLineSeparation rdf:type owl:DatatypeProperty ;
                                                     rdfs:domain [ rdf:type owl:Class ;
                                                                   owl:unionOf ( era:SubsetWithCommonCharacteristics
                                                                                 era:Track
                                                                               )
                                                                 ] ;
                                                     rdfs:range xsd:anyURI ;
                                                     era:rinfIndex "1.1.1.2.5.5" ;
                                                     dct:created "2023-03-14" ;
                                                     rdfs:comment "Name and/or reference of the document specifying the restriction(s) related to the position of Multiple Traction unit(s) to comply with contact line separation."@en ;
                                                     rdfs:isDefinedBy <http://data.europa.eu/949/> ;
                                                     rdfs:label "Document with restriction related to the position of Multiple Traction unit(s) to comply with contact line separation"@en ;
                                                     vs:term_status "stable" .


###  http://data.europa.eu/949/documentRestrictionPowerConsumption
era:documentRestrictionPowerConsumption rdf:type owl:DatatypeProperty ;
                                        rdfs:domain [ rdf:type owl:Class ;
                                                      owl:unionOf ( era:SubsetWithCommonCharacteristics
                                                                    era:Track
                                                                  )
                                                    ] ;
                                        rdfs:range xsd:anyURI ;
                                        era:rinfIndex "1.1.1.2.5.4" ;
                                        dct:created "2023-03-14" ;
                                        rdfs:comment "Name and/or reference of the document specifying the restriction(s) related to power consumption of specific electric traction unit(s)."@en ;
                                        rdfs:isDefinedBy <http://data.europa.eu/949/> ;
                                        rdfs:label "Document with restriction related to power consumption of specific electric traction unit(s)"@en ;
                                        vs:term_status "stable" .


###  http://data.europa.eu/949/drivingCabs
era:drivingCabs rdf:type owl:DatatypeProperty ,
                         owl:FunctionalProperty ;
                rdfs:domain era:VehicleType ;
                rdfs:range xsd:integer ;
                era:eratvIndex "4.1.1" ;
                dct:created "2021-08-24"^^xsd:date ;
                dct:modified "2021-08-24"^^xsd:date ;
                rdfs:comment "Number of driving cabs. For wagons the number of driving cabs is to be set to zero (0)."@en ;
                rdfs:isDefinedBy <http://data.europa.eu/949/> ;
                rdfs:label "Driving cabs"@en ;
                vs:term_status "stable" .


###  http://data.europa.eu/949/eddyCurrentBrakePrevention
era:eddyCurrentBrakePrevention rdf:type owl:DatatypeProperty ,
                                        owl:FunctionalProperty ;
                               rdfs:domain era:VehicleType ;
                               rdfs:range xsd:boolean ;
                               era:eratvIndex "4.7.4.1.2" ;
                               dct:created "2020-08-24"^^xsd:date ;
                               dct:modified "2020-11-03"^^xsd:date ;
                               rdfs:comment "Possibility of preventing the use of the eddy current track brake (only if fitted with eddy current brake)"@en ;
                               rdfs:isDefinedBy <http://data.europa.eu/949/> ;
                               rdfs:label "Eddy current brake prevention"@en ;
                               vs:term_status "stable" .


###  http://data.europa.eu/949/eddyCurrentBrakingConditionsDocument
era:eddyCurrentBrakingConditionsDocument rdf:type owl:DatatypeProperty ;
                                         rdfs:domain [ rdf:type owl:Class ;
                                                       owl:unionOf ( era:SubsetWithCommonCharacteristics
                                                                     era:Track
                                                                   )
                                                     ] ;
                                         rdfs:range xsd:anyURI ;
                                         era:appendixD2Index "3.4.5" ;
                                         era:rinfIndex "1.1.1.1.6.4" ;
                                         era:usedInRCCCalculations "true"^^xsd:boolean ;
                                         dct:created "2020-08-24"^^xsd:date ;
                                         dct:modified "2021-09-10"^^xsd:date ;
                                         dct:source <https://eur-lex.europa.eu/eli/reg_impl/2019/773/oj> ;
                                         rdfs:comment """Electronic document available in two EU languages from the IM stored by the Agency with conditions for the use of eddy current brakes identified in 1.1.1.1.6.2.
In https://eur-lex.europa.eu/eli/reg_impl/2019/773/oj 3.4.5 Permissibility to use Eddy-current brake."""@en ;
                                         rdfs:isDefinedBy <http://data.europa.eu/949/> ;
                                         rdfs:label "Document with the conditions for the use of eddy current brakes"@en ;
                                         vs:term_status "stable" .


###  http://data.europa.eu/949/eddyCurrentBrakingFitted
era:eddyCurrentBrakingFitted rdf:type owl:DatatypeProperty ,
                                      owl:FunctionalProperty ;
                             rdfs:domain era:VehicleType ;
                             rdfs:range xsd:boolean ;
                             era:eratvIndex "4.7.4.1.1"^^xsd:string ;
                             dct:created "2022-09-06"^^xsd:date ;
                             rdfs:comment "Eddy current track brake fitted. New property defined to distinghish it from eddyCurrentBraking which is a RINF SKOS property."@en ;
                             rdfs:isDefinedBy "http://data.europa.eu/949/"^^xsd:anyURI ;
                             rdfs:label "Eddy current braking fitted"@en ;
                             vs:term_status "stable" .


###  http://data.europa.eu/949/emergencyBrake
era:emergencyBrake rdf:type owl:DatatypeProperty ,
                            owl:FunctionalProperty ;
                   rdfs:domain era:VehicleType ;
                   rdfs:range xsd:string ;
                   era:eratvIndex "4.7.5" ;
                   dct:created "2020-08-24"^^xsd:date ;
                   dct:modified "2021-08-26"^^xsd:date ;
                   rdfs:comment "Stopping distance and deceleration profile for each load condition per design maximum speed."@en ;
                   rdfs:isDefinedBy <http://data.europa.eu/949/> ;
                   rdfs:label "Emergency braking"@en ;
                   vs:term_status "stable" .


###  http://data.europa.eu/949/endIntrinsicCoordinate
era:endIntrinsicCoordinate rdf:type owl:DatatypeProperty ;
                           rdfs:domain era:NetElement ;
                           rdfs:range xsd:double ;
                           dct:created "2021-04-01"^^xsd:date ;
                           dct:modified "2021-04-01"^^xsd:date ;
                           rdfs:comment "Indicates the coordinate point where a linear object ends."@en ;
                           rdfs:isDefinedBy <http://data.europa.eu/949/> ;
                           rdfs:label "End intrinsic coordinate"@en ;
                           vs:term_status "stable" .


###  http://data.europa.eu/949/energyMeterInstalled
era:energyMeterInstalled rdf:type owl:DatatypeProperty ;
                         rdfs:domain era:VehicleType ;
                         rdfs:range xsd:boolean ;
                         era:eratvIndex "4.10.12" ;
                         dct:created "2021-08-31"^^xsd:date ;
                         dct:modified "2021-08-31"^^xsd:date ;
                         rdfs:comment "TSI conform energy meter for billing purposes installed on board."@en ;
                         rdfs:isDefinedBy <http://data.europa.eu/949/> ;
                         rdfs:label "Energy meter installed"@en ;
                         vs:term_status "stable" .


###  http://data.europa.eu/949/energySupplyMaxPower
era:energySupplyMaxPower rdf:type owl:DatatypeProperty ;
                         rdfs:domain era:VehicleType ;
                         rdfs:range xsd:double ;
                         era:eratvIndex "4.10.2" ;
                         dct:created "2021-08-31"^^xsd:date ;
                         dct:modified "2021-08-31"^^xsd:date ;
                         rdfs:comment "Maximum power (to be indicated for each energy supply system the vehicle is equipped for), given in kW."@en ;
                         rdfs:isDefinedBy <http://data.europa.eu/949/> ;
                         rdfs:label "Energy supply max power"@en ;
                         vs:term_status "stable" .


###  http://data.europa.eu/949/energySupplySystemTSICompliant
era:energySupplySystemTSICompliant rdf:type owl:DatatypeProperty ;
                                   rdfs:domain era:ContactLineSystem ;
                                   rdfs:range xsd:boolean ;
                                   era:rinfIndex "1.1.1.2.2.1.2.1" ;
                                   era:usedInRCCCalculations "true"^^xsd:boolean ;
                                   dct:created "2020-08-24"^^xsd:date ;
                                   dct:modified "2021-08-06"^^xsd:date ;
                                   rdfs:comment "Indication if the traction supply system (nominal voltage and frequency) is fully compliant with TSI."@en ;
                                   rdfs:isDefinedBy <http://data.europa.eu/949/> ;
                                   rdfs:label "Energy supply system TSI compliant"@en ;
                                   vs:term_status "stable" .


###  http://data.europa.eu/949/etcsDataCommApp
era:etcsDataCommApp rdf:type owl:DatatypeProperty ,
                             owl:FunctionalProperty ;
                    rdfs:domain era:VehicleType ;
                    rdfs:range xsd:string ;
                    era:eratvIndex "4.13.2.9" ;
                    dct:created "2021-08-31"^^xsd:date ;
                    dct:modified "2021-08-31"^^xsd:date ;
                    rdfs:comment "Data communication application for ETCS implementation."@en ;
                    rdfs:isDefinedBy <http://data.europa.eu/949/> ;
                    rdfs:label "ETCS data communication application"@en ;
                    vs:term_status "stable" .


###  http://data.europa.eu/949/etcsErrorCorrectionsOnboard
era:etcsErrorCorrectionsOnboard rdf:type owl:DatatypeProperty ;
                                rdfs:domain [ rdf:type owl:Class ;
                                              owl:unionOf ( era:SubsetWithCommonCharacteristics
                                                            era:Track
                                                          )
                                            ] ;
                                rdfs:range xsd:anyURI ;
                                era:rinfIndex "1.1.1.3.1.2" ;
                                dct:created "2023-03-14"^^xsd:date ;
                                rdfs:comment "List of unacceptable errors impacting the IM network that are required to be solved in the on-board according to the CCS TSI point 7.2.10.3 specification maintenance point."@en ;
                                rdfs:isDefinedBy <http://data.europa.eu/949/> ;
                                rdfs:label "ETCS error corrections required for the on-board"@en ;
                                vs:term_status "stable" .


###  http://data.europa.eu/949/etcsImplementsLevelCrossingProcedure
era:etcsImplementsLevelCrossingProcedure rdf:type owl:DatatypeProperty ;
                                         rdfs:domain [ rdf:type owl:Class ;
                                                       owl:unionOf ( era:SubsetWithCommonCharacteristics
                                                                     era:Track
                                                                   )
                                                     ] ;
                                         rdfs:range xsd:boolean ;
                                         era:appendixD3Index "1.2" ;
                                         era:rinfIndex "1.1.1.3.2.13" ,
                                                       "1.2.1.1.1.13" ;
                                         dct:created "2022-11-04"^^xsd:date ;
                                         rdfs:comment "If the trackside does not implement any solution to cover defective LXs (which are normally protected by means of a technical system), then drivers will be required to comply with instructions received from other sources."@en ;
                                         rdfs:isDefinedBy <http://data.europa.eu/949/> ;
                                         rdfs:label "ETCS trackside implements level crossing procedure or an equivalent solution"@en ;
                                         vs:term_status "stable" .


###  http://data.europa.eu/949/etcsInfillLineAccess
era:etcsInfillLineAccess rdf:type owl:DatatypeProperty ,
                                  owl:FunctionalProperty ;
                         rdfs:domain [ rdf:type owl:Class ;
                                       owl:unionOf ( era:SubsetWithCommonCharacteristics
                                                     era:Track
                                                   )
                                     ] ;
                         rdfs:range xsd:boolean ;
                         era:rinfIndex "1.1.1.3.2.3" ,
                                       "1.2.1.1.1.3" ;
                         dct:created "2021-08-08"^^xsd:date ;
                         dct:modified "2021-09-12"^^xsd:date ;
                         rdfs:comment "Indication whether infill is required to access the line for safety reasons."@en ;
                         rdfs:isDefinedBy <http://data.europa.eu/949/> ;
                         rdfs:label "ETCS infill necessary for line access"@en ;
                         vs:term_status "stable" .


###  http://data.europa.eu/949/etcsNationalApplications
era:etcsNationalApplications rdf:type owl:DatatypeProperty ;
                             rdfs:domain era:VehicleType ;
                             rdfs:range xsd:string ;
                             era:eratvIndex "4.13.1.4" ;
                             dct:created "2021-08-31"^^xsd:date ;
                             dct:modified "2021-08-31"^^xsd:date ;
                             rdfs:comment "ETCS national applications implemented (NID_XUSER of Packet 44)."@en ;
                             rdfs:isDefinedBy <http://data.europa.eu/949/> ;
                             rdfs:label "ETCS national applications"@en ;
                             vs:term_status "stable" .


###  http://data.europa.eu/949/etcsNationalPacket44
era:etcsNationalPacket44 rdf:type owl:DatatypeProperty ,
                                  owl:FunctionalProperty ;
                         rdfs:domain [ rdf:type owl:Class ;
                                       owl:unionOf ( era:SubsetWithCommonCharacteristics
                                                     era:Track
                                                   )
                                     ] ;
                         rdfs:range xsd:boolean ;
                         era:rinfIndex "1.1.1.3.2.5" ,
                                       "1.2.1.1.1.5" ;
                         dct:created "2021-08-08"^^xsd:date ;
                         dct:modified "2021-09-12"^^xsd:date ;
                         rdfs:comment "Indication whether data for national packet 44 applications is transmitted between track and train."@en ;
                         rdfs:isDefinedBy <http://data.europa.eu/949/> ;
                         rdfs:label "ETCS national packet 44 application implemented"@en ;
                         vs:term_status "stable" .


###  http://data.europa.eu/949/etcsOnBoardImplementation
era:etcsOnBoardImplementation rdf:type owl:DatatypeProperty ,
                                       owl:FunctionalProperty ;
                              rdfs:domain era:VehicleType ;
                              rdfs:range xsd:string ;
                              era:eratvIndex "4.13.1.7" ;
                              dct:created "2021-08-31"^^xsd:date ;
                              dct:modified "2021-08-31"^^xsd:date ;
                              rdfs:comment "ETCS on-board implementation."@en ;
                              rdfs:isDefinedBy <http://data.europa.eu/949/> ;
                              rdfs:label "ETCS on-board implementation"@en ;
                              vs:term_status "stable" .


###  http://data.europa.eu/949/etcsOptionalFunctions
era:etcsOptionalFunctions rdf:type owl:DatatypeProperty ;
                          rdfs:domain [ rdf:type owl:Class ;
                                        owl:unionOf ( era:SubsetWithCommonCharacteristics
                                                      era:Track
                                                    )
                                      ] ;
                          rdfs:range xsd:string ;
                          era:rinfIndex "1.1.1.3.2.7" ;
                          dct:created "2021-08-08"^^xsd:date ;
                          dct:modified "2023-03-14"^^xsd:date ;
                          rdfs:comment "Deprecated according to the ammendment to the Regulation (EU) 2019/777. Optional ETCS functions which might improve operation on the line."@en ;
                          rdfs:isDefinedBy <http://data.europa.eu/949/> ;
                          rdfs:label "ETCS optional functions"@en ;
                          owl:deprecated "true"^^xsd:boolean ;
                          vs:term_status "unstable" .


###  http://data.europa.eu/949/etcsSystemFunctionalitiesNextFiveYears
era:etcsSystemFunctionalitiesNextFiveYears rdf:type owl:DatatypeProperty ;
                                           rdfs:subPropertyOf owl:topDataProperty ;
                                           rdfs:domain [ rdf:type owl:Class ;
                                                         owl:unionOf ( era:SubsetWithCommonCharacteristics
                                                                       era:Track
                                                                     )
                                                       ] ;
                                           rdfs:range xsd:anyURI ;
                                           era:rinfIndex "1.1.1.3.2.19" ,
                                                         "1.2.1.1.1.20" ;
                                           dct:created "2023-03-14"^^xsd:date ;
                                           rdfs:comment "List of ETCS system version 2.2 or 3.0 functionalities to be required in the next 5 years according to CCS TSI point 6.1.1.2 and Appendix G."@en ;
                                           rdfs:isDefinedBy <http://data.europa.eu/949/> ;
                                           rdfs:label "ETCS system version 2.2 or 3.0 functionalities to be required in the next 5 years"@en ;
                                           vs:term_status "stable" .


###  http://data.europa.eu/949/etcsTransmitsTrackConditions
era:etcsTransmitsTrackConditions rdf:type owl:DatatypeProperty ;
                                 rdfs:domain [ rdf:type owl:Class ;
                                               owl:unionOf ( era:SubsetWithCommonCharacteristics
                                                             era:Track
                                                           )
                                             ] ;
                                 rdfs:range xsd:boolean ;
                                 era:appendixD3Index "1.1" ;
                                 era:rinfIndex "1.1.1.3.2.12" ,
                                               "1.2.1.1.1.12" ;
                                 dct:created "2022-11-04"^^xsd:date ;
                                 dct:modified "2023-03-14"^^xsd:date ;
                                 rdfs:comment """According to the specification referenced in Appendix A-1, index [C]
If the trackside does not provide Track Conditions, the driver will need to be informed about such conditions via alternative methods."""@en ;
                                 rdfs:isDefinedBy <http://data.europa.eu/949/> ;
                                 rdfs:label "Is the ETCS trackside engineered to transmit Track Conditions"@en ;
                                 vs:term_status "stable" .


###  http://data.europa.eu/949/ferromagneticWheelMaterial
era:ferromagneticWheelMaterial rdf:type owl:DatatypeProperty ;
                               rdfs:domain era:VehicleType ;
                               rdfs:range xsd:boolean ;
                               era:eratvIndex "4.14.2.12" ;
                               dct:created "2021-09-01"^^xsd:date ;
                               dct:modified "2021-09-01"^^xsd:date ;
                               rdfs:comment "Wheel material is ferromagnetic."@en ;
                               rdfs:isDefinedBy <http://data.europa.eu/949/> ;
                               rdfs:label "Ferromagnetic wheel material"@en ;
                               vs:term_status "stable" .


###  http://data.europa.eu/949/fixedSeats
era:fixedSeats rdf:type owl:DatatypeProperty ;
               rdfs:domain era:VehicleType ;
               rdfs:range xsd:string ;
               era:eratvIndex "4.12.1.1" ;
               dct:created "2021-08-31"^^xsd:date ;
               dct:modified "2021-08-31"^^xsd:date ;
               rdfs:comment "Number of fixed seats."@en ;
               rdfs:isDefinedBy <http://data.europa.eu/949/> ;
               rdfs:label "Fixed seats"@en ;
               vs:term_status "stable" .


###  http://data.europa.eu/949/flangeLubeForbidden
era:flangeLubeForbidden rdf:type owl:DatatypeProperty ,
                                 owl:FunctionalProperty ;
                        rdfs:domain [ rdf:type owl:Class ;
                                      owl:unionOf ( era:SubsetWithCommonCharacteristics
                                                    era:Track
                                                  )
                                    ] ;
                        rdfs:range xsd:boolean ;
                        era:rinfIndex "1.1.1.1.7.1" ;
                        dct:created "2021-08-08"^^xsd:date ;
                        dct:modified "2021-09-11"^^xsd:date ;
                        rdfs:comment "Indication whether the use of on-board device for flange lubrication is forbidden"@en ;
                        rdfs:isDefinedBy <http://data.europa.eu/949/> ;
                        rdfs:label "Use of flange lubrication forbidden"@en ;
                        vs:term_status "stable" .


###  http://data.europa.eu/949/flangeLubeRules
era:flangeLubeRules rdf:type owl:DatatypeProperty ;
                    rdfs:domain era:TrainDetectionSystem ;
                    rdfs:range xsd:boolean ;
                    era:rinfIndex "1.1.1.3.7.20" ;
                    dct:created "2021-08-08"^^xsd:date ;
                    dct:modified "2023-03-14"^^xsd:date ;
                    rdfs:comment "Deprecated according to the ammendment to the Regulation (EU) 2019/777. Indication whether rules for activation or deactivation of flange lubrication exist."@en ;
                    rdfs:isDefinedBy <http://data.europa.eu/949/> ;
                    rdfs:label "Existence of rules on on-board flange lubrication"@en ;
                    owl:deprecated "true"^^xsd:boolean ;
                    vs:term_status "stable" .


###  http://data.europa.eu/949/flangeLubricationFitted
era:flangeLubricationFitted rdf:type owl:DatatypeProperty ;
                            rdfs:domain era:VehicleType ;
                            rdfs:range xsd:boolean ;
                            era:eratvIndex "4.9.3.1" ;
                            dct:created "2021-08-31"^^xsd:date ;
                            dct:modified "2021-08-31"^^xsd:date ;
                            rdfs:comment "Indicates if the vehicle type is fitted for flange lubrication."@en ;
                            rdfs:isDefinedBy <http://data.europa.eu/949/> ;
                            rdfs:label "Flange lubrication fitted"@en ;
                            vs:term_status "stable" .


###  http://data.europa.eu/949/frenchTrainDetectionSystemLimitationApplicable
era:frenchTrainDetectionSystemLimitationApplicable rdf:type owl:DatatypeProperty ;
                                                   rdfs:domain era:FrenchTrainDetectionSystemLimitation ;
                                                   rdfs:range xsd:boolean ;
                                                   era:rinfIndex "1.1.1.3.7.1.4" ;
                                                   era:usedInRCCCalculations "true"^^xsd:boolean ;
                                                   dct:created "2023-04-05"^^xsd:date ;
                                                   rdfs:comment "Part of the section with train detection limitation that indicates if it is applicable. Only for the French network."@en ;
                                                   rdfs:isDefinedBy <http://data.europa.eu/949/> ;
                                                   rdfs:label "Section with train detection limitation is applicable, only for the French network"@en ;
                                                   vs:term_status "stable" .


###  http://data.europa.eu/949/gaugingCheckLocation
era:gaugingCheckLocation rdf:type owl:DatatypeProperty ;
                         rdfs:domain [ rdf:type owl:Class ;
                                       owl:unionOf ( era:SubsetWithCommonCharacteristics
                                                     era:Track
                                                   )
                                     ] ;
                         rdfs:range xsd:string ;
                         era:rinfIndex "1.1.1.1.3.1.2" ,
                                       "1.2.1.0.3.5" ;
                         era:usedInRCCCalculations "true"^^xsd:boolean ;
                         dct:created "2020-07-29"^^xsd:date ;
                         dct:modified "2023-03-14"^^xsd:date ;
                         rdfs:comment "Location of particular points requiring specific checks due to deviations from gauging referred to in 1.1.1.1.3.1.1."@en ;
                         rdfs:isDefinedBy <http://data.europa.eu/949/> ;
                         rdfs:label "Railway location of particular points requiring specific checks"@en ;
                         vs:term_status "stable" .


###  http://data.europa.eu/949/gaugingTransversalDocument
era:gaugingTransversalDocument rdf:type owl:DatatypeProperty ;
                               rdfs:domain [ rdf:type owl:Class ;
                                             owl:unionOf ( era:SubsetWithCommonCharacteristics
                                                           era:Track
                                                         )
                                           ] ;
                               rdfs:range xsd:anyURI ;
                               era:rinfIndex "1.1.1.1.3.1.3" ,
                                             "1.2.1.0.3.6" ;
                               era:usedInRCCCalculations "true"^^xsd:boolean ;
                               dct:created "2020-08-24"^^xsd:date ;
                               dct:modified "2023-03-14"^^xsd:date ;
                               rdfs:comment "Electronic document available from the IM stored by the Agency with the transversal section of the particular points requiring specific checks due to deviations from gauging referred to in 1.1.1.1.3.1.1. Where relevant, guidance for the check with the particular point may be attached to the document with the transversal section."@en ;
                               rdfs:isDefinedBy <http://data.europa.eu/949/> ;
                               rdfs:label "Document with the transversal section of the particular points requiring specific checks"@en ;
                               vs:term_status "stable" .


###  http://data.europa.eu/949/gprsForETCS
era:gprsForETCS rdf:type owl:DatatypeProperty ,
                         owl:FunctionalProperty ;
                rdfs:domain [ rdf:type owl:Class ;
                              owl:unionOf ( era:SubsetWithCommonCharacteristics
                                            era:Track
                                          )
                            ] ;
                rdfs:range xsd:boolean ;
                era:rinfIndex "1.1.1.3.3.3.2" ,
                              "1.2.1.1.2.3.2" ;
                dct:created "2021-08-08"^^xsd:date ;
                dct:modified "2021-09-12"^^xsd:date ;
                rdfs:comment "Indication if GPRS can be used for ETCS."@en ;
                rdfs:isDefinedBy <http://data.europa.eu/949/> ;
                rdfs:label "GPRS for ETCS"@en ;
                vs:term_status "stable" .


###  http://data.europa.eu/949/gprsImplementationArea
era:gprsImplementationArea rdf:type owl:DatatypeProperty ;
                           rdfs:domain [ rdf:type owl:Class ;
                                         owl:unionOf ( era:SubsetWithCommonCharacteristics
                                                       era:Track
                                                     )
                                       ] ;
                           rdfs:range xsd:string ;
                           era:rinfIndex "1.1.1.3.3.3.3" ,
                                         "1.2.1.1.2.3.3" ;
                           dct:created "2021-08-09"^^xsd:date ;
                           dct:modified "2021-09-12"^^xsd:date ;
                           rdfs:comment "Indication of the area in which GPRS can be used for ETCS."@en ;
                           rdfs:isDefinedBy <http://data.europa.eu/949/> ;
                           rdfs:label "Area of implementation of GPRS"@en ;
                           vs:term_status "stable" .


###  http://data.europa.eu/949/gradient
era:gradient rdf:type owl:DatatypeProperty ,
                      owl:FunctionalProperty ;
             rdfs:domain era:Siding ;
             rdfs:range xsd:double ;
             era:rinfIndex "1.2.2.0.3.1" ;
             era:usedInRCCCalculations "true"^^xsd:boolean ;
             dct:created "2021-08-10"^^xsd:date ;
             dct:modified "2021-08-10"^^xsd:date ;
             dct:source <https://rsm-evolution.org/220927_RSM/EARoot/EA2/EA1/EA166.html> ;
             rdfs:comment "Maximum value of the gradient for stabling tracks expressed in millimetres per metre."@en ;
             rdfs:isDefinedBy <http://data.europa.eu/949/> ;
             rdfs:label "Gradient for stabling tracks"@en ;
             vs:term_status "stable" .


###  http://data.europa.eu/949/gradientProfile
era:gradientProfile rdf:type owl:DatatypeProperty ;
                    rdfs:domain [ rdf:type owl:Class ;
                                  owl:unionOf ( era:SubsetWithCommonCharacteristics
                                                era:Track
                                              )
                                ] ;
                    rdfs:range xsd:string ;
                    era:appendixD2Index "3.2.1" ,
                                        "3.2.2" ;
                    era:rinfIndex "1.1.1.1.3.6" ;
                    era:usedInRCCCalculations "true"^^xsd:boolean ;
                    dct:created "2020-08-24"^^xsd:date ;
                    dct:modified "2021-09-10"^^xsd:date ;
                    dct:source <https://rsm-evolution.org/220927_RSM/EARoot/EA2/EA1/EA166.html> ;
                    rdfs:comment """Sequence of gradient values and locations of change in gradient.
In https://eur-lex.europa.eu/eli/reg_impl/2019/773/oj 3.2.1 Gradient percentage, 3.2.2 Gradient location."""@en ;
                    rdfs:isDefinedBy <http://data.europa.eu/949/> ;
                    rdfs:label "Gradient profile"@en ;
                    vs:term_status "stable" .


###  http://data.europa.eu/949/gsmRAdditionalInfo
era:gsmRAdditionalInfo rdf:type owl:DatatypeProperty ;
                       rdfs:domain [ rdf:type owl:Class ;
                                     owl:unionOf ( era:SubsetWithCommonCharacteristics
                                                   era:Track
                                                 )
                                   ] ;
                       rdfs:range xsd:string ;
                       era:rinfIndex "1.1.1.3.3.3.1" ,
                                     "1.2.1.1.2.3.1" ;
                       dct:created "2021-08-08"^^xsd:date ;
                       dct:modified "2021-09-12"^^xsd:date ;
                       rdfs:comment "Any additional information on network characteristics or corresponding document available from the IM and stored by the Agency, e.g.; interference level, leading to the recommendation of additional on-board protection."@en ;
                       rdfs:isDefinedBy <http://data.europa.eu/949/> ;
                       rdfs:label "Additional information on network characteristics"@en ;
                       vs:term_status "stable" .


###  http://data.europa.eu/949/gsmRNoCoverage
era:gsmRNoCoverage rdf:type owl:DatatypeProperty ,
                            owl:FunctionalProperty ;
                   rdfs:domain [ rdf:type owl:Class ;
                                 owl:unionOf ( era:SubsetWithCommonCharacteristics
                                               era:Track
                                             )
                               ] ;
                   rdfs:range xsd:boolean ;
                   era:rinfIndex "1.1.1.3.3.8" ,
                                 "1.2.1.1.2.8" ;
                   dct:created "2021-08-09"^^xsd:date ;
                   dct:modified "2021-09-12"^^xsd:date ;
                   rdfs:comment "Indication if there is no GSMR coverage."@en ;
                   rdfs:isDefinedBy <http://data.europa.eu/949/> ;
                   rdfs:label "No GSM-R coverage"@en ;
                   vs:term_status "stable" .


###  http://data.europa.eu/949/gsmRSetsInDrivingCab
era:gsmRSetsInDrivingCab rdf:type owl:DatatypeProperty ;
                         rdfs:domain era:VehicleType ;
                         rdfs:range xsd:integer ;
                         era:eratvIndex "4.13.2.2" ;
                         dct:created "2021-08-31"^^xsd:date ;
                         dct:modified "2021-08-31"^^xsd:date ;
                         rdfs:comment "Number of GSM-R mobile sets in driving cab for data transmission."@en ;
                         rdfs:isDefinedBy <http://data.europa.eu/949/> ;
                         rdfs:label "GSM-R sets in driving cab"@en ;
                         vs:term_status "stable" .


###  http://data.europa.eu/949/gsmrErrorCorrectionsOnboard
era:gsmrErrorCorrectionsOnboard rdf:type owl:DatatypeProperty ;
                                rdfs:domain [ rdf:type owl:Class ;
                                              owl:unionOf ( era:SubsetWithCommonCharacteristics
                                                            era:Track
                                                          )
                                            ] ;
                                rdfs:range xsd:anyURI ;
                                era:rinfIndex "1.1.1.3.3.11" ;
                                dct:created "2023-03-14"^^xsd:date ;
                                rdfs:comment "List of unacceptable errors impacting the IM network that are required to be solved in the on-board according to the CCS TSI point 7.2.10.3 specification maintenance point."@en ;
                                rdfs:isDefinedBy <http://data.europa.eu/949/> ;
                                rdfs:label "GSM-R error corrections required for the on-board"@en ;
                                vs:term_status "stable" .


###  http://data.europa.eu/949/gsmrForcedDeregistrationFunctionalNumber
era:gsmrForcedDeregistrationFunctionalNumber rdf:type owl:DatatypeProperty ;
                                             rdfs:domain [ rdf:type owl:Class ;
                                                           owl:unionOf ( era:SubsetWithCommonCharacteristics
                                                                         era:Track
                                                                       )
                                                         ] ;
                                             rdfs:range xsd:boolean ;
                                             era:appendixD3Index "2.1" ;
                                             era:rinfIndex "1.1.1.3.3.11" ,
                                                           "1.2.1.1.2.11" ;
                                             dct:created "2022-11-07"^^xsd:date ;
                                             dct:modified "2023-03-14"^^xsd:date ;
                                             rdfs:comment "This feature will condition the applicable operational rules for drivers and signallers when dealing with cab radios registered under wrong numbers."@en ;
                                             rdfs:isDefinedBy <http://data.europa.eu/949/> ;
                                             rdfs:label "GSM-R network is configured to allow forced de-registration of a functional number by another driver"@en ;
                                             vs:term_status "stable" .


###  http://data.europa.eu/949/hasAdditionalBrakingInformation
era:hasAdditionalBrakingInformation rdf:type owl:DatatypeProperty ,
                                             owl:FunctionalProperty ;
                                    rdfs:domain [ rdf:type owl:Class ;
                                                  owl:unionOf ( era:SubsetWithCommonCharacteristics
                                                                era:Track
                                                              )
                                                ] ;
                                    rdfs:range xsd:boolean ;
                                    era:rinfIndex "1.1.1.3.11.2" ;
                                    era:usedInRCCCalculations "true"^^xsd:boolean ;
                                    dct:created "2020-08-24"^^xsd:date ;
                                    dct:modified "2021-09-12"^^xsd:date ;
                                    rdfs:comment "Availability by the IM of additional information as defined in point (2) of point 4.2.2.6.2 of OPE TSI."@en ;
                                    rdfs:isDefinedBy <http://data.europa.eu/949/> ;
                                    rdfs:label "Availability by the IM of additional information"@en ;
                                    vs:term_status "stable" .


###  http://data.europa.eu/949/hasAutomaticDroppingDevice
era:hasAutomaticDroppingDevice rdf:type owl:DatatypeProperty ,
                                        owl:FunctionalProperty ;
                               rdfs:domain era:VehicleType ;
                               rdfs:range xsd:boolean ;
                               era:eratvIndex "4.10.11" ;
                               dct:created "2020-08-25"^^xsd:date ;
                               dct:modified "2020-11-03"^^xsd:date ;
                               rdfs:comment "Automatic dropping device (ADD) fitted (to be indicated for each energy supply system the vehicle is equipped for)."@en ;
                               rdfs:isDefinedBy <http://data.europa.eu/949/> ;
                               rdfs:label "Has automatic dropping device"@en ;
                               vs:term_status "stable" .


###  http://data.europa.eu/949/hasBallast
era:hasBallast rdf:type owl:DatatypeProperty ,
                        owl:FunctionalProperty ;
               rdfs:domain [ rdf:type owl:Class ;
                             owl:unionOf ( era:SubsetWithCommonCharacteristics
                                           era:Track
                                         )
                           ] ;
               rdfs:range xsd:boolean ;
               era:rinfIndex "1.1.1.1.4.4" ;
               dct:created "2021-08-03"^^xsd:date ;
               dct:modified "2021-09-10"^^xsd:date ;
               rdfs:comment "Specifies whether track construction is with sleepers embedded in ballast or not."@en ;
               rdfs:isDefinedBy <http://data.europa.eu/949/> ;
               rdfs:label "Existence of ballast"@en ;
               vs:term_status "stable" .


###  http://data.europa.eu/949/hasCantDefficiencyCompensation
era:hasCantDefficiencyCompensation rdf:type owl:DatatypeProperty ;
                                   rdfs:domain era:VehicleType ;
                                   rdfs:range xsd:boolean ;
                                   era:eratvIndex "4.6.2" ;
                                   dct:created "2021-08-26"^^xsd:date ;
                                   dct:modified "2021-08-26"^^xsd:date ;
                                   rdfs:comment "Vehicle equipped with a cant deficiency compensation system (tilting vehicle)."@en ;
                                   rdfs:isDefinedBy <http://data.europa.eu/949/> ;
                                   rdfs:label "Has cant defficiency compensation"@en ;
                                   vs:term_status "stable" .


###  http://data.europa.eu/949/hasCurrentLimitation
era:hasCurrentLimitation rdf:type owl:DatatypeProperty ,
                                  owl:FunctionalProperty ;
                         rdfs:domain era:VehicleType ;
                         rdfs:range xsd:boolean ;
                         era:eratvIndex "4.10.14" ;
                         dct:created "2020-08-24"^^xsd:date ;
                         dct:modified "2020-11-03"^^xsd:date ;
                         rdfs:comment "Electric units equipped with power or current limitation function."@en ;
                         rdfs:isDefinedBy <http://data.europa.eu/949/> ;
                         rdfs:label "Has current limitation"@en ;
                         vs:term_status "stable" .


###  http://data.europa.eu/949/hasETCSRestrictionsConditions
era:hasETCSRestrictionsConditions rdf:type owl:DatatypeProperty ,
                                           owl:FunctionalProperty ;
                                  rdfs:domain [ rdf:type owl:Class ;
                                                owl:unionOf ( era:SubsetWithCommonCharacteristics
                                                              era:Track
                                                            )
                                              ] ;
                                  rdfs:range xsd:boolean ;
                                  era:rinfIndex "1.1.1.3.2.6" ,
                                                "1.2.1.1.1.6" ;
                                  dct:created "2021-08-08"^^xsd:date ;
                                  dct:modified "2021-09-12"^^xsd:date ;
                                  rdfs:comment "Indication whether restrictions or conditions due to partial compliance with the CCS TSI â Commission Regulation (EU) 2016/919 (5) exist."@en ;
                                  rdfs:isDefinedBy <http://data.europa.eu/949/> ;
                                  rdfs:label "Existence of operating restrictions or conditions"@en ;
                                  vs:term_status "stable" .


###  http://data.europa.eu/949/hasElectricShoreSupply
era:hasElectricShoreSupply rdf:type owl:DatatypeProperty ,
                                    owl:FunctionalProperty ;
                           rdfs:domain era:Siding ;
                           rdfs:range xsd:boolean ;
                           era:rinfIndex "1.2.2.0.4.6" ;
                           dct:created "2021-08-10"^^xsd:date ;
                           dct:modified "2021-08-10"^^xsd:date ;
                           rdfs:comment "Indication whether an installation for electric shore supply exists (fixed installation for servicing trains)."@en ;
                           rdfs:isDefinedBy <http://data.europa.eu/949/> ;
                           rdfs:label "Existence of electric shore supply"@en ;
                           vs:term_status "stable" .


###  http://data.europa.eu/949/hasEmergencyPlan
era:hasEmergencyPlan rdf:type owl:DatatypeProperty ,
                              owl:FunctionalProperty ;
                     rdfs:domain era:Tunnel ;
                     rdfs:range xsd:boolean ;
                     era:rinfIndex "1.1.1.1.8.9" ,
                                   "1.2.1.0.5.6" ,
                                   "1.2.2.0.5.6" ;
                     dct:created "2021-08-03"^^xsd:date ;
                     dct:modified "2021-08-10"^^xsd:date ;
                     rdfs:comment "Indication whether emergency plan exists."@en ;
                     rdfs:isDefinedBy <http://data.europa.eu/949/> ;
                     rdfs:label "Existence of emergency plan"@en ;
                     vs:term_status "stable" .


###  http://data.europa.eu/949/hasEvacuationAndRescuePoints
era:hasEvacuationAndRescuePoints rdf:type owl:DatatypeProperty ;
                                 rdfs:domain era:Tunnel ;
                                 rdfs:range xsd:boolean ;
                                 era:appendixD2Index "3.2.3" ;
                                 era:rinfIndex "1.1.1.1.8.13" ,
                                               "1.2.1.0.5.11" ,
                                               "1.2.2.0.5.10" ;
                                 dct:created "2022-10-27"^^xsd:date ;
                                 dct:modified "2023-03-14"^^xsd:date ;
                                 dct:source <https://eur-lex.europa.eu/eli/reg_impl/2019/773/oj> ;
                                 rdfs:comment """Indication of existence of evacuation and rescue points.
In https://eur-lex.europa.eu/eli/reg_impl/2019/773/oj 3.2.3 Tunnels: location, name, length, specific information such as the existence of walkways and points of safe egress as well as the location of safe areas where evacuation of passengers may take place; fire safety categorisation."""@en ;
                                 rdfs:isDefinedBy <http://data.europa.eu/949/> ;
                                 rdfs:label "Existence of evacuation and rescue points"@en ;
                                 vs:term_status "stable" .


###  http://data.europa.eu/949/hasExternalCleaning
era:hasExternalCleaning rdf:type owl:DatatypeProperty ,
                                 owl:FunctionalProperty ;
                        rdfs:domain era:Siding ;
                        rdfs:range xsd:boolean ;
                        era:rinfIndex "1.2.2.0.4.2" ;
                        dct:created "2021-08-10"^^xsd:date ;
                        dct:modified "2021-08-10"^^xsd:date ;
                        rdfs:comment "Indication whether exists an installation for external cleaning facility (fixed installation for servicing trains) as defined in INF TSIs."@en ;
                        rdfs:isDefinedBy <http://data.europa.eu/949/> ;
                        rdfs:label "Existence of external cleaning facilities"@en ;
                        vs:term_status "stable" .


###  http://data.europa.eu/949/hasHotAxleBoxDetector
era:hasHotAxleBoxDetector rdf:type owl:DatatypeProperty ,
                                   owl:FunctionalProperty ;
                          rdfs:domain [ rdf:type owl:Class ;
                                        owl:unionOf ( era:SubsetWithCommonCharacteristics
                                                      era:Track
                                                    )
                                      ] ;
                          rdfs:range xsd:boolean ;
                          era:rinfIndex "1.1.1.1.7.4" ;
                          era:usedInRCCCalculations "true"^^xsd:boolean ;
                          dct:created "2020-08-24"^^xsd:date ;
                          dct:modified "2021-09-11"^^xsd:date ;
                          rdfs:comment "Existence of trackside hot axle box detector (HABD)."@en ;
                          rdfs:isDefinedBy <http://data.europa.eu/949/> ;
                          rdfs:label "Existence of trackside hot axle box detector (HABD)"@en ;
                          vs:term_status "stable" .


###  http://data.europa.eu/949/hasLevelCrossings
era:hasLevelCrossings rdf:type owl:DatatypeProperty ,
                               owl:FunctionalProperty ;
                      rdfs:domain [ rdf:type owl:Class ;
                                    owl:unionOf ( era:SubsetWithCommonCharacteristics
                                                  era:Track
                                                )
                                  ] ;
                      rdfs:range xsd:boolean ;
                      era:rinfIndex "1.1.1.1.7.2" ;
                      dct:created "2021-08-03"^^xsd:date ;
                      dct:modified "2021-09-11"^^xsd:date ;
                      rdfs:comment "Indication whether level crossings (including pedestrian track crossing) exist on the section of line."@en ;
                      rdfs:isDefinedBy <http://data.europa.eu/949/> ;
                      rdfs:label "Existence of level crossings"@en ;
                      vs:term_status "stable" .


###  http://data.europa.eu/949/hasLubricationDevicePrevention
era:hasLubricationDevicePrevention rdf:type owl:DatatypeProperty ;
                                   rdfs:domain era:VehicleType ;
                                   rdfs:range xsd:boolean ;
                                   era:eratvIndex "4.9.3.2" ;
                                   dct:created "2021-08-31"^^xsd:date ;
                                   dct:modified "2021-08-31"^^xsd:date ;
                                   rdfs:comment "Possibility of preventing the use of the lubrication device (only if fitted with flange lubrication)."@en ;
                                   rdfs:isDefinedBy <http://data.europa.eu/949/> ;
                                   rdfs:label "Has lubrication device prevention"@en ;
                                   vs:term_status "stable" .


###  http://data.europa.eu/949/hasOtherTrainProtection
era:hasOtherTrainProtection rdf:type owl:DatatypeProperty ,
                                     owl:FunctionalProperty ;
                            rdfs:domain [ rdf:type owl:Class ;
                                          owl:unionOf ( era:SubsetWithCommonCharacteristics
                                                        era:Track
                                                      )
                                        ] ;
                            rdfs:range xsd:boolean ;
                            era:rinfIndex "1.1.1.3.5.1" ;
                            dct:created "2021-08-09"^^xsd:date ;
                            dct:modified "2023-03-14"^^xsd:date ;
                            rdfs:comment "Deprecated according to the ammendment to the Regulation (EU) 2019/777. Indication if other train protection, control and warning systems in normal operation are installed lineside."@en ;
                            rdfs:isDefinedBy <http://data.europa.eu/949/> ;
                            rdfs:label "Existence of other train protection, control and warning systems installed"@en ;
                            owl:deprecated "true"^^xsd:boolean ;
                            vs:term_status "unstable" .


###  http://data.europa.eu/949/hasParkingBrake
era:hasParkingBrake rdf:type owl:DatatypeProperty ,
                             owl:FunctionalProperty ;
                    rdfs:domain era:VehicleType ;
                    rdfs:range xsd:boolean ;
                    era:eratvIndex "4.7.3.4" ;
                    dct:created "2021-08-26"^^xsd:date ;
                    dct:modified "2021-08-26"^^xsd:date ;
                    rdfs:comment "Indicates if a vehicle type has parking brake."@en ;
                    rdfs:isDefinedBy <http://data.europa.eu/949/> ;
                    rdfs:label "Has parking brake"@en ;
                    vs:term_status "stable" .


###  http://data.europa.eu/949/hasPlatformCurvature
era:hasPlatformCurvature rdf:type owl:DatatypeProperty ;
                         rdfs:domain era:Platform ;
                         rdfs:range xsd:boolean ;
                         era:appendixD2Index "2.3.8" ;
                         era:rinfIndex "1.2.1.0.6.8" ;
                         dct:created "2022-10-27"^^xsd:date ;
                         dct:modified "2023-03-14"^^xsd:date ;
                         dct:source <https://eur-lex.europa.eu/eli/reg_impl/2019/773/oj> ;
                         rdfs:comment """Indication of the existence of the curvature of the platform.
In https://eur-lex.europa.eu/eli/reg_impl/2019/773/oj 2.3.8 Curvature of platforms."""@en ;
                         rdfs:isDefinedBy <http://data.europa.eu/949/> ;
                         rdfs:label "Existence of  platform curvature"@en ;
                         vs:term_status "stable" .


###  http://data.europa.eu/949/hasRefuelling
era:hasRefuelling rdf:type owl:DatatypeProperty ,
                           owl:FunctionalProperty ;
                  rdfs:domain era:Siding ;
                  rdfs:range xsd:boolean ;
                  era:rinfIndex "1.2.2.0.4.4" ;
                  dct:created "2021-08-10"^^xsd:date ;
                  dct:modified "2021-08-10"^^xsd:date ;
                  rdfs:comment "Indication whether exists an installation for refuelling (fixed installation for servicing trains) as defined in INF TSIs."@en ;
                  rdfs:isDefinedBy <http://data.europa.eu/949/> ;
                  rdfs:label "Existence of refuelling"@en ;
                  vs:term_status "stable" .


###  http://data.europa.eu/949/hasRegenerativeBrake
era:hasRegenerativeBrake rdf:type owl:DatatypeProperty ,
                                  owl:FunctionalProperty ;
                         rdfs:domain era:VehicleType ;
                         rdfs:range xsd:boolean ;
                         era:eratvIndex "4.7.4.3.1" ;
                         dct:created "2020-08-24"^^xsd:date ;
                         dct:modified "2021-08-06"^^xsd:date ;
                         rdfs:comment "Indication whether regenerative braking is permitted or not."@en ;
                         rdfs:isDefinedBy <http://data.europa.eu/949/> ;
                         rdfs:label "Permission for regenerative braking"@en ;
                         vs:term_status "stable" .


###  http://data.europa.eu/949/hasSandRestocking
era:hasSandRestocking rdf:type owl:DatatypeProperty ,
                               owl:FunctionalProperty ;
                      rdfs:domain era:Siding ;
                      rdfs:range xsd:boolean ;
                      era:rinfIndex "1.2.2.0.4.5" ;
                      dct:created "2021-08-10"^^xsd:date ;
                      dct:modified "2021-08-10"^^xsd:date ;
                      rdfs:comment "Indication whether an installation for sand restocking exists (fixed installation for servicing trains)."@en ;
                      rdfs:isDefinedBy <http://data.europa.eu/949/> ;
                      rdfs:label "Existence of sand restocking"@en ;
                      vs:term_status "stable" .


###  http://data.europa.eu/949/hasSandingPrevention
era:hasSandingPrevention rdf:type owl:DatatypeProperty ;
                         rdfs:domain era:VehicleType ;
                         rdfs:range xsd:boolean ;
                         era:eratvIndex "4.14.2.12" ;
                         dct:created "2021-09-01"^^xsd:date ;
                         dct:modified "2021-09-01"^^xsd:date ;
                         rdfs:comment "Possibility of preventing the use of sanding."@en ;
                         rdfs:isDefinedBy <http://data.europa.eu/949/> ;
                         rdfs:label "Has sanding prevention"@en ;
                         vs:term_status "stable" .


###  http://data.europa.eu/949/hasSchematicOverviewOPDigitalForm
era:hasSchematicOverviewOPDigitalForm rdf:type owl:DatatypeProperty ;
                                      rdfs:domain era:OperationalPoint ;
                                      rdfs:range xsd:boolean ;
                                      era:rinfIndex "1.2.0.0.0.7" ;
                                      dct:created "2023-03-14"^^xsd:date ;
                                      rdfs:comment "The existence of a schematic overview of the operational point in digital form"@en ;
                                      rdfs:isDefinedBy <http://data.europa.eu/949/> ;
                                      rdfs:label "Has schematic overview in digital form"@en ;
                                      vs:term_status "stable" .


###  http://data.europa.eu/949/hasSevereWeatherConditions
era:hasSevereWeatherConditions rdf:type owl:DatatypeProperty ,
                                        owl:FunctionalProperty ;
                               rdfs:domain [ rdf:type owl:Class ;
                                             owl:unionOf ( era:SubsetWithCommonCharacteristics
                                                           era:Track
                                                         )
                                           ] ;
                               rdfs:range xsd:boolean ;
                               era:rinfIndex "1.1.1.1.2.8" ;
                               era:usedInRCCCalculations "true"^^xsd:boolean ;
                               dct:created "2020-08-24"^^xsd:date ;
                               dct:modified "2021-09-10"^^xsd:date ;
                               rdfs:comment "Climatic conditions on the line are severe according to European standard."@en ;
                               rdfs:isDefinedBy <http://data.europa.eu/949/> ;
                               rdfs:label "Existence of severe climatic conditions"@en ;
                               vs:term_status "stable" .


###  http://data.europa.eu/949/hasShuntingRestrictions
era:hasShuntingRestrictions rdf:type owl:DatatypeProperty ,
                                     owl:FunctionalProperty ;
                            rdfs:domain era:VehicleType ;
                            rdfs:range xsd:boolean ;
                            era:eratvIndex "4.8.3" ;
                            dct:created "2021-08-31"^^xsd:date ;
                            dct:modified "2021-08-31"^^xsd:date ;
                            rdfs:comment "Indicates the presence of shunting restrictions."@en ;
                            rdfs:isDefinedBy <http://data.europa.eu/949/> ;
                            rdfs:label "Has shunting restrictions"@en ;
                            vs:term_status "stable" .


###  http://data.europa.eu/949/hasSystemSeparation
era:hasSystemSeparation rdf:type owl:DatatypeProperty ,
                                 owl:FunctionalProperty ;
                        rdfs:domain [ rdf:type owl:Class ;
                                      owl:unionOf ( era:SubsetWithCommonCharacteristics
                                                    era:Track
                                                  )
                                    ] ;
                        rdfs:range xsd:boolean ;
                        era:rinfIndex "1.1.1.2.4.2.1" ;
                        dct:created "2021-08-08"^^xsd:date ;
                        dct:modified "2021-09-12"^^xsd:date ;
                        rdfs:comment "Indication of existence of system separation."@en ;
                        rdfs:isDefinedBy <http://data.europa.eu/949/> ;
                        rdfs:label "System separation"@en ;
                        vs:term_status "stable" .


###  http://data.europa.eu/949/hasTSITrainDetection
era:hasTSITrainDetection rdf:type owl:DatatypeProperty ;
                         rdfs:domain [ rdf:type owl:Class ;
                                       owl:unionOf ( era:SubsetWithCommonCharacteristics
                                                     era:Track
                                                   )
                                     ] ;
                         rdfs:range xsd:boolean ;
                         era:rinfIndex "1.1.1.3.4.1" ,
                                       "1.2.1.1.3.1" ;
                         dct:created "2021-08-09"^^xsd:date ;
                         dct:modified "2021-09-12"^^xsd:date ;
                         rdfs:comment "Indication if there is any train detection system installed and fully compliant with the CCS TSI."@en ;
                         rdfs:isDefinedBy <http://data.europa.eu/949/> ;
                         rdfs:label "Existence of train detection system fully compliant with the TSI"@en ;
                         vs:term_status "stable" .


###  http://data.europa.eu/949/hasToiletDischarge
era:hasToiletDischarge rdf:type owl:DatatypeProperty ,
                                owl:FunctionalProperty ;
                       rdfs:domain era:Siding ;
                       rdfs:range xsd:boolean ;
                       era:rinfIndex "1.2.2.0.4.1" ;
                       dct:created "2021-08-10"^^xsd:date ;
                       dct:modified "2021-08-10"^^xsd:date ;
                       rdfs:comment "Indication whether exists an installation for toilet discharge (fixed installation for servicing trains) as defined in INF TSIs."@en ;
                       rdfs:isDefinedBy <http://data.europa.eu/949/> ;
                       rdfs:label "Existence of toilet discharge"@en ;
                       vs:term_status "stable" .


###  http://data.europa.eu/949/hasTrainIntegrityConfirmation
era:hasTrainIntegrityConfirmation rdf:type owl:DatatypeProperty ,
                                           owl:FunctionalProperty ;
                                  rdfs:domain era:VehicleType ;
                                  rdfs:range xsd:boolean ;
                                  era:eratvIndex "4.13.1.9" ;
                                  dct:created "2020-08-31"^^xsd:date ;
                                  dct:modified "2021-09-12"^^xsd:date ;
                                  rdfs:comment "Indication of on-board management system about completeness of the train information."@en ;
                                  rdfs:isDefinedBy <http://data.europa.eu/949/> ;
                                  rdfs:label "Has train integrity confirmation"@en ;
                                  vs:term_status "stable" .


###  http://data.europa.eu/949/hasWalkway
era:hasWalkway rdf:type owl:DatatypeProperty ;
               rdfs:domain era:Tunnel ;
               rdfs:range xsd:boolean ;
               era:appendixD2Index "3.2.3" ;
               era:rinfIndex "1.1.1.1.8.12" ,
                             "1.2.1.0.5.10" ,
                             "1.2.2.0.5.9" ;
               dct:created "2022-10-27"^^xsd:date ;
               dct:modified "2023-03-14"^^xsd:date ;
               dct:source <https://eur-lex.europa.eu/eli/reg_impl/2019/773/oj> ;
               rdfs:comment """Indication of existence of walkways.
In https://eur-lex.europa.eu/eli/reg_impl/2019/773/oj 3.2.3 Tunnels: location, name, length, specific information such as the existence of walkways and points of safe egress as well as the location of safe areas where evacuation of passengers may take place; fire safety categorisation"""@en ;
               rdfs:isDefinedBy <http://data.europa.eu/949/> ;
               rdfs:label "Existence of walkways"@en ;
               vs:term_status "stable" .


###  http://data.europa.eu/949/hasWaterRestocking
era:hasWaterRestocking rdf:type owl:DatatypeProperty ,
                                owl:FunctionalProperty ;
                       rdfs:domain era:Siding ;
                       rdfs:range xsd:boolean ;
                       era:rinfIndex "1.2.2.0.4.3" ;
                       dct:created "2021-08-10"^^xsd:date ;
                       dct:modified "2021-08-10"^^xsd:date ;
                       rdfs:comment "Indication whether exists an installation for water restocking (fixed installation for servicing trains) as defined in INF TSIs."@en ;
                       rdfs:isDefinedBy <http://data.europa.eu/949/> ;
                       rdfs:label "Existence of water restocking"@en ;
                       vs:term_status "stable" .


###  http://data.europa.eu/949/hasWheelSlideProtectionSystem
era:hasWheelSlideProtectionSystem rdf:type owl:DatatypeProperty ,
                                           owl:FunctionalProperty ;
                                  rdfs:domain era:VehicleType ;
                                  rdfs:range xsd:boolean ;
                                  era:eratvIndex "4.7.8" ;
                                  dct:created "2021-08-31"^^xsd:date ;
                                  dct:modified "2021-08-31"^^xsd:date ;
                                  rdfs:comment "Indicates the presence of a wheel slide protection system."@en ;
                                  rdfs:isDefinedBy <http://data.europa.eu/949/> ;
                                  rdfs:label "Has wheel slide protection system"@en ;
                                  vs:term_status "stable" .


###  http://data.europa.eu/949/highSpeedLoadModelCompliance
era:highSpeedLoadModelCompliance rdf:type owl:DatatypeProperty ,
                                          owl:FunctionalProperty ;
                                 rdfs:domain [ rdf:type owl:Class ;
                                               owl:unionOf ( era:SubsetWithCommonCharacteristics
                                                             era:Track
                                                           )
                                             ] ;
                                 rdfs:range xsd:boolean ;
                                 era:rinfIndex "1.1.1.1.2.4.2" ;
                                 era:usedInRCCCalculations "true"^^xsd:boolean ;
                                 dct:created "2020-08-24"^^xsd:date ;
                                 dct:modified "2023-03-14"^^xsd:date ;
                                 rdfs:comment """For sections of line with a maximum permitted speed of 200 km/h or more.
Information regarding the procedure to be used to perform the dynamic compatibility check."""@en ;
                                 rdfs:isDefinedBy <http://data.europa.eu/949/> ;
                                 rdfs:label "Compliance of structures with the High Speed Load Model (HSLM) dynamic load model"@en ;
                                 vs:term_status "stable" .


###  http://data.europa.eu/949/hotAxleBoxDetectorGeneration
era:hotAxleBoxDetectorGeneration rdf:type owl:DatatypeProperty ,
                                          owl:FunctionalProperty ;
                                 rdfs:domain [ rdf:type owl:Class ;
                                               owl:unionOf ( era:SubsetWithCommonCharacteristics
                                                             era:Track
                                                           )
                                             ] ;
                                 rdfs:range xsd:string ;
                                 era:rinfIndex "1.1.1.1.7.7" ;
                                 era:usedInRCCCalculations "true"^^xsd:boolean ;
                                 dct:created "2020-08-24"^^xsd:date ;
                                 dct:modified "2021-09-11"^^xsd:date ;
                                 rdfs:comment """Specific for the French Italian and Swedish networks.
Generation of trackside hot axle box detector."""@en ;
                                 rdfs:isDefinedBy <http://data.europa.eu/949/> ;
                                 rdfs:label "Generation of trackside HABD"@en ;
                                 vs:term_status "stable" .


###  http://data.europa.eu/949/hotAxleBoxDetectorIdentification
era:hotAxleBoxDetectorIdentification rdf:type owl:DatatypeProperty ,
                                              owl:FunctionalProperty ;
                                     rdfs:domain [ rdf:type owl:Class ;
                                                   owl:unionOf ( era:SubsetWithCommonCharacteristics
                                                                 era:Track
                                                               )
                                                 ] ;
                                     rdfs:range xsd:string ;
                                     era:rinfIndex "1.1.1.1.7.6" ;
                                     era:usedInRCCCalculations "true"^^xsd:boolean ;
                                     dct:created "2020-08-24"^^xsd:date ;
                                     dct:modified "2021-09-11"^^xsd:date ;
                                     rdfs:comment """ISpecific for the French, Italian and Swedish networks.
Applicable if trackside HABD is not TSI compliant, identification of trackside hot axle box detector."""@en ;
                                     rdfs:isDefinedBy <http://data.europa.eu/949/> ;
                                     rdfs:label "Identification of trackside HABD"@en ;
                                     vs:term_status "stable" .


###  http://data.europa.eu/949/hotAxleBoxDetectorLocation
era:hotAxleBoxDetectorLocation rdf:type owl:DatatypeProperty ;
                               rdfs:domain [ rdf:type owl:Class ;
                                             owl:unionOf ( era:SubsetWithCommonCharacteristics
                                                           era:Track
                                                         )
                                           ] ;
                               rdfs:range xsd:double ;
                               era:rinfIndex "1.1.1.1.7.8" ;
                               era:usedInRCCCalculations "true"^^xsd:boolean ;
                               dct:created "2020-08-24"^^xsd:date ;
                               dct:modified "2021-09-11"^^xsd:date ;
                               rdfs:comment """Specific for the French Italian and Swedish networks.
Applicable if trackside HABD is not TSI compliant, localisation of trackside hot axle box detector."""@en ;
                               rdfs:isDefinedBy <http://data.europa.eu/949/> ;
                               rdfs:label "Railway location of trackside HABD"@en ;
                               vs:term_status "stable" .


###  http://data.europa.eu/949/hotAxleBoxDetectorTSICompliant
era:hotAxleBoxDetectorTSICompliant rdf:type owl:DatatypeProperty ,
                                            owl:FunctionalProperty ;
                                   rdfs:domain [ rdf:type owl:Class ;
                                                 owl:unionOf ( era:SubsetWithCommonCharacteristics
                                                               era:Track
                                                             )
                                               ] ;
                                   rdfs:range xsd:boolean ;
                                   era:rinfIndex "1.1.1.1.7.5" ;
                                   era:usedInRCCCalculations "true"^^xsd:boolean ;
                                   dct:created "2020-08-24"^^xsd:date ;
                                   dct:modified "2021-09-11"^^xsd:date ;
                                   rdfs:comment """Specific for the French, Italian and Swedish networks.
Trackside hot axle box detector TSI compliant."""@en ;
                                   rdfs:isDefinedBy <http://data.europa.eu/949/> ;
                                   rdfs:label "Trackside HABD TSI compliant"@en ;
                                   vs:term_status "stable" .


###  http://data.europa.eu/949/imCode
era:imCode rdf:type owl:DatatypeProperty ;
           rdfs:subPropertyOf dct:identifier ;
           rdf:type owl:FunctionalProperty ;
           rdfs:domain era:InfrastructureManager ;
           rdfs:range xsd:string ;
           era:appendixD2Index "1.1" ;
           era:rinfIndex "1.1.0.0.0.1" ,
                         "1.1.1.1.8.1" ,
                         "1.2.1.0.0.1" ,
                         "1.2.1.0.5.1" ,
                         "1.2.1.0.6.1" ,
                         "1.2.2.0.0.1" ,
                         "1.2.2.0.5.1" ;
           dct:created "2021-08-02"^^xsd:date ;
           dct:modified "2023-03-14"^^xsd:date ;
           dct:source <https://eur-lex.europa.eu/eli/reg_impl/2019/773/oj> ;
           rdfs:comment """Infrastructure manager means anybody or undertaking that is responsible in particular for establishing and maintaining railway infrastructure or a part thereof.
In https://eur-lex.europa.eu/eli/reg_impl/2019/773/oj  1.1 infrastructure manager's Name."""@en ;
           rdfs:isDefinedBy <http://data.europa.eu/949/> ;
           rdfs:label "IM's code"@en ;
           vs:term_status "stable" .


###  http://data.europa.eu/949/instructionsSwitchRadioSystems
era:instructionsSwitchRadioSystems rdf:type owl:DatatypeProperty ;
                                   rdfs:domain [ rdf:type owl:Class ;
                                                 owl:unionOf ( era:SubsetWithCommonCharacteristics
                                                               era:Track
                                                             )
                                               ] ;
                                   rdfs:range xsd:anyURI ;
                                   era:appendixD2Index "3.4.4" ;
                                   era:rinfIndex "1.1.1.3.8.2.1" ,
                                                 "1.2.1.1.7.2.1" ;
                                   dct:created "2022-10-28"^^xsd:date ;
                                   dct:modified "2023-03-14"^^xsd:date ;
                                   dct:source <https://eur-lex.europa.eu/eli/reg_impl/2019/773/oj> ;
                                   rdfs:comment """Name and/or reference of the document specifying the Special instructions to switch over between different radio systems.
In https://eur-lex.europa.eu/eli/reg_impl/2019/773/oj 3.4.4 Special instructions (location) to switch over between different radio systems."""@en ;
                                   rdfs:isDefinedBy <http://data.europa.eu/949/> ;
                                   rdfs:label "Special instructions to switch over between different radio systems"@en ;
                                   vs:term_status "stable" .


###  http://data.europa.eu/949/isQuietRoute
era:isQuietRoute rdf:type owl:DatatypeProperty ,
                          owl:FunctionalProperty ;
                 rdfs:domain [ rdf:type owl:Class ;
                               owl:unionOf ( era:SubsetWithCommonCharacteristics
                                             era:Track
                                           )
                             ] ;
                 rdfs:range xsd:boolean ;
                 era:rinfIndex "1.1.1.1.7.11" ;
                 dct:created "2020-11-04"^^xsd:date ;
                 dct:modified "2021-09-12"^^xsd:date ;
                 rdfs:comment "Belonging to a âquieter routeâ in accordance with Article 5b of NOI TSI."@en ;
                 rdfs:isDefinedBy <http://data.europa.eu/949/> ;
                 rdfs:label "Belonging to a quieter route"@en ;
                 vs:term_status "stable" .


###  http://data.europa.eu/949/kilometer
era:kilometer rdf:type owl:DatatypeProperty ;
              rdfs:domain era:LineReference ;
              rdfs:range xsd:double ;
              era:appendixD2Index "2.2.2" ;
              era:rinfIndex "1.1.1.1.8.12.1" ,
                            "1.1.1.1.8.13.1" ,
                            "1.1.1.3.14.3" ,
                            "1.2.0.0.0.6" ,
                            "1.2.1.0.5.10.1" ,
                            "1.2.1.0.5.11.1" ,
                            "1.2.1.0.8.3" ,
                            "1.2.2.0.5.10.1" ,
                            "1.2.2.0.5.9.1" ;
              dct:created "2021-01-29"^^xsd:date ;
              dct:modified "2021-01-29"^^xsd:date ;
              dct:source <https://eur-lex.europa.eu/eli/reg_impl/2019/773/oj> ;
              rdfs:comment """Distance measured in kilometers from the origin of a national railway line.
In https://eur-lex.europa.eu/eli/reg_impl/2019/773/oj 2.2.2 Principal locations (stations, yards, junctions, freight terminals) and their position relative to the line."""@en ;
              rdfs:isDefinedBy <http://data.europa.eu/949/> ;
              rdfs:label "Kilometer"@en ;
              vs:term_status "stable" .


###  http://data.europa.eu/949/length
era:length rdf:type owl:DatatypeProperty ,
                    owl:FunctionalProperty ;
           rdfs:domain era:Feature ;
           rdfs:range xsd:double ;
           era:appendixD2Index "2.3.6" ;
           era:eratvIndex "4.8.1" ;
           era:rinfIndex "1.1.0.0.0.5" ,
                         "1.1.1.1.8.12.1" ,
                         "1.1.1.1.8.13.1" ,
                         "1.1.1.1.8.7" ,
                         "1.1.1.3.14.5" ,
                         "1.2.1.0.5.10.1" ,
                         "1.2.1.0.5.11.1" ,
                         "1.2.1.0.5.5" ,
                         "1.2.1.0.6.4" ,
                         "1.2.2.0.2.1" ,
                         "1.2.2.0.5.10.1" ,
                         "1.2.2.0.5.5" ,
                         "1.2.2.0.5.9.1" ;
           era:usedInRCCCalculations "true"^^xsd:boolean ;
           dct:created "2021-04-01"^^xsd:date ;
           dct:modified "2021-08-11"^^xsd:date ;
           dct:source <https://eur-lex.europa.eu/eli/reg_impl/2019/773/oj> ;
           rdfs:comment """Length of a physical object, which can be a section of line, a tunnel, a platform, etc.
Length of section of line (1.1.0.0.0.5), length between operational points at start and end of section of line.
In https://eur-lex.europa.eu/eli/reg_impl/2019/773/oj 2.3.6 Length of platforms."""@en ;
           rdfs:isDefinedBy <http://data.europa.eu/949/> ;
           rdfs:label "Length"@en ;
           vs:term_status "stable" .


###  http://data.europa.eu/949/letterMarking
era:letterMarking rdf:type owl:DatatypeProperty ;
                  rdfs:domain era:VehicleType ;
                  rdfs:range xsd:string ;
                  era:eratvIndex "4.1.7" ;
                  dct:created "2021-08-25"^^xsd:date ;
                  dct:modified "2021-08-25"^^xsd:date ;
                  rdfs:comment "letter marking"@en ;
                  rdfs:isDefinedBy <http://data.europa.eu/949/> ;
                  rdfs:label "Letter marking"@en ;
                  vs:term_status "stable" .


###  http://data.europa.eu/949/linearCoordinate
era:linearCoordinate rdf:type owl:DatatypeProperty ;
                     rdfs:range xsd:double ;
                     dct:created "2021-04-01"^^xsd:date ;
                     dct:modified "2021-04-01"^^xsd:date ;
                     rdfs:comment "Indicates the position of an object within a linear positioning system. For example, relative to a national railway line."@en ;
                     rdfs:isDefinedBy <http://data.europa.eu/949/> ;
                     rdfs:label "Linear coordinate"@en ;
                     vs:term_status "stable" .


###  http://data.europa.eu/949/linesideDistanceIndicationFrequency
era:linesideDistanceIndicationFrequency rdf:type owl:DatatypeProperty ;
                                        rdfs:domain [ rdf:type owl:Class ;
                                                      owl:unionOf ( era:SubsetWithCommonCharacteristics
                                                                    era:Track
                                                                  )
                                                    ] ;
                                        rdfs:range xsd:integer ;
                                        era:appendixD2Index "3.1.3" ;
                                        era:rinfIndex "1.1.1.0.0.3" ;
                                        dct:created "2022-10-27"^^xsd:date ;
                                        dct:modified "2023-03-14"^^xsd:date ;
                                        dct:source <https://eur-lex.europa.eu/eli/reg_impl/2019/773/oj> ;
                                        rdfs:comment """Frequency of track lineside distance indications.
In https://eur-lex.europa.eu/eli/reg_impl/2019/773/oj 3.1.3 Lineside indications of distance (frequency, appearance and positioning)."""@en ;
                                        rdfs:isDefinedBy <http://data.europa.eu/949/> ;
                                        rdfs:label "Lineside distance indication frequency"@en ;
                                        vs:term_status "stable" .


###  http://data.europa.eu/949/loadCapabilitySpeed
era:loadCapabilitySpeed rdf:type owl:DatatypeProperty ;
                        rdfs:domain era:LoadCapability ;
                        rdfs:range xsd:integer ;
                        era:rinfIndex "1.1.1.1.2.4" ;
                        era:usedInRCCCalculations "true"^^xsd:boolean ;
                        dct:created "2023-01-20"^^xsd:date ;
                        rdfs:comment """Part of the load capability of a track that corresponds to the speed of the load model. 
The load capability is a value selected from the list of load models representing: line category which is amended by value of speed [km/h] permitted for a specific load model. The list of values may also be Route Availability which is amended by value of speed [miles/h] permitted for a specific load model."""@en ;
                        rdfs:isDefinedBy <http://data.europa.eu/949/> ;
                        rdfs:label "Load capability speed"@en ;
                        vs:term_status "stable" .


###  http://data.europa.eu/949/loadingPlatformHeight
era:loadingPlatformHeight rdf:type owl:DatatypeProperty ;
                          rdfs:domain era:VehicleType ;
                          rdfs:range xsd:integer ;
                          era:eratvIndex "4.8.7" ;
                          dct:created "2021-08-31"^^xsd:date ;
                          dct:modified "2021-08-31"^^xsd:date ;
                          rdfs:comment "Height of loading platform (for flat wagons and combined transport), given in mm."@en ;
                          rdfs:isDefinedBy <http://data.europa.eu/949/> ;
                          rdfs:label "Loading platform height"@en ;
                          vs:term_status "stable" .


###  http://data.europa.eu/949/localRulesOrRestrictions
era:localRulesOrRestrictions rdf:type owl:DatatypeProperty ;
                             rdfs:domain [ rdf:type owl:Class ;
                                           owl:unionOf ( era:OperationalPoint
                                                         era:Track
                                                       )
                                         ] ;
                             rdfs:range xsd:boolean ;
                             era:rinfIndex "1.1.1.4.1" ,
                                           "1.2.3.1" ;
                             dct:created "2021-08-09"^^xsd:date ;
                             dct:modified "2021-09-12"^^xsd:date ;
                             rdfs:comment "Existence of rules and restrictions of a strictly local nature."@en ;
                             rdfs:isDefinedBy <http://data.europa.eu/949/> ;
                             rdfs:label "Existence of rules and restrictions of a strictly local nature."@en ;
                             vs:term_status "stable" .


###  http://data.europa.eu/949/localRulesOrRestrictionsDoc
era:localRulesOrRestrictionsDoc rdf:type owl:DatatypeProperty ;
                                rdfs:domain [ rdf:type owl:Class ;
                                              owl:unionOf ( era:OperationalPoint
                                                            era:Track
                                                          )
                                            ] ;
                                rdfs:range xsd:anyURI ;
                                era:rinfIndex "1.1.1.4.2" ,
                                              "1.2.3.2" ;
                                dct:created "2021-08-09"^^xsd:date ;
                                dct:modified "2023-01-20"^^xsd:date ;
                                rdfs:comment "Electronic document available from the IM stored by the Agency providing additional information."@en ;
                                rdfs:isDefinedBy <http://data.europa.eu/949/> ;
                                rdfs:label "Documents regarding the rules or restrictions of a strictly local nature available by the IM"@en ;
                                vs:term_status "stable" .


###  http://data.europa.eu/949/mNvderun
era:mNvderun rdf:type owl:DatatypeProperty ;
             rdfs:domain [ rdf:type owl:Class ;
                           owl:unionOf ( era:SubsetWithCommonCharacteristics
                                         era:Track
                                       )
                         ] ;
             rdfs:range xsd:boolean ;
             era:appendixD3Index "1.5.10" ;
             era:rinfIndex "1.1.1.3.2.16.10" ,
                           "1.2.1.1.1.16.10Â " ;
             dct:created "2022-11-07"^^xsd:date ;
             dct:modified "2023-03-14"^^xsd:date ;
             rdfs:comment """Entry of Driver ID permitted while running. According to the specification referenced in Appendix A-1, index [C]. 
In https://www.era.europa.eu/sites/default/files/filesystem/ertms/ccs_tsi_annex_a_-_mandatory_specifications/set_of_specifications_3_etcs_b3_r2_gsm-r_b1/index004_-_subset-026_v360.zip
 Subset 26, chapter 7. 7.5.1.75 M_NVDERUN."""@en ;
             rdfs:isDefinedBy <http://data.europa.eu/949/> ;
             rdfs:label "M_NVDERUN"@en ;
             vs:term_status "stable" .


###  http://data.europa.eu/949/magneticBrakePrevention
era:magneticBrakePrevention rdf:type owl:DatatypeProperty ,
                                     owl:FunctionalProperty ;
                            rdfs:domain era:VehicleType ;
                            rdfs:range xsd:boolean ;
                            era:eratvIndex "4.7.4.2.2" ;
                            dct:created "2020-08-24"^^xsd:date ;
                            dct:modified "2021-04-13"^^xsd:date ;
                            rdfs:comment "Possibility of preventing the use of the magnetic track brake (only if fitted with magnetic brake)"@en ;
                            rdfs:isDefinedBy <http://data.europa.eu/949/> ;
                            rdfs:label "Magnetic brake prevention"@en ;
                            vs:term_status "stable" .


###  http://data.europa.eu/949/magneticBrakingConditionsDocument
era:magneticBrakingConditionsDocument rdf:type owl:DatatypeProperty ;
                                      rdfs:domain [ rdf:type owl:Class ;
                                                    owl:unionOf ( era:SubsetWithCommonCharacteristics
                                                                  era:Track
                                                                )
                                                  ] ;
                                      rdfs:range xsd:anyURI ;
                                      era:appendixD2Index "3.4.6" ;
                                      era:rinfIndex "1.1.1.1.6.5" ;
                                      era:usedInRCCCalculations "true"^^xsd:boolean ;
                                      dct:created "2020-08-24"^^xsd:date ;
                                      dct:modified "2021-09-11"^^xsd:date ;
                                      dct:source <https://eur-lex.europa.eu/eli/reg_impl/2019/773/oj> ;
                                      rdfs:comment """Electronic document available in two EU languages from the IM stored by the Agency with conditions for the use of magnetic brakes identified in 1.1.1.1.6.3.
In https://eur-lex.europa.eu/eli/reg_impl/2019/773/oj 3.4.6 Permissibility to use magnetic brake."""@en ;
                                      rdfs:isDefinedBy <http://data.europa.eu/949/> ;
                                      rdfs:label "Document with the conditions for the use of magnetic brakes"@en ;
                                      vs:term_status "stable" .


###  http://data.europa.eu/949/magneticBrakingFitted
era:magneticBrakingFitted rdf:type owl:DatatypeProperty ;
                          rdfs:domain era:VehicleType ;
                          rdfs:range xsd:boolean ;
                          era:eratvIndex "4.7.4.2.1" ;
                          dct:created "2022-09-12"^^xsd:date ;
                          rdfs:comment "Magnetic track brake fitted. New property defined to distinguish it from magneticBraking which is a RINF SKOS property."@en ;
                          rdfs:isDefinedBy "http://data.europa.eu/949/"^^xsd:anyURI ;
                          rdfs:label "Magnetic braking fitted"@en ;
                          vs:term_status "stable" .


###  http://data.europa.eu/949/massPerWheel
era:massPerWheel rdf:type owl:DatatypeProperty ,
                          owl:FunctionalProperty ;
                 rdfs:domain era:VehicleType ;
                 rdfs:range xsd:integer ;
                 era:eratvIndex "4.5.6" ;
                 dct:created "2021-08-26"^^xsd:date ;
                 dct:modified "2021-08-26"^^xsd:date ;
                 rdfs:comment "Mass per wheel, given in kg."@en ;
                 rdfs:isDefinedBy <http://data.europa.eu/949/> ;
                 rdfs:label "Mass per wheel"@en ;
                 vs:term_status "stable" .


###  http://data.europa.eu/949/maxCurrentStandstillPantograph
era:maxCurrentStandstillPantograph rdf:type owl:DatatypeProperty ,
                                            owl:FunctionalProperty ;
                                   rdfs:domain [ rdf:type owl:Class ;
                                                 owl:unionOf ( era:ContactLineSystem
                                                               era:Siding
                                                               era:VehicleType
                                                             )
                                               ] ;
                                   rdfs:range xsd:double ;
                                   era:appendixD2Index "3.3.8" ;
                                   era:eratvIndex "4.10.4" ;
                                   era:rinfIndex "1.1.1.2.2.3" ,
                                                 "1.2.2.0.6.1" ;
                                   era:usedInRCCCalculations "true"^^xsd:boolean ;
                                   dct:created "2020-08-25"^^xsd:date ;
                                   dct:modified "2021-09-12"^^xsd:date ;
                                   dct:source <https://eur-lex.europa.eu/eli/reg_impl/2019/773/oj> ;
                                   rdfs:comment """Indication of the maximum allowable train current at standstill expressed in amperes. 
In https://eur-lex.europa.eu/eli/reg_impl/2019/773/oj 3.3.8 Maximum current at standstill per pantograph."""@en ;
                                   rdfs:isDefinedBy <http://data.europa.eu/949/> ;
                                   rdfs:label "Maximum current at standstill per pantograph"@en ;
                                   vs:term_status "stable" .


###  http://data.europa.eu/949/maxDistConsecutiveAxles
era:maxDistConsecutiveAxles rdf:type owl:DatatypeProperty ;
                            rdfs:domain [ rdf:type owl:Class ;
                                          owl:unionOf ( era:TrainDetectionSystem
                                                        era:VehicleType
                                                      )
                                        ] ;
                            rdfs:range xsd:integer ;
                            era:eratvIndex "4.14.2.1" ;
                            era:rinfIndex "1.1.1.3.7.2.2" ;
                            dct:created "2021-08-08"^^xsd:date ;
                            dct:modified "2023-03-14"^^xsd:date ;
                            rdfs:comment "Deprecated according to the ammendment to the Regulation (EU) 2019/777. However, the parameter remains as it is also an ERATV parameter. Indication of maximum permitted distance between two consecutive axles in case of TSI non-compliance, given in millimetres."@en ;
                            rdfs:isDefinedBy <http://data.europa.eu/949/> ;
                            rdfs:label "Maximum permitted distance between two consecutive axles in case of TSI non-compliance"@en ;
                            vs:term_status "stable" .


###  http://data.europa.eu/949/maxDistEndTrainFirstAxle
era:maxDistEndTrainFirstAxle rdf:type owl:DatatypeProperty ;
                             rdfs:domain era:TrainDetectionSystem ;
                             rdfs:range xsd:integer ;
                             era:rinfIndex "1.1.1.3.7.5" ;
                             dct:created "2021-08-08"^^xsd:date ;
                             dct:modified "2023-03-14"^^xsd:date ;
                             rdfs:comment "Deprecated according to the ammendment to the Regulation (EU) 2019/777. Indication of maximum distance between end of train and first axle, given in millimetres, applicable for both sides (front and rear) of a vehicle or train."@en ;
                             rdfs:isDefinedBy <http://data.europa.eu/949/> ;
                             rdfs:label "Maximum distance between end of train and first axle"@en ;
                             owl:deprecated "true"^^xsd:boolean ;
                             vs:term_status "stable" .


###  http://data.europa.eu/949/maxFlangeHeight
era:maxFlangeHeight rdf:type owl:DatatypeProperty ;
                    rdfs:domain [ rdf:type owl:Class ;
                                  owl:unionOf ( era:TrainDetectionSystem
                                                era:VehicleType
                                              )
                                ] ;
                    rdfs:range xsd:double ;
                    era:eratvIndex "4.14.2.9" ;
                    era:rinfIndex "1.1.1.3.7.10" ;
                    dct:created "2021-08-08"^^xsd:date ;
                    dct:modified "2023-03-14"^^xsd:date ;
                    rdfs:comment "Deprecated according to the ammendment to the Regulation (EU) 2019/777. However, the parameter remains as it is also an ERATV parameter. Maximum permitted flange height, given in millimiters."@en ;
                    rdfs:isDefinedBy <http://data.europa.eu/949/> ;
                    rdfs:label "Maximum permitted height of the flange"@en ;
                    vs:term_status "stable" .


###  http://data.europa.eu/949/maxImpedanceWheelset
era:maxImpedanceWheelset rdf:type owl:DatatypeProperty ;
                         rdfs:domain [ rdf:type owl:Class ;
                                       owl:unionOf ( era:TrainDetectionSystem
                                                     era:VehicleType
                                                   )
                                     ] ;
                         rdfs:range xsd:double ;
                         era:eratvIndex "4.14.2.16" ;
                         era:rinfIndex "1.1.1.3.7.15.2" ;
                         dct:created "2021-08-08"^^xsd:date ;
                         dct:modified "2023-03-14"^^xsd:date ;
                         rdfs:comment "Deprecated according to the ammendment to the Regulation (EU) 2019/777. The value of maximum permitted impedance given in ohm in case of TSI non-compliance."@en ;
                         rdfs:isDefinedBy <http://data.europa.eu/949/> ;
                         rdfs:label "Maximum permitted impedance between opposite wheels of a wheelset when not TSI compliant"@en ;
                         vs:term_status "stable" .


###  http://data.europa.eu/949/maxLengthVehicleNose
era:maxLengthVehicleNose rdf:type owl:DatatypeProperty ;
                         rdfs:domain era:VehicleType ;
                         rdfs:range xsd:integer ;
                         era:eratvIndex "4.14.2.4" ;
                         dct:created "2021-09-01"^^xsd:date ;
                         dct:modified "2021-09-01"^^xsd:date ;
                         rdfs:comment "Maximum length of the vehicle nose."@en ;
                         rdfs:isDefinedBy <http://data.europa.eu/949/> ;
                         rdfs:label "Maximum length vehicle nose"@en ;
                         vs:term_status "stable" .


###  http://data.europa.eu/949/maxTrainCurrent
era:maxTrainCurrent rdf:type owl:DatatypeProperty ;
                    rdfs:domain era:ContactLineSystem ;
                    rdfs:range xsd:integer ;
                    era:appendixD2Index "3.3.2" ;
                    era:rinfIndex "1.1.1.2.2.2" ;
                    dct:created "2021-08-06"^^xsd:date ;
                    dct:modified "2021-08-06"^^xsd:date ;
                    dct:source "https://wiki2.railml.org/wiki/IS:maxTrainCurrent_electrification"^^xsd:anyURI ;
                    rdfs:comment """Indication of the maximum allowable train current expressed in amperes.
In https://eur-lex.europa.eu/eli/reg_impl/2019/773/oj 3.3.2 Maximum train current."""@en ;
                    rdfs:isDefinedBy <http://data.europa.eu/949/> ;
                    rdfs:label "Maximum train current"@en ;
                    vs:term_status "stable" .


###  http://data.europa.eu/949/maximumAltitude
era:maximumAltitude rdf:type owl:DatatypeProperty ,
                             owl:FunctionalProperty ;
                    rdfs:domain [ rdf:type owl:Class ;
                                  owl:unionOf ( era:SubsetWithCommonCharacteristics
                                                era:Track
                                              )
                                ] ;
                    rdfs:range xsd:double ;
                    era:rinfIndex "1.1.1.1.2.7" ;
                    dct:created "2021-08-03"^^xsd:date ;
                    dct:modified "2022-10-20"^^xsd:date ;
                    rdfs:comment "HighFest point of the section of line above sea level in reference to Normal Amsterdam's Peil (NAP)."@en ;
                    rdfs:isDefinedBy <http://data.europa.eu/949/> ;
                    rdfs:label "Maximum altitude"@en ;
                    vs:term_status "stable" .


###  http://data.europa.eu/949/maximumAverageDeceleration
era:maximumAverageDeceleration rdf:type owl:DatatypeProperty ,
                                        owl:FunctionalProperty ;
                               rdfs:domain era:VehicleType ;
                               rdfs:range xsd:double ;
                               era:eratvIndex "4.7.1" ;
                               dct:created "2021-08-26"^^xsd:date ;
                               dct:modified "2021-08-26"^^xsd:date ;
                               rdfs:comment "Maximum train deceleration given in m/sÂ²."@en ;
                               rdfs:isDefinedBy <http://data.europa.eu/949/> ;
                               rdfs:label "Maximum average deceleration"@en ;
                               vs:term_status "stable" .


###  http://data.europa.eu/949/maximumBrakeThermalEnergyCapacity
era:maximumBrakeThermalEnergyCapacity rdf:type owl:DatatypeProperty ,
                                               owl:FunctionalProperty ;
                                      rdfs:domain era:VehicleType ;
                                      rdfs:range xsd:integer ;
                                      era:eratvIndex "4.7.2.1.6" ;
                                      dct:created "2021-08-26"^^xsd:date ;
                                      dct:modified "2021-08-26"^^xsd:date ;
                                      rdfs:comment "Maximum brake thermal energy capacity given in kJ"@en ;
                                      rdfs:isDefinedBy <http://data.europa.eu/949/> ;
                                      rdfs:label "Maximum brake thermal energy capacity"@en ;
                                      vs:term_status "stable" .


###  http://data.europa.eu/949/maximumBrakingDistance
era:maximumBrakingDistance rdf:type owl:DatatypeProperty ,
                                    owl:FunctionalProperty ;
                           rdfs:domain [ rdf:type owl:Class ;
                                         owl:unionOf ( era:SubsetWithCommonCharacteristics
                                                       era:Track
                                                     )
                                       ] ;
                           rdfs:range xsd:integer ;
                           era:rinfIndex "1.1.1.3.11.1" ;
                           era:usedInRCCCalculations "true"^^xsd:boolean ;
                           dct:created "2020-08-24"^^xsd:date ;
                           dct:modified "2021-09-12"^^xsd:date ;
                           rdfs:comment "The maximum value of the braking distance [in meters] of a train shall be given for the maximum line speed."@en ;
                           rdfs:isDefinedBy <http://data.europa.eu/949/> ;
                           rdfs:label "Maximum braking distance requested"@en ;
                           vs:term_status "stable" .


###  http://data.europa.eu/949/maximumContactWireHeight
era:maximumContactWireHeight rdf:type owl:DatatypeProperty ,
                                      owl:FunctionalProperty ;
                             rdfs:domain [ rdf:type owl:Class ;
                                           owl:unionOf ( era:SubsetWithCommonCharacteristics
                                                         era:Track
                                                         era:VehicleType
                                                       )
                                         ] ;
                             rdfs:range xsd:double ;
                             era:eratvIndex "4.10.5" ;
                             era:rinfIndex "1.1.1.2.2.5" ;
                             era:usedInRCCCalculations "true"^^xsd:boolean ;
                             dct:created "2020-08-25"^^xsd:date ;
                             dct:modified "2021-09-11"^^xsd:date ;
                             rdfs:comment "Indication of the maximum contact wire height expressed in metres."@en ;
                             rdfs:isDefinedBy <http://data.europa.eu/949/> ;
                             rdfs:label "Maximum contact wire height"@en ;
                             vs:term_status "stable" .


###  http://data.europa.eu/949/maximumDesignSpeed
era:maximumDesignSpeed rdf:type owl:DatatypeProperty ,
                                owl:FunctionalProperty ;
                       rdfs:domain era:VehicleType ;
                       rdfs:range xsd:integer ;
                       era:eratvIndex "4.1.2.1" ;
                       dct:created "2020-08-24"^^xsd:date ;
                       dct:modified "2020-11-03"^^xsd:date ;
                       rdfs:comment "Maximum design speed."@en ;
                       rdfs:isDefinedBy <http://data.europa.eu/949/> ;
                       rdfs:label "Maximum design speed"@en ;
                       vs:term_status "stable" .


###  http://data.europa.eu/949/maximumInterferenceCurrent
era:maximumInterferenceCurrent rdf:type owl:DatatypeProperty ;
                               rdfs:domain era:TrainDetectionSystem ;
                               rdfs:range xsd:integer ;
                               era:rinfIndex "1.1.1.3.4.2.1" ,
                                             "1.2.1.1.3.2.1" ;
                               dct:created "2023-03-14"^^xsd:date ;
                               rdfs:comment "Maximum interference current limits allowed for track circuits for a defined frequency band."@en ;
                               rdfs:isDefinedBy <http://data.europa.eu/949/> ;
                               rdfs:label "Maximum interference current"@en ;
                               vs:term_status "stable" .


###  http://data.europa.eu/949/maximumLocomotivesCoupled
era:maximumLocomotivesCoupled rdf:type owl:DatatypeProperty ,
                                       owl:FunctionalProperty ;
                              rdfs:domain era:VehicleType ;
                              rdfs:range xsd:integer ;
                              era:eratvIndex "4.1.5" ;
                              dct:created "2021-08-25"^^xsd:date ;
                              dct:modified "2021-08-25"^^xsd:date ;
                              rdfs:comment "Maximum number of trainsets or locomotives coupled together in multiple operation."@en ;
                              rdfs:isDefinedBy <http://data.europa.eu/949/> ;
                              rdfs:label "Maximum locomotives coupled"@en ;
                              vs:term_status "stable" .


###  http://data.europa.eu/949/maximumMagneticFieldDirectionX
era:maximumMagneticFieldDirectionX rdf:type owl:DatatypeProperty ;
                                   rdfs:domain era:MaximumMagneticField ;
                                   rdfs:range xsd:integer ;
                                   era:rinfIndex "1.1.1.3.4.2.3" ,
                                                 "1.2.1.1.3.2.3" ;
                                   dct:created "2023-03-14"^^xsd:date ;
                                   rdfs:comment "The maximum magnetic field limits allowed for axle counters (in dBÂµA/m) for a defined frequency band. Direction X."@en ;
                                   rdfs:isDefinedBy <http://data.europa.eu/949/> ;
                                   rdfs:label "Maximum magnetic field direction X"@en ;
                                   vs:term_status "stable" .


###  http://data.europa.eu/949/maximumMagneticFieldDirectionY
era:maximumMagneticFieldDirectionY rdf:type owl:DatatypeProperty ;
                                   rdfs:domain era:MaximumMagneticField ;
                                   rdfs:range xsd:integer ;
                                   era:rinfIndex "1.1.1.3.4.2.3" ,
                                                 "1.2.1.1.3.2.3" ;
                                   dct:created "2023-03-14"^^xsd:date ;
                                   rdfs:comment "The maximum magnetic field limits allowed for axle counters (in dBÂµA/m) for a defined frequency band. Direction Y."@en ;
                                   rdfs:isDefinedBy <http://data.europa.eu/949/> ;
                                   rdfs:label "Maximum magnetic field direction Y"@en ;
                                   vs:term_status "stable" .


###  http://data.europa.eu/949/maximumMagneticFieldDirectionZ
era:maximumMagneticFieldDirectionZ rdf:type owl:DatatypeProperty ;
                                   rdfs:domain era:MaximumMagneticField ;
                                   rdfs:range xsd:integer ;
                                   era:rinfIndex "1.1.1.3.4.2.3" ,
                                                 "1.2.1.1.3.2.3" ;
                                   dct:created "2023-03-14"^^xsd:date ;
                                   rdfs:comment "The maximum magnetic field limits allowed for axle counters (in dBÂµA/m) for a defined frequency band. Direction Z."@en ;
                                   rdfs:isDefinedBy <http://data.europa.eu/949/> ;
                                   rdfs:label "Maximum magnetic field direction Z"@en ;
                                   vs:term_status "stable" .


###  http://data.europa.eu/949/maximumPermittedSpeed
era:maximumPermittedSpeed rdf:type owl:DatatypeProperty ,
                                   owl:FunctionalProperty ;
                          rdfs:domain [ rdf:type owl:Class ;
                                        owl:unionOf ( era:SubsetWithCommonCharacteristics
                                                      era:Track
                                                    )
                                      ] ;
                          rdfs:range xsd:integer ;
                          era:appendixD2Index "3.1.4" ;
                          era:rinfIndex "1.1.1.1.2.5" ;
                          era:usedInRCCCalculations "true"^^xsd:boolean ;
                          dct:created "2020-08-24"^^xsd:date ;
                          dct:modified "2023-03-14"^^xsd:date ;
                          rdfs:comment """Nominal maximum operational speed on the line as a result of infrastructure, energy and control, command and signalling subsystem characteristics expressed in kilometres/hour.
In https://eur-lex.europa.eu/eli/reg_impl/2019/773/oj 3.1.4 Maximum permissible speed for each track, including, if necessary, differential speeds relating to certain types of train."""@en ;
                          rdfs:isDefinedBy <http://data.europa.eu/949/> ;
                          rdfs:label "Maximum permitted speed"@en ;
                          vs:term_status "stable" .


###  http://data.europa.eu/949/maximumServiceBrake
era:maximumServiceBrake rdf:type owl:DatatypeProperty ,
                                 owl:FunctionalProperty ;
                        rdfs:domain era:VehicleType ;
                        rdfs:range xsd:string ;
                        era:eratvIndex "4.7.7" ;
                        dct:created "2021-08-26"^^xsd:date ;
                        dct:modified "2021-08-26"^^xsd:date ;
                        rdfs:comment "At maximum service brake: Stopping distance, Maximum deceleration, for the load condition 'design mass under normal payload' at the design maximum speed."@en ;
                        rdfs:isDefinedBy <http://data.europa.eu/949/> ;
                        rdfs:label "Maximum service break"@en ;
                        vs:term_status "stable" .


###  http://data.europa.eu/949/maximumSpeedAndCantDeficiency
era:maximumSpeedAndCantDeficiency rdf:type owl:DatatypeProperty ,
                                           owl:FunctionalProperty ;
                                  rdfs:domain era:VehicleType ;
                                  rdfs:range xsd:string ;
                                  era:eratvIndex "4.6.4" ;
                                  dct:created "2020-08-24"^^xsd:date ;
                                  dct:isReplacedBy era:MaximumSpeedAndCantDeficiency ,
                                                   era:vehicleTypeMaximumCantDeficiency ,
                                                   era:vehicleTypeMaximumSpeed ,
                                                   era:vehicleTypeMaximumSpeedAndCantDeficiency ;
                                  dct:modified "2023-04-05"^^xsd:date ;
                                  rdfs:comment """Combination of maximum speed and maximum cant deficiency for which the vehicle was assessed.

This property was before an object skos property. The values for this property do not come from a list of predefined values. Thus, the original object property was replaced by this datatype property with range xsd:string.
Deprecated because of replacement by a class and two integer properties. The reason is that the property represents two concepts: [number] km/h for maximum speed - [number] mm for maximum cant deificency."""@en ;
                                  rdfs:isDefinedBy <http://data.europa.eu/949/> ;
                                  rdfs:label "Maximum speed and cant deficiency"@en ;
                                  owl:deprecated "true"^^xsd:boolean ;
                                  vs:term_status "stable" .


###  http://data.europa.eu/949/maximumSpeedEmpty
era:maximumSpeedEmpty rdf:type owl:DatatypeProperty ;
                      rdfs:domain era:VehicleType ;
                      rdfs:range xsd:integer ;
                      era:eratvIndex "4.1.2.2" ;
                      dct:created "2021-08-24"^^xsd:date ;
                      dct:modified "2021-08-24"^^xsd:date ;
                      rdfs:comment "Maximum speed when empty."@en ;
                      rdfs:isDefinedBy <http://data.europa.eu/949/> ;
                      rdfs:label "Maximum speed empty"@en ;
                      vs:term_status "stable" .


###  http://data.europa.eu/949/maximumTemperature
era:maximumTemperature rdf:type owl:DatatypeProperty ;
                       rdfs:domain [ rdf:type owl:Class ;
                                     owl:unionOf ( era:SubsetWithCommonCharacteristics
                                                   era:Track
                                                   era:VehicleType
                                                 )
                                   ] ;
                       rdfs:range xsd:integer ;
                       era:eratvIndex "4.3.1" ;
                       era:rinfIndex "1.1.1.1.2.6" ;
                       era:usedInRCCCalculations "true"^^xsd:boolean ;
                       dct:created "2020-08-24"^^xsd:date ;
                       dct:modified "2021-09-10"^^xsd:date ;
                       rdfs:comment "Maximum tempertaure allowed for unrestricted operation access, according to European standard."@en ;
                       rdfs:isDefinedBy <http://data.europa.eu/949/> ;
                       rdfs:label "Temperature range (maximum)"@en ;
                       vs:term_status "stable" .


###  http://data.europa.eu/949/maximumTrainDeceleration
era:maximumTrainDeceleration rdf:type owl:DatatypeProperty ,
                                      owl:FunctionalProperty ;
                             rdfs:domain [ rdf:type owl:Class ;
                                           owl:unionOf ( era:SubsetWithCommonCharacteristics
                                                         era:Track
                                                       )
                                         ] ;
                             rdfs:range xsd:double ;
                             era:rinfIndex "1.1.1.1.6.1" ;
                             era:usedInRCCCalculations "true"^^xsd:boolean ;
                             dct:created "2020-08-24"^^xsd:date ;
                             dct:modified "2021-09-10"^^xsd:date ;
                             rdfs:comment "Limit for longitudinal track resistance given as a maximum allowed train deceleration and expressed in metres per square second."@en ;
                             rdfs:isDefinedBy <http://data.europa.eu/949/> ;
                             rdfs:label "Maximum train deceleration"@en ;
                             vs:term_status "stable" .


###  http://data.europa.eu/949/meetsRequirementVehicleAuthorisation
era:meetsRequirementVehicleAuthorisation rdf:type owl:DatatypeProperty ;
                                         rdfs:domain era:VehicleType ;
                                         rdfs:range xsd:string ;
                                         era:eratvIndex "4.1.8" ;
                                         dct:created "2021-08-25"^^xsd:date ;
                                         dct:modified "2021-08-25"^^xsd:date ;
                                         rdfs:comment "Type meets the requirements necessary for validity of the vehicle authorisation granted by one Member State in other MSs."@en ;
                                         rdfs:isDefinedBy <http://data.europa.eu/949/> ;
                                         rdfs:label "Meets requirement vehicle authorization"@en ;
                                         vs:term_status "stable" .


###  http://data.europa.eu/949/minAxleLoad
era:minAxleLoad rdf:type owl:DatatypeProperty ,
                         owl:FunctionalProperty ;
                rdfs:domain [ rdf:type owl:Class ;
                              owl:unionOf ( era:MinAxleLoadVehicleCategory
                                            era:VehicleType
                                          )
                            ] ;
                rdfs:range xsd:double ;
                era:eratvIndex "4.14.2.10" ;
                dct:created "2021-08-08"^^xsd:date ;
                dct:modified "2023-03-14"^^xsd:date ;
                rdfs:comment "Minimum permitted axle load, given in tons."@en ,
                             "Should be deprecated according to the ammendment to the Regulation (EU) 2019/777 but remains because it is also a parameter of ERATV."@en ;
                rdfs:isDefinedBy <http://data.europa.eu/949/> ;
                rdfs:label "Minimum permitted axle load"@en ;
                vs:term_status "stable" .


###  http://data.europa.eu/949/minDistConsecutiveAxles
era:minDistConsecutiveAxles rdf:type owl:DatatypeProperty ;
                            rdfs:domain era:VehicleType ;
                            rdfs:range xsd:integer ;
                            era:eratvIndex "4.14.2.2" ;
                            dct:created "2021-08-08"^^xsd:date ;
                            dct:modified "2023-03-14"^^xsd:date ;
                            rdfs:comment "Deprecated according to the ammendment to the Regulation (EU) 2019/777. However, the parameter remains as it is also an ERATV parameter. RINF index has been deleted."@en ,
                                         "Indication of minimum permitted distance between two consecutive axles, given in millimetres."@en ;
                            rdfs:isDefinedBy <http://data.europa.eu/949/> ;
                            rdfs:label "Minimum permitted distance between two consecutive axles"@en ;
                            vs:term_status "stable" .


###  http://data.europa.eu/949/minDistFirstLastAxle
era:minDistFirstLastAxle rdf:type owl:DatatypeProperty ;
                         rdfs:domain era:VehicleType ;
                         rdfs:range xsd:integer ;
                         era:eratvIndex "4.14.2.3" ;
                         dct:created "2021-08-08"^^xsd:date ;
                         dct:modified "2023-03-14"^^xsd:date ;
                         rdfs:comment "Deprecated according to the ammendment to the Regulation (EU) 2019/777. However, the parameter remains as it is also an ERATV parameter. RINF index has been deleted"@en ,
                                      "Indication of minimum permitted distance between first and last axles, given in millimetres."@en ;
                         rdfs:isDefinedBy <http://data.europa.eu/949/> ;
                         rdfs:label "Minimum permitted distance between first and last axle"@en ;
                         vs:term_status "stable" .


###  http://data.europa.eu/949/minFlangeHeight
era:minFlangeHeight rdf:type owl:DatatypeProperty ;
                    rdfs:domain era:VehicleType ;
                    rdfs:range xsd:double ;
                    era:eratvIndex "4.14.2.8" ;
                    dct:created "2021-08-08"^^xsd:date ;
                    dct:modified "2021-09-01"^^xsd:date ;
                    rdfs:comment "Deprecated according to the ammendment to the Regulation (EU) 2019/777. However, the parameter remains as it is also an ERATV parameter. RINF index has been deleted"@en ,
                                 "Minimum permitted flange height, given in millimiters."@en ;
                    rdfs:isDefinedBy <http://data.europa.eu/949/> ;
                    rdfs:label "Minimum permitted height of the flange"@en ;
                    vs:term_status "stable" .


###  http://data.europa.eu/949/minFlangeThickness
era:minFlangeThickness rdf:type owl:DatatypeProperty ;
                       rdfs:domain era:VehicleType ;
                       rdfs:range xsd:double ;
                       era:eratvIndex "4.14.2.7" ;
                       dct:created "2021-08-08"^^xsd:date ;
                       dct:modified "2021-09-01"^^xsd:date ;
                       rdfs:comment "Deprecated according to the ammendment to the Regulation (EU) 2019/777. However, the parameter remains as it is also an ERATV parameter. RINF index has been deleted"@en ,
                                    "Minimum permitted flange thickness, given in millimiters."@en ;
                       rdfs:isDefinedBy <http://data.europa.eu/949/> ;
                       rdfs:label "Minimum permitted thickness of the flange"@en ;
                       vs:term_status "stable" .


###  http://data.europa.eu/949/minRimWidth
era:minRimWidth rdf:type owl:DatatypeProperty ;
                rdfs:domain era:VehicleType ;
                rdfs:range xsd:double ;
                era:eratvIndex "4.14.2.5" ;
                dct:created "2021-08-08"^^xsd:date ;
                dct:modified "2023-03-14"^^xsd:date ;
                rdfs:comment "Deprecated according to the ammendment to the Regulation (EU) 2019/777. However, the parameter remains as it is also an ERATV parameter. RINF index has been deleted."@en ;
                rdfs:isDefinedBy <http://data.europa.eu/949/> ;
                rdfs:label "Minimum permitted width of the rim"@en ;
                vs:term_status "stable" .


###  http://data.europa.eu/949/minVehicleImpedance
era:minVehicleImpedance rdf:type owl:DatatypeProperty ;
                        rdfs:domain [ rdf:type owl:Class ;
                                      owl:unionOf ( era:TrainDetectionSystem
                                                    era:VehicleType
                                                  )
                                    ] ;
                        rdfs:range xsd:string ;
                        era:eratvIndex "4.14.2.17" ;
                        era:rinfIndex "1.1.1.3.4.2.2" ,
                                      "1.2.1.1.3.2.2" ;
                        dct:created "2021-09-01"^^xsd:date ;
                        dct:modified "2023-03-14"^^xsd:date ;
                        rdfs:comment """Impedance as defined in the specification referenced in Appendix A-1, index [D].
Impedance as defined in point 3.2.2.1 of ERA/ERTMS/033281 V5.
Minimum vehicle impedance (between wheels and pantograph) (only for vehicles equipped for 1500V or 3000V DC)."""@en ;
                        rdfs:isDefinedBy <http://data.europa.eu/949/> ;
                        rdfs:label "Vehicle impedance"@en ;
                        vs:term_status "stable" ;
                        skos:altLabel "Minimum vehicle impedance"@en .


###  http://data.europa.eu/949/minWheelDiameter
era:minWheelDiameter rdf:type owl:DatatypeProperty ;
                     rdfs:domain era:VehicleType ;
                     rdfs:range xsd:integer ;
                     era:eratvIndex "4.14.2.6" ;
                     dct:created "2021-08-08"^^xsd:date ;
                     dct:modified "2023-03-14"^^xsd:date ;
                     rdfs:comment "Deprecated according to the ammendment to the Regulation (EU) 2019/777. However, the parameter remains as it is also an ERATV parameter. RINF index has been deleted."@en ,
                                  "Minimum permitted wheel diameter, given in millimiters."@en ;
                     rdfs:isDefinedBy <http://data.europa.eu/949/> ;
                     rdfs:label "Minimum permitted wheel diameter"@en ;
                     vs:term_status "stable" .


###  http://data.europa.eu/949/minimumConcaveVerticalRadius
era:minimumConcaveVerticalRadius rdf:type owl:DatatypeProperty ,
                                          owl:FunctionalProperty ;
                                 rdfs:domain era:VehicleType ;
                                 rdfs:range xsd:integer ;
                                 era:eratvIndex "4.8.6" ;
                                 dct:created "2020-08-24"^^xsd:date ;
                                 dct:modified "2020-11-03"^^xsd:date ;
                                 rdfs:comment "Minimum vertical concave curve radius capability."@en ;
                                 rdfs:isDefinedBy <http://data.europa.eu/949/> ;
                                 rdfs:label "Minimum concave vertical radius"@en ;
                                 vs:term_status "stable" .


###  http://data.europa.eu/949/minimumContactWireHeight
era:minimumContactWireHeight rdf:type owl:DatatypeProperty ,
                                      owl:FunctionalProperty ;
                             rdfs:domain [ rdf:type owl:Class ;
                                           owl:unionOf ( era:SubsetWithCommonCharacteristics
                                                         era:Track
                                                         era:VehicleType
                                                       )
                                         ] ;
                             rdfs:range xsd:double ;
                             era:eratvIndex "4.10.5" ;
                             era:rinfIndex "1.1.1.2.2.6" ;
                             era:usedInRCCCalculations "true"^^xsd:boolean ;
                             dct:created "2020-08-25"^^xsd:date ;
                             dct:modified "2021-09-11"^^xsd:date ;
                             rdfs:comment "Indication of the minimum contact wire height expressed in metres."@en ;
                             rdfs:isDefinedBy <http://data.europa.eu/949/> ;
                             rdfs:label "Minimum contact wire height"@en ;
                             vs:term_status "stable" .


###  http://data.europa.eu/949/minimumConvexVerticalRadius
era:minimumConvexVerticalRadius rdf:type owl:DatatypeProperty ,
                                         owl:FunctionalProperty ;
                                rdfs:domain era:VehicleType ;
                                rdfs:range xsd:integer ;
                                era:eratvIndex "4.8.5" ;
                                dct:created "2020-08-24"^^xsd:date ;
                                dct:modified "2020-11-03"^^xsd:date ;
                                rdfs:comment "Minimum vertical convex curve radius capability."@en ;
                                rdfs:isDefinedBy <http://data.europa.eu/949/> ;
                                rdfs:label "Minimum convex vertical radius"@en ;
                                vs:term_status "stable" .


###  http://data.europa.eu/949/minimumHorizontalRadius
era:minimumHorizontalRadius rdf:type owl:DatatypeProperty ,
                                     owl:FunctionalProperty ;
                            rdfs:domain [ rdf:type owl:Class ;
                                          owl:unionOf ( era:Siding
                                                        era:SubsetWithCommonCharacteristics
                                                        era:Track
                                                        era:VehicleType
                                                      )
                                        ] ;
                            rdfs:range xsd:integer ;
                            era:eratvIndex "4.8.4" ;
                            era:rinfIndex "1.1.1.1.3.7" ,
                                          "1.2.2.0.3.2" ;
                            era:usedInRCCCalculations "true"^^xsd:boolean ;
                            dct:created "2020-08-24"^^xsd:date ;
                            dct:modified "2021-09-10"^^xsd:date ;
                            rdfs:comment "Radius of the smallest horizontal curve of the track in metres."@en ;
                            rdfs:isDefinedBy <http://data.europa.eu/949/> ;
                            rdfs:label "Minimum radius of horizontal curve"@en ;
                            vs:term_status "stable" .


###  http://data.europa.eu/949/minimumTemperature
era:minimumTemperature rdf:type owl:DatatypeProperty ;
                       rdfs:domain [ rdf:type owl:Class ;
                                     owl:unionOf ( era:SubsetWithCommonCharacteristics
                                                   era:Track
                                                   era:VehicleType
                                                 )
                                   ] ;
                       rdfs:range xsd:integer ;
                       era:eratvIndex "4.3.1" ;
                       era:rinfIndex "1.1.1.1.2.6" ;
                       era:usedInRCCCalculations "true"^^xsd:boolean ;
                       dct:created "2020-08-24"^^xsd:date ;
                       dct:modified "2021-09-10"^^xsd:date ;
                       rdfs:comment "Minimum tempertaure allowed for unrestricted operation access, according to European standard."@en ;
                       rdfs:isDefinedBy <http://data.europa.eu/949/> ;
                       rdfs:label "Temperature range (minimum)"@en ;
                       vs:term_status "stable" .


###  http://data.europa.eu/949/minimumVerticalRadius
era:minimumVerticalRadius rdf:type owl:DatatypeProperty ,
                                   owl:FunctionalProperty ;
                          rdfs:domain era:Siding ;
                          rdfs:range xsd:string ;
                          era:rinfIndex "1.2.2.0.3.3" ;
                          dct:created "2020-08-24"^^xsd:date ;
                          dct:isReplacedBy era:minimumVerticalRadiusCrest ,
                                           era:minimumVerticalRadiusHollow ;
                          dct:modified "2023-04-05"^^xsd:date ;
                          rdfs:comment """Radius of the smallest vertical curve expressed in metres. 
Deprecated because of replacement by  two integer properties The reason is that the property is composed of two values: The first âNNNâ is a value of crest, the second âNNNâ is a value of hollow, both expressed in metres."""@en ;
                          rdfs:isDefinedBy <http://data.europa.eu/949/> ;
                          rdfs:label "Minimum radius of vertical curve"@en ;
                          owl:deprecated "true"^^xsd:boolean ;
                          vs:term_status "stable" .


###  http://data.europa.eu/949/minimumVerticalRadiusCrest
era:minimumVerticalRadiusCrest rdf:type owl:DatatypeProperty ;
                               rdfs:domain era:Siding ;
                               rdfs:range xsd:integer ;
                               era:rinfIndex "1.2.2.0.3.3" ;
                               era:usedInRCCCalculations "true"^^xsd:boolean ;
                               dct:created "2023-04-05" ;
                               rdfs:comment """Part of the minimum radius of vertical curve that indicates the crest. 
The minimum radius of vertical curve is the radius of the smallest vertical curve expressed in metres."""@en ;
                               rdfs:isDefinedBy <http://data.europa.eu/949/> ;
                               rdfs:label "Minimum radius of vertical curve crest"@en ;
                               vs:term_status "stable" .


###  http://data.europa.eu/949/minimumVerticalRadiusHollow
era:minimumVerticalRadiusHollow rdf:type owl:DatatypeProperty ;
                                rdfs:domain era:Siding ;
                                rdfs:range xsd:integer ;
                                era:rinfIndex "1.2.2.0.3.3" ;
                                era:usedInRCCCalculations "true"^^xsd:boolean ;
                                dct:created "2023-04-05" ;
                                rdfs:comment """Part of the minimum radius of vertical curve that indicates the hollow. 
The minimum radius of vertical curve is the radius of the smallest vertical curve expressed in metres."""@en ;
                                rdfs:isDefinedBy <http://data.europa.eu/949/> ;
                                rdfs:label "Minimum radius of vertical curve hollow"@en ;
                                vs:term_status "stable" .


###  http://data.europa.eu/949/minimumWheelDiameter
era:minimumWheelDiameter rdf:type owl:DatatypeProperty ,
                                  owl:FunctionalProperty ;
                         rdfs:domain [ rdf:type owl:Class ;
                                       owl:unionOf ( era:SubsetWithCommonCharacteristics
                                                     era:Track
                                                     era:VehicleType
                                                   )
                                     ] ;
                         rdfs:range xsd:integer ;
                         era:eratvIndex "4.8.2" ;
                         era:rinfIndex "1.1.1.1.5.2" ;
                         era:usedInRCCCalculations "true"^^xsd:boolean ;
                         dct:created "2020-08-24"^^xsd:date ;
                         dct:modified "2021-09-10"^^xsd:date ;
                         rdfs:comment "Maximum unguided length of fixed obtuse crossings is based on a minimum wheel diameter in service expressed in millimetres."@en ;
                         rdfs:isDefinedBy <http://data.europa.eu/949/> ;
                         rdfs:label "Minimum wheel diameter for fixed obtuse crossings"@en ;
                         vs:term_status "stable" .


###  http://data.europa.eu/949/multipleTrainProtectionRequired
era:multipleTrainProtectionRequired rdf:type owl:DatatypeProperty ,
                                             owl:FunctionalProperty ;
                                    rdfs:domain [ rdf:type owl:Class ;
                                                  owl:unionOf ( era:SubsetWithCommonCharacteristics
                                                                era:Track
                                                              )
                                                ] ;
                                    rdfs:range xsd:boolean ;
                                    era:rinfIndex "1.1.1.3.5.2" ;
                                    dct:created "2021-08-09"^^xsd:date ;
                                    dct:modified "2023-03-14"^^xsd:date ;
                                    rdfs:comment "Deprecated according to the ammendment to the Regulation (EU) 2019/777. Indication whether more than one train protection, control and warning system is required to be on-board and active simultaneously."@en ;
                                    rdfs:isDefinedBy <http://data.europa.eu/949/> ;
                                    rdfs:label "Need for more than one train protection, control and warning system required on board"@en ;
                                    owl:deprecated "true"^^xsd:boolean ;
                                    vs:term_status "unstable" .


###  http://data.europa.eu/949/nationalLoadCapability
era:nationalLoadCapability rdf:type owl:DatatypeProperty ;
                           rdfs:domain [ rdf:type owl:Class ;
                                         owl:unionOf ( era:SubsetWithCommonCharacteristics
                                                       era:Track
                                                     )
                                       ] ;
                           rdfs:range xsd:string ;
                           era:rinfIndex "1.1.1.1.2.4.1" ;
                           era:usedInRCCCalculations "true"^^xsd:boolean ;
                           dct:created "2020-08-24"^^xsd:date ;
                           dct:modified "2021-09-10"^^xsd:date ;
                           rdfs:comment "National classification for load capability."@en ;
                           rdfs:isDefinedBy <http://data.europa.eu/949/> ;
                           rdfs:label "National classification for load capability"@en ;
                           vs:term_status "stable" .


###  http://data.europa.eu/949/nationalRollingStockFireCategory
era:nationalRollingStockFireCategory rdf:type owl:DatatypeProperty ,
                                              owl:FunctionalProperty ;
                                     rdfs:domain era:Tunnel ;
                                     rdfs:range xsd:string ;
                                     era:rinfIndex "1.1.1.1.8.11" ,
                                                   "1.2.1.0.5.8" ,
                                                   "1.2.2.0.5.8" ;
                                     era:usedInRCCCalculations "true"^^xsd:boolean ;
                                     dct:created "2020-07-29"^^xsd:date ;
                                     dct:modified "2021-08-10"^^xsd:date ;
                                     rdfs:comment "Categorisation how a passenger train with a fire on board will continue to operate for a defined time period â according to national rules if they exist"@en ;
                                     rdfs:isDefinedBy <http://data.europa.eu/949/> ;
                                     rdfs:label "National fire category of rolling stock required"@en ;
                                     vs:term_status "stable" .


###  http://data.europa.eu/949/nationalValuesBrakeModel
era:nationalValuesBrakeModel rdf:type owl:DatatypeProperty ;
                             rdfs:domain [ rdf:type owl:Class ;
                                           owl:unionOf ( era:SubsetWithCommonCharacteristics
                                                         era:Track
                                                       )
                                         ] ;
                             rdfs:range xsd:string ;
                             era:rinfIndex "1.1.1.3.2.16.13" ,
                                           "1.2.1.1.1.16.13" ;
                             dct:created "2023-03-14"^^xsd:date ;
                             rdfs:comment """Set of parameters for adapting the braking curves calculated by the ETCS on-board system to match accuracy, performance and safety margins imposed by the infrastructure manager.
It copies the content of Packet 3 or of Packet 203 as defined in the specification referenced in Appendix A-1, index [C]. 
It copies the content of Packet 3 (for M_VERSION above 2.0) as defined in SRS 7.4.2.1.1 or of Packet 203 (for M_VERSION 1.1) , as defined in SRS 6.5.1.5.22,"""@en ;
                             rdfs:isDefinedBy "http://data.europa.eu/949/" ;
                             rdfs:label "National Values used for the brake model"@en ;
                             vs:term_status "stable" .


###  http://data.europa.eu/949/nonCodedRestrictions
era:nonCodedRestrictions rdf:type owl:DatatypeProperty ,
                                  owl:FunctionalProperty ;
                         rdfs:domain era:VehicleType ;
                         rdfs:range xsd:string ;
                         dct:created "2022-06-15"^^xsd:date ;
                         dct:modified "2022-06-15"^^xsd:date ;
                         rdfs:comment "Denotes a non coded restrictions for this particular vehicleType, as a set of sentences."@en ;
                         rdfs:isDefinedBy <http://data.europa.eu/949/> ;
                         rdfs:label "Non coded restrictions"@en ;
                         vs:term_status "stable" .


###  http://data.europa.eu/949/numberElementsRakeFreightWagons
era:numberElementsRakeFreightWagons rdf:type owl:DatatypeProperty ;
                                    rdfs:domain era:VehicleType ;
                                    rdfs:range xsd:integer ;
                                    era:eratvIndex "4.1.6" ;
                                    dct:created "2021-08-25"^^xsd:date ;
                                    dct:modified "2021-08-25"^^xsd:date ;
                                    rdfs:comment "Number of elements in the rake of freight wagons (only for subcategory 'rake of freight wagons')"@en ;
                                    rdfs:isDefinedBy <http://data.europa.eu/949/> ;
                                    rdfs:label "Number elements rake freight wagons"@en ;
                                    vs:term_status "stable" .


###  http://data.europa.eu/949/numberOfPantographsInContactWithOCL
era:numberOfPantographsInContactWithOCL rdf:type owl:DatatypeProperty ,
                                                 owl:FunctionalProperty ;
                                        rdfs:domain era:VehicleType ;
                                        rdfs:range xsd:integer ;
                                        era:eratvIndex "4.10.7" ;
                                        dct:created "2020-08-25"^^xsd:date ;
                                        dct:modified "2020-11-19"^^xsd:date ;
                                        rdfs:comment "Number of pantographs in contact with the overhead contact line (OCL) (to be indicated for each energy supply system the vehicle is equipped for)."@en ;
                                        rdfs:isDefinedBy <http://data.europa.eu/949/> ;
                                        rdfs:label "Number of pantographs in contact with OCL"@en ;
                                        vs:term_status "stable" .


###  http://data.europa.eu/949/numberOfToilets
era:numberOfToilets rdf:type owl:DatatypeProperty ;
                    rdfs:domain era:VehicleType ;
                    rdfs:range xsd:integer ;
                    era:eratvIndex "4.12.1.2" ;
                    dct:created "2021-08-31"^^xsd:date ;
                    dct:modified "2021-08-31"^^xsd:date ;
                    rdfs:comment "Number of toilets."@en ;
                    rdfs:isDefinedBy <http://data.europa.eu/949/> ;
                    rdfs:label "Number of toilets"@en ;
                    vs:term_status "stable" .


###  http://data.europa.eu/949/oclType
era:oclType rdf:type owl:DatatypeProperty ;
            rdfs:domain era:VehicleType ;
            rdfs:range xsd:string ;
            era:eratvIndex "4.10.9" ;
            dct:created "2020-08-25"^^xsd:date ;
            dct:modified "2020-10-03"^^xsd:date ;
            rdfs:comment "OCL type."@en ;
            rdfs:isDefinedBy <http://data.europa.eu/949/> ;
            rdfs:label "Ocl type"@en ;
            vs:term_status "stable" .


###  http://data.europa.eu/949/opName
era:opName rdf:type owl:DatatypeProperty ,
                    owl:FunctionalProperty ;
           rdfs:domain era:OperationalPoint ;
           rdfs:range xsd:string ;
           era:appendixD2Index "2.3.1" ;
           era:rinfIndex "1.2.0.0.0.1" ;
           dct:created "2021-09-13"^^xsd:date ;
           dct:modified "2021-09-13"^^xsd:date ;
           dct:source <https://eur-lex.europa.eu/eli/reg_impl/2019/773/oj> ;
           rdfs:comment """Name normally related to the town or village or to traffic control purpose.
In https://eur-lex.europa.eu/eli/reg_impl/2019/773/oj 2.3.1 Name of location."""@en ;
           rdfs:isDefinedBy <http://data.europa.eu/949/> ;
           rdfs:label "Name of Operational point"@en ;
           vs:term_status "stable" .


###  http://data.europa.eu/949/opTypeGaugeChangeover
era:opTypeGaugeChangeover rdf:type owl:DatatypeProperty ,
                                   owl:FunctionalProperty ;
                          rdfs:domain era:OperationalPoint ;
                          rdfs:range xsd:string ;
                          era:rinfIndex "1.2.0.0.0.4.1" ;
                          era:usedInRCCCalculations "true"^^xsd:boolean ;
                          dct:created "2021-08-11"^^xsd:date ;
                          dct:modified "2021-08-11"^^xsd:date ;
                          rdfs:comment "Type of track gauge changeover facility."@en ;
                          rdfs:isDefinedBy <http://data.europa.eu/949/> ;
                          rdfs:label "Type of track gauge changeover facility"@en ;
                          vs:term_status "stable" .


###  http://data.europa.eu/949/parkingBrake
era:parkingBrake rdf:type owl:DatatypeProperty ;
                 rdfs:domain era:VehicleType ;
                 rdfs:range xsd:boolean ;
                 era:eratvIndex "4.7.3" ;
                 dct:created "2022-04-11"^^xsd:date ;
                 dct:modified "2022-04-11"^^xsd:date ;
                 rdfs:comment "Indicates whether all vehicles of this type must be equipped with a parking brake."@en ;
                 rdfs:isDefinedBy <http://data.europa.eu/949/> ;
                 rdfs:label "Parking brake"@en ;
                 vs:term_status "stable" .


###  http://data.europa.eu/949/parkingBrakeMandatory
era:parkingBrakeMandatory rdf:type owl:DatatypeProperty ;
                          rdfs:domain era:VehicleType ;
                          rdfs:range xsd:boolean ;
                          era:eratvIndex "4.7.3.1" ;
                          dct:created "2021-08-26"^^xsd:date ;
                          dct:modified "2021-08-26"^^xsd:date ;
                          rdfs:comment "All vehicles of this type must be equipped with a parking brake (parking brake mandatory for vehicles of this type)."@en ;
                          rdfs:isDefinedBy <http://data.europa.eu/949/> ;
                          rdfs:label "Parking brake mandatory"@en ;
                          vs:term_status "stable" .


###  http://data.europa.eu/949/parkingBrakeMaximumGradient
era:parkingBrakeMaximumGradient rdf:type owl:DatatypeProperty ,
                                         owl:FunctionalProperty ;
                                rdfs:domain era:VehicleType ;
                                rdfs:range xsd:double ;
                                era:eratvIndex "4.7.3.3" ;
                                dct:created "2020-08-24"^^xsd:date ;
                                dct:modified "2020-11-03"^^xsd:date ;
                                rdfs:comment "Maximum gradient on which the unit is kept immobilised by the parking brake alone (if the vehicle is fitted with it)."@en ;
                                rdfs:isDefinedBy <http://data.europa.eu/949/> ;
                                rdfs:label "Parking brake maximum gradient"@en ;
                                vs:term_status "stable" .


###  http://data.europa.eu/949/passByNoiseLevel
era:passByNoiseLevel rdf:type owl:DatatypeProperty ;
                     rdfs:domain era:VehicleType ;
                     rdfs:range xsd:double ;
                     era:eratvIndex "4.11.1" ;
                     dct:created "2021-08-31"^^xsd:date ;
                     dct:modified "2021-08-31"^^xsd:date ;
                     rdfs:comment "Pass-by noise level given in dB(A)."@en ;
                     rdfs:isDefinedBy <http://data.europa.eu/949/> ;
                     rdfs:label "Pass-by noise level"@en ;
                     vs:term_status "stable" .


###  http://data.europa.eu/949/permissiblePayload
era:permissiblePayload rdf:type owl:DatatypeProperty ,
                                owl:FunctionalProperty ;
                       rdfs:domain era:VehicleType ;
                       rdfs:range xsd:string ;
                       era:eratvIndex "4.5.1" ;
                       dct:created "2020-08-24"^^xsd:date ;
                       dct:modified "2020-11-03"^^xsd:date ;
                       rdfs:comment "Permissible payload for different line categories."@en ;
                       rdfs:isDefinedBy <http://data.europa.eu/949/> ;
                       rdfs:label "Permissible payload"@en ;
                       vs:term_status "stable" .


###  http://data.europa.eu/949/permissionChargingElectricEnergyTractionStandstill
era:permissionChargingElectricEnergyTractionStandstill rdf:type owl:DatatypeProperty ;
                                                       rdfs:subPropertyOf owl:topDataProperty ;
                                                       rdfs:domain era:ContactLineSystem ;
                                                       rdfs:range xsd:boolean ;
                                                       era:rinfIndex "1.2.1.0.7.1" ;
                                                       dct:created "2023-03-14"^^xsd:date ;
                                                       rdfs:comment "Point at which IM authorises charging of electric energy storage for traction purposes at standstill."@en ;
                                                       rdfs:isDefinedBy <http://data.europa.eu/949/> ;
                                                       rdfs:label "Permission for charging electric energy storage for traction purposes at standstill"@en ;
                                                       vs:term_status "stable" .


###  http://data.europa.eu/949/permitUseReflectivePlates
era:permitUseReflectivePlates rdf:type owl:DatatypeProperty ;
                              rdfs:domain [ rdf:type owl:Class ;
                                            owl:unionOf ( era:SubsetWithCommonCharacteristics
                                                          era:Track
                                                        )
                                          ] ;
                              rdfs:range xsd:boolean ;
                              era:rinfIndex "1.1.1.1.7.12" ;
                              dct:created "2023-03-14"^^xsd:date ;
                              rdfs:comment "Sections where is permitted to use the reflective plates on rail freight corridors, with a view to prioritise the current bottlenecks. Specific case for Belgium, France, Italy, Portugal and Spain until 1.1.2026."@en ;
                              rdfs:isDefinedBy <http://data.europa.eu/949/> ;
                              rdfs:label "Permit of use of reflective plates"@en ;
                              vs:term_status "stable" .


###  http://data.europa.eu/949/permittedContactForce
era:permittedContactForce rdf:type owl:DatatypeProperty ,
                                   owl:FunctionalProperty ;
                          rdfs:domain [ rdf:type owl:Class ;
                                        owl:unionOf ( era:SubsetWithCommonCharacteristics
                                                      era:Track
                                                    )
                                      ] ;
                          rdfs:range xsd:string ;
                          era:rinfIndex "1.1.1.2.5.2" ;
                          era:usedInRCCCalculations "true"^^xsd:boolean ;
                          dct:created "2020-08-25"^^xsd:date ;
                          dct:modified "2021-09-12"^^xsd:date ;
                          rdfs:comment "Indication of contact force allowed expressed in newtons."@en ;
                          rdfs:isDefinedBy <http://data.europa.eu/949/> ;
                          rdfs:label "Contact force permitted"@en ;
                          vs:term_status "stable" .


###  http://data.europa.eu/949/phaseInfo
era:phaseInfo rdf:type owl:DatatypeProperty ,
                       owl:FunctionalProperty ;
              rdfs:domain [ rdf:type owl:Class ;
                            owl:unionOf ( era:SubsetWithCommonCharacteristics
                                          era:Track
                                        )
                          ] ;
              rdfs:range xsd:string ;
              era:rinfIndex "1.1.1.2.4.1.2" ;
              dct:created "2021-08-08"^^xsd:date ;
              dct:isReplacedBy era:phaseInfoLength ,
                               era:phaseInfoPantographLowered ,
                               era:phaseInfoSwitchOffBreaker ,
                               "http://data.europa.eu/949/PhaseInfo" ,
                               "http://data.europa.eu/949/phaseInfoKm" ,
                               "http://data.europa.eu/949/trackPhaseInfo" ;
              dct:modified "2023-04-05"^^xsd:date ;
              rdfs:comment """Indication of required several information on phase separation. 
Deprecated because of replacement by three properties. The reason is that the property is composed of three values: length [NNN]â â the length of the phase separation in metres; switch off breaker [Y/N], single selection of âY=yesâ or âN=noâ to show whether the breaker has to be switched off; and lower pantograph [Y/N]â, single selection of âY=yesâ or âN=noâ to show whether the pantograph has to be lowered,  Km [NNN.NNN] - the location from the start of the line where the new value is valid."""@en ;
              rdfs:isDefinedBy <http://data.europa.eu/949/> ;
              rdfs:label "Information on phase separation"@en ;
              owl:deprecated "true"^^xsd:boolean ;
              vs:term_status "stable" .


###  http://data.europa.eu/949/phaseInfoKm
era:phaseInfoKm rdf:type owl:DatatypeProperty ;
                rdfs:domain era:PhaseInfo ;
                rdfs:range xsd:double ;
                era:rinfIndex "1.1.1.2.4.1.2" ;
                dct:creator "2023-04-05"^^xsd:date ;
                rdfs:comment """Part of the phase info of a track that indicates the location from the start of the line where the new value is valid.
The phase info is the indication of required several information on phase separation."""@en ;
                rdfs:isDefinedBy <http://data.europa.eu/949/> ;
                rdfs:label "Phase info Km"@en ;
                vs:term_status "stable" .


###  http://data.europa.eu/949/phaseInfoLength
era:phaseInfoLength rdf:type owl:DatatypeProperty ;
                    rdfs:domain era:PhaseInfo ;
                    rdfs:range xsd:integer ;
                    era:rinfIndex "1.1.1.2.4.1.2" ;
                    dct:created "2023-04-05"^^xsd:date ;
                    rdfs:comment """Part of the phase info of a track that corresponds to the length of the phase separation in metres. 
The phase info is the indication of required several information on phase separation."""@en ;
                    rdfs:isDefinedBy <http://data.europa.eu/949/> ;
                    rdfs:label "Phase info length"@en ;
                    vs:term_status "stable" .


###  http://data.europa.eu/949/phaseInfoPantographLowered
era:phaseInfoPantographLowered rdf:type owl:DatatypeProperty ;
                               rdfs:domain era:PhaseInfo ;
                               rdfs:range xsd:boolean ;
                               era:rinfIndex "1.1.1.2.4.1.2" ;
                               dct:created "2023-04-05"^^xsd:date ;
                               rdfs:comment """Part of the phase info of a track that shows whether a pantograph has to be lowered.
The phase info is the indication of required several information on phase separation."""@en ;
                               rdfs:isDefinedBy <http://data.europa.eu/949/> ;
                               rdfs:label "Phase info pantograph lowered"@en ;
                               vs:term_status "stable" .


###  http://data.europa.eu/949/phaseInfoSwitchOffBreaker
era:phaseInfoSwitchOffBreaker rdf:type owl:DatatypeProperty ;
                              rdfs:domain era:PhaseInfo ;
                              rdfs:range xsd:boolean ;
                              era:rinfIndex "1.1.1.2.4.1.2" ;
                              dct:created "2023-04-05"^^xsd:date ;
                              rdfs:comment """Part of the phase info of a track that shows whether the breaker has to be switched off.
The phase info is the indication of required several information on phase separation."""@en ;
                              rdfs:isDefinedBy <http://data.europa.eu/949/> ;
                              rdfs:label "Phase info switch off breaker"@en ;
                              vs:term_status "stable" .


###  http://data.europa.eu/949/phaseSeparation
era:phaseSeparation rdf:type owl:DatatypeProperty ,
                             owl:FunctionalProperty ;
                    rdfs:domain [ rdf:type owl:Class ;
                                  owl:unionOf ( era:SubsetWithCommonCharacteristics
                                                era:Track
                                              )
                                ] ;
                    rdfs:range xsd:boolean ;
                    era:rinfIndex "1.1.1.2.4.1.1" ;
                    dct:created "2021-08-08"^^xsd:date ;
                    dct:modified "2021-09-12"^^xsd:date ;
                    rdfs:comment "Indication of existence of phase separation and required information."@en ;
                    rdfs:isDefinedBy <http://data.europa.eu/949/> ;
                    rdfs:label "Phase separation"@en ;
                    vs:term_status "stable" .


###  http://data.europa.eu/949/platformId
era:platformId rdf:type owl:DatatypeProperty ,
                        owl:FunctionalProperty ;
               rdfs:domain era:Platform ;
               rdfs:range xsd:string ;
               era:appendixD2Index "2.3.5" ;
               era:rinfIndex "1.2.1.0.6.2" ;
               dct:created "2021-09-13"^^xsd:date ;
               dct:modified "2023-03-14"^^xsd:date ;
               dct:source <https://eur-lex.europa.eu/eli/reg_impl/2019/773/oj> ;
               rdfs:comment """Unique platform identification or platform number within an Operational Point.
In 2.3.5 https://eur-lex.europa.eu/eli/reg_impl/2019/773/oj Identification of platforms."""@en ;
               rdfs:isDefinedBy <http://data.europa.eu/949/> ;
               rdfs:label "Platform id"@en ;
               vs:term_status "stable" .


###  http://data.europa.eu/949/portableBoardingAids
era:portableBoardingAids rdf:type owl:DatatypeProperty ;
                         rdfs:domain era:VehicleType ;
                         rdfs:range xsd:string ;
                         era:eratvIndex "4.12.3.3" ;
                         dct:created "2021-08-31"^^xsd:date ;
                         dct:modified "2021-08-31"^^xsd:date ;
                         rdfs:comment "Description of any portable boarding aids if considered in the design of the vehicle for meeting the PRM TSI requirements."@en ;
                         rdfs:isDefinedBy <http://data.europa.eu/949/> ;
                         rdfs:label "Portable boarding aids"@en ;
                         vs:term_status "stable" .


###  http://data.europa.eu/949/preventRegenerativeBrakeUse
era:preventRegenerativeBrakeUse rdf:type owl:DatatypeProperty ,
                                         owl:FunctionalProperty ;
                                rdfs:domain era:VehicleType ;
                                rdfs:range xsd:boolean ;
                                era:eratvIndex "4.7.4.3.2" ;
                                dct:created "2020-08-24"^^xsd:date ;
                                dct:modified "2020-11-03"^^xsd:date ;
                                rdfs:comment "Possibility of preventing the use of the regenerative brake (only if fitted with regenerative brake)."@en ;
                                rdfs:isDefinedBy <http://data.europa.eu/949/> ;
                                rdfs:label "Prevent regenerative brake use"@en ;
                                vs:term_status "stable" .


###  http://data.europa.eu/949/prioritySeats
era:prioritySeats rdf:type owl:DatatypeProperty ;
                  rdfs:domain era:VehicleType ;
                  rdfs:range xsd:string ;
                  era:eratvIndex "4.12.2.1" ;
                  dct:created "2021-08-31"^^xsd:date ;
                  dct:modified "2021-08-31"^^xsd:date ;
                  rdfs:comment "Number of priority seats."@en ;
                  rdfs:isDefinedBy <http://data.europa.eu/949/> ;
                  rdfs:label "Priority seats"@en ;
                  vs:term_status "stable" .


###  http://data.europa.eu/949/prmAccessibleToilets
era:prmAccessibleToilets rdf:type owl:DatatypeProperty ;
                         rdfs:domain era:VehicleType ;
                         rdfs:range xsd:integer ;
                         era:eratvIndex "4.12.2.3" ;
                         dct:created "2021-08-31"^^xsd:date ;
                         dct:modified "2021-08-31"^^xsd:date ;
                         rdfs:comment "Number of PRM accessible toilets."@en ;
                         rdfs:isDefinedBy <http://data.europa.eu/949/> ;
                         rdfs:label "Prm accessible toilets"@en ;
                         vs:term_status "stable" .


###  http://data.europa.eu/949/publicNetworkRoaming
era:publicNetworkRoaming rdf:type owl:DatatypeProperty ,
                                  owl:FunctionalProperty ;
                         rdfs:domain [ rdf:type owl:Class ;
                                       owl:unionOf ( era:SubsetWithCommonCharacteristics
                                                     era:Track
                                                   )
                                     ] ;
                         rdfs:range xsd:boolean ;
                         era:rinfIndex "1.1.1.3.3.6" ,
                                       "1.2.1.1.2.6" ;
                         dct:created "2021-08-09"^^xsd:date ;
                         dct:modified "2021-09-12"^^xsd:date ;
                         rdfs:comment """Existence of roaming to a public network 
In case of Y, provide the name of the public network under parameter 1.1.1.3.3.7."""@en ;
                         rdfs:isDefinedBy <http://data.europa.eu/949/> ;
                         rdfs:label "GSM-R existence of roaming to public networks"@en ;
                         vs:term_status "stable" .


###  http://data.europa.eu/949/publicNetworkRoamingDetails
era:publicNetworkRoamingDetails rdf:type owl:DatatypeProperty ,
                                         owl:FunctionalProperty ;
                                rdfs:domain [ rdf:type owl:Class ;
                                              owl:unionOf ( era:SubsetWithCommonCharacteristics
                                                            era:Track
                                                          )
                                            ] ;
                                rdfs:range xsd:string ;
                                era:rinfIndex "1.1.1.3.3.7" ,
                                              "1.2.1.1.2.7" ;
                                dct:created "2021-08-09"^^xsd:date ;
                                dct:modified "2023-04-05"^^xsd:date ;
                                rdfs:comment """If roaming to public networks is configured, please indicate to which networks, 
for which users and in which areas."""@en ;
                                rdfs:isDefinedBy <http://data.europa.eu/949/> ;
                                rdfs:label "GSM-R details on roaming to public networks"@en ;
                                owl:deprecated "true"^^xsd:boolean ;
                                vs:term_status "stable" .


###  http://data.europa.eu/949/qNvsbtsmperm
era:qNvsbtsmperm rdf:type owl:DatatypeProperty ;
                 rdfs:domain [ rdf:type owl:Class ;
                               owl:unionOf ( era:SubsetWithCommonCharacteristics
                                             era:Track
                                           )
                             ] ;
                 rdfs:range xsd:boolean ;
                 era:rinfIndex "1.1.1.3.2.16.12" ,
                               "1.2.1.1.1.16.12" ;
                 dct:created "2023-03-14"^^xsd:date ;
                 rdfs:comment "Permission to use service brake in target speed monitoring."@en ;
                 rdfs:isDefinedBy <http://data.europa.eu/949/> ;
                 rdfs:label "Q_NVSBTSMPERM"@en ;
                 vs:term_status "stable" .


###  http://data.europa.eu/949/quasiStaticGuidingForce
era:quasiStaticGuidingForce rdf:type owl:DatatypeProperty ;
                            rdfs:domain era:VehicleType ;
                            rdfs:range xsd:double ;
                            era:eratvIndex "4.5.4" ;
                            dct:created "2021-08-26"^^xsd:date ;
                            dct:modified "2021-08-26"^^xsd:date ;
                            rdfs:comment "Quasi-static guiding force (if exceeds the limit defined in TSI or not defined in the TSI), given in kN."@en ;
                            rdfs:isDefinedBy <http://data.europa.eu/949/> ;
                            rdfs:label "Quasi static guiding force"@en ;
                            vs:term_status "stable" .


###  http://data.europa.eu/949/radioNetworkId
era:radioNetworkId rdf:type owl:DatatypeProperty ;
                   rdfs:domain [ rdf:type owl:Class ;
                                 owl:unionOf ( era:SubsetWithCommonCharacteristics
                                               era:Track
                                             )
                               ] ;
                   rdfs:range xsd:integer ;
                   era:rinfIndex "1.1.1.3.3.12" ,
                                 "1.2.1.1.2.13" ;
                   dct:created "2023-03-14"^^xsd:date ;
                   rdfs:comment "Unique identification of the GSM-R network the calling mobile station has to register with, as defined in the specification referenced in Appendix A-1, index [C]."@en ;
                   rdfs:isDefinedBy <http://data.europa.eu/949/> ;
                   rdfs:label "Radio Network ID"@en ;
                   vs:term_status "stable" .


###  http://data.europa.eu/949/radioSwitchOverSpecialConditions
era:radioSwitchOverSpecialConditions rdf:type owl:DatatypeProperty ;
                                     rdfs:domain era:VehicleType ;
                                     rdfs:range xsd:string ;
                                     era:eratvIndex "4.13.2.4" ;
                                     dct:created "2021-08-31"^^xsd:date ;
                                     dct:modified "2021-08-31"^^xsd:date ;
                                     rdfs:comment "Special conditions implemented on-board to switch over between different radio systems. Given as combination of systems installed on board ('System XX'_'System YY')."@en ;
                                     rdfs:isDefinedBy <http://data.europa.eu/949/> ;
                                     rdfs:label "Radio switch over special conditions"@en ;
                                     vs:term_status "stable" .


###  http://data.europa.eu/949/railInclinationMeasurement
era:railInclinationMeasurement rdf:type owl:DatatypeProperty ,
                                        owl:FunctionalProperty ;
                               rdfs:domain [ rdf:type owl:Class ;
                                             owl:unionOf ( era:SubsetWithCommonCharacteristics
                                                           era:Track
                                                         )
                                           ] ;
                               rdfs:range xsd:integer ;
                               era:rinfIndex "1.1.1.1.4.3" ;
                               dct:created "2022-09-06"^^xsd:date ;
                               dct:description "http://data.europa.eu/949/railInclination"^^xsd:anyURI ;
                               rdfs:comment """An angle defining the inclination of the head of a rail relative to the running surface. 
This is a RINF parameter treated as an integer. It has been defined in order to distinguish it from the ERATV parameter, railInclination, which is a SKOS."""@en ,
                                            "The reason for deprecation is that the definition of this property is being rolled back, as before, the property railInclination is a SKOS for both RINF and ERATV."@en ;
                               rdfs:isDefinedBy "http://data.europa.eu/949/"^^xsd:anyURI ;
                               rdfs:label "Rail inclination measurement"@en ;
                               owl:deprecated "true"^^xsd:boolean ;
                               vs:term_status "stable" .


###  http://data.europa.eu/949/railSystemType
era:railSystemType rdf:type owl:DatatypeProperty ;
                   rdfs:domain era:SubsetWithCommonCharacteristics ;
                   rdfs:range xsd:string ;
                   dct:created "2022-11-04"^^xsd:date ;
                   rdfs:comment "Type of railway system. Can be \"High-speed\" or \"Conventional\"."@en ;
                   rdfs:isDefinedBy <http://data.europa.eu/949/> ;
                   rdfs:label "Rail system type"@en ;
                   vs:term_status "stable" .


###  http://data.europa.eu/949/raisedPantographsDistance
era:raisedPantographsDistance rdf:type owl:DatatypeProperty ;
                              rdfs:domain era:RaisedPantographsDistanceAndSpeed ;
                              rdfs:range xsd:integer ;
                              era:rinfIndex "1.1.1.2.3.3" ;
                              era:usedInRCCCalculations "true"^^xsd:boolean ;
                              dct:created "2023-04-05"^^xsd:date ;
                              rdfs:comment """Part of the raised pantographs dustance and speed of a track that corresponds to the minimum distance between pantographs, in metres.
The raised pantographs distance and speed is  the indication of maximum number of raised pantographs per train allowed and minimum spacing centre line to centre line of adjacent pantograph heads, expressed in metres, at the given speed."""@en ;
                              rdfs:isDefinedBy <http://data.europa.eu/949/> ;
                              rdfs:label "Raised pantographs distance"@en ;
                              vs:term_status "stable" .


###  http://data.europa.eu/949/raisedPantographsDistanceAndSpeed
era:raisedPantographsDistanceAndSpeed rdf:type owl:DatatypeProperty ;
                                      rdfs:domain [ rdf:type owl:Class ;
                                                    owl:unionOf ( era:SubsetWithCommonCharacteristics
                                                                  era:Track
                                                                )
                                                  ] ;
                                      rdfs:range xsd:string ;
                                      era:appendixD2Index "3.3.4" ;
                                      era:rinfIndex "1.1.1.2.3.3" ;
                                      dct:created "2020-08-25"^^xsd:date ;
                                      dct:modified "2023-04-05"^^xsd:date ;
                                      dct:source <https://eur-lex.europa.eu/eli/reg_impl/2019/773/oj> ;
                                      rdfs:comment """Indication of maximum number of raised pantographs per train allowed and minimum spacing centre line to centre line of adjacent pantograph heads, expressed in metres, at the given speed.
In https://eur-lex.europa.eu/eli/reg_impl/2019/773/oj 3.3.4 Restriction related to the position of Multiple Traction unit(s) to comply with contact line separation (position of pantograph).
Deprecated because of replacement by a class and three integer properties The reason is that the property is composed of three values: [N] is number of pantographs; [NNN] is minimum distance between pantographs, in metres; [NNN] is the speed considered in km/h."""@en ;
                                      rdfs:isDefinedBy <http://data.europa.eu/949/> ;
                                      rdfs:label "Requirements for number of raised pantographs and spacing between them, at the given speed"@en ;
                                      owl:deprecated "true"^^xsd:boolean ;
                                      vs:term_status "stable" .


###  http://data.europa.eu/949/raisedPantographsNumber
era:raisedPantographsNumber rdf:type owl:DatatypeProperty ;
                            rdfs:domain era:RaisedPantographsDistanceAndSpeed ;
                            rdfs:range xsd:integer ;
                            era:rinfIndex "1.1.1.2.3.3" ;
                            era:usedInRCCCalculations "true"^^xsd:boolean ;
                            dct:created "2023-04-05"^^xsd:date ;
                            rdfs:comment "Number of pantographs."@en ;
                            rdfs:isDefinedBy <http://data.europa.eu/949/> ;
                            rdfs:label """Part of the raised pantographs distance and speed of a track that corresponds to the number of pantographs. 
The raised pantographs distance and speed is  the indication of maximum number of raised pantographs per train allowed and minimum spacing centre line to centre line of adjacent pantograph heads, expressed in metres, at the given speed"""@en ;
                            vs:term_status "stable" .


###  http://data.europa.eu/949/raisedPantographsSpeed
era:raisedPantographsSpeed rdf:type owl:DatatypeProperty ;
                           rdfs:domain era:RaisedPantographsDistanceAndSpeed ;
                           rdfs:range xsd:integer ;
                           era:rinfIndex "1.1.1.2.3.3" ;
                           era:usedInRCCCalculations "true"^^xsd:boolean ;
                           dct:created "2023-04-05"^^xsd:date ;
                           rdfs:comment """Part of the raised pantographs distance and speed of a track that corresponds to the speed considered in km/h. 
The raised pantographs distance and speed is  the indication of maximum number of raised pantographs per train allowed and minimum spacing centre line to centre line of adjacent pantograph heads, expressed in metres, at the given speed"""@en ;
                           rdfs:isDefinedBy <http://data.europa.eu/949/> ;
                           rdfs:label "Raised pantographs speed"@en ;
                           vs:term_status "stable" .


###  http://data.europa.eu/949/redLightsRequired
era:redLightsRequired rdf:type owl:DatatypeProperty ,
                               owl:FunctionalProperty ;
                      rdfs:domain [ rdf:type owl:Class ;
                                    owl:unionOf ( era:SubsetWithCommonCharacteristics
                                                  era:Track
                                                )
                                  ] ;
                      rdfs:range xsd:boolean ;
                      era:rinfIndex "1.1.1.1.7.10" ;
                      dct:created "2021-08-08"^^xsd:date ;
                      dct:modified "2021-09-12"^^xsd:date ;
                      rdfs:comment "Sections where two steady red lights are required in accordance with OPE TSI"@en ;
                      rdfs:isDefinedBy <http://data.europa.eu/949/> ;
                      rdfs:label "Steady red lights required"@en ;
                      vs:term_status "stable" .


###  http://data.europa.eu/949/referencePassByNoiseLevel
era:referencePassByNoiseLevel rdf:type owl:DatatypeProperty ;
                              rdfs:domain era:VehicleType ;
                              rdfs:range xsd:boolean ;
                              era:eratvIndex "4.11.2" ;
                              dct:created "2021-08-31"^^xsd:date ;
                              dct:modified "2021-08-31"^^xsd:date ;
                              rdfs:comment "Pass-by noise level was measured under reference conditions."@en ;
                              rdfs:isDefinedBy <http://data.europa.eu/949/> ;
                              rdfs:label "Reference pass-by noise level"@en ;
                              vs:term_status "stable" .


###  http://data.europa.eu/949/relativeDistanceDangerPoint
era:relativeDistanceDangerPoint rdf:type owl:DatatypeProperty ;
                                rdfs:domain era:Signal ;
                                rdfs:range xsd:integer ;
                                era:rinfIndex "1.1.1.3.14.4" ,
                                              "1.2.1.0.8.4" ;
                                dct:created "2023-03-14"^^xsd:date ;
                                rdfs:comment "Distance in meters to the danger point."@en ;
                                rdfs:isDefinedBy <http://data.europa.eu/949/> ;
                                rdfs:label "Relative distance of the danger point"@en ;
                                vs:term_status "stable" .


###  http://data.europa.eu/949/relativePosition
era:relativePosition rdf:type owl:DatatypeProperty ;
                     rdfs:range xsd:double ;
                     dct:created "2021-04-01"^^xsd:date ;
                     dct:modified "2021-04-01"^^xsd:date ;
                     rdfs:comment "Indicates the position of an object relative to the linear coordinates of the associated topological object."@en ;
                     rdfs:isDefinedBy <http://data.europa.eu/949/> ;
                     rdfs:label "Relative position"@en ;
                     vs:term_status "stable" .


###  http://data.europa.eu/949/requiredSandingOverride
era:requiredSandingOverride rdf:type owl:DatatypeProperty ;
                            rdfs:domain era:TrainDetectionSystem ;
                            rdfs:range xsd:boolean ;
                            era:appendixD2Index "3.2.6" ;
                            era:rinfIndex "1.1.1.3.7.18" ;
                            dct:created "2021-08-08"^^xsd:date ;
                            dct:modified "2023-03-14"^^xsd:date ;
                            dct:source <https://eur-lex.europa.eu/eli/reg_impl/2019/773/oj> ;
                            rdfs:comment """Deprecated according to the ammendment to the Regulation (EU) 2019/777. Indication whether possibility to activate/deactivate sanding devices by driver, according to instructions from the Infrastructure Manager, is required or not.
In  https://eur-lex.europa.eu/eli/reg_impl/2019/773/oj 3.2.6 Locations of areas designated for testing the sanding equipment (if existing)."""@en ;
                            rdfs:isDefinedBy <http://data.europa.eu/949/> ;
                            rdfs:label "Sanding override by driver required"@en ;
                            owl:deprecated "true"^^xsd:boolean ;
                            vs:term_status "stable" .


###  http://data.europa.eu/949/schematicOverviewOP
era:schematicOverviewOP rdf:type owl:DatatypeProperty ;
                        rdfs:domain era:OperationalPoint ;
                        rdfs:range xsd:anyURI ;
                        era:rinfIndex "1.2.0.0.0.7.1" ;
                        dct:created "2023-03-14"^^xsd:date ;
                        rdfs:comment "Document providing the schematic overview of the  operational point."@en ;
                        rdfs:isDefinedBy <http://data.europa.eu/949/> ;
                        rdfs:label "Schematic overview of the operational point"@en ;
                        vs:term_status "stable" .


###  http://data.europa.eu/949/shortestDistanceBetweenPantographsInContactWithOCL
era:shortestDistanceBetweenPantographsInContactWithOCL rdf:type owl:DatatypeProperty ,
                                                                owl:FunctionalProperty ;
                                                       rdfs:domain era:VehicleType ;
                                                       rdfs:range xsd:string ;
                                                       era:eratvIndex "4.10.8" ;
                                                       dct:created "2020-08-25"^^xsd:date ;
                                                       dct:modified "2021-09-15"^^xsd:date ;
                                                       rdfs:comment "Shortest distance between two pantographs in contact with the OCL (to be indicated for each energy supply system the vehicle is equipped for; to be indicated for single and, if applicable, multiple operation) (only if number of raised pantographs is more than 1)."@en ;
                                                       rdfs:isDefinedBy <http://data.europa.eu/949/> ;
                                                       rdfs:label "Shortest distance between pantographs in contact with OCL"@en ;
                                                       vs:term_status "stable" .


###  http://data.europa.eu/949/sidingId
era:sidingId rdf:type owl:DatatypeProperty ;
             rdfs:subPropertyOf dct:identifier ;
             rdf:type owl:FunctionalProperty ;
             rdfs:domain era:Siding ;
             rdfs:range xsd:string ;
             era:appendixD2Index "2.2.1" ,
                                 "2.2.1.4" ;
             era:rinfIndex "1.2.2.0.0.2" ;
             dct:created "2021-09-13"^^xsd:date ;
             dct:modified "2023-03-14"^^xsd:date ;
             dct:source <https://eur-lex.europa.eu/eli/reg_impl/2019/773/oj> ;
             rdfs:comment """Unique siding identification or number within an Operational Point.
IN https://eur-lex.europa.eu/eli/reg_impl/2019/773/oj 2.2.1 Indication of running lines, loops catch/trap points and access to sidings."""@en ;
             rdfs:isDefinedBy <http://data.europa.eu/949/> ;
             rdfs:label "Identification of siding"@en ;
             vs:term_status "stable" .


###  http://data.europa.eu/949/signalId
era:signalId rdf:type owl:DatatypeProperty ;
             rdfs:subPropertyOf dct:identifier ;
             rdfs:domain era:Signal ;
             rdfs:range xsd:string ;
             era:rinfIndex "1.1.1.3.14.1" ,
                           "1.2.1.0.8.1" ;
             dct:created "2023-03-14"^^xsd:date ;
             rdfs:comment "Identifier of signal"@en ;
             rdfs:isDefinedBy <http://data.europa.eu/949/> ;
             rdfs:label "Name of signal"@en ;
             vs:term_status "stable" .


###  http://data.europa.eu/949/sleepingPlaces
era:sleepingPlaces rdf:type owl:DatatypeProperty ;
                   rdfs:domain era:VehicleType ;
                   rdfs:range xsd:string ;
                   era:eratvIndex "4.12.1.3" ;
                   dct:created "2021-08-31"^^xsd:date ;
                   dct:modified "2021-09-15"^^xsd:date ;
                   rdfs:comment "Number of sleeping places."@en ;
                   rdfs:isDefinedBy <http://data.europa.eu/949/> ;
                   rdfs:label "Sleeping places"@en ;
                   vs:term_status "stable" .


###  http://data.europa.eu/949/specificInformation
era:specificInformation rdf:type owl:DatatypeProperty ,
                                 owl:FunctionalProperty ;
                        rdfs:domain [ rdf:type owl:Class ;
                                      owl:unionOf ( era:SubsetWithCommonCharacteristics
                                                    era:Track
                                                  )
                                    ] ;
                        rdfs:range xsd:string ;
                        era:rinfIndex "1.1.1.1.3.5.1" ;
                        dct:created "2021-08-03"^^xsd:date ;
                        dct:modified "2021-09-10"^^xsd:date ;
                        rdfs:comment "Any relevant information from the IM relating to the line layout."@en ;
                        rdfs:isDefinedBy <http://data.europa.eu/949/> ;
                        rdfs:label "Specific information"@en ;
                        vs:term_status "stable" .


###  http://data.europa.eu/949/startIntrinsicCoordinate
era:startIntrinsicCoordinate rdf:type owl:DatatypeProperty ;
                             rdfs:domain era:NetElement ;
                             rdfs:range xsd:double ;
                             dct:created "2021-04-01"^^xsd:date ;
                             dct:modified "2021-04-01"^^xsd:date ;
                             rdfs:comment "Indicates the coordinate point where a linear object begins."@en ;
                             rdfs:isDefinedBy <http://data.europa.eu/949/> ;
                             rdfs:label "Start intrinsic coordinate"@en ;
                             vs:term_status "stable" .


###  http://data.europa.eu/949/startingNoiseLevel
era:startingNoiseLevel rdf:type owl:DatatypeProperty ;
                       rdfs:domain era:VehicleType ;
                       rdfs:range xsd:double ;
                       era:eratvIndex "4.11.4" ;
                       dct:created "2021-08-31"^^xsd:date ;
                       dct:modified "2021-08-31"^^xsd:date ;
                       rdfs:comment "starting noise level given in dB(A)."@en ;
                       rdfs:isDefinedBy <http://data.europa.eu/949/> ;
                       rdfs:label "Starting noise level"@en ;
                       vs:term_status "stable" .


###  http://data.europa.eu/949/staticAxleLoadExceptionalPayload
era:staticAxleLoadExceptionalPayload rdf:type owl:DatatypeProperty ,
                                              owl:FunctionalProperty ;
                                     rdfs:domain era:VehicleType ;
                                     rdfs:range xsd:double ;
                                     era:eratvIndex "4.5.3.3" ;
                                     dct:created "2020-08-24"^^xsd:date ;
                                     dct:modified "2020-11-03"^^xsd:date ;
                                     rdfs:comment "Static axle load under exceptional payload."@en ;
                                     rdfs:isDefinedBy <http://data.europa.eu/949/> ;
                                     rdfs:label "Static axle load under exceptional payload"@en ;
                                     vs:term_status "stable" .


###  http://data.europa.eu/949/staticAxleLoadNormalPayload
era:staticAxleLoadNormalPayload rdf:type owl:DatatypeProperty ,
                                         owl:FunctionalProperty ;
                                rdfs:domain era:VehicleType ;
                                rdfs:range xsd:double ;
                                era:eratvIndex "4.5.3.2" ;
                                dct:created "2020-08-24"^^xsd:date ;
                                dct:modified "2020-11-03"^^xsd:date ;
                                rdfs:comment "Static axle load under normal payload."@en ;
                                rdfs:isDefinedBy <http://data.europa.eu/949/> ;
                                rdfs:label "Static axle load under normal payload"@en ;
                                vs:term_status "stable" .


###  http://data.europa.eu/949/staticAxleLoadWorkingOrder
era:staticAxleLoadWorkingOrder rdf:type owl:DatatypeProperty ,
                                        owl:FunctionalProperty ;
                               rdfs:domain era:VehicleType ;
                               rdfs:range xsd:double ;
                               era:eratvIndex "4.5.3.1" ;
                               dct:created "2020-08-24"^^xsd:date ;
                               dct:modified "2020-11-03"^^xsd:date ;
                               rdfs:comment "Static axle load in working order."@en ;
                               rdfs:isDefinedBy <http://data.europa.eu/949/> ;
                               rdfs:label "Static axle load in working order"@en ;
                               vs:term_status "stable" .


###  http://data.europa.eu/949/stationaryNoiseLevel
era:stationaryNoiseLevel rdf:type owl:DatatypeProperty ;
                         rdfs:domain era:VehicleType ;
                         rdfs:range xsd:double ;
                         era:eratvIndex "4.11.3" ;
                         dct:created "2021-08-31"^^xsd:date ;
                         dct:modified "2021-08-31"^^xsd:date ;
                         rdfs:comment "stationary noise level given in dB(A)."@en ;
                         rdfs:isDefinedBy <http://data.europa.eu/949/> ;
                         rdfs:label "Stationary noise level"@en ;
                         vs:term_status "stable" .


###  http://data.europa.eu/949/structuralCategory
era:structuralCategory rdf:type owl:DatatypeProperty ;
                       rdfs:domain era:VehicleType ;
                       rdfs:range xsd:string ;
                       era:eratvIndex "4.1.10" ;
                       dct:created "2021-08-25"^^xsd:date ;
                       dct:modified "2021-08-25"^^xsd:date ;
                       rdfs:comment "Structural category."@en ;
                       rdfs:isDefinedBy <http://data.europa.eu/949/> ;
                       rdfs:label "Structural category"@en ;
                       vs:term_status "stable" .


###  http://data.europa.eu/949/structureCheckLocation
era:structureCheckLocation rdf:type owl:DatatypeProperty ;
                           rdfs:domain [ rdf:type owl:Class ;
                                         owl:unionOf ( era:SubsetWithCommonCharacteristics
                                                       era:Track
                                                     )
                                       ] ;
                           rdfs:range xsd:double ;
                           era:rinfIndex "1.1.1.1.2.4.3" ;
                           era:usedInRCCCalculations "true"^^xsd:boolean ;
                           dct:created "2020-08-24"^^xsd:date ;
                           dct:modified "2023-03-14"^^xsd:date ;
                           rdfs:comment "Localisation of structures requiring specific checks."@en ;
                           rdfs:isDefinedBy <http://data.europa.eu/949/> ;
                           rdfs:label "Railway location of structures requiring specific checks"@en ;
                           vs:term_status "stable" .


###  http://data.europa.eu/949/subsetName
era:subsetName rdf:type owl:DatatypeProperty ;
               rdfs:domain era:SubsetWithCommonCharacteristics ;
               rdfs:range xsd:string ;
               dct:created "2023-03-14"^^xsd:date ;
               rdfs:comment "A subset of common characteristics is identified with a unique name/id, for example \"ETCSbaseline2\" which will describe all ETCS National values (1.1.1.3.2.16 group) and it will be the same for a part of the network (set of tracks)."@en ;
               rdfs:isDefinedBy <http://data.europa.eu/949/> ;
               rdfs:label "Name of a subset with common characteristics"@en ;
               vs:term_status "stable" .


###  http://data.europa.eu/949/switchProtectControlWarning
era:switchProtectControlWarning rdf:type owl:DatatypeProperty ,
                                         owl:FunctionalProperty ;
                                rdfs:domain [ rdf:type owl:Class ;
                                              owl:unionOf ( era:SubsetWithCommonCharacteristics
                                                            era:Track
                                                          )
                                            ] ;
                                rdfs:range xsd:boolean ;
                                era:rinfIndex "1.1.1.3.8.1" ,
                                              "1.2.1.1.7.1" ;
                                dct:created "2021-08-09"^^xsd:date ;
                                dct:modified "2021-09-12"^^xsd:date ;
                                rdfs:comment "Indication whether a switch over between different systems whilst running exist."@en ;
                                rdfs:isDefinedBy <http://data.europa.eu/949/> ;
                                rdfs:label "Existence of switch over between different protection, control and warning systems while running"@en ;
                                vs:term_status "stable" .


###  http://data.europa.eu/949/switchRadioSystem
era:switchRadioSystem rdf:type owl:DatatypeProperty ,
                               owl:FunctionalProperty ;
                      rdfs:domain [ rdf:type owl:Class ;
                                    owl:unionOf ( era:SubsetWithCommonCharacteristics
                                                  era:Track
                                                )
                                  ] ;
                      rdfs:range xsd:boolean ;
                      era:rinfIndex "1.1.1.3.8.2" ,
                                    "1.2.1.1.7.2" ;
                      dct:created "2021-08-09"^^xsd:date ;
                      dct:modified "2021-09-12"^^xsd:date ;
                      rdfs:comment "Indication whether a switch over between different radio systems and no communication system whilst running exist."@en ;
                      rdfs:isDefinedBy <http://data.europa.eu/949/> ;
                      rdfs:label "Existence of switch over between different radio systems"@en ;
                      vs:term_status "stable" .


###  http://data.europa.eu/949/systemSeparationInfo
era:systemSeparationInfo rdf:type owl:DatatypeProperty ,
                                  owl:FunctionalProperty ;
                         rdfs:domain [ rdf:type owl:Class ;
                                       owl:unionOf ( era:SubsetWithCommonCharacteristics
                                                     era:Track
                                                   )
                                     ] ;
                         rdfs:range xsd:string ;
                         era:rinfIndex "1.1.1.2.4.2.2" ;
                         dct:created "2021-08-08"^^xsd:date ;
                         dct:isReplacedBy era:SystemSeparationInfo ,
                                          era:systemSeparationInfoKm ,
                                          era:systemSeparationInfoLength ,
                                          era:systemSeparationInfoSwitchOffBreaker ,
                                          era:systemSeparationLoweredPantograph ,
                                          era:trackSystemSeparationInfo ;
                         dct:modified "2023-04-05"^^xsd:date ;
                         rdfs:comment """Indication of required several information on system separation.
Deprecated because of replacement by four properties. The reason is that the property is composed of four values: length [NNN], the length of the system separation in metres; switch off breaker [Y/N]. Single selection of âY=yesâ or âN=noâ to show whether the breaker has to be switched off;  lower pantograph [Y/N]. Single selection of âY=yesâ or âN=noâ to show whether the pantograph has to be lowered, and [CharacterString]  to show whether the supply system has to be changed."""@en ;
                         rdfs:isDefinedBy <http://data.europa.eu/949/> ;
                         rdfs:label "Information on system separation"@en ;
                         owl:deprecated "true"^^xsd:boolean ;
                         vs:term_status "stable" .


###  http://data.europa.eu/949/systemSeparationInfoChangeSupplySystem
era:systemSeparationInfoChangeSupplySystem rdf:type owl:DatatypeProperty ;
                                           rdfs:domain era:SystemSeparationInfo ;
                                           rdfs:range xsd:string ;
                                           era:rinfIndex "1.1.1.2.4.2.2" ;
                                           dct:created "2023-04-05"^^xsd:date ;
                                           rdfs:comment """Part of the system separation info of a track that shows whether the supply system has to be changed.
The system separation info is the Indication of required several information on system separation."""@en ;
                                           rdfs:isDefinedBy <http://data.europa.eu/949/> ;
                                           rdfs:label "System separation info change supply system"@en ;
                                           vs:term_status "stable" .


###  http://data.europa.eu/949/systemSeparationInfoKm
era:systemSeparationInfoKm rdf:type owl:DatatypeProperty ;
                           rdfs:domain era:PhaseInfo ;
                           rdfs:range xsd:double ;
                           era:rinfIndex "1.1.1.2.4.2.2" ;
                           dct:created "2023-04-05"^^xsd:date ;
                           rdfs:comment """Part of the system separation info of a track.  Indicates the the location from the start of the line where the new value is valid.
The system separation info is the Indication of required several information on system separation."""@en ;
                           rdfs:isDefinedBy <http://data.europa.eu/949/> ;
                           rdfs:label "System separation info Km"@en ;
                           vs:term_status "stable" .


###  http://data.europa.eu/949/systemSeparationInfoLength
era:systemSeparationInfoLength rdf:type owl:DatatypeProperty ;
                               rdfs:domain era:SystemSeparationInfo ;
                               rdfs:range xsd:integer ;
                               era:rinfIndex "1.1.1.2.4.2.2" ;
                               dct:created "2023-04-05"^^xsd:date ;
                               rdfs:comment """Part of the system separation info of a track that shows the length of the system separation in metres.
The system separation info is the Indication of required several information on system separation."""@en ;
                               rdfs:isDefinedBy <http://data.europa.eu/949/> ;
                               rdfs:label "System separation info length"@en ;
                               vs:term_status "stable" .


###  http://data.europa.eu/949/systemSeparationInfoPantographLowered
era:systemSeparationInfoPantographLowered rdf:type owl:DatatypeProperty ;
                                          rdfs:domain era:SystemSeparationInfo ;
                                          rdfs:range xsd:boolean ;
                                          era:rinfIndex "1.1.1.2.4.2.2" ;
                                          dct:created "2023-04-05"^^xsd:date ;
                                          rdfs:comment """Part of the system separation info of a track that shows whether the pantograph has to be lowered.
The system separation info is the Indication of required several information on system separation."""@en ;
                                          rdfs:isDefinedBy <http://data.europa.eu/949/> ;
                                          rdfs:label "System separation info  pantograph lowered"@en ;
                                          vs:term_status "stable" .


###  http://data.europa.eu/949/systemSeparationInfoSwitchOffBreaker
era:systemSeparationInfoSwitchOffBreaker rdf:type owl:DatatypeProperty ;
                                         rdfs:domain era:SystemSeparationInfo ;
                                         rdfs:range xsd:boolean ;
                                         era:rinfIndex "1.1.1.2.4.2.2" ;
                                         dct:created "2023-04-05"^^xsd:date ;
                                         rdfs:comment """Part of the system separation info of a track that shows whether the breaker has to be switched off.
The system separation info is the Indication of required several information on system separation."""@en ;
                                         rdfs:isDefinedBy <http://data.europa.eu/949/> ;
                                         rdfs:label "System separation info switch off breaker"@en ;
                                         vs:term_status "stable" .


###  http://data.europa.eu/949/tNvcontact
era:tNvcontact rdf:type owl:DatatypeProperty ;
               rdfs:domain [ rdf:type owl:Class ;
                             owl:unionOf ( era:SubsetWithCommonCharacteristics
                                           era:Track
                                         )
                           ] ;
               rdfs:range xsd:integer ;
               era:appendixD3Index "1.5.8" ;
               era:rinfIndex "1.1.1.3.2.16.8" ,
                             "1.2.1.1.1.16.8Â " ;
               dct:created "2022-11-07"^^xsd:date ;
               dct:modified "2023-03-14"^^xsd:date ;
               rdfs:comment """Maximum time without a safe message from Radio Block Center before train reacts in seconds. 
According the specification referenced in Appendix A-1, index [C]. 
In https://www.era.europa.eu/sites/default/files/filesystem/ertms/ccs_tsi_annex_a_-_mandatory_specifications/set_of_specifications_3_etcs_b3_r2_gsm-r_b1/index004_-_subset-026_v360.zip
 Subset 26, chapter 7. 7.5.1.148 T_NVCONTACT."""@en ;
               rdfs:isDefinedBy <http://data.europa.eu/949/> ;
               rdfs:label "T_NVCONTACT"@en ;
               vs:term_status "stable" .


###  http://data.europa.eu/949/tNvovtrp
era:tNvovtrp rdf:type owl:DatatypeProperty ;
             rdfs:domain [ rdf:type owl:Class ;
                           owl:unionOf ( era:SubsetWithCommonCharacteristics
                                         era:Track
                                       )
                         ] ;
             rdfs:range xsd:integer ;
             era:appendixD3Index "1.5.6" ;
             era:rinfIndex "1.1.1.3.2.16.6" ,
                           "1.2.1.1.1.16.6Â " ;
             dct:created "2022-11-07"^^xsd:date ;
             dct:modified "2023-03-14"^^xsd:date ;
             rdfs:comment """MMaximum time for overriding the train trip in seconds. 
According to the specification referenced in Appendix A-1, index [C]. 
In https://www.era.europa.eu/sites/default/files/filesystem/ertms/ccs_tsi_annex_a_-_mandatory_specifications/set_of_specifications_3_etcs_b3_r2_gsm-r_b1/index004_-_subset-026_v360.zip
 Subset 26, chapter 7. 7.5.1.149 T_NVOVTRP."""@en ;
             rdfs:isDefinedBy <http://data.europa.eu/949/> ;
             rdfs:label "T_NVOVTRP"@en ;
             vs:term_status "stable" .


###  http://data.europa.eu/949/tafTAPCode
era:tafTAPCode rdf:type owl:DatatypeProperty ;
               rdfs:subPropertyOf dct:identifier ;
               rdf:type owl:FunctionalProperty ;
               rdfs:domain era:OperationalPoint ;
               rdfs:range xsd:string ;
               era:appendixD2Index "2.2.2" ;
               era:rinfIndex "1.2.0.0.0.3" ;
               dct:created "2020-07-29"^^xsd:date ;
               dct:modified "2021-08-11"^^xsd:date ;
               rdfs:comment "Primary code developed for TAF/TAP."@en ;
               rdfs:isDefinedBy <http://data.europa.eu/949/> ;
               rdfs:label "Primary location code developed for information exchange in accordance with the TSIs relating to telematics applications."@en ;
               vs:term_status "stable" .


###  http://data.europa.eu/949/tenGISId
era:tenGISId rdf:type owl:DatatypeProperty ,
                      owl:FunctionalProperty ;
             rdfs:domain [ rdf:type owl:Class ;
                           owl:unionOf ( era:SubsetWithCommonCharacteristics
                                         era:Track
                                       )
                         ] ;
             rdfs:range xsd:string ;
             era:rinfIndex "1.1.1.1.2.1.2" ;
             dct:created "2021-08-03"^^xsd:date ;
             dct:modified "2021-09-10"^^xsd:date ;
             rdfs:comment "Indication of the GIS identity (GIS ID) of the section of TEN-T database to which the track belongs."@en ;
             rdfs:isDefinedBy <http://data.europa.eu/949/> ;
             rdfs:label "TEN GIS identity"@en ;
             vs:term_status "stable" .


###  http://data.europa.eu/949/thermalCapacityDistance
era:thermalCapacityDistance rdf:type owl:DatatypeProperty ,
                                     owl:FunctionalProperty ;
                            rdfs:domain era:VehicleType ;
                            rdfs:range xsd:double ;
                            era:eratvIndex "4.7.2.1.4" ;
                            dct:created "2020-08-24"^^xsd:date ;
                            dct:modified "2020-11-03"^^xsd:date ;
                            rdfs:comment "Thermal capacity distance. If no reference case is indicated."@en ;
                            rdfs:isDefinedBy <http://data.europa.eu/949/> ;
                            rdfs:label "Thermal capacity distance"@en ;
                            vs:term_status "stable" .


###  http://data.europa.eu/949/thermalCapacityGradient
era:thermalCapacityGradient rdf:type owl:DatatypeProperty ,
                                     owl:FunctionalProperty ;
                            rdfs:domain era:VehicleType ;
                            rdfs:range xsd:double ;
                            era:eratvIndex "4.7.2.1.3" ;
                            dct:created "2020-08-24"^^xsd:date ;
                            dct:modified "2020-11-03"^^xsd:date ;
                            rdfs:comment "Thermal capacity gradient. If no reference case is indicated."@en ;
                            rdfs:isDefinedBy <http://data.europa.eu/949/> ;
                            rdfs:label "Thermal capacity gradient"@en ;
                            vs:term_status "stable" .


###  http://data.europa.eu/949/thermalCapacitySpeed
era:thermalCapacitySpeed rdf:type owl:DatatypeProperty ,
                                  owl:FunctionalProperty ;
                         rdfs:domain era:VehicleType ;
                         rdfs:range xsd:double ;
                         era:eratvIndex "4.7.2.1.2" ;
                         dct:created "2020-08-24"^^xsd:date ;
                         dct:modified "2020-11-03"^^xsd:date ;
                         rdfs:comment "Thermal capacity speed. If no reference case is indicated."@en ;
                         rdfs:isDefinedBy <http://data.europa.eu/949/> ;
                         rdfs:label "Thermal capacity speed"@en ;
                         vs:term_status "stable" .


###  http://data.europa.eu/949/thermalCapacityTime
era:thermalCapacityTime rdf:type owl:DatatypeProperty ,
                                 owl:FunctionalProperty ;
                        rdfs:domain era:VehicleType ;
                        rdfs:range xsd:integer ;
                        era:eratvIndex "4.7.2.1.5" ;
                        dct:created "2020-08-24"^^xsd:date ;
                        dct:modified "2020-11-03"^^xsd:date ;
                        rdfs:comment "Thermal capacity time. If no reference case is indicated."@en ;
                        rdfs:isDefinedBy <http://data.europa.eu/949/> ;
                        rdfs:label "Thermal capacity time"@en ;
                        vs:term_status "stable" .


###  http://data.europa.eu/949/tiltingSupported
era:tiltingSupported rdf:type owl:DatatypeProperty ;
                     rdfs:domain [ rdf:type owl:Class ;
                                   owl:unionOf ( era:SubsetWithCommonCharacteristics
                                                 era:Track
                                               )
                                 ] ;
                     rdfs:range xsd:boolean ;
                     era:rinfIndex "1.1.1.3.12.1" ;
                     dct:created "2021-08-09"^^xsd:date ;
                     dct:modified "2023-03-14"^^xsd:date ;
                     rdfs:comment "Deprecated according to the ammendment to the Regulation (EU) 2019/777. Indication whether tilting functions are supported by ETCS."@en ;
                     rdfs:isDefinedBy <http://data.europa.eu/949/> ;
                     rdfs:label "Indication whether tilting functions are supported by ETCS"@en ;
                     owl:deprecated "true"^^xsd:boolean ;
                     vs:term_status "stable" .


###  http://data.europa.eu/949/totalVehicleMass
era:totalVehicleMass rdf:type owl:DatatypeProperty ,
                              owl:FunctionalProperty ;
                     rdfs:domain era:VehicleType ;
                     rdfs:range xsd:integer ;
                     era:eratvIndex "4.5.5" ;
                     dct:created "2021-08-26"^^xsd:date ;
                     dct:modified "2021-08-26"^^xsd:date ;
                     rdfs:comment "Total vehicle mass (for each vehicle of the unit), given in kg."@en ;
                     rdfs:isDefinedBy <http://data.europa.eu/949/> ;
                     rdfs:label "Total vehicle mass"@en ;
                     vs:term_status "stable" .


###  http://data.europa.eu/949/trackId
era:trackId rdf:type owl:DatatypeProperty ;
            rdfs:subPropertyOf dct:identifier ;
            rdf:type owl:FunctionalProperty ;
            rdfs:domain era:Track ;
            rdfs:range xsd:string ;
            era:appendixD2Index "2.2.1.1" ;
            era:rinfIndex "1.1.1.0.0.1" ,
                          "1.2.1.0.0.2" ;
            dct:created "2021-09-09"^^xsd:date ;
            dct:modified "2021-09-09"^^xsd:date ;
            dct:source <https://eur-lex.europa.eu/eli/reg_impl/2019/773/oj> ;
            rdfs:comment """Unique track identification or unique track number within a Section of Line.
In https://eur-lex.europa.eu/eli/reg_impl/2019/773/oj 2.2.1 Indication of running lines, loops catch/trap points and access to sidings, 2.3.4 Identification and plan of tracks, including switches, 2.3.9 Identification of loops."""@en ;
            rdfs:isDefinedBy <http://data.europa.eu/949/> ;
            rdfs:label "Identification of track"@en ;
            vs:term_status "stable" .


###  http://data.europa.eu/949/trainControlSwitchOverSpecialConditions
era:trainControlSwitchOverSpecialConditions rdf:type owl:DatatypeProperty ;
                                            rdfs:domain era:VehicleType ;
                                            rdfs:range xsd:string ;
                                            era:eratvIndex "4.13.1.6" ;
                                            dct:created "2021-08-31"^^xsd:date ;
                                            dct:modified "2021-08-31"^^xsd:date ;
                                            rdfs:comment "Special conditions implemented on-board to switch over between different train protection control and warning systems. Given as combination of systems installed on board ('System XX'_'System YY')."@en ;
                                            rdfs:isDefinedBy <http://data.europa.eu/949/> ;
                                            rdfs:label "Train control switch over special conditions"@en ;
                                            vs:term_status "stable" .


###  http://data.europa.eu/949/trainDetectionSystemSpecificCheckDocument
era:trainDetectionSystemSpecificCheckDocument rdf:type owl:DatatypeProperty ;
                                              rdfs:domain era:TrainDetectionSystem ;
                                              rdfs:range xsd:anyURI ;
                                              era:rinfIndex "1.1.1.3.7.1.3" ,
                                                            "1.2.1.1.6.2" ;
                                              era:usedInRCCCalculations "true"^^xsd:boolean ;
                                              dct:created "2021-08-03"^^xsd:date ;
                                              dct:modified "2022-12-13"^^xsd:date ;
                                              rdfs:comment "Electronic document from the IM stored by the Agency with precise values in accordance with TSI CCS Article13 and the specification referenced in Appendix A-1, index [D], for the specific check to be performed for train detection systems identified in 1.1.1.3.7.1.2.  and 1.2.1.1.6.1"@en ;
                                              rdfs:isDefinedBy <http://data.europa.eu/949/> ;
                                              rdfs:label "Document with the procedure(s) related to the type of train detection systems declared in 1.2.1.1.6.1"@en ;
                                              vs:term_status "stable" .


###  http://data.europa.eu/949/trainIntegrityOnBoardRequired
era:trainIntegrityOnBoardRequired rdf:type owl:DatatypeProperty ,
                                           owl:FunctionalProperty ;
                                  rdfs:domain [ rdf:type owl:Class ;
                                                owl:unionOf ( era:SubsetWithCommonCharacteristics
                                                              era:Track
                                                            )
                                              ] ;
                                  rdfs:range xsd:boolean ;
                                  era:rinfIndex "1.1.1.3.2.8" ,
                                                "1.2.1.1.1.8" ;
                                  era:usedInRCCCalculations "true"^^xsd:boolean ;
                                  dct:created "2020-08-31"^^xsd:date ;
                                  dct:modified "2021-09-12"^^xsd:date ;
                                  rdfs:comment "Indication whether train confirmation from on-board is required to access the line for safety reasons."@en ;
                                  rdfs:isDefinedBy <http://data.europa.eu/949/> ;
                                  rdfs:label "Train integrity confirmation from on-board (not from driver) necessary for line access"@en ;
                                  vs:term_status "stable" .


###  http://data.europa.eu/949/transportableOnFerry
era:transportableOnFerry rdf:type owl:DatatypeProperty ;
                         rdfs:domain era:VehicleType ;
                         rdfs:range xsd:boolean ;
                         era:eratvIndex "4.8.8" ;
                         dct:created "2021-08-31"^^xsd:date ;
                         dct:modified "2021-08-31"^^xsd:date ;
                         rdfs:comment "Indicates the suitability for transport on ferries."@en ;
                         rdfs:isDefinedBy <http://data.europa.eu/949/> ;
                         rdfs:label "Transportable on ferry"@en ;
                         vs:term_status "stable" .


###  http://data.europa.eu/949/tsiCompliant
era:tsiCompliant rdf:type owl:DatatypeProperty ;
                 rdfs:range xsd:boolean ;
                 dct:created "2020-11-03"^^xsd:date ;
                 dct:modified "2023-01-23"^^xsd:date ;
                 rdfs:comment "Indicates if a certain property is TSI compliant."@en ,
                              "The reason for deprecation is that it is used in SKOS \"OtherPantographHeads\" and \"TsiPantographHeads\" to indicate in the first case if a SKOS concept is not tsiCompliant (false) and in the second case that the concept is tsiCompliant (true). These two SKOS were originally one SKOS, \"PantographHeads\". Currently with the two SKOS the property is redundant."@en ;
                 rdfs:isDefinedBy <http://data.europa.eu/949/> ;
                 rdfs:label "Tsi compliant"@en ;
                 owl:deprecated "true"^^xsd:boolean ;
                 vs:term_status "stable" .


###  http://data.europa.eu/949/tsiSwitchCrossing
era:tsiSwitchCrossing rdf:type owl:DatatypeProperty ,
                               owl:FunctionalProperty ;
                      rdfs:domain [ rdf:type owl:Class ;
                                    owl:unionOf ( era:SubsetWithCommonCharacteristics
                                                  era:Track
                                                )
                                  ] ;
                      rdfs:range xsd:boolean ;
                      era:rinfIndex "1.1.1.1.5.1" ;
                      dct:created "2021-08-03"^^xsd:date ;
                      dct:modified "2021-09-10"^^xsd:date ;
                      rdfs:comment "Switches and crossings are maintained to in service limit dimension as specified in TSI."@en ;
                      rdfs:isDefinedBy <http://data.europa.eu/949/> ;
                      rdfs:label "TSI compliance of in service values for switches and crossings"@en ;
                      vs:term_status "stable" .


###  http://data.europa.eu/949/tunnelDocRef
era:tunnelDocRef rdf:type owl:DatatypeProperty ;
                 rdfs:domain era:Tunnel ;
                 rdfs:range xsd:anyURI ;
                 era:rinfIndex "1.1.1.1.8.8.2" ;
                 dct:created "2021-08-03"^^xsd:date ;
                 dct:modified "2021-08-03"^^xsd:date ;
                 rdfs:comment "Electronic document available from the IM stored by the Agency with precise description of the clearance gauge and geometry of the tunnel."@en ;
                 rdfs:isDefinedBy <http://data.europa.eu/949/> ;
                 rdfs:label "Reference to a document available from the IM with precise description of the tunnel"@en ;
                 vs:term_status "stable" .


###  http://data.europa.eu/949/tunnelIdentification
era:tunnelIdentification rdf:type owl:DatatypeProperty ;
                         rdfs:subPropertyOf dct:identifier ;
                         rdf:type owl:FunctionalProperty ;
                         rdfs:domain era:Tunnel ;
                         rdfs:range xsd:string ;
                         era:appendixD2Index "3.2.3" ;
                         era:rinfIndex "1.1.1.1.8.2" ,
                                       "1.2.1.0.5.2" ,
                                       "1.2.2.0.5.2" ;
                         dct:created "2021-08-03"^^xsd:date ;
                         dct:modified "2021-09-13"^^xsd:date ;
                         dct:source <https://eur-lex.europa.eu/eli/reg_impl/2019/773/oj> ;
                         rdfs:comment """Unique tunnel identification or unique number within Member State.
In https://eur-lex.europa.eu/eli/reg_impl/2019/773/oj 3.2.3 Tunnels: location, name, length, specific information such as the existence of walkways and points of safe egress as well as the location of safe areas where evacuation of passengers may take place; fire safety categorisation."""@en ;
                         rdfs:isDefinedBy <http://data.europa.eu/949/> ;
                         rdfs:label "Tunnel identification"@en ;
                         vs:term_status "stable" .


###  http://data.europa.eu/949/tunnelKilometerEnd
era:tunnelKilometerEnd rdf:type owl:DatatypeProperty ;
                       rdfs:domain era:Tunnel ;
                       rdfs:range xsd:double ;
                       era:rinfIndex "1.1.1.1.8.4" ;
                       dct:created "2023-03-14"^^xsd:date ;
                       rdfs:comment "Kilometer of the line at the end of a tunnel."@en ;
                       rdfs:isDefinedBy <http://data.europa.eu/949/> ;
                       rdfs:label "Tunnel kilometer end"@en ;
                       vs:term_status "stable" .


###  http://data.europa.eu/949/tunnelKilometerStart
era:tunnelKilometerStart rdf:type owl:DatatypeProperty ;
                         rdfs:domain era:Tunnel ;
                         rdfs:range xsd:double ;
                         era:rinfIndex "1.1.1.1.8.3" ;
                         dct:created "2023-03-14"^^xsd:date ;
                         rdfs:comment "Geographical coordinates in decimal degrees and km of the line at the beginning of a tunnel."@en ;
                         rdfs:isDefinedBy <http://data.europa.eu/949/> ;
                         rdfs:label "Tunnel kilometer start"@en ;
                         vs:term_status "stable" .


###  http://data.europa.eu/949/typeVersionNumber
era:typeVersionNumber rdf:type owl:DatatypeProperty ,
                               owl:FunctionalProperty ;
                      rdfs:domain era:VehicleType ;
                      rdfs:range xsd:string ;
                      dct:created "2020-11-22"^^xsd:date ;
                      dct:modified "2020-11-22"^^xsd:date ;
                      rdfs:comment "Serial number that identifies a vehicle type."@en ;
                      rdfs:isDefinedBy <http://data.europa.eu/949/> ;
                      rdfs:label "Type version number"@en ;
                      vs:term_status "stable" .


###  http://data.europa.eu/949/umax2
era:umax2 rdf:type owl:DatatypeProperty ;
          rdfs:domain era:ContactLineSystem ;
          rdfs:range xsd:integer ;
          era:rinfIndex "1.1.1.2.2.1.3" ;
          era:usedInRCCCalculations "true"^^xsd:boolean ;
          dct:created "2020-08-24"^^xsd:date ;
          dct:modified "2021-08-06"^^xsd:date ;
          rdfs:comment "Highest non-permanent voltage (Umax2) for France on lines not compliant with values defined in the the specification referenced in Appendix A-2, index [1]."@en ;
          rdfs:isDefinedBy <http://data.europa.eu/949/> ;
          rdfs:label "Umax2 for lines referred to in sections 7.4.2.2.1 and 7.4.2.11.1 of Regulation (EU)1301/2014."@en ;
          vs:term_status "stable" .


###  http://data.europa.eu/949/uopid
era:uopid rdf:type owl:DatatypeProperty ;
          rdfs:subPropertyOf dct:identifier ;
          rdf:type owl:FunctionalProperty ;
          rdfs:domain era:OperationalPoint ;
          rdfs:range xsd:string ;
          era:appendixD2Index "2.2.2" ;
          era:rinfIndex "1.2.0.0.0.2" ;
          dct:created "2020-07-29"^^xsd:date ;
          dct:modified "2021-08-11"^^xsd:date ;
          dct:source <https://eur-lex.europa.eu/eli/reg_impl/2019/773/oj> ;
          rdfs:comment """Code composed of country code and alphanumeric operational point code, as defined in RINF.
In https://eur-lex.europa.eu/eli/reg_impl/2019/773/oj 2.2.2 Principal locations (stations, yards, junctions, freight terminals) and their position relative to the line."""@en ;
          rdfs:isDefinedBy <http://data.europa.eu/949/> ;
          rdfs:label "Unique OP ID"@en ;
          vs:term_status "stable" .


###  http://data.europa.eu/949/usesGroup555
era:usesGroup555 rdf:type owl:DatatypeProperty ,
                          owl:FunctionalProperty ;
                 rdfs:domain [ rdf:type owl:Class ;
                               owl:unionOf ( era:SubsetWithCommonCharacteristics
                                             era:Track
                                             era:VehicleType
                                           )
                             ] ;
                 rdfs:range xsd:boolean ;
                 era:eratvIndex "4.13.2.12" ;
                 era:rinfIndex "1.1.1.3.3.4" ,
                               "1.2.1.1.2.4" ;
                 era:usedInRCCCalculations "true"^^xsd:boolean ;
                 dct:created "2020-08-31"^^xsd:date ;
                 dct:modified "2021-09-12"^^xsd:date ;
                 rdfs:comment "Indication if group 555 is used."@en ;
                 rdfs:isDefinedBy <http://data.europa.eu/949/> ;
                 rdfs:label "GSM-R use of group 555"@en ;
                 vs:term_status "stable" .


###  http://data.europa.eu/949/vNvallowovtrp
era:vNvallowovtrp rdf:type owl:DatatypeProperty ;
                  rdfs:domain [ rdf:type owl:Class ;
                                owl:unionOf ( era:SubsetWithCommonCharacteristics
                                              era:Track
                                            )
                              ] ;
                  rdfs:range xsd:integer ;
                  era:appendixD3Index "1.5.3" ;
                  era:rinfIndex "1.1.1.3.2.16.3" ,
                                "1.2.1.1.1.16.3Â " ;
                  dct:created "2022-11-07"^^xsd:date ;
                  dct:modified "2023-03-14"^^xsd:date ;
                  rdfs:comment """Speed limit allowing the driver to select the âoverrideâ function
in km/h
According to the specification referenced in Appendix A-1, index [C]. 
In https://www.era.europa.eu/sites/default/files/filesystem/ertms/ccs_tsi_annex_a_-_mandatory_specifications/set_of_specifications_3_etcs_b3_r2_gsm-r_b1/index004_-_subset-026_v360.zip
 Chapter 7. 7.5.1.161"""@en ;
                  rdfs:isDefinedBy <http://data.europa.eu/949/> ;
                  rdfs:label "V_NVALLOWOVTRP"@en ;
                  vs:term_status "stable" .


###  http://data.europa.eu/949/vNvsupovtrp
era:vNvsupovtrp rdf:type owl:DatatypeProperty ;
                rdfs:domain [ rdf:type owl:Class ;
                              owl:unionOf ( era:SubsetWithCommonCharacteristics
                                            era:Track
                                          )
                            ] ;
                rdfs:range xsd:integer ;
                era:appendixD3Index "1.5.4" ;
                era:rinfIndex "1.1.1.3.2.16.4" ,
                              "1.2.1.1.1.16.4Â " ;
                dct:created "2022-11-07"^^xsd:date ;
                dct:modified "2023-03-14"^^xsd:date ;
                rdfs:comment """Override speed limit to be supervised when the âoverrideâ function is active  in km/h
According to the specification referenced in Appendix A-1, index [C]. 
In https://www.era.europa.eu/sites/default/files/filesystem/ertms/ccs_tsi_annex_a_-_mandatory_specifications/set_of_specifications_3_etcs_b3_r2_gsm-r_b1/index004_-_subset-026_v360.zip
 Subset 26, chapter 7. 7.5.1.163 V_NVSUPOVTRP."""@en ;
                rdfs:isDefinedBy <http://data.europa.eu/949/> ;
                rdfs:label "V_NVSUPOVTRP"@en ;
                vs:term_status "stable" .


###  http://data.europa.eu/949/validityEndDate
era:validityEndDate rdf:type owl:DatatypeProperty ;
                    rdfs:domain era:InfrastructureObject ;
                    rdfs:range xsd:date ;
                    dct:created "2022-10-19"^^xsd:date ;
                    rdfs:comment "Defines the validity end date (e.g., an operational point that is not valid anymore), so that it is possible to filter out those that are not applicable for a specific application (e.g., for route planning)"@en ;
                    rdfs:isDefinedBy "http://data.europa.eu/949/"^^xsd:anyURI ;
                    rdfs:label "Validity end date"@en ;
                    vs:term_status "stable" .


###  http://data.europa.eu/949/validityStartDate
era:validityStartDate rdf:type owl:DatatypeProperty ;
                      rdfs:domain era:InfrastructureObject ;
                      rdfs:range xsd:date ;
                      dct:created "2022-10-20"^^xsd:date ;
                      rdfs:comment "Defines the validity start date (e.g., an operational point that is not valid now since it is planned for the future), so that it is possible to filter out those that are not applicable for a specific application (e.g., for route planning)"@en ;
                      rdfs:isDefinedBy "http://data.europa.eu/949/"^^xsd:anyURI ;
                      rdfs:label "Validity start date"@en ;
                      vs:term_status "stable" .


###  http://data.europa.eu/949/vehicleContactForce
era:vehicleContactForce rdf:type owl:DatatypeProperty ,
                                 owl:FunctionalProperty ;
                        rdfs:domain era:VehicleType ;
                        rdfs:range xsd:integer ;
                        era:eratvIndex "4.10.15" ;
                        dct:created "2020-08-25"^^xsd:date ;
                        dct:modified "2020-11-03"^^xsd:date ;
                        rdfs:comment "Mean contact force."@en ;
                        rdfs:isDefinedBy <http://data.europa.eu/949/> ;
                        rdfs:label "Vehicle contact force"@en ;
                        vs:term_status "stable" .


###  http://data.europa.eu/949/vehicleKinematicGaugeOther
era:vehicleKinematicGaugeOther rdf:type owl:DatatypeProperty ;
                               rdfs:domain era:VehicleType ;
                               rdfs:range xsd:string ;
                               era:eratvIndex "4.2.2" ;
                               dct:created "2022-05-30" ;
                               rdfs:comment "Vehicle kinematic gauge  that corresponds to other gauges assessed using the kinematic method"@en ;
                               rdfs:isDefinedBy <http://data.europa.eu/949/> ;
                               rdfs:label "Vehicle kinematic gauge other"@en ;
                               vs:term_status "stable" .


###  http://data.europa.eu/949/vehicleMaxSandingOutput
era:vehicleMaxSandingOutput rdf:type owl:DatatypeProperty ;
                            rdfs:domain era:VehicleType ;
                            rdfs:range xsd:string ;
                            era:eratvIndex "4.14.2.13" ;
                            dct:created "2021-09-01"^^xsd:date ;
                            dct:modified "2021-09-01"^^xsd:date ;
                            rdfs:comment "Vehicle Maximum sanding output, given in grams per second."@en ;
                            rdfs:isDefinedBy <http://data.europa.eu/949/> ;
                            rdfs:label "Vehicle max sanding output"@en ;
                            vs:term_status "stable" .


###  http://data.europa.eu/949/vehicleNumber
era:vehicleNumber rdf:type owl:DatatypeProperty ;
                  rdfs:domain era:Vehicle ;
                  rdfs:range xsd:string ;
                  dct:created "2020-11-24"^^xsd:date ;
                  dct:modified "2020-11-24"^^xsd:date ;
                  rdfs:comment "Identification number of a vehicle or wagon."@en ;
                  rdfs:isDefinedBy <http://data.europa.eu/949/> ;
                  rdfs:label "Vehicle number"@en ;
                  vs:term_status "stable" .


###  http://data.europa.eu/949/vehiclePantographHead
era:vehiclePantographHead rdf:type owl:DatatypeProperty ;
                          rdfs:domain era:VehicleType ;
                          rdfs:range xsd:string ;
                          era:eratvIndex "4.10.6" ;
                          dct:created "2020-08-25"^^xsd:date ;
                          dct:modified "2020-11-03"^^xsd:date ;
                          rdfs:comment "Pantograph head geometry (to be indicated for each energy supply system the vehicle is equipped for)."@en ;
                          rdfs:isDefinedBy <http://data.europa.eu/949/> ;
                          rdfs:label "Vehicle pantograph head"@en ;
                          vs:term_status "stable" .


###  http://data.europa.eu/949/vehicleSeries
era:vehicleSeries rdf:type owl:DatatypeProperty ;
                  rdfs:domain era:Vehicle ;
                  rdfs:range xsd:string ;
                  dct:created "2020-11-22"^^xsd:date ;
                  dct:modified "2020-11-22"^^xsd:date ;
                  rdfs:comment "Manufacturing series of a vehicle."@en ;
                  rdfs:isDefinedBy <http://data.europa.eu/949/> ;
                  rdfs:label "Vehicle series"@en ;
                  vs:term_status "unstable" .


###  http://data.europa.eu/949/vehicleTypeMaximumCantDeficiency
era:vehicleTypeMaximumCantDeficiency rdf:type owl:DatatypeProperty ;
                                     rdfs:domain era:MaximumSpeedAndCantDeficiency ;
                                     rdfs:range xsd:integer ;
                                     era:eratvIndex "4.6.4" ;
                                     dct:created "2023-04-05"^^xsd:date ;
                                     rdfs:comment "Part of the combination of maximum speed and maximum cant deficiency for which the vehicle was assessed. Corresponds to the maximum cant deficiency."@en ;
                                     rdfs:isDefinedBy <http://data.europa.eu/949/> ;
                                     rdfs:label "Vehicle type maximum cant deficiency"@en ;
                                     vs:term_status "stable" .


###  http://data.europa.eu/949/vehicleTypeMaximumSpeed
era:vehicleTypeMaximumSpeed rdf:type owl:DatatypeProperty ;
                            rdfs:domain era:MaximumSpeedAndCantDeficiency ;
                            rdfs:range xsd:integer ;
                            era:eratvIndex "4.6.4" ;
                            dct:created "2023-04-05"^^xsd:date ;
                            rdfs:comment "Part of the combination of maximum speed and maximum cant deficiency for which the vehicle was assessed. Corresponds to the maximum speed."@en ;
                            rdfs:isDefinedBy <http://data.europa.eu/949/> ;
                            rdfs:label "Vehicle type maximum speed"@en ;
                            vs:term_status "stable" .


###  http://data.europa.eu/949/vehicleTypesCompatibleTrafficLoad
era:vehicleTypesCompatibleTrafficLoad rdf:type owl:DatatypeProperty ;
                                      rdfs:domain [ rdf:type owl:Class ;
                                                    owl:unionOf ( era:SubsetWithCommonCharacteristics
                                                                  era:Track
                                                                )
                                                  ] ;
                                      rdfs:range xsd:anyURI ;
                                      era:rinfIndex "1.1.1.5.1" ;
                                      dct:created "2023-03-14"^^xsd:date ;
                                      rdfs:comment "The infrastructure managers shall provide through RINF the information to the RU regarding list of vehicle types compatible with the route for which they have already verified compatibility for parameter Traffic load and load carrying capacity of infrastructure and train detection systems, where such information is available."@en ;
                                      rdfs:isDefinedBy <http://data.europa.eu/949/> ;
                                      rdfs:label "List of vehicle types already identified as compatible with Traffic load and load carrying capacity of infrastructure and train detection systems"@en ;
                                      vs:term_status "unstable" .


###  http://data.europa.eu/949/vehiclesCompatibleTrafficLoad
era:vehiclesCompatibleTrafficLoad rdf:type owl:DatatypeProperty ;
                                  rdfs:domain [ rdf:type owl:Class ;
                                                owl:unionOf ( era:SubsetWithCommonCharacteristics
                                                              era:Track
                                                            )
                                              ] ;
                                  rdfs:range xsd:anyURI ;
                                  era:rinfIndex "1.1.1.5.2" ;
                                  dct:created "2023-03-14"^^xsd:date ;
                                  rdfs:comment "The infrastructure managers shall provide through RINF the information or a document to the RU regarding list of vehicle(s) compatible with the route for which they have already verified compatibility for parameter Traffic load and load carrying capacity of infrastructure and train detection systems, where such information is available."@en ;
                                  rdfs:isDefinedBy <http://data.europa.eu/949/> ;
                                  rdfs:label "List of vehicles already identified as compatible with Traffic load and load carrying capacity of infrastructure and train detection systems"@en ;
                                  vs:term_status "unstable" .


###  http://data.europa.eu/949/vehiclesComposingFixedFormation
era:vehiclesComposingFixedFormation rdf:type owl:DatatypeProperty ,
                                             owl:FunctionalProperty ;
                                    rdfs:domain era:VehicleType ;
                                    rdfs:range xsd:integer ;
                                    era:eratvIndex "4.1.12" ;
                                    dct:created "2021-08-25"^^xsd:date ;
                                    dct:modified "2021-08-25"^^xsd:date ;
                                    rdfs:comment "Number of vehicles composing the fixed formation (for fixed formation only). Note: the value is mandatory for all vehicle categories. If the vehicle is composed of only one car, the indicated value shall be '1'."@en ;
                                    rdfs:isDefinedBy <http://data.europa.eu/949/> ;
                                    rdfs:label "Vehicles composing fixed formation"@en ;
                                    vs:term_status "stable" .


###  http://data.europa.eu/949/verificationCCS
era:verificationCCS rdf:type owl:DatatypeProperty ;
                    rdfs:domain [ rdf:type owl:Class ;
                                  owl:unionOf ( era:SubsetWithCommonCharacteristics
                                                era:Track
                                              )
                                ] ;
                    rdfs:range xsd:string ;
                    era:rinfIndex "1.1.1.3.1.1" ;
                    dct:created "2021-08-08"^^xsd:date ;
                    dct:modified "2022-07-28"^^xsd:date ;
                    rdfs:comment "Unique number for EC declarations in accordance with Commission Implementing Regulation (EU) 2019/250"@en ;
                    rdfs:isDefinedBy <http://data.europa.eu/949/> ;
                    rdfs:label "EC declaration of verification for track (CCS)"@en ;
                    vs:term_status "stable" .


###  http://data.europa.eu/949/verificationENE
era:verificationENE rdf:type owl:DatatypeProperty ;
                    rdfs:domain [ rdf:type owl:Class ;
                                  owl:unionOf ( era:SubsetWithCommonCharacteristics
                                                era:Track
                                              )
                                ] ;
                    rdfs:range xsd:string ;
                    era:rinfIndex "1.1.1.2.1.1" ;
                    dct:created "2021-08-08"^^xsd:date ;
                    dct:modified "2021-09-11"^^xsd:date ;
                    rdfs:comment "Unique number for EC declarations in accordance with Commission Implementing Regulation (EU) 2019/250."@en ;
                    rdfs:isDefinedBy <http://data.europa.eu/949/> ;
                    rdfs:label "EC declaration of verification for track (ENE)"@en ;
                    vs:term_status "stable" .


###  http://data.europa.eu/949/verificationINF
era:verificationINF rdf:type owl:DatatypeProperty ;
                    rdfs:domain [ rdf:type owl:Class ;
                                  owl:unionOf ( era:Siding
                                                era:Track
                                              )
                                ] ;
                    rdfs:range xsd:string ;
                    era:rinfIndex "1.1.1.1.1.1" ,
                                  "1.2.1.0.1.1" ,
                                  "1.2.2.0.1.1" ;
                    dct:created "2021-08-03"^^xsd:date ;
                    dct:modified "2023-03-14"^^xsd:date ;
                    rdfs:comment """Unique number for EC declarations in accordance with Commission Implementing Regulation (EU) 2019/250.
In https://eur-lex.europa.eu/legal-content/EN/TXT/HTML/?uri=CELEX:32019R0777&from=EN"""@en ;
                    rdfs:isDefinedBy <http://data.europa.eu/949/> ;
                    rdfs:label "EC declaration of verification for track/siding [INF]"@en ;
                    vs:term_status "stable" .


###  http://data.europa.eu/949/verificationSRT
era:verificationSRT rdf:type owl:DatatypeProperty ;
                    rdfs:domain era:Tunnel ;
                    rdfs:range xsd:string ;
                    era:rinfIndex "1.1.1.1.8.5" ,
                                  "1.2.1.0.5.3" ,
                                  "1.2.2.0.5.3" ;
                    dct:created "2021-08-03"^^xsd:date ;
                    dct:modified "2021-09-02"^^xsd:date ;
                    rdfs:comment "Unique number for EC declarations in accordance with Commission Implementing Regulation (EU) 2019/250."@en ;
                    rdfs:isDefinedBy <http://data.europa.eu/949/> ;
                    rdfs:label "EC declaration of verification for tunnel (SRT)"@en ;
                    vs:term_status "stable" .


###  http://data.europa.eu/949/voiceOperationalCommImpl
era:voiceOperationalCommImpl rdf:type owl:DatatypeProperty ,
                                      owl:FunctionalProperty ;
                             rdfs:domain era:VehicleType ;
                             rdfs:range xsd:string ;
                             era:eratvIndex "4.13.2.6" ;
                             dct:created "2021-08-31"^^xsd:date ;
                             dct:modified "2021-08-31"^^xsd:date ;
                             rdfs:comment "Voice and operational communication implementation."@en ;
                             rdfs:isDefinedBy <http://data.europa.eu/949/> ;
                             rdfs:label "Voice operational communication implementation"@en ;
                             vs:term_status "stable" .


###  http://data.europa.eu/949/wheelSetGaugeTransformationMethod
era:wheelSetGaugeTransformationMethod rdf:type owl:DatatypeProperty ;
                                      rdfs:domain era:VehicleType ;
                                      rdfs:range xsd:string ;
                                      era:eratvIndex "4.1.3.b" ;
                                      dct:created "2021-08-25"^^xsd:date ;
                                      dct:modified "2021-08-25"^^xsd:date ;
                                      rdfs:comment "Wheel gauge transformation method. Defined if more than one wheel gauges have been selected."@en ;
                                      rdfs:isDefinedBy <http://data.europa.eu/949/> ;
                                      rdfs:label "Wheel set gauge transformation method"@en ;
                                      vs:term_status "stable" .


###  http://data.europa.eu/949/wheelchairSleepingPlaces
era:wheelchairSleepingPlaces rdf:type owl:DatatypeProperty ;
                             rdfs:domain era:VehicleType ;
                             rdfs:range xsd:string ;
                             era:eratvIndex "4.12.2.4" ;
                             dct:created "2021-08-31"^^xsd:date ;
                             dct:modified "2021-08-31"^^xsd:date ;
                             rdfs:comment "Number of wheelchair accessible sleeping places."@en ;
                             rdfs:isDefinedBy <http://data.europa.eu/949/> ;
                             rdfs:label "Wheelchair sleeping spaces"@en ;
                             vs:term_status "stable" .


###  http://data.europa.eu/949/wheelchairSpaces
era:wheelchairSpaces rdf:type owl:DatatypeProperty ;
                     rdfs:domain era:VehicleType ;
                     rdfs:range xsd:integer ;
                     era:eratvIndex "4.12.2.2" ;
                     dct:created "2021-08-31"^^xsd:date ;
                     dct:modified "2023-01-23"^^xsd:date ;
                     rdfs:comment "Number of wheelchair spaces."@en ;
                     rdfs:isDefinedBy <http://data.europa.eu/949/> ;
                     rdfs:label "Wheelchair spaces"@en ;
                     vs:term_status "stable" .


###  http://purl.org/dc/terms/identifier
dct:identifier rdf:type owl:DatatypeProperty .


###  http://schema.org/url
<http://schema.org/url> rdf:type owl:DatatypeProperty .


###  http://www.w3.org/ns/org#identifier
org:identifier rdf:type owl:DatatypeProperty .


###  http://xmlns.com/foaf/0.1/name
<http://xmlns.com/foaf/0.1/name> rdf:type owl:DatatypeProperty .


###  http://xmlns.com/foaf/0.1/nick
<http://xmlns.com/foaf/0.1/nick> rdf:type owl:DatatypeProperty .


#################################################################
#    Classes
#################################################################

###  http://data.europa.eu/949/Border
era:Border rdf:type owl:Class ;
           rdfs:subClassOf era:OperationalPoint ;
           dct:modified "2022-10-27"^^xsd:date ;
           dct:source "https://wiki3.railml.org/wiki/IS:border"^^xsd:anyURI ;
           rdfs:comment "The reason for deprecation of the Border is that it has no usage and is already represented in the SKOS OperationalPointTypes. This concept was  included as part of the LD4RAIL-242 Create functional prototype of the new vocabulary (D-B2-A2) issue, https://citnet.tech.ec.europa.eu/CITnet/confluence/pages/viewpage.action?pageId=1122974879."@en ;
           rdfs:isDefinedBy <http://data.europa.eu/949/> ;
           rdfs:label "Border"@en ;
           owl:deprecated "true"^^xsd:boolean ;
           skos:definition "A border point is used to separate the railway network due to different reasons. Typical examples are country borders, the change of owning infrastructure manager or the border of a station."@en .


###  http://data.europa.eu/949/Certificate
era:Certificate rdf:type owl:Class ;
                dct:created "2022-06-15"^^xsd:date ;
                dct:modified "2022-06-15"^^xsd:date ;
                rdfs:isDefinedBy <http://data.europa.eu/949/> ;
                rdfs:label "Certificate"@en ;
                vs:term_status "stable" .


###  http://data.europa.eu/949/ContactLineSystem
era:ContactLineSystem rdf:type owl:Class ;
                      era:rinfIndex "1.1.1.2.2" ;
                      dct:created "2021-08-04"^^xsd:date ;
                      dct:modified "2021-08-04"^^xsd:date ;
                      rdfs:comment "System that is used to transmit electrical energy to road or rail vehicles."@en ;
                      rdfs:isDefinedBy <http://data.europa.eu/949/> ;
                      rdfs:label "Contact Line System"@en ;
                      vs:term_status "stable" .


###  http://data.europa.eu/949/ETCSLevel
era:ETCSLevel rdf:type owl:Class ;
              era:rinfIndex "1.1.1.3.2" ;
              dct:created "2021-08-07"^^xsd:date ;
              dct:modified "2021-08-07"^^xsd:date ;
              rdfs:comment "ERTMS / ETCS application level related to the track side equipment."@en ;
              rdfs:isDefinedBy <http://data.europa.eu/949/> ;
              rdfs:label "ETCS Level"@en ;
              vs:term_status "stable" .


###  http://data.europa.eu/949/Feature
era:Feature rdf:type owl:Class ;
            rdfs:subClassOf gsp:Feature ;
            dct:created "2022-07-07"@en ;
            dct:modified "2022-10-27"^^xsd:date ;
            rdfs:comment "Class that encompasses the features that are part of the physical infrastructure (class InfrastructureObject) and the topological objects (class TopologicalObject). It is a subclass of the geographical Feature class that has a spatial representation."@en ;
            rdfs:isDefinedBy <http://data.europa.eu/949/> ;
            rdfs:label "ERA Feature"@en .


###  http://data.europa.eu/949/FrenchTrainDetectionSystemLimitation
era:FrenchTrainDetectionSystemLimitation rdf:type owl:Class ;
                                         dct:created "2023-04-05"^^xsd:date ;
                                         rdfs:comment """Specific for route compatibility check on French network. Sections with: 
-1 Tonnage circulated per track is inferior to 15000 tons/day/track 
-2 Directional Interlocking 
-3 45-second delay for directional interlocking 
-4 Installation with track circuit announcement 
-5 Absence of a shunting assistance pedal in the normal direction of circulation for non-reversible double track lines 
-6 Absence of a shunting assistance pedal regardless of the direction of traffic for single track lines and tracks for two way working 
-7 Absence of a pedal announcement mechanism 
-8 45-second delay for specific announcement reset devices"""@en ;
                                         rdfs:isDefinedBy <http://data.europa.eu/949/> ;
                                         rdfs:label "Section with train detection limitation, only for the French network"@en ;
                                         vs:term_status "stable" .


###  http://data.europa.eu/949/InfrastructureManager
era:InfrastructureManager rdf:type owl:Class ;
                          rdfs:subClassOf org:Organization ;
                          rdfs:comment "The infrastructure manager owns and operates the railway network and related infrastructure."@en ;
                          rdfs:isDefinedBy <http://data.europa.eu/949/> ;
                          rdfs:label "Infrastructure manager"@en ;
                          rdfs:seeAlso "https://wiki3.railml.org/wiki/CO:infrastructureManager"^^xsd:anyURI ;
                          skos:scopeNote "See point (2) of Article 3 of Directive 2012/34/EU of the European Parliament and of the Council establishing a single European railway area."@en .


###  http://data.europa.eu/949/InfrastructureObject
era:InfrastructureObject rdf:type owl:Class ;
                         rdfs:subClassOf era:Feature ;
                         dct:created "2022-07-07" ;
                         dct:modified "2022-10-27"^^xsd:date ;
                         rdfs:comment """This class encompasses all those classes that represent features that are  implemented in the European railway infrastructure. It is a subclass of the ERA Feature that has a spatial representation. It covers tracks, platforms, signals, tunnels, operational points, and sections of line.
A feature that belongs to the infrastructure can be abstracted (hasAbstraction) as a topological object. It also is related to the infrastructure manager through the property infrastructureMgr."""@en ;
                         rdfs:isDefinedBy <http://data.europa.eu/949/> ;
                         rdfs:label "Infrastructure object"@en ;
                         rdfs:seeAlso <https://wiki3.railml.org/DataModel/3.2/IS/EARoot/EA246.htm> .


###  http://data.europa.eu/949/LineReference
era:LineReference rdf:type owl:Class ;
                  dct:created "2021-01-29"^^xsd:date ;
                  dct:modified "2021-01-29"^^xsd:date ;
                  rdfs:comment "A reference to a specific national railway line."@en ,
                               "Railway location" ;
                  rdfs:isDefinedBy <http://data.europa.eu/949/> ;
                  rdfs:label "Railway location"@en ;
                  vs:term_status "stable" ;
                  skos:altLabel "Linear reference" .


###  http://data.europa.eu/949/LoadCapability
era:LoadCapability rdf:type owl:Class ;
                   dct:created "2023-03-14"^^xsd:date ;
                   rdfs:comment """A combination of the line category and speed at the weakest point of the track. 
Each track can have several load capability (structured) values, and each one has values for load model line category and load model speed."""@en ,
                                "This class together with properties loadCapabilityLineCategory and loadCapabilitySpeed replaces the previous loadCapability SKOS property."@en ;
                   rdfs:isDefinedBy <http://data.europa.eu/949/> ;
                   rdfs:label "Load capability"@en ;
                   vs:term_status "stable" .


###  http://data.europa.eu/949/Manufacturer
era:Manufacturer rdf:type owl:Class ;
                 rdfs:subClassOf org:Organization ;
                 dct:created "2020-11-19"^^xsd:date ;
                 dct:modified "2020-11-19"^^xsd:date ;
                 rdfs:comment "A company or organization that manufactures vehicles."@en ;
                 rdfs:isDefinedBy <http://data.europa.eu/949/> ;
                 rdfs:label "Manufacturer"@en ;
                 vs:term_status "stable" .


###  http://data.europa.eu/949/MaximumMagneticField
era:MaximumMagneticField rdf:type owl:Class ;
                         dct:created "2023-03-14"^^xsd:date ;
                         rdfs:comment """The maximum magnetic field limits allowed for axle counters (in dBÂµA/m) for a defined frequency band.
It should be provided in 3 directions."""@en ;
                         rdfs:isDefinedBy <http://data.europa.eu/949/> ;
                         rdfs:label "Maximum magnetic field"@en ;
                         vs:term_status "stable" .


###  http://data.europa.eu/949/MaximumSpeedAndCantDeficiency
era:MaximumSpeedAndCantDeficiency rdf:type owl:Class ;
                                  dct:created "2023-04-05" ;
                                  rdfs:comment "Combination of maximum speed and maximum cant deficiency for which the vehicle was assessed."@en ;
                                  rdfs:isDefinedBy <http://data.europa.eu/949/> ;
                                  rdfs:label "Maximum speed and cant deficiency"@en ;
                                  vs:term_status "stable" .


###  http://data.europa.eu/949/MinAxleLoadVehicleCategory
era:MinAxleLoadVehicleCategory rdf:type owl:Class ;
                               dct:created "2023-01-25"^^xsd:date ;
                               dct:modified "2023-03-14"@en ;
                               rdfs:comment "Deprecated according to the ammendment to the Regulation (EU) 2019/777. Represents information that indicates the load given in tons depending of the category of vehicle. Its properties are minAxleLoadVehicleCategory and minAxleLoad."@en ;
                               rdfs:isDefinedBy <http://data.europa.eu/949/> ;
                               rdfs:label "Min axle load vehicle category"@en ;
                               owl:deprecated "true"^^xsd:boolean ;
                               vs:term_status "stable" .


###  http://data.europa.eu/949/NationalRailwayLine
era:NationalRailwayLine rdf:type owl:Class ;
                        dct:created "2021-01-25"^^xsd:date ;
                        dct:modified "2021-08-03"^^xsd:date ;
                        rdfs:comment "Railway line within a member state."@en ;
                        rdfs:isDefinedBy <http://data.europa.eu/949/> ;
                        rdfs:label "National railway line"@en ;
                        rdfs:seeAlso <https://wiki3.railml.org/DataModel/3.2/IS/EARoot/EA210.htm> ;
                        vs:term_status "stable" .


###  http://data.europa.eu/949/NetElement
era:NetElement rdf:type owl:Class ;
               rdfs:subClassOf era:TopologicalObject ;
               dct:created "2021-04-01"^^xsd:date ;
               dct:modified "2021-04-01"^^xsd:date ;
               rdfs:comment "Base class for defining nodes in the connectivity graph representing the topological network."@en ;
               rdfs:isDefinedBy <http://data.europa.eu/949/> ;
               rdfs:label "Net Element"@en ;
               rdfs:seeAlso <https://rsm-evolution.org/220927_RSM/EARoot/EA2/EA2/EA287.html> ,
                            <https://wiki3.railml.org/DataModel/3.2/IS/EARoot/EA227.htm> ,
                            "http://wiki.railtopomodel.org/index.php?title=Main_Page" ;
               vs:term_status "stable" .


###  http://data.europa.eu/949/NetRelation
era:NetRelation rdf:type owl:Class ;
                rdfs:subClassOf era:TopologicalObject ;
                dct:created "2021-04-01"^^xsd:date ;
                dct:modified "2021-04-01"^^xsd:date ;
                rdfs:comment "Base class for defining edges in the connectivity graph representing the topological network."@en ;
                rdfs:isDefinedBy <http://data.europa.eu/949/> ;
                rdfs:label "Net Relation"@en ;
                rdfs:seeAlso <https://rsm-evolution.org/220927_RSM/EARoot/EA2/EA2/EA292.html> ,
                             <https://wiki3.railml.org/DataModel/3.2/IS/EARoot/EA230.htm> ,
                             "http://wiki.railtopomodel.org/index.php?title=Main_Page" ;
                vs:term_status "stable" .


###  http://data.europa.eu/949/OperationalPoint
era:OperationalPoint rdf:type owl:Class ;
                     rdfs:subClassOf era:InfrastructureObject ;
                     era:appendixD2Index "2.1.2" ;
                     era:rinfIndex 1.2 ;
                     dct:created "2020-07-29"^^xsd:date ;
                     dct:modified "2022-07-07"^^xsd:date ;
                     rdfs:comment """An operational point (OP) means any location for train service operations, where train services may begin and end or change route, and where passenger or freight services may be provided; operational point also means any location at boundaries between Member States or infrastructure managers.
In https://eur-lex.europa.eu/eli/reg_impl/2019/773/oj 2.1.2 Principal locations (stations, yards, junctions, freight terminals)."""@en ;
                     rdfs:isDefinedBy <http://data.europa.eu/949/> ;
                     rdfs:label "Operational Point"@en ;
                     rdfs:seeAlso <https://wiki3.railml.org/DataModel/3.2/IS/EARoot/EA238.htm> ;
                     vs:term_status "stable" .


###  http://data.europa.eu/949/PhaseInfo
era:PhaseInfo rdf:type owl:Class ;
              dct:created "2023-04-05"^^xsd:date ;
              rdfs:comment "Indication of required several information on phase separation."@en ;
              rdfs:isDefinedBy <http://data.europa.eu/949/> ;
              rdfs:label "Phase info"@en ;
              vs:term_status era:stable .


###  http://data.europa.eu/949/Platform
era:Platform rdf:type owl:Class ;
             rdfs:subClassOf era:InfrastructureObject ;
             era:rinfIndex "1.2.1.0.6" ;
             dct:created "2021-08-02"^^xsd:date ;
             dct:modified "2022-07-07"^^xsd:date ;
             rdfs:comment "Platform for the purpose of RINF is understood as a platform edge. A platform concerns only the part of the structure neighbouring to the track (interfaced with trains)."@en ;
             rdfs:isDefinedBy <http://data.europa.eu/949/> ;
             rdfs:label "Platform"@en ;
             rdfs:seeAlso <https://wiki3.railml.org/DataModel/3.2/IS/EARoot/EA250.htm> ;
             vs:term_status "stable" .


###  http://data.europa.eu/949/RaisedPantographsDistanceAndSpeed
era:RaisedPantographsDistanceAndSpeed rdf:type owl:Class ;
                                      dct:created "2023-04-05"^^xsd:date ;
                                      rdfs:isDefinedBy <http://data.europa.eu/949/> ;
                                      rdfs:label """Indication of maximum number of raised pantographs per train allowed and minimum spacing centre line to centre line of adjacent pantograph heads, expressed in metres, at the given speed.
Each track can have several raised pantographs per train allowed (structured) values, and each one has values for number of pantographs, minimum distance between pantographs, in metres, and speed considered in km/h."""@en ,
                                                 "Raised pantographs distance and speed"@en ;
                                      vs:term_status "stable" .


###  http://data.europa.eu/949/SectionOfLine
era:SectionOfLine rdf:type owl:Class ;
                  rdfs:subClassOf era:InfrastructureObject ,
                                  [ rdf:type owl:Restriction ;
                                    owl:onProperty era:lineNationalId ;
                                    owl:qualifiedCardinality "1"^^xsd:nonNegativeInteger ;
                                    owl:onClass era:NationalRailwayLine
                                  ] ,
                                  [ rdf:type owl:Restriction ;
                                    owl:onProperty era:opEnd ;
                                    owl:qualifiedCardinality "1"^^xsd:nonNegativeInteger ;
                                    owl:onClass era:OperationalPoint
                                  ] ,
                                  [ rdf:type owl:Restriction ;
                                    owl:onProperty era:opStart ;
                                    owl:qualifiedCardinality "1"^^xsd:nonNegativeInteger ;
                                    owl:onClass era:OperationalPoint
                                  ] ;
                  era:appendixD2Index "2.1.1" ;
                  era:rinfIndex 1.1 ;
                  <http://purl.org/dc/elements/1.1/source> <https://eur-lex.europa.eu/eli/reg_impl/2019/773/oj> ;
                  dct:created "2021-04-02"^^xsd:date ;
                  dct:modified "2022-07-07"^^xsd:date ;
                  rdfs:comment """A section of line means the part of line between adjacent operational points and may consist of several tracks.
In https://eur-lex.europa.eu/eli/reg_impl/2019/773/oj 2.1.1 Line sections."""@en ;
                  rdfs:isDefinedBy <http://data.europa.eu/949/> ;
                  rdfs:label "Section Of Line"@en ;
                  vs:term_status "stable" .


###  http://data.europa.eu/949/Siding
era:Siding rdf:type owl:Class ;
           rdfs:subClassOf era:Track ;
           era:rinfIndex "1.2.2" ;
           dct:created "2021-08-10"^^xsd:date ;
           dct:modified "2022-10-27"^^xsd:date ;
           dct:source "Official Journal of the European Union L 139 I/85" ;
           rdfs:comment "Sidings are all those tracks where running trains in service movements ends and which are not used for operational routing of a train."@en ;
           rdfs:isDefinedBy <http://data.europa.eu/949/> ;
           rdfs:label "Siding"@en ;
           vs:term_status "stable" ;
           skos:definition "Siding Any track(s) within an operational point which is not used for operational routing of a train."@en .


###  http://data.europa.eu/949/Signal
era:Signal rdf:type owl:Class ;
           rdfs:subClassOf era:InfrastructureObject ;
           era:rinfIndex "1.2.1.0.8" ;
           <http://purl.org/dc/elements/1.1/source> <https://eur-lex.europa.eu/eli/reg_impl/2019/773/oj> ;
           dct:created "2021-04-01"^^xsd:date ;
           dct:modified "2022-10-27"^^xsd:date ;
           rdfs:comment """A railway signal is an installation next to the railway track for signalling the maximum allowed speed in the next block section to the train driver.
Definition RSM: Apparatus by means of which a conventional visual or acoustic indication is given, generally concerning the movements of railway vehicles."""@en ;
           rdfs:isDefinedBy <http://data.europa.eu/949/> ;
           rdfs:label "Signal"@en ;
           rdfs:seeAlso <https://rsm-evolution.org/220927_RSM/EARoot/EA4/EA3/EA978.html> ,
                        <https://wiki3.railml.org/DataModel/3.2/IS/EARoot/EA271.htm> ;
           vs:term_status "stable" .


###  http://data.europa.eu/949/SpecialArea
era:SpecialArea rdf:type owl:Class ;
                rdfs:subClassOf era:InfrastructureObject ;
                <http://purl.org/dc/elements/1.1/source> <https://eur-lex.europa.eu/eli/reg_impl/2019/773/oj> ;
                dct:created "2022-10-27"@en ;
                rdfs:comment "Encompasses all those areas or sections such as safe areas, restricted areas (non-stopping areas or industrial risk locations)."@en ;
                rdfs:isDefinedBy <http://data.europa.eu/949/> ;
                rdfs:label "Special area"@en ;
                rdfs:seeAlso <https://wiki3.railml.org/DataModel/3.2/IS/EARoot/EA258.htm> ;
                vs:term_status "stable" .


###  http://data.europa.eu/949/SpecialTunnelArea
era:SpecialTunnelArea rdf:type owl:Class ;
                      rdfs:subClassOf era:SpecialArea ;
                      <http://purl.org/dc/elements/1.1/source> <https://eur-lex.europa.eu/eli/reg_impl/2019/773/oj> ;
                      dct:created "2022-10-27"@en ;
                      rdfs:comment "Area or location within a tunnel where  there is a walkway, evacuation and rescue points."@en ;
                      rdfs:isDefinedBy <http://data.europa.eu/949/> ;
                      rdfs:label "Special tunnel area"@en ;
                      vs:term_status "stable" .


###  http://data.europa.eu/949/SubsetWithCommonCharacteristics
era:SubsetWithCommonCharacteristics rdf:type owl:Class ;
                                    dct:created "2022-11-04"^^xsd:date ;
                                    dct:modified "2023-03-14"^^xsd:date ;
                                    rdfs:comment "Subset of items shared by sections of lines and/or operational points of a member state. For the purposes of the register of infrastructure, each infrastructure manager shall describe its railway network at least by sections of line and operational points and optionally via common characteristic subsets."@en ;
                                    rdfs:isDefinedBy <http://data.europa.eu/949/> ;
                                    rdfs:label "Subset with common characteristics"@en ;
                                    vs:term_status "stable" .


###  http://data.europa.eu/949/SystemSeparationInfo
era:SystemSeparationInfo rdf:type owl:Class ;
                         dct:created "2023-04-05"^^xsd:date ;
                         rdfs:comment "Indication of required several information on system separation."@en ;
                         rdfs:isDefinedBy "http://data.europa.eu/949/"^^xsd:date ;
                         rdfs:label "System separation info"@en ;
                         vs:term_status "stable" .


###  http://data.europa.eu/949/TopologicalObject
era:TopologicalObject rdf:type owl:Class ;
                      rdfs:subClassOf era:Feature ;
                      dct:created "2022-05-04"^^xsd:date ;
                      rdfs:comment "Top level class for the the track network described as a topological node edge model"@en ;
                      rdfs:isDefinedBy <http://data.europa.eu/949/> ;
                      rdfs:label "Topological Object"@en ;
                      rdfs:seeAlso <https://wiki3.railml.org/DataModel/3.2/IS/EARoot/EA386.htm> ;
                      vs:term_status "unstable" .


###  http://data.europa.eu/949/Track
era:Track rdf:type owl:Class ;
          rdfs:subClassOf era:InfrastructureObject ;
          era:rinfIndex "1.1.1" ;
          dct:created "2020-07-29"^^xsd:date ;
          dct:modified "2022-07-07"^^xsd:date ;
          rdfs:comment "A running track that is used for train service movements."@en ;
          rdfs:isDefinedBy <http://data.europa.eu/949/> ;
          rdfs:label "Track"@en ;
          rdfs:seeAlso <https://wiki3.railml.org/DataModel/3.2/IS/EARoot/EA400.htm> ;
          vs:term_status "stable" .


###  http://data.europa.eu/949/TrainDetectionSystem
era:TrainDetectionSystem rdf:type owl:Class ;
                         era:rinfIndex "1.1.1.3.4" ;
                         dct:created "2021-08-07"^^xsd:date ;
                         dct:modified "2021-08-07"^^xsd:date ;
                         rdfs:comment "System used to detect the position of vehicles in the railway track."@en ;
                         rdfs:isDefinedBy <http://data.europa.eu/949/> ;
                         rdfs:label "Train Detection System"@en ;
                         rdfs:seeAlso <https://wiki3.railml.org/DataModel/3.2/IS/EARoot/EA402.htm> ;
                         vs:term_status "stable" .


###  http://data.europa.eu/949/Tunnel
era:Tunnel rdf:type owl:Class ;
           rdfs:subClassOf era:InfrastructureObject ;
           era:rinfIndex "1.2.2.0.5" ;
           <http://purl.org/dc/elements/1.1/source> <https://eur-lex.europa.eu/eli/reg_impl/2019/773/oj> ;
           dct:created "2020-07-29"^^xsd:date ;
           dct:modified "2022-07-07"^^xsd:date ;
           rdfs:comment "A railway tunnel is an excavation or a construction around the track provided to allow the railway to pass for example higher land, buildings or water."@en ;
           rdfs:isDefinedBy <http://data.europa.eu/949/> ;
           rdfs:label "Tunnel"@en ;
           vs:term_status "stable" .


###  http://data.europa.eu/949/Vehicle
era:Vehicle rdf:type owl:Class ;
            dct:created "2020-11-22"^^xsd:date ;
            dct:modified "2020-11-22"^^xsd:date ;
            rdfs:comment "A specific vehicle or wagon able to operate over railway lines."@en ;
            rdfs:isDefinedBy <http://data.europa.eu/949/> ;
            rdfs:label "Vehicle"@en ;
            vs:term_status "stable" .


###  http://data.europa.eu/949/VehicleKeeper
era:VehicleKeeper rdf:type owl:Class ;
                  rdfs:subClassOf org:Organization ;
                  dct:created "2020-11-23"^^xsd:date ;
                  dct:modified "2020-11-23"^^xsd:date ;
                  rdfs:comment "A company or organization that owns or operates a certain vehicle."@en ;
                  rdfs:isDefinedBy <http://data.europa.eu/949/> ;
                  rdfs:label "Vehicle Keeper"@en ;
                  vs:term_status "stable" .


###  http://data.europa.eu/949/VehicleType
era:VehicleType rdf:type owl:Class ;
                rdfs:subClassOf [ rdf:type owl:Restriction ;
                                  owl:onProperty era:manufacturer ;
                                  owl:qualifiedCardinality "1"^^xsd:nonNegativeInteger ;
                                  owl:onClass era:Manufacturer
                                ] ;
                dct:created "2020-07-29"^^xsd:date ;
                dct:modified "2020-07-29"^^xsd:date ;
                rdfs:comment "A vehicle type that has been authorized to operate on the EU railway infrastructure."@en ;
                rdfs:isDefinedBy <http://data.europa.eu/949/> ;
                rdfs:label "Vehicle Type"@en ;
                vs:term_status "stable" .


###  http://www.opengis.net/ont/geosparql#Feature
gsp:Feature rdf:type owl:Class .


###  http://www.opengis.net/ont/geosparql#Geometry
gsp:Geometry rdf:type owl:Class .


###  http://www.w3.org/1999/02/22-rdf-syntax-ns#Bag
rdf:Bag rdf:type owl:Class .


###  http://www.w3.org/2000/01/rdf-schema#Resource
rdfs:Resource rdf:type owl:Class .


###  http://www.w3.org/2003/01/geo/wgs84_pos#Point
wgs:Point rdf:type owl:Class ;
          rdfs:subClassOf wgs:SpatialThing ;
          rdfs:comment """ 
Uniquely identified by lat/long/alt. i.e.

spaciallyIntersects(P1, P2) :- lat(P1, LAT), long(P1, LONG), alt(P1, ALT),
  lat(P2, LAT), long(P2, LONG), alt(P2, ALT).

sameThing(P1, P2) :- type(P1, Point), type(P2, Point), spaciallyIntersects(P1, P2).
  """ ,
                       """A point, typically described using a coordinate system relative to Earth, such as WGS84.
  """ ;
          rdfs:label "Point" .


###  http://www.w3.org/2003/01/geo/wgs84_pos#SpatialThing
wgs:SpatialThing rdf:type owl:Class ;
                 rdfs:comment """Anything with spatial extent, i.e. size, shape, or position.
 e.g. people, places, bowling balls, as well as abstract areas like cubes.
""" ;
                 rdfs:label "SpatialThing" .


###  http://www.w3.org/2004/02/skos/core#Concept
skos:Concept rdf:type owl:Class .


###  http://www.w3.org/ns/org#Organization
org:Organization rdf:type owl:Class .


#################################################################
#    Individuals
#################################################################

###  http://data.europa.eu/949/concepts/op-types/borderStation
opTypes:borderStation rdf:type owl:NamedIndividual .


###  http://data.europa.eu/949/concepts/op-types/station
opTypes:station rdf:type owl:NamedIndividual .


#################################################################
#    Annotations
#################################################################

gsp:asWKT era:rinfIndex "1.1.1.3.14.6" ,
                        "1.1.0.0.1.1" ,
                        "1.1.1.0.1.1" ,
                        "1.2.0.0.0.5" ;
          era:appendixD2Index "2.1.1" ,
                              "2.1.2" ,
                              "2.2.2" ;
          era:rinfIndex "1.2.1.0.8.5" .


wgs: <http://purl.org/dc/elements/1.1/date> "$Date: 2009/04/20 15:00:30 $" ;
     rdfs:label "geo" ;
     <http://purl.org/dc/elements/1.1/description> """A vocabulary for representing latitude, longitude and 
 altitude information in the WGS84 geodetic reference datum. 
 Version $Id: wgs84_pos.rdf,v 1.22 2009/04/20 15:00:30 timbl Exp $. See http://www.w3.org/2003/01/geo/ for more details.""" ;
     rdfs:comment """
Recent changes to this namespace:
$Log: wgs84_pos.rdf,v $
Revision 1.22  2009/04/20 15:00:30  timbl
Remove the time bits which have been deal with elsewhere eg in iCal.

Revision 1.21  2009/04/20 12:52:47  timbl
try again

Revision 1.20  2009/04/20 12:42:11  timbl
Add Event (edited ages ago and never checked in), and location (following discussion http://chatlogs.planetrdf.com/swig/2009-04-20#T12-36-09)

Revision 1.19  2009/04/20 12:36:31  timbl
Add Event (edited ages ago and never checked in), and location (following discussion http://chatlogs.planetrdf.com/swig/2009-04-20#T12-36-09)

Revision 1.18  2006/02/01 22:01:04  danbri
Clarified that lat and long are decimal degrees, and that alt is decimal metres about local reference ellipsoid

Revision 1.17  2004/02/06 17:38:12  danbri
Fixed a bad commit screwup

Revision 1.15  2003/04/19 11:24:08  danbri
Fixed the typo even more.

Revision 1.14  2003/04/19 11:16:56  danbri
fixed a typo

Revision 1.13  2003/02/19 22:27:27  connolly
relaxed domain constraints on lat/long/alt from Point to SpatialThing

Revision 1.12  2003/01/12 01:41:41  danbri
Trying local copy of XSLT doc.

Revision 1.11  2003/01/12 01:20:18  danbri
added a link to morten's xslt rdfs viewer.

Revision 1.10  2003/01/11 18:56:49  danbri
Removed datatype range from lat and long properties, since they would
have required each occurance of the property to mention the datatype.

Revision 1.9  2003/01/11 11:41:31  danbri
Another typo; repaired rdfs:Property to rdf:Property x4

Revision 1.8  2003/01/11 11:05:02  danbri
Added an rdfs:range for each lat/long/alt property,
http://www.w3.org/2001/XMLSchema#float

Revision 1.7  2003/01/10 20:25:16  danbri
Longer rdfs:comment for Point, trying to be Earth-centric and neutral about
coordinate system(s) at the same time. Feedback welcomed.

Revision 1.6  2003/01/10 20:18:30  danbri
Added CVS log comments into the RDF/XML as an rdfs:comment property of the
vocabulary. Note that this is not common practice (but seems both harmless
and potentially useful).


revision 1.5
date: 2003/01/10 20:14:31;  author: danbri;  state: Exp;  lines: +16 -5
Updated schema:
Added a dc:date, added url for more info. Changed the rdfs:label of the
namespace from gp to geo. Added a class Point, set as the rdfs:domain of
each property. Added XML comment on the lat_long property suggesting that
we might not need it (based on #rdfig commentary from implementors).

revision 1.4
date: 2003/01/10 20:01:07;  author: danbri;  state: Exp;  lines: +6 -5
Fixed typo; several rdfs:about attributes are now rdf:about. Thanks to MortenF in
#rdfig for catching this error.

revision 1.3
date: 2003/01/10 11:59:03;  author: danbri;  state: Exp;  lines: +4 -3
fixed buglet in vocab, added more wgs links

revision 1.2
date: 2003/01/10 11:01:11;  author: danbri;  state: Exp;  lines: +4 -4
Removed alt from the as-a-flat-string property, and switched from
space separated to comma separated.

revision 1.1
date: 2003/01/10 10:53:23;  author: danbri;  state: Exp;
basic geo vocab

""" ;
     <http://purl.org/dc/elements/1.1/title> "WGS84 Geo Positioning: an RDF vocabulary" .


wgs:lat_long rdfs:comment "A comma-separated representation of a latitude, longitude coordinate." ;
             rdfs:label "Lat/long" .


wgs:location rdfs:label "Location" ;
             rdfs:comment """The relation between something and the point, 
 or other geometrical thing in space, where it is.  For example, the realtionship between
 a radio tower and a Point with a given lat and long.
 Or a relationship between a park and its outline as a closed arc of points, or a road and
 its location as a arc (a sequence of points).
 Clearly in practice there will be limit to the accuracy of any such statement, but one would expect
 an accuracy appropriate for the size of the object and uses such as mapping .
 """ ;
             era:rinfIndex "1.1.0.0.1.1" ,
                           "1.1.1.3.14.6" ,
                           "1.2.1.0.8.5" ,
                           "1.2.0.0.0.5" ;
             era:usedInRCCCalculations "true"^^xsd:boolean ;
             era:rinfIndex "1.1.1.0.1.1" .


###  Generated by the OWL API (version 4.5.9.2019-02-01T07:24:44Z) https://github.com/owlcs/owlapi
